<?xml version = '1.0' encoding = 'UTF-8'?>
<rdf:RDF xmlns="http://vcd.vicomtech.org/ontology/automotive#" xml:base="http://vcd.vicomtech.org/ontology/automotive" xmlns:owl="http://www.w3.org/2002/07/owl#" xmlns:rdfs="http://www.w3.org/2000/01/rdf-schema#" xmlns:rdf="http://www.w3.org/1999/02/22-rdf-syntax-ns#" xmlns:xsd="http://www.w3.org/2001/XMLSchema#" xmlns:dcterms="http://unknown.prefix/dcterms#">
  <owl:Ontology rdf:about="http://vcd.vicomtech.org/ontology/automotive#" />
  <!-- 
    ///////////////////////////////////////////////////////////////////////////////////////
    //
    // Annotation properties
    //
    ///////////////////////////////////////////////////////////////////////////////////////
     -->
  <!-- http://unknown.prefix/dcterms#description -->
  <owl:AnnotationProperty rdf:about="http://unknown.prefix/dcterms#description" />
  <!-- 
    ///////////////////////////////////////////////////////////////////////////////////////
    //
    // Classes
    //
    ///////////////////////////////////////////////////////////////////////////////////////
     -->
  <!-- http://vcd.vicomtech.org/ontology/automotive#Accessories -->
  <owl:Class rdf:about="http://vcd.vicomtech.org/ontology/automotive#Accessories">
    <rdfs:label xml:lang="en">Accessories</rdfs:label>
    <rdfs:subClassOf rdf:resource="http://vcd.vicomtech.org/ontology/automotive#Attribute" />
    <dcterms:description xml:lang="en">A thing which can be added to something else in order to make it more useful, versatile, or attractive.</dcterms:description>
  </owl:Class>
  <!-- http://vcd.vicomtech.org/ontology/automotive#Action -->
  <owl:Class rdf:about="http://vcd.vicomtech.org/ontology/automotive#Action">
    <rdfs:label xml:lang="en">Action</rdfs:label>
    <rdfs:subClassOf rdf:resource="http://www.w3.org/2002/07/owl#Thing" />
    <dcterms:description xml:lang="en">A maneuver performed by an object to achieve an end. Could be done to change the initial state or to keep the stationary state.</dcterms:description>
  </owl:Class>
  <!-- http://vcd.vicomtech.org/ontology/automotive#ActiveSafety -->
  <owl:Class rdf:about="http://vcd.vicomtech.org/ontology/automotive#ActiveSafety">
    <rdfs:label xml:lang="en">Active safety</rdfs:label>
    <rdfs:subClassOf rdf:resource="http://vcd.vicomtech.org/ontology/automotive#Safety" />
    <dcterms:description xml:lang="en">Is used to refer to technology assisting in the prevention of a crash.</dcterms:description>
  </owl:Class>
  <!-- http://vcd.vicomtech.org/ontology/automotive#Adult -->
  <owl:Class rdf:about="http://vcd.vicomtech.org/ontology/automotive#Adult">
    <rdfs:label xml:lang="en">Adult</rdfs:label>
    <rdfs:subClassOf rdf:resource="http://vcd.vicomtech.org/ontology/automotive#Pedestrian" />
    <dcterms:description xml:lang="en">A human who is fully grown or developed.</dcterms:description>
  </owl:Class>
  <!-- http://vcd.vicomtech.org/ontology/automotive#Age -->
  <owl:Class rdf:about="http://vcd.vicomtech.org/ontology/automotive#Age">
    <rdfs:label xml:lang="en">Age</rdfs:label>
    <rdfs:subClassOf rdf:resource="http://vcd.vicomtech.org/ontology/automotive#Attribute" />
    <dcterms:description xml:lang="en">The length of time that a person has lived or a thing has existed.</dcterms:description>
  </owl:Class>
  <!-- http://vcd.vicomtech.org/ontology/automotive#Aircraft -->
  <owl:Class rdf:about="http://vcd.vicomtech.org/ontology/automotive#Aircraft">
    <rdfs:label xml:lang="en">Aircraft</rdfs:label>
    <rdfs:subClassOf rdf:resource="http://vcd.vicomtech.org/ontology/automotive#Vehicle" />
    <dcterms:description xml:lang="en">An aeroplane, helicopter or other machine capable of flight.</dcterms:description>
  </owl:Class>
  <!-- http://vcd.vicomtech.org/ontology/automotive#Ambulance -->
  <owl:Class rdf:about="http://vcd.vicomtech.org/ontology/automotive#Ambulance">
    <rdfs:label xml:lang="en">Ambulance</rdfs:label>
    <rdfs:subClassOf rdf:resource="http://vcd.vicomtech.org/ontology/automotive#EmergencyVehicle" />
    <dcterms:description xml:lang="en">A road vehicle equipped for taking sick or injured people to and from hospital, especially in emergencies.</dcterms:description>
  </owl:Class>
  <!-- http://vcd.vicomtech.org/ontology/automotive#Animal -->
  <owl:Class rdf:about="http://vcd.vicomtech.org/ontology/automotive#Animal">
    <rdfs:label xml:lang="en">Animal</rdfs:label>
    <rdfs:subClassOf rdf:resource="http://vcd.vicomtech.org/ontology/automotive#Dynamic" />
    <dcterms:description xml:lang="en">A living organism that feeds on organic matter, typically having specialized sense organs and nervous system and able to respond rapidly to stimuli.</dcterms:description>
  </owl:Class>
  <!-- http://vcd.vicomtech.org/ontology/automotive#Approaching -->
  <owl:Class rdf:about="http://vcd.vicomtech.org/ontology/automotive#Approaching">
    <rdfs:label xml:lang="en">Approaching</rdfs:label>
    <rdfs:subClassOf rdf:resource="http://vcd.vicomtech.org/ontology/automotive#MovingManeuver" />
    <dcterms:description xml:lang="en">The action of getting closer to a junction, crosswalk or other object.</dcterms:description>
  </owl:Class>
  <!-- http://vcd.vicomtech.org/ontology/automotive#Arrow -->
  <owl:Class rdf:about="http://vcd.vicomtech.org/ontology/automotive#Arrow">
    <rdfs:label xml:lang="en">Arrow</rdfs:label>
    <rdfs:subClassOf rdf:resource="http://vcd.vicomtech.org/ontology/automotive#Marking" />
    <dcterms:description xml:lang="en">Direction arrows used on the approach to busy multi-lane junctions to give drivers advance indication of the correct lane.</dcterms:description>
  </owl:Class>
  <!-- http://vcd.vicomtech.org/ontology/automotive#ArrowLeftTurn -->
  <owl:Class rdf:about="http://vcd.vicomtech.org/ontology/automotive#ArrowLeftTurn">
    <rdfs:label xml:lang="en">Arrow left turn</rdfs:label>
    <rdfs:subClassOf rdf:resource="http://vcd.vicomtech.org/ontology/automotive#Arrow" />
    <dcterms:description xml:lang="en">Arrow indicating a left turn.</dcterms:description>
  </owl:Class>
  <!-- http://vcd.vicomtech.org/ontology/automotive#ArrowLeftrightTurn -->
  <owl:Class rdf:about="http://vcd.vicomtech.org/ontology/automotive#ArrowLeftrightTurn">
    <rdfs:label xml:lang="en">Arrow leftright turn</rdfs:label>
    <rdfs:subClassOf rdf:resource="http://vcd.vicomtech.org/ontology/automotive#Arrow" />
    <dcterms:description xml:lang="en">A two headed arrow indicating a left and right turn.</dcterms:description>
  </owl:Class>
  <!-- http://vcd.vicomtech.org/ontology/automotive#ArrowRightTurn -->
  <owl:Class rdf:about="http://vcd.vicomtech.org/ontology/automotive#ArrowRightTurn">
    <rdfs:label xml:lang="en">Arrow right turn</rdfs:label>
    <rdfs:subClassOf rdf:resource="http://vcd.vicomtech.org/ontology/automotive#Arrow" />
    <dcterms:description xml:lang="en">Arrow indicating a right turn.</dcterms:description>
  </owl:Class>
  <!-- http://vcd.vicomtech.org/ontology/automotive#ArrowThru -->
  <owl:Class rdf:about="http://vcd.vicomtech.org/ontology/automotive#ArrowThru">
    <rdfs:label xml:lang="en">Arrow thru</rdfs:label>
    <rdfs:subClassOf rdf:resource="http://vcd.vicomtech.org/ontology/automotive#Arrow" />
    <dcterms:description xml:lang="en">Arrow marking pointing straight ahead.</dcterms:description>
  </owl:Class>
  <!-- http://vcd.vicomtech.org/ontology/automotive#ArrowThruleftTurn -->
  <owl:Class rdf:about="http://vcd.vicomtech.org/ontology/automotive#ArrowThruleftTurn">
    <rdfs:label xml:lang="en">Arrow thruleft turn</rdfs:label>
    <rdfs:subClassOf rdf:resource="http://vcd.vicomtech.org/ontology/automotive#Arrow" />
    <dcterms:description xml:lang="en">A two-headed arrow with one head pointing straight ahead and the other pointing to the left.</dcterms:description>
  </owl:Class>
  <!-- http://vcd.vicomtech.org/ontology/automotive#ArrowThrurightTurn -->
  <owl:Class rdf:about="http://vcd.vicomtech.org/ontology/automotive#ArrowThrurightTurn">
    <rdfs:label xml:lang="en">Arrow thruright turn</rdfs:label>
    <rdfs:subClassOf rdf:resource="http://vcd.vicomtech.org/ontology/automotive#Arrow" />
    <dcterms:description xml:lang="en">A two-headed arrow with one head pointing straight ahead and the other pointing to the right.</dcterms:description>
  </owl:Class>
  <!-- http://vcd.vicomtech.org/ontology/automotive#ArrowUturn -->
  <owl:Class rdf:about="http://vcd.vicomtech.org/ontology/automotive#ArrowUturn">
    <rdfs:label xml:lang="en">U turn arrow</rdfs:label>
    <rdfs:subClassOf rdf:resource="http://vcd.vicomtech.org/ontology/automotive#Arrow" />
    <dcterms:description xml:lang="en">U-shaped arrow indicating that a change of direction can be done.</dcterms:description>
  </owl:Class>
  <!-- http://vcd.vicomtech.org/ontology/automotive#Attribute -->
  <owl:Class rdf:about="http://vcd.vicomtech.org/ontology/automotive#Attribute">
    <rdfs:label xml:lang="en">Attribute</rdfs:label>
    <rdfs:subClassOf rdf:resource="http://www.w3.org/2002/07/owl#Thing" />
    <dcterms:description xml:lang="en">A quality or feature regarded as a characteristic or inherent part of someone or something.</dcterms:description>
  </owl:Class>
  <!-- http://vcd.vicomtech.org/ontology/automotive#Back -->
  <owl:Class rdf:about="http://vcd.vicomtech.org/ontology/automotive#Back">
    <rdfs:label xml:lang="en">Back</rdfs:label>
    <rdfs:subClassOf rdf:resource="http://vcd.vicomtech.org/ontology/automotive#TrafficSign" />
    <dcterms:description xml:lang="en">Back side of traffic signs.</dcterms:description>
  </owl:Class>
  <!-- http://vcd.vicomtech.org/ontology/automotive#Banner -->
  <owl:Class rdf:about="http://vcd.vicomtech.org/ontology/automotive#Banner">
    <rdfs:label xml:lang="en">Banner</rdfs:label>
    <rdfs:subClassOf rdf:resource="http://vcd.vicomtech.org/ontology/automotive#Signs" />
    <dcterms:description xml:lang="en">Typically a flag, made of textile or plastic.</dcterms:description>
  </owl:Class>
  <!-- http://vcd.vicomtech.org/ontology/automotive#Barrier -->
  <owl:Class rdf:about="http://vcd.vicomtech.org/ontology/automotive#Barrier">
    <rdfs:label xml:lang="en">Barrier</rdfs:label>
    <rdfs:subClassOf rdf:resource="http://vcd.vicomtech.org/ontology/automotive#Construction" />
    <dcterms:description xml:lang="en">A fence or other obstacle that prevents movement or access.</dcterms:description>
  </owl:Class>
  <!-- http://vcd.vicomtech.org/ontology/automotive#Bench -->
  <owl:Class rdf:about="http://vcd.vicomtech.org/ontology/automotive#Bench">
    <rdfs:label xml:lang="en">Bench</rdfs:label>
    <rdfs:subClassOf rdf:resource="http://vcd.vicomtech.org/ontology/automotive#RoadsideObject" />
    <dcterms:description xml:lang="en">A place to sit down.</dcterms:description>
  </owl:Class>
  <!-- http://vcd.vicomtech.org/ontology/automotive#Bendy -->
  <owl:Class rdf:about="http://vcd.vicomtech.org/ontology/automotive#Bendy">
    <rdfs:label xml:lang="en">Bendy</rdfs:label>
    <rdfs:subClassOf rdf:resource="http://vcd.vicomtech.org/ontology/automotive#Bus" />
    <dcterms:description xml:lang="en">An articulated vehicle used in public transportation. It is usually a single-decker, and comprises two or more rigid sections linked by a pivoting joint (articulation) enclosed by protectuve bellows inside and outside and a cover plate on the floor.</dcterms:description>
  </owl:Class>
  <!-- http://vcd.vicomtech.org/ontology/automotive#Bicycle -->
  <owl:Class rdf:about="http://vcd.vicomtech.org/ontology/automotive#Bicycle">
    <rdfs:label xml:lang="en">Bicycle</rdfs:label>
    <rdfs:subClassOf rdf:resource="http://vcd.vicomtech.org/ontology/automotive#Cycle" />
    <dcterms:description xml:lang="en">A vehicle consisting of two wheels held in a frame one behind the other, propelled by pedals and steered with handlebars attached to the front wheel.</dcterms:description>
  </owl:Class>
  <!-- http://vcd.vicomtech.org/ontology/automotive#BikeLane -->
  <owl:Class rdf:about="http://vcd.vicomtech.org/ontology/automotive#BikeLane">
    <rdfs:label xml:lang="en">Bike lane</rdfs:label>
    <rdfs:subClassOf rdf:resource="http://vcd.vicomtech.org/ontology/automotive#Flat" />
    <dcterms:description xml:lang="en">Paved areas intended for bicycle use only. Contains only regions or ground specifically designated for cyclists where pedestrians and cars should not enter.</dcterms:description>
  </owl:Class>
  <!-- http://vcd.vicomtech.org/ontology/automotive#BikeRack -->
  <owl:Class rdf:about="http://vcd.vicomtech.org/ontology/automotive#BikeRack">
    <rdfs:label xml:lang="en">Bike rack</rdfs:label>
    <rdfs:subClassOf rdf:resource="http://vcd.vicomtech.org/ontology/automotive#RoadsideObject" />
    <dcterms:description xml:lang="en">A construction to place and lock a bike.</dcterms:description>
  </owl:Class>
  <!-- http://vcd.vicomtech.org/ontology/automotive#Billboard -->
  <owl:Class rdf:about="http://vcd.vicomtech.org/ontology/automotive#Billboard">
    <rdfs:label xml:lang="en">Billboard</rdfs:label>
    <rdfs:subClassOf rdf:resource="http://vcd.vicomtech.org/ontology/automotive#Signs" />
    <dcterms:description xml:lang="en">Advertisements placed in public space and also those mounted on buildings.</dcterms:description>
  </owl:Class>
  <!-- http://vcd.vicomtech.org/ontology/automotive#Bird -->
  <owl:Class rdf:about="http://vcd.vicomtech.org/ontology/automotive#Bird">
    <rdfs:label xml:lang="en">Bird</rdfs:label>
    <rdfs:subClassOf rdf:resource="http://vcd.vicomtech.org/ontology/automotive#Animal" />
    <dcterms:description xml:lang="en">A creature (animal) with feathers and wings, usually able to fly. Includes birds on the ground.</dcterms:description>
  </owl:Class>
  <!-- http://vcd.vicomtech.org/ontology/automotive#BlurredArea -->
  <owl:Class rdf:about="http://vcd.vicomtech.org/ontology/automotive#BlurredArea">
    <rdfs:label xml:lang="en">Blurred area</rdfs:label>
    <rdfs:subClassOf rdf:resource="http://vcd.vicomtech.org/ontology/automotive#Void" />
    <dcterms:description xml:lang="en">An indistinct area.</dcterms:description>
  </owl:Class>
  <!-- http://vcd.vicomtech.org/ontology/automotive#Boat -->
  <owl:Class rdf:about="http://vcd.vicomtech.org/ontology/automotive#Boat">
    <rdfs:label xml:lang="en">Boat</rdfs:label>
    <rdfs:subClassOf rdf:resource="http://vcd.vicomtech.org/ontology/automotive#WaterVehicle" />
    <dcterms:description xml:lang="en">Vehicle suitable for riding/sailing on water. Propelled by oars, sails or an engine.</dcterms:description>
  </owl:Class>
  <!-- http://vcd.vicomtech.org/ontology/automotive#Bridge -->
  <owl:Class rdf:about="http://vcd.vicomtech.org/ontology/automotive#Bridge">
    <rdfs:label xml:lang="en">Bridge</rdfs:label>
    <rdfs:subClassOf rdf:resource="http://vcd.vicomtech.org/ontology/automotive#Structure" />
    <dcterms:description xml:lang="en">A structure carrying a road, path, railway, etc. across a river, road, or other obstacle.</dcterms:description>
  </owl:Class>
  <!-- http://vcd.vicomtech.org/ontology/automotive#BrokenStop -->
  <owl:Class rdf:about="http://vcd.vicomtech.org/ontology/automotive#BrokenStop">
    <rdfs:label xml:lang="en">Broken stop</rdfs:label>
    <rdfs:subClassOf rdf:resource="http://vcd.vicomtech.org/ontology/automotive#WhiteLines" />
  </owl:Class>
  <!-- http://vcd.vicomtech.org/ontology/automotive#Building -->
  <owl:Class rdf:about="http://vcd.vicomtech.org/ontology/automotive#Building">
    <rdfs:label xml:lang="en">Building</rdfs:label>
    <rdfs:subClassOf rdf:resource="http://vcd.vicomtech.org/ontology/automotive#Structure" />
    <dcterms:description xml:lang="en">A structure with a roof and walls, such as a house or factory.</dcterms:description>
  </owl:Class>
  <!-- http://vcd.vicomtech.org/ontology/automotive#Bump -->
  <owl:Class rdf:about="http://vcd.vicomtech.org/ontology/automotive#Bump">
    <rdfs:label xml:lang="en">Bump</rdfs:label>
    <rdfs:subClassOf rdf:resource="http://vcd.vicomtech.org/ontology/automotive#Marking" />
    <dcterms:description xml:lang="en">A marking indicating speed reduction.</dcterms:description>
  </owl:Class>
  <!-- http://vcd.vicomtech.org/ontology/automotive#Bus -->
  <owl:Class rdf:about="http://vcd.vicomtech.org/ontology/automotive#Bus">
    <rdfs:label xml:lang="en">Bus</rdfs:label>
    <rdfs:subClassOf rdf:resource="http://vcd.vicomtech.org/ontology/automotive#RoadVehicle" />
    <dcterms:description xml:lang="en">A large motor vehicle, having a long body, equipped with seats or benches for passengers, usually operating as part of a scheduled service; omnibus.</dcterms:description>
  </owl:Class>
  <!-- http://vcd.vicomtech.org/ontology/automotive#Capacity -->
  <owl:Class rdf:about="http://vcd.vicomtech.org/ontology/automotive#Capacity">
    <rdfs:label xml:lang="en">Capacity</rdfs:label>
    <rdfs:subClassOf rdf:resource="http://vcd.vicomtech.org/ontology/automotive#Attribute" />
    <dcterms:description xml:lang="en">The maximum amount of people the vehicle can transport. Depends on the number of seats.</dcterms:description>
  </owl:Class>
  <!-- http://vcd.vicomtech.org/ontology/automotive#Car -->
  <owl:Class rdf:about="http://vcd.vicomtech.org/ontology/automotive#Car">
    <rdfs:label xml:lang="en">Car</rdfs:label>
    <rdfs:subClassOf rdf:resource="http://vcd.vicomtech.org/ontology/automotive#RoadVehicle" />
    <dcterms:description xml:lang="en">A road vehicle with an engine, four wheels, and seats for a small number of people.</dcterms:description>
  </owl:Class>
  <!-- http://vcd.vicomtech.org/ontology/automotive#CarMount -->
  <owl:Class rdf:about="http://vcd.vicomtech.org/ontology/automotive#CarMount">
    <rdfs:label xml:lang="en">Car mount</rdfs:label>
    <rdfs:subClassOf rdf:resource="http://vcd.vicomtech.org/ontology/automotive#Void" />
    <dcterms:description xml:lang="en">Mount used to hold the camera while capturing.</dcterms:description>
  </owl:Class>
  <!-- http://vcd.vicomtech.org/ontology/automotive#Caravan -->
  <owl:Class rdf:about="http://vcd.vicomtech.org/ontology/automotive#Caravan">
    <rdfs:label xml:lang="en">Caravan</rdfs:label>
    <rdfs:subClassOf rdf:resource="http://vcd.vicomtech.org/ontology/automotive#RoadVehicle" />
    <dcterms:description xml:lang="en">A road vehicle equipped for living in, typically towed by a car and used for holidays.</dcterms:description>
  </owl:Class>
  <!-- http://vcd.vicomtech.org/ontology/automotive#CarryingObject -->
  <owl:Class rdf:about="http://vcd.vicomtech.org/ontology/automotive#CarryingObject">
    <rdfs:label xml:lang="en">Carrying object</rdfs:label>
    <rdfs:subClassOf rdf:resource="http://vcd.vicomtech.org/ontology/automotive#Attribute" />
    <dcterms:description xml:lang="en">Any object carried by a human.</dcterms:description>
  </owl:Class>
  <!-- http://vcd.vicomtech.org/ontology/automotive#CatchBasin -->
  <owl:Class rdf:about="http://vcd.vicomtech.org/ontology/automotive#CatchBasin">
    <rdfs:label xml:lang="en">Catch basin</rdfs:label>
    <rdfs:subClassOf rdf:resource="http://vcd.vicomtech.org/ontology/automotive#RoadsideObject" />
    <dcterms:description xml:lang="en">Sewage water draigane, typically with a grid on top or inlet of a curb.</dcterms:description>
  </owl:Class>
  <!-- http://vcd.vicomtech.org/ontology/automotive#CctvCamera -->
  <owl:Class rdf:about="http://vcd.vicomtech.org/ontology/automotive#CctvCamera">
    <rdfs:label xml:lang="en">CCTV camera</rdfs:label>
    <rdfs:subClassOf rdf:resource="http://vcd.vicomtech.org/ontology/automotive#RoadsideObject" />
    <dcterms:description xml:lang="en">Surveillance camera mounted in public space.</dcterms:description>
  </owl:Class>
  <!-- http://vcd.vicomtech.org/ontology/automotive#Child -->
  <owl:Class rdf:about="http://vcd.vicomtech.org/ontology/automotive#Child">
    <rdfs:label xml:lang="en">Child</rdfs:label>
    <rdfs:subClassOf rdf:resource="http://vcd.vicomtech.org/ontology/automotive#Pedestrian" />
    <dcterms:description xml:lang="en">A young human being below the age of puberty or below the legal age of majority.</dcterms:description>
  </owl:Class>
  <!-- http://vcd.vicomtech.org/ontology/automotive#City -->
  <owl:Class rdf:about="http://vcd.vicomtech.org/ontology/automotive#City">
    <rdfs:label xml:lang="en">City</rdfs:label>
    <rdfs:subClassOf rdf:resource="http://vcd.vicomtech.org/ontology/automotive#Static" />
    <dcterms:description xml:lang="en">A large town.</dcterms:description>
  </owl:Class>
  <!-- http://vcd.vicomtech.org/ontology/automotive#Clothes -->
  <owl:Class rdf:about="http://vcd.vicomtech.org/ontology/automotive#Clothes">
    <rdfs:label xml:lang="en">Clothes</rdfs:label>
    <rdfs:subClassOf rdf:resource="http://vcd.vicomtech.org/ontology/automotive#Attribute" />
    <dcterms:description xml:lang="en">Items worn to cover the human body.</dcterms:description>
  </owl:Class>
  <!-- http://vcd.vicomtech.org/ontology/automotive#Cloudy -->
  <owl:Class rdf:about="http://vcd.vicomtech.org/ontology/automotive#Cloudy">
    <rdfs:label xml:lang="en">Cloudy</rdfs:label>
    <rdfs:subClassOf rdf:resource="http://vcd.vicomtech.org/ontology/automotive#Weather" />
    <dcterms:description xml:lang="en">Full of or overcast by clouds.</dcterms:description>
  </owl:Class>
  <!-- http://vcd.vicomtech.org/ontology/automotive#Color -->
  <owl:Class rdf:about="http://vcd.vicomtech.org/ontology/automotive#Color">
    <rdfs:label xml:lang="en">Color</rdfs:label>
    <rdfs:subClassOf rdf:resource="http://vcd.vicomtech.org/ontology/automotive#Attribute" />
  </owl:Class>
  <!-- http://vcd.vicomtech.org/ontology/automotive#Connectivity -->
  <owl:Class rdf:about="http://vcd.vicomtech.org/ontology/automotive#Connectivity">
    <rdfs:label xml:lang="en">Connectivity</rdfs:label>
    <rdfs:subClassOf rdf:resource="http://vcd.vicomtech.org/ontology/automotive#Attribute" />
    <dcterms:description xml:lang="en">The ability to link to and communicate with other computer systems, electronic devices, software, or Internet via USB, Bluetooth or Wi-Fi.</dcterms:description>
  </owl:Class>
  <!-- http://vcd.vicomtech.org/ontology/automotive#Construction -->
  <owl:Class rdf:about="http://vcd.vicomtech.org/ontology/automotive#Construction">
    <rdfs:label xml:lang="en">Construction</rdfs:label>
    <rdfs:subClassOf rdf:resource="http://vcd.vicomtech.org/ontology/automotive#Static" />
    <dcterms:description xml:lang="en">A building or other structure.</dcterms:description>
  </owl:Class>
  <!-- http://vcd.vicomtech.org/ontology/automotive#ConstructionVehicle -->
  <owl:Class rdf:about="http://vcd.vicomtech.org/ontology/automotive#ConstructionVehicle">
    <rdfs:label xml:lang="en">Construction vehicle</rdfs:label>
    <rdfs:subClassOf rdf:resource="http://vcd.vicomtech.org/ontology/automotive#RoadVehicle" />
    <dcterms:description xml:lang="en">Refers to heavy-duty vehicles, specially designed for executing construction tasks.</dcterms:description>
  </owl:Class>
  <!-- http://vcd.vicomtech.org/ontology/automotive#ConstructionWorker -->
  <owl:Class rdf:about="http://vcd.vicomtech.org/ontology/automotive#ConstructionWorker">
    <rdfs:label xml:lang="en">Construction worker</rdfs:label>
    <rdfs:subClassOf rdf:resource="http://vcd.vicomtech.org/ontology/automotive#Adult" />
    <dcterms:description xml:lang="en">A person (Human) who works in the construction industry.</dcterms:description>
  </owl:Class>
  <!-- http://vcd.vicomtech.org/ontology/automotive#Crossing -->
  <owl:Class rdf:about="http://vcd.vicomtech.org/ontology/automotive#Crossing">
    <rdfs:label xml:lang="en">Crossing</rdfs:label>
    <rdfs:subClassOf rdf:resource="http://vcd.vicomtech.org/ontology/automotive#MovingManeuver" />
    <dcterms:description xml:lang="en">The action of crossing either a juntion or a crosswalk.</dcterms:description>
  </owl:Class>
  <!-- http://vcd.vicomtech.org/ontology/automotive#Crosswalk -->
  <owl:Class rdf:about="http://vcd.vicomtech.org/ontology/automotive#Crosswalk">
    <rdfs:label xml:lang="en">Crosswalk</rdfs:label>
    <rdfs:subClassOf rdf:resource="http://vcd.vicomtech.org/ontology/automotive#Marking" />
    <dcterms:description xml:lang="en">A marked part of a road where pedestrians have right of way to cross; a pedestrian crossing.</dcterms:description>
  </owl:Class>
  <!-- http://vcd.vicomtech.org/ontology/automotive#CrosswalkPlain -->
  <owl:Class rdf:about="http://vcd.vicomtech.org/ontology/automotive#CrosswalkPlain">
    <rdfs:label xml:lang="en">Crosswalk plain</rdfs:label>
    <rdfs:subClassOf rdf:resource="http://vcd.vicomtech.org/ontology/automotive#Crosswalk" />
    <dcterms:description xml:lang="en">Region of a road which is meant to cross the street but not marked with a zebra pattern, instead two parallel lines indicate the crosswalk. The road surface is marked as plain crosswalk, the two lines indicating the border are marked as general markings.</dcterms:description>
  </owl:Class>
  <!-- http://vcd.vicomtech.org/ontology/automotive#CrosswalkZebra -->
  <owl:Class rdf:about="http://vcd.vicomtech.org/ontology/automotive#CrosswalkZebra">
    <rdfs:label xml:lang="en">Crosswalk zebra</rdfs:label>
    <rdfs:subClassOf rdf:resource="http://vcd.vicomtech.org/ontology/automotive#Crosswalk" />
    <dcterms:description xml:lang="en">Crosswalk indicated by a zebra pattern.</dcterms:description>
  </owl:Class>
  <!-- http://vcd.vicomtech.org/ontology/automotive#Curb -->
  <owl:Class rdf:about="http://vcd.vicomtech.org/ontology/automotive#Curb">
    <rdfs:label xml:lang="en">Curb</rdfs:label>
    <rdfs:subClassOf rdf:resource="http://vcd.vicomtech.org/ontology/automotive#Barrier" />
    <dcterms:description xml:lang="en">Is the edge where a raised sidewalk or road median/central reservation meets a street or other roadway.</dcterms:description>
  </owl:Class>
  <!-- http://vcd.vicomtech.org/ontology/automotive#CurbCut -->
  <owl:Class rdf:about="http://vcd.vicomtech.org/ontology/automotive#CurbCut">
    <rdfs:label xml:lang="en">Curb cut</rdfs:label>
    <rdfs:subClassOf rdf:resource="http://vcd.vicomtech.org/ontology/automotive#Flat" />
    <dcterms:description xml:lang="en">Lowered curbs or curb cuts which can be driven over.</dcterms:description>
  </owl:Class>
  <!-- http://vcd.vicomtech.org/ontology/automotive#Curbstone -->
  <owl:Class rdf:about="http://vcd.vicomtech.org/ontology/automotive#Curbstone">
    <rdfs:label xml:lang="en">Curbstone</rdfs:label>
    <rdfs:subClassOf rdf:resource="http://vcd.vicomtech.org/ontology/automotive#RoadsideObject" />
    <dcterms:description xml:lang="en">A long, narrow stone or concrete block, laid end to end with others to form a kerb.  variant spelling of kerbstone.</dcterms:description>
  </owl:Class>
  <!-- http://vcd.vicomtech.org/ontology/automotive#CyberSecurity -->
  <owl:Class rdf:about="http://vcd.vicomtech.org/ontology/automotive#CyberSecurity">
    <rdfs:label xml:lang="en">Cyber security</rdfs:label>
    <rdfs:subClassOf rdf:resource="http://vcd.vicomtech.org/ontology/automotive#Security" />
    <dcterms:description xml:lang="en">Cybersecurity, within the context of road vehicles, is the protection of automotive electronic systems, communication networks, control algorithms, software, users, and underlying data from malicious attacks, damage, unauthorized access, or manipulation.</dcterms:description>
  </owl:Class>
  <!-- http://vcd.vicomtech.org/ontology/automotive#Cycle -->
  <owl:Class rdf:about="http://vcd.vicomtech.org/ontology/automotive#Cycle">
    <rdfs:label xml:lang="en">Cycle</rdfs:label>
    <rdfs:subClassOf rdf:resource="http://vcd.vicomtech.org/ontology/automotive#RoadVehicle" />
    <dcterms:description xml:lang="en">Comprises two-wheeled vehicles.</dcterms:description>
  </owl:Class>
  <!-- http://vcd.vicomtech.org/ontology/automotive#Cyclist -->
  <owl:Class rdf:about="http://vcd.vicomtech.org/ontology/automotive#Cyclist">
    <rdfs:label rdf:datatype="http://www.w3.org/2001/XMLSchema#string">Cyclist</rdfs:label>
    <rdfs:subClassOf rdf:resource="http://vcd.vicomtech.org/ontology/automotive#Rider" />
    <dcterms:description xml:lang="en">A person who rides a bicycle. Dows not include the bicycle or persons moving a bike while walking.</dcterms:description>
  </owl:Class>
  <!-- http://vcd.vicomtech.org/ontology/automotive#Debris -->
  <owl:Class rdf:about="http://vcd.vicomtech.org/ontology/automotive#Debris">
    <rdfs:label xml:lang="en">Debris</rdfs:label>
    <rdfs:subClassOf rdf:resource="http://vcd.vicomtech.org/ontology/automotive#MovableObject" />
    <dcterms:description xml:lang="en">Scattered pieces of rubbish or remains. Loose natural material consisting especially of broken pieces of rock.</dcterms:description>
  </owl:Class>
  <!-- http://vcd.vicomtech.org/ontology/automotive#Doors -->
  <owl:Class rdf:about="http://vcd.vicomtech.org/ontology/automotive#Doors">
    <rdfs:label xml:lang="en">Doors</rdfs:label>
    <rdfs:subClassOf rdf:resource="http://vcd.vicomtech.org/ontology/automotive#Attribute" />
    <dcterms:description xml:lang="en">Refers to the number of doors of the vehicle including the boot.</dcterms:description>
  </owl:Class>
  <!-- http://vcd.vicomtech.org/ontology/automotive#DoubleBrokenWhite -->
  <owl:Class rdf:about="http://vcd.vicomtech.org/ontology/automotive#DoubleBrokenWhite">
    <rdfs:label xml:lang="en">Double broken white</rdfs:label>
    <rdfs:subClassOf rdf:resource="http://vcd.vicomtech.org/ontology/automotive#WhiteLines" />
    <dcterms:description xml:lang="en">A double row of thicker short broken lines can be seen on a major road indicating that you need to give way they can also be used at mini-roundabouts.</dcterms:description>
  </owl:Class>
  <!-- http://vcd.vicomtech.org/ontology/automotive#DoubleBrokenYellow -->
  <owl:Class rdf:about="http://vcd.vicomtech.org/ontology/automotive#DoubleBrokenYellow">
    <rdfs:label xml:lang="en">Double broken yellow</rdfs:label>
    <rdfs:subClassOf rdf:resource="http://vcd.vicomtech.org/ontology/automotive#YellowLines" />
    <dcterms:description xml:lang="en">A double row of thicker short broken lines can be seen on a major road indicating that you need to give way they can also be used at mini-roundabouts.</dcterms:description>
  </owl:Class>
  <!-- http://vcd.vicomtech.org/ontology/automotive#DoubleSolidWhite -->
  <owl:Class rdf:about="http://vcd.vicomtech.org/ontology/automotive#DoubleSolidWhite">
    <rdfs:label xml:lang="en">Double solid white</rdfs:label>
    <rdfs:subClassOf rdf:resource="http://vcd.vicomtech.org/ontology/automotive#WhiteLines" />
    <dcterms:description xml:lang="en">Two solid lines that indicate a lane barrier between a regular use and a preferential use lane, such as a carpool/HOV. Never change lanes while in these lanes.</dcterms:description>
  </owl:Class>
  <!-- http://vcd.vicomtech.org/ontology/automotive#DoubleSolidYellow -->
  <owl:Class rdf:about="http://vcd.vicomtech.org/ontology/automotive#DoubleSolidYellow">
    <rdfs:label xml:lang="en">Double solid yellow</rdfs:label>
    <rdfs:subClassOf rdf:resource="http://vcd.vicomtech.org/ontology/automotive#YellowLines" />
    <dcterms:description xml:lang="en">Two solid lines that indicate a lane barrier between a regular use and a preferential use lane, such as a carpool/HOV. Never change lanes while in these lanes.</dcterms:description>
  </owl:Class>
  <!-- http://vcd.vicomtech.org/ontology/automotive#DrivableCobblestone -->
  <owl:Class rdf:about="http://vcd.vicomtech.org/ontology/automotive#DrivableCobblestone">
    <rdfs:label xml:lang="en">Drivable cobblestone</rdfs:label>
    <rdfs:subClassOf rdf:resource="http://vcd.vicomtech.org/ontology/automotive#RoadType" />
    <dcterms:description xml:lang="en">A road with a surface formed by naturally rounded stones.</dcterms:description>
  </owl:Class>
  <!-- http://vcd.vicomtech.org/ontology/automotive#Driveaway -->
  <owl:Class rdf:about="http://vcd.vicomtech.org/ontology/automotive#Driveaway">
    <rdfs:label xml:lang="en">Driveaway</rdfs:label>
    <rdfs:subClassOf rdf:resource="http://vcd.vicomtech.org/ontology/automotive#MovingManeuver" />
    <dcterms:description xml:lang="en">The action perforned when a vehicle starts moving.</dcterms:description>
  </owl:Class>
  <!-- http://vcd.vicomtech.org/ontology/automotive#DrivingStraight -->
  <owl:Class rdf:about="http://vcd.vicomtech.org/ontology/automotive#DrivingStraight">
    <rdfs:label xml:lang="en">Driving straight</rdfs:label>
    <rdfs:subClassOf rdf:resource="http://vcd.vicomtech.org/ontology/automotive#MovingManeuver" />
    <dcterms:description xml:lang="en">The action of driving following the current road path.</dcterms:description>
  </owl:Class>
  <!-- http://vcd.vicomtech.org/ontology/automotive#Drizzly -->
  <owl:Class rdf:about="http://vcd.vicomtech.org/ontology/automotive#Drizzly">
    <rdfs:label xml:lang="en">Drizzly</rdfs:label>
    <rdfs:subClassOf rdf:resource="http://vcd.vicomtech.org/ontology/automotive#Weather" />
    <dcterms:description xml:lang="en">Weather characterized or marked by very light rain.</dcterms:description>
  </owl:Class>
  <!-- http://vcd.vicomtech.org/ontology/automotive#Dustbin -->
  <owl:Class rdf:about="http://vcd.vicomtech.org/ontology/automotive#Dustbin">
    <rdfs:label xml:lang="en">Dustbin</rdfs:label>
    <rdfs:subClassOf rdf:resource="http://vcd.vicomtech.org/ontology/automotive#RoadObstacles" />
    <dcterms:description xml:lang="en">A container for household refuse, especially one kept outside.</dcterms:description>
  </owl:Class>
  <!-- http://vcd.vicomtech.org/ontology/automotive#Dynamic -->
  <owl:Class rdf:about="http://vcd.vicomtech.org/ontology/automotive#Dynamic">
    <rdfs:label xml:lang="en">Dynamic</rdfs:label>
    <rdfs:subClassOf rdf:resource="http://vcd.vicomtech.org/ontology/automotive#Object" />
    <dcterms:description xml:lang="en">Dynamic objects are characterized by the hability to perform an activity, change their state or move.</dcterms:description>
  </owl:Class>
  <!-- http://vcd.vicomtech.org/ontology/automotive#EgoVehicle -->
  <owl:Class rdf:about="http://vcd.vicomtech.org/ontology/automotive#EgoVehicle">
    <rdfs:label xml:lang="en">Ego vehicle</rdfs:label>
    <rdfs:subClassOf rdf:resource="http://vcd.vicomtech.org/ontology/automotive#RoadVehicle" />
    <dcterms:description xml:lang="en">A vehicle with sensors and other detection systems. The vehicle under test.</dcterms:description>
  </owl:Class>
  <!-- http://vcd.vicomtech.org/ontology/automotive#ElectronicTraffic -->
  <owl:Class rdf:about="http://vcd.vicomtech.org/ontology/automotive#ElectronicTraffic">
    <rdfs:label xml:lang="en">Electronic traffic</rdfs:label>
    <rdfs:subClassOf rdf:resource="http://vcd.vicomtech.org/ontology/automotive#Void" />
    <dcterms:description xml:lang="en">Traffic enhanced with electronic equipment.</dcterms:description>
  </owl:Class>
  <!-- http://vcd.vicomtech.org/ontology/automotive#EmergencyVehicle -->
  <owl:Class rdf:about="http://vcd.vicomtech.org/ontology/automotive#EmergencyVehicle">
    <rdfs:label xml:lang="en">Emergency vehicle</rdfs:label>
    <rdfs:subClassOf rdf:resource="http://vcd.vicomtech.org/ontology/automotive#RoadVehicle" />
    <dcterms:description xml:lang="en">Any vehicle that is designated and authorized to respond to an emergency in a life-threatening situation.</dcterms:description>
  </owl:Class>
  <!-- http://vcd.vicomtech.org/ontology/automotive#FallBehind -->
  <owl:Class rdf:about="http://vcd.vicomtech.org/ontology/automotive#FallBehind">
    <rdfs:label xml:lang="en">Fall behind</rdfs:label>
    <rdfs:subClassOf rdf:resource="http://vcd.vicomtech.org/ontology/automotive#MovingManeuver" />
    <dcterms:description xml:lang="en">The action of driving slower than its lead vehicle and is also decelerating.</dcterms:description>
  </owl:Class>
  <!-- http://vcd.vicomtech.org/ontology/automotive#Fence -->
  <owl:Class rdf:about="http://vcd.vicomtech.org/ontology/automotive#Fence">
    <rdfs:label xml:lang="en">Fence</rdfs:label>
    <rdfs:subClassOf rdf:resource="http://vcd.vicomtech.org/ontology/automotive#Barrier" />
    <dcterms:description xml:lang="en">A building for housing a motor vehicle or vehicles.</dcterms:description>
  </owl:Class>
  <!-- http://vcd.vicomtech.org/ontology/automotive#FireHydrant -->
  <owl:Class rdf:about="http://vcd.vicomtech.org/ontology/automotive#FireHydrant">
    <rdfs:label xml:lang="en">Fire hydrant</rdfs:label>
    <rdfs:subClassOf rdf:resource="http://vcd.vicomtech.org/ontology/automotive#RoadsideObject" />
    <dcterms:description xml:lang="en">Water outlet typically used by fire-fighters.</dcterms:description>
  </owl:Class>
  <!-- http://vcd.vicomtech.org/ontology/automotive#Flat -->
  <owl:Class rdf:about="http://vcd.vicomtech.org/ontology/automotive#Flat">
    <rdfs:label xml:lang="en">Flat</rdfs:label>
    <rdfs:subClassOf rdf:resource="http://vcd.vicomtech.org/ontology/automotive#Construction" />
    <dcterms:description xml:lang="en">Objects or areas without raised areas or indentations.</dcterms:description>
  </owl:Class>
  <!-- http://vcd.vicomtech.org/ontology/automotive#Foggy -->
  <owl:Class rdf:about="http://vcd.vicomtech.org/ontology/automotive#Foggy">
    <rdfs:label xml:lang="en">Foggy</rdfs:label>
    <rdfs:subClassOf rdf:resource="http://vcd.vicomtech.org/ontology/automotive#Weather" />
    <dcterms:description xml:lang="en">Thick with or having much fig; misty.</dcterms:description>
  </owl:Class>
  <!-- http://vcd.vicomtech.org/ontology/automotive#Following -->
  <owl:Class rdf:about="http://vcd.vicomtech.org/ontology/automotive#Following">
    <rdfs:label xml:lang="en">Following</rdfs:label>
    <rdfs:subClassOf rdf:resource="http://vcd.vicomtech.org/ontology/automotive#MovingManeuver" />
    <dcterms:description xml:lang="en">When the vehicle is driving with the same velocity as the vehicle in front.</dcterms:description>
  </owl:Class>
  <!-- http://vcd.vicomtech.org/ontology/automotive#Footwalk -->
  <owl:Class rdf:about="http://vcd.vicomtech.org/ontology/automotive#Footwalk">
    <rdfs:label xml:lang="en">Footwalk</rdfs:label>
    <rdfs:subClassOf rdf:resource="http://vcd.vicomtech.org/ontology/automotive#Flat" />
    <dcterms:description xml:lang="en">A surface paved or constructed for walking along often with a handrail (as on a bridge or on a parapet).</dcterms:description>
  </owl:Class>
  <!-- http://vcd.vicomtech.org/ontology/automotive#Front -->
  <owl:Class rdf:about="http://vcd.vicomtech.org/ontology/automotive#Front">
    <rdfs:label xml:lang="en">Front</rdfs:label>
    <rdfs:subClassOf rdf:resource="http://vcd.vicomtech.org/ontology/automotive#TrafficSign" />
    <dcterms:description xml:lang="en">Front side of a traffic sign.</dcterms:description>
  </owl:Class>
  <!-- http://vcd.vicomtech.org/ontology/automotive#FuelType -->
  <owl:Class rdf:about="http://vcd.vicomtech.org/ontology/automotive#FuelType">
    <rdfs:label xml:lang="en">Fuel type</rdfs:label>
    <rdfs:subClassOf rdf:resource="http://vcd.vicomtech.org/ontology/automotive#Attribute" />
    <dcterms:description xml:lang="en">Refers to how the vehicle is propelled.</dcterms:description>
  </owl:Class>
  <!-- http://vcd.vicomtech.org/ontology/automotive#Garage -->
  <owl:Class rdf:about="http://vcd.vicomtech.org/ontology/automotive#Garage">
    <rdfs:label xml:lang="en">Garage</rdfs:label>
    <rdfs:subClassOf rdf:resource="http://vcd.vicomtech.org/ontology/automotive#Barrier" />
    <dcterms:description xml:lang="en">A building for housing a motor vehicle or vehicles.</dcterms:description>
  </owl:Class>
  <!-- http://vcd.vicomtech.org/ontology/automotive#Gender -->
  <owl:Class rdf:about="http://vcd.vicomtech.org/ontology/automotive#Gender">
    <rdfs:label xml:lang="en">Gender</rdfs:label>
    <rdfs:subClassOf rdf:resource="http://vcd.vicomtech.org/ontology/automotive#Attribute" />
    <dcterms:description xml:lang="en">Either of the two sexes (male and female).</dcterms:description>
  </owl:Class>
  <!-- http://vcd.vicomtech.org/ontology/automotive#GlidingOnWheels -->
  <owl:Class rdf:about="http://vcd.vicomtech.org/ontology/automotive#GlidingOnWheels">
    <rdfs:label xml:lang="en">Gliding on wheels</rdfs:label>
    <rdfs:subClassOf rdf:resource="http://vcd.vicomtech.org/ontology/automotive#MovingManeuver" />
    <dcterms:description xml:lang="en">Gliding is an energy-efficient driving mode achieved by turning off the internal combustion engine while the vehicle is still moving in order to save fuel.</dcterms:description>
  </owl:Class>
  <!-- http://vcd.vicomtech.org/ontology/automotive#GroundAnimal -->
  <owl:Class rdf:about="http://vcd.vicomtech.org/ontology/automotive#GroundAnimal">
    <rdfs:label xml:lang="en">Ground animal</rdfs:label>
    <rdfs:subClassOf rdf:resource="http://vcd.vicomtech.org/ontology/automotive#Animal" />
    <dcterms:description xml:lang="en">Animals which move on the ground.</dcterms:description>
  </owl:Class>
  <!-- http://vcd.vicomtech.org/ontology/automotive#GuardRail -->
  <owl:Class rdf:about="http://vcd.vicomtech.org/ontology/automotive#GuardRail">
    <rdfs:label xml:lang="en">Guard rail</rdfs:label>
    <rdfs:subClassOf rdf:resource="http://vcd.vicomtech.org/ontology/automotive#Barrier" />
    <dcterms:description xml:lang="en">A strong fence at the side of a road or in the middle of an expressway, intended to reduce the risk of serious accidents; a crash barrier.</dcterms:description>
  </owl:Class>
  <!-- http://vcd.vicomtech.org/ontology/automotive#Hair -->
  <owl:Class rdf:about="http://vcd.vicomtech.org/ontology/automotive#Hair">
    <rdfs:label xml:lang="en">Hair</rdfs:label>
    <rdfs:subClassOf rdf:resource="http://vcd.vicomtech.org/ontology/automotive#Attribute" />
    <dcterms:description xml:lang="en">Descriptive term used to refer to the type of hair of a person.</dcterms:description>
  </owl:Class>
  <!-- http://vcd.vicomtech.org/ontology/automotive#Halt -->
  <owl:Class rdf:about="http://vcd.vicomtech.org/ontology/automotive#Halt">
    <rdfs:label xml:lang="en">Halt</rdfs:label>
    <rdfs:subClassOf rdf:resource="http://vcd.vicomtech.org/ontology/automotive#MovingManeuver" />
    <dcterms:description xml:lang="en">The action of braking till coming to a halt.</dcterms:description>
  </owl:Class>
  <!-- http://vcd.vicomtech.org/ontology/automotive#Height -->
  <owl:Class rdf:about="http://vcd.vicomtech.org/ontology/automotive#Height">
    <rdfs:label xml:lang="en">Height</rdfs:label>
    <rdfs:subClassOf rdf:resource="http://vcd.vicomtech.org/ontology/automotive#Attribute" />
    <dcterms:description xml:lang="en">The measurement of someone or something from head to foot or from base to top.</dcterms:description>
  </owl:Class>
  <!-- http://vcd.vicomtech.org/ontology/automotive#Human -->
  <owl:Class rdf:about="http://vcd.vicomtech.org/ontology/automotive#Human">
    <rdfs:label xml:lang="en">Human</rdfs:label>
    <rdfs:subClassOf rdf:resource="http://vcd.vicomtech.org/ontology/automotive#Dynamic" />
    <dcterms:description xml:lang="en">A bipedal primate mammal (Homo sapiens). A person.</dcterms:description>
  </owl:Class>
  <!-- http://vcd.vicomtech.org/ontology/automotive#Intersection -->
  <owl:Class rdf:about="http://vcd.vicomtech.org/ontology/automotive#Intersection">
    <rdfs:label xml:lang="en">Intersection</rdfs:label>
    <rdfs:subClassOf rdf:resource="http://vcd.vicomtech.org/ontology/automotive#Flat" />
    <dcterms:description xml:lang="en">An intersection is an at-grade junction where two or more roads or streets meet or cross.</dcterms:description>
  </owl:Class>
  <!-- http://vcd.vicomtech.org/ontology/automotive#IrrelevantSign -->
  <owl:Class rdf:about="http://vcd.vicomtech.org/ontology/automotive#IrrelevantSign">
    <rdfs:label xml:lang="en">Irrelevant sign</rdfs:label>
    <rdfs:subClassOf rdf:resource="http://vcd.vicomtech.org/ontology/automotive#Signs" />
  </owl:Class>
  <!-- http://vcd.vicomtech.org/ontology/automotive#JunctionBox -->
  <owl:Class rdf:about="http://vcd.vicomtech.org/ontology/automotive#JunctionBox">
    <rdfs:label xml:lang="en">Junction-box</rdfs:label>
    <rdfs:subClassOf rdf:resource="http://vcd.vicomtech.org/ontology/automotive#RoadsideObject" />
    <dcterms:description xml:lang="en">An electrical junction box can contain junctions of electric wires and/or cables.</dcterms:description>
  </owl:Class>
  <!-- http://vcd.vicomtech.org/ontology/automotive#Lane -->
  <owl:Class rdf:about="http://vcd.vicomtech.org/ontology/automotive#Lane">
    <rdfs:label rdf:datatype="http://www.w3.org/2001/XMLSchema#string">Lane</rdfs:label>
    <rdfs:subClassOf rdf:resource="http://vcd.vicomtech.org/ontology/automotive#Flat" />
    <dcterms:description rdf:datatype="http://www.w3.org/2001/XMLSchema#string">A division of a road marked off with painted lines and intended to separate single lines of traffic according to speed or direction.</dcterms:description>
  </owl:Class>
  <!-- http://vcd.vicomtech.org/ontology/automotive#LaneChange -->
  <owl:Class rdf:about="http://vcd.vicomtech.org/ontology/automotive#LaneChange">
    <rdfs:label xml:lang="en">Lane change</rdfs:label>
    <rdfs:subClassOf rdf:resource="http://vcd.vicomtech.org/ontology/automotive#MovingManeuver" />
    <dcterms:description xml:lang="en">An action performed with the aim of moving to the concurrent lane.</dcterms:description>
  </owl:Class>
  <!-- http://vcd.vicomtech.org/ontology/automotive#LaneChangingIntoLeft -->
  <owl:Class rdf:about="http://vcd.vicomtech.org/ontology/automotive#LaneChangingIntoLeft">
    <rdfs:label xml:lang="en">Lane changing into left</rdfs:label>
    <rdfs:subClassOf rdf:resource="http://vcd.vicomtech.org/ontology/automotive#LaneChange" />
    <dcterms:description xml:lang="en">The action of moving to the left lane.</dcterms:description>
  </owl:Class>
  <!-- http://vcd.vicomtech.org/ontology/automotive#LaneChangingIntoRight -->
  <owl:Class rdf:about="http://vcd.vicomtech.org/ontology/automotive#LaneChangingIntoRight">
    <rdfs:label xml:lang="en">Lane changing into right</rdfs:label>
    <rdfs:subClassOf rdf:resource="http://vcd.vicomtech.org/ontology/automotive#LaneChange" />
    <dcterms:description xml:lang="en">The action of moving to the right lane.</dcterms:description>
  </owl:Class>
  <!-- http://vcd.vicomtech.org/ontology/automotive#LaneChangingLeft -->
  <owl:Class rdf:about="http://vcd.vicomtech.org/ontology/automotive#LaneChangingLeft">
    <rdfs:label rdf:datatype="http://www.w3.org/2001/XMLSchema#string">Lane changing left</rdfs:label>
    <rdfs:subClassOf rdf:resource="http://vcd.vicomtech.org/ontology/automotive#LaneChange" />
    <dcterms:description xml:lang="en">The action of moving to the left lane.</dcterms:description>
  </owl:Class>
  <!-- http://vcd.vicomtech.org/ontology/automotive#LaneChangingRight -->
  <owl:Class rdf:about="http://vcd.vicomtech.org/ontology/automotive#LaneChangingRight">
    <rdfs:label xml:lang="en">Lane changing right</rdfs:label>
    <rdfs:subClassOf rdf:resource="http://vcd.vicomtech.org/ontology/automotive#LaneChange" />
    <dcterms:description xml:lang="en">The action of moving to the right lane.</dcterms:description>
  </owl:Class>
  <!-- http://vcd.vicomtech.org/ontology/automotive#LaneDivider -->
  <owl:Class rdf:about="http://vcd.vicomtech.org/ontology/automotive#LaneDivider">
    <rdfs:label xml:lang="en">Lane divider</rdfs:label>
    <rdfs:subClassOf rdf:resource="http://vcd.vicomtech.org/ontology/automotive#RoadsideObject" />
    <dcterms:description xml:lang="en">A barrier placed between the lanes of a highway to divide the traffic moving in opposite directions.</dcterms:description>
  </owl:Class>
  <!-- http://vcd.vicomtech.org/ontology/automotive#LaneMarking -->
  <owl:Class rdf:about="http://vcd.vicomtech.org/ontology/automotive#LaneMarking">
    <rdfs:label xml:lang="en">Lane marking</rdfs:label>
    <rdfs:subClassOf rdf:resource="http://vcd.vicomtech.org/ontology/automotive#Marking" />
    <dcterms:description xml:lang="en">Markings delimiting the lanes along the road.</dcterms:description>
  </owl:Class>
  <!-- http://vcd.vicomtech.org/ontology/automotive#LossOfControl -->
  <owl:Class rdf:about="http://vcd.vicomtech.org/ontology/automotive#LossOfControl">
    <rdfs:label xml:lang="en">Loss of control</rdfs:label>
    <rdfs:subClassOf rdf:resource="http://vcd.vicomtech.org/ontology/automotive#MovingManeuver" />
    <dcterms:description xml:lang="en">The action of losing the control of the vehicle which usually leads to an incident.</dcterms:description>
  </owl:Class>
  <!-- http://vcd.vicomtech.org/ontology/automotive#Mailbox -->
  <owl:Class rdf:about="http://vcd.vicomtech.org/ontology/automotive#Mailbox">
    <rdfs:label xml:lang="en">Mailbox</rdfs:label>
    <rdfs:subClassOf rdf:resource="http://vcd.vicomtech.org/ontology/automotive#RoadsideObject" />
    <dcterms:description xml:lang="en">A box to put mail into.</dcterms:description>
  </owl:Class>
  <!-- http://vcd.vicomtech.org/ontology/automotive#Manhole -->
  <owl:Class rdf:about="http://vcd.vicomtech.org/ontology/automotive#Manhole">
    <rdfs:label xml:lang="en">Manhole</rdfs:label>
    <rdfs:subClassOf rdf:resource="http://vcd.vicomtech.org/ontology/automotive#RoadsideObject" />
    <dcterms:description xml:lang="en">Opening in road to access canal system. Has to be big enough to fit a person and includes squared ones.</dcterms:description>
  </owl:Class>
  <!-- http://vcd.vicomtech.org/ontology/automotive#Manufacturer -->
  <owl:Class rdf:about="http://vcd.vicomtech.org/ontology/automotive#Manufacturer">
    <rdfs:label xml:lang="en">Manufacturer</rdfs:label>
    <rdfs:subClassOf rdf:resource="http://vcd.vicomtech.org/ontology/automotive#Attribute" />
    <dcterms:description xml:lang="en">A person or company that makes goods for sale; the brand of the vehicle.</dcterms:description>
  </owl:Class>
  <!-- http://vcd.vicomtech.org/ontology/automotive#Marking -->
  <owl:Class rdf:about="http://vcd.vicomtech.org/ontology/automotive#Marking">
    <rdfs:label xml:lang="en">Marking</rdfs:label>
    <rdfs:subClassOf rdf:resource="http://vcd.vicomtech.org/ontology/automotive#Flat" />
    <dcterms:description xml:lang="en">A mark or patten of marks delimiting a concrete area of the road.</dcterms:description>
  </owl:Class>
  <!-- http://vcd.vicomtech.org/ontology/automotive#Media -->
  <owl:Class rdf:about="http://vcd.vicomtech.org/ontology/automotive#Media">
    <rdfs:label xml:lang="en">Media</rdfs:label>
    <rdfs:subClassOf rdf:resource="http://vcd.vicomtech.org/ontology/automotive#Attribute" />
    <dcterms:description xml:lang="en">Media are the communication outlets or tools used to store and deliver information or data (VD, SD, Sat Nac).</dcterms:description>
  </owl:Class>
  <!-- http://vcd.vicomtech.org/ontology/automotive#Misc -->
  <owl:Class rdf:about="http://vcd.vicomtech.org/ontology/automotive#Misc">
    <rdfs:label xml:lang="en">Misc</rdfs:label>
    <rdfs:subClassOf rdf:resource="http://vcd.vicomtech.org/ontology/automotive#RoadVehicle" />
    <dcterms:description xml:lang="en">Miscellaneous; Objects of various types or from different sources.</dcterms:description>
  </owl:Class>
  <!-- http://vcd.vicomtech.org/ontology/automotive#Misty -->
  <owl:Class rdf:about="http://vcd.vicomtech.org/ontology/automotive#Misty">
    <rdfs:label xml:lang="en">Misty</rdfs:label>
    <rdfs:subClassOf rdf:resource="http://vcd.vicomtech.org/ontology/automotive#Weather" />
    <dcterms:description xml:lang="en">Covered by a cloudlike aggregation of minute globules of water suspended in the atmosphere at or near the earth&amp;#39;s surface, reducing visibility to a lesser degree than fog.</dcterms:description>
  </owl:Class>
  <!-- http://vcd.vicomtech.org/ontology/automotive#Model -->
  <owl:Class rdf:about="http://vcd.vicomtech.org/ontology/automotive#Model">
    <rdfs:label xml:lang="en">Model</rdfs:label>
    <rdfs:subClassOf rdf:resource="http://vcd.vicomtech.org/ontology/automotive#Attribute" />
    <dcterms:description xml:lang="en">The type or design of the vehicle.</dcterms:description>
  </owl:Class>
  <!-- http://vcd.vicomtech.org/ontology/automotive#Motorcycle -->
  <owl:Class rdf:about="http://vcd.vicomtech.org/ontology/automotive#Motorcycle">
    <rdfs:label xml:lang="en">Motorcycle</rdfs:label>
    <rdfs:subClassOf rdf:resource="http://vcd.vicomtech.org/ontology/automotive#Cycle" />
    <dcterms:description xml:lang="en">A two-wheeled vehicle that is powered by a motor and has no pedals.</dcterms:description>
  </owl:Class>
  <!-- http://vcd.vicomtech.org/ontology/automotive#Motorcyclist -->
  <owl:Class rdf:about="http://vcd.vicomtech.org/ontology/automotive#Motorcyclist">
    <rdfs:label xml:lang="en">Motorcyclist</rdfs:label>
    <rdfs:subClassOf rdf:resource="http://vcd.vicomtech.org/ontology/automotive#Rider" />
    <dcterms:description xml:lang="en">A person who rides a motorcycle. Includes passengers.</dcterms:description>
  </owl:Class>
  <!-- http://vcd.vicomtech.org/ontology/automotive#Mountain -->
  <owl:Class rdf:about="http://vcd.vicomtech.org/ontology/automotive#Mountain">
    <rdfs:label xml:lang="en">Mountain</rdfs:label>
    <rdfs:subClassOf rdf:resource="http://vcd.vicomtech.org/ontology/automotive#Nature" />
    <dcterms:description xml:lang="en">Distant elevations of the ground.</dcterms:description>
  </owl:Class>
  <!-- http://vcd.vicomtech.org/ontology/automotive#MovableObject -->
  <owl:Class rdf:about="http://vcd.vicomtech.org/ontology/automotive#MovableObject">
    <rdfs:label xml:lang="en">Movable object</rdfs:label>
    <rdfs:subClassOf rdf:resource="http://vcd.vicomtech.org/ontology/automotive#Static" />
    <dcterms:description xml:lang="en">An object capable of being moved.</dcterms:description>
  </owl:Class>
  <!-- http://vcd.vicomtech.org/ontology/automotive#MovingManeuver -->
  <owl:Class rdf:about="http://vcd.vicomtech.org/ontology/automotive#MovingManeuver">
    <rdfs:label xml:lang="en">Moving maneuver</rdfs:label>
    <rdfs:subClassOf rdf:resource="http://vcd.vicomtech.org/ontology/automotive#Action" />
    <dcterms:description xml:lang="en">A maneuver performed to change the initial state of the object.</dcterms:description>
  </owl:Class>
  <!-- http://vcd.vicomtech.org/ontology/automotive#MovingStraight -->
  <owl:Class rdf:about="http://vcd.vicomtech.org/ontology/automotive#MovingStraight">
    <rdfs:label xml:lang="en">Moving straight</rdfs:label>
    <rdfs:subClassOf rdf:resource="http://vcd.vicomtech.org/ontology/automotive#MovingManeuver" />
    <dcterms:description xml:lang="en">The action of moving following the current path.</dcterms:description>
  </owl:Class>
  <!-- http://vcd.vicomtech.org/ontology/automotive#Nationality -->
  <owl:Class rdf:about="http://vcd.vicomtech.org/ontology/automotive#Nationality">
    <rdfs:label xml:lang="en">Nationality</rdfs:label>
    <rdfs:subClassOf rdf:resource="http://vcd.vicomtech.org/ontology/automotive#Attribute" />
    <dcterms:description xml:lang="en">The status of belonging to a particular nation.</dcterms:description>
  </owl:Class>
  <!-- http://vcd.vicomtech.org/ontology/automotive#Nature -->
  <owl:Class rdf:about="http://vcd.vicomtech.org/ontology/automotive#Nature">
    <rdfs:label xml:lang="en">Nature</rdfs:label>
    <rdfs:subClassOf rdf:resource="http://vcd.vicomtech.org/ontology/automotive#Static" />
    <dcterms:description xml:lang="en">The phenomena of the physical world collectively, including plants, animals, the landscape, and other features and products of the earth, as opposed to humans or human creations.</dcterms:description>
  </owl:Class>
  <!-- http://vcd.vicomtech.org/ontology/automotive#NonDrivableStreet -->
  <owl:Class rdf:about="http://vcd.vicomtech.org/ontology/automotive#NonDrivableStreet">
    <rdfs:label xml:lang="en">Non drivable street</rdfs:label>
    <rdfs:subClassOf rdf:resource="http://vcd.vicomtech.org/ontology/automotive#RoadType" />
    <dcterms:description xml:lang="en">A road where is not allowed to drive any king of vehicle.</dcterms:description>
  </owl:Class>
  <!-- http://vcd.vicomtech.org/ontology/automotive#NormalStreet -->
  <owl:Class rdf:about="http://vcd.vicomtech.org/ontology/automotive#NormalStreet">
    <rdfs:label xml:lang="en">Normal street</rdfs:label>
    <rdfs:subClassOf rdf:resource="http://vcd.vicomtech.org/ontology/automotive#RoadType" />
    <dcterms:description xml:lang="en">Street with no restriction.</dcterms:description>
  </owl:Class>
  <!-- http://vcd.vicomtech.org/ontology/automotive#Object -->
  <owl:Class rdf:about="http://vcd.vicomtech.org/ontology/automotive#Object">
    <rdfs:label xml:lang="en">Object</rdfs:label>
    <rdfs:subClassOf rdf:resource="http://www.w3.org/2002/07/owl#Thing" />
    <dcterms:description xml:lang="en">An object is any material thing that can be seen and touched.</dcterms:description>
  </owl:Class>
  <!-- http://vcd.vicomtech.org/ontology/automotive#OldMarkingWhite -->
  <owl:Class rdf:about="http://vcd.vicomtech.org/ontology/automotive#OldMarkingWhite">
    <rdfs:label xml:lang="en">Old marking white</rdfs:label>
    <rdfs:subClassOf rdf:resource="http://vcd.vicomtech.org/ontology/automotive#WhiteLines" />
    <dcterms:description xml:lang="en">An old marking that is still visible.</dcterms:description>
  </owl:Class>
  <!-- http://vcd.vicomtech.org/ontology/automotive#OldMarkingYellow -->
  <owl:Class rdf:about="http://vcd.vicomtech.org/ontology/automotive#OldMarkingYellow">
    <rdfs:label xml:lang="en">Old marking yellow</rdfs:label>
    <rdfs:subClassOf rdf:resource="http://vcd.vicomtech.org/ontology/automotive#YellowLines" />
    <dcterms:description xml:lang="en">An old marking that is still visible.</dcterms:description>
  </owl:Class>
  <!-- http://vcd.vicomtech.org/ontology/automotive#OtherBarrier -->
  <owl:Class rdf:about="http://vcd.vicomtech.org/ontology/automotive#OtherBarrier">
    <rdfs:label xml:lang="en">Other barrier</rdfs:label>
    <rdfs:subClassOf rdf:resource="http://vcd.vicomtech.org/ontology/automotive#Barrier" />
  </owl:Class>
  <!-- http://vcd.vicomtech.org/ontology/automotive#OtherRider -->
  <owl:Class rdf:about="http://vcd.vicomtech.org/ontology/automotive#OtherRider">
    <rdfs:label xml:lang="en">Other rider</rdfs:label>
    <rdfs:subClassOf rdf:resource="http://vcd.vicomtech.org/ontology/automotive#Rider" />
    <dcterms:description xml:lang="en">A person who rides a vehicle other than a motorcycle or a bicycle. For examples, vehicles like ricksaw, wheeled char, scooter, mobility-scooter, etc.</dcterms:description>
  </owl:Class>
  <!-- http://vcd.vicomtech.org/ontology/automotive#Overpass -->
  <owl:Class rdf:about="http://vcd.vicomtech.org/ontology/automotive#Overpass">
    <rdfs:label xml:lang="en">Overpass</rdfs:label>
    <rdfs:subClassOf rdf:resource="http://vcd.vicomtech.org/ontology/automotive#Barrier" />
    <dcterms:description xml:lang="en">A crossing of two highways or of a highway and pedestrian path or railroad at different levels where clearance to traffic on the lower level is obtained by elevating the higher level also : the upper level of such a crossing.</dcterms:description>
  </owl:Class>
  <!-- http://vcd.vicomtech.org/ontology/automotive#Parked -->
  <owl:Class rdf:about="http://vcd.vicomtech.org/ontology/automotive#Parked">
    <rdfs:label xml:lang="en">Parked</rdfs:label>
    <rdfs:subClassOf rdf:resource="http://vcd.vicomtech.org/ontology/automotive#StationaryManeuver" />
    <dcterms:description xml:lang="en">The action of being stopped an leaving the vehicle temporarily in that spot.</dcterms:description>
  </owl:Class>
  <!-- http://vcd.vicomtech.org/ontology/automotive#ParkedIn -->
  <owl:Class rdf:about="http://vcd.vicomtech.org/ontology/automotive#ParkedIn">
    <rdfs:label xml:lang="en">Parked in</rdfs:label>
    <rdfs:subClassOf rdf:resource="http://vcd.vicomtech.org/ontology/automotive#StationaryManeuver" />
    <dcterms:description xml:lang="en">The action of being stopped an leaving the vehicle temporarily in that spot.</dcterms:description>
  </owl:Class>
  <!-- http://vcd.vicomtech.org/ontology/automotive#Parking -->
  <owl:Class rdf:about="http://vcd.vicomtech.org/ontology/automotive#Parking">
    <rdfs:label xml:lang="en">Parking</rdfs:label>
    <rdfs:subClassOf rdf:resource="http://vcd.vicomtech.org/ontology/automotive#MovingManeuver" />
  </owl:Class>
  <!-- http://vcd.vicomtech.org/ontology/automotive#ParkingLot -->
  <owl:Class rdf:about="http://vcd.vicomtech.org/ontology/automotive#ParkingLot">
    <rdfs:label xml:lang="en">Parking lot</rdfs:label>
    <rdfs:subClassOf rdf:resource="http://vcd.vicomtech.org/ontology/automotive#Flat" />
    <dcterms:description xml:lang="en">A building, or an area under a building, where cars can be parked.</dcterms:description>
  </owl:Class>
  <!-- http://vcd.vicomtech.org/ontology/automotive#ParkingSign -->
  <owl:Class rdf:about="http://vcd.vicomtech.org/ontology/automotive#ParkingSign">
    <rdfs:label xml:lang="en">Parking sign</rdfs:label>
    <rdfs:subClassOf rdf:resource="http://vcd.vicomtech.org/ontology/automotive#Signs" />
    <dcterms:description xml:lang="en">A sign that gives information about a parking space.</dcterms:description>
  </owl:Class>
  <!-- http://vcd.vicomtech.org/ontology/automotive#Passing -->
  <owl:Class rdf:about="http://vcd.vicomtech.org/ontology/automotive#Passing">
    <rdfs:label xml:lang="en">Passing</rdfs:label>
    <rdfs:subClassOf rdf:resource="http://vcd.vicomtech.org/ontology/automotive#MovingManeuver" />
    <dcterms:description xml:lang="en">When a vehicle is driving past another vehicle in a neighboring lane.</dcterms:description>
  </owl:Class>
  <!-- http://vcd.vicomtech.org/ontology/automotive#PassiveSafety -->
  <owl:Class rdf:about="http://vcd.vicomtech.org/ontology/automotive#PassiveSafety">
    <rdfs:label xml:lang="en">Passive safety</rdfs:label>
    <rdfs:subClassOf rdf:resource="http://vcd.vicomtech.org/ontology/automotive#Safety" />
    <dcterms:description xml:lang="en">Is used to refer to components of the vehicle (primarily airbags, seatbelts and the physical structure of the vehicle) that help to protect occupants during a crash.</dcterms:description>
  </owl:Class>
  <!-- http://vcd.vicomtech.org/ontology/automotive#Pedestrian -->
  <owl:Class rdf:about="http://vcd.vicomtech.org/ontology/automotive#Pedestrian">
    <rdfs:label xml:lang="en">Pedestrian</rdfs:label>
    <rdfs:subClassOf rdf:resource="http://vcd.vicomtech.org/ontology/automotive#Human" />
    <dcterms:description xml:lang="en">Persons moving by their own legs, sitting or in any unusual pose but not meant to drive a vehicle.</dcterms:description>
  </owl:Class>
  <!-- http://vcd.vicomtech.org/ontology/automotive#PedestrianArea -->
  <owl:Class rdf:about="http://vcd.vicomtech.org/ontology/automotive#PedestrianArea">
    <rdfs:label xml:lang="en">Pedestrian area</rdfs:label>
    <rdfs:subClassOf rdf:resource="http://vcd.vicomtech.org/ontology/automotive#Flat" />
    <dcterms:description xml:lang="en">Areas solely to be used by pedestrians. E.g. inner city areas, parks, shopping zones, etc.</dcterms:description>
  </owl:Class>
  <!-- http://vcd.vicomtech.org/ontology/automotive#PersonalMobility -->
  <owl:Class rdf:about="http://vcd.vicomtech.org/ontology/automotive#PersonalMobility">
    <rdfs:label xml:lang="en">Personal mobility</rdfs:label>
    <rdfs:subClassOf rdf:resource="http://vcd.vicomtech.org/ontology/automotive#WheeledSlow" />
  </owl:Class>
  <!-- http://vcd.vicomtech.org/ontology/automotive#PhoneBooth -->
  <owl:Class rdf:about="http://vcd.vicomtech.org/ontology/automotive#PhoneBooth">
    <rdfs:label xml:lang="en">Phone booth</rdfs:label>
    <rdfs:subClassOf rdf:resource="http://vcd.vicomtech.org/ontology/automotive#RoadsideObject" />
    <dcterms:description xml:lang="en">A public call box typically equipped with a payphone.</dcterms:description>
  </owl:Class>
  <!-- http://vcd.vicomtech.org/ontology/automotive#PhysicalSecurity -->
  <owl:Class rdf:about="http://vcd.vicomtech.org/ontology/automotive#PhysicalSecurity">
    <rdfs:label xml:lang="en">Physical security</rdfs:label>
    <rdfs:subClassOf rdf:resource="http://vcd.vicomtech.org/ontology/automotive#Security" />
    <dcterms:description xml:lang="en">Physical security describes security measures that are designed to deny unauthorized access to facilities, equipment and resources and to protect personnel and property from damage or harm (such as espionage, theft, or terrorist attacks).</dcterms:description>
  </owl:Class>
  <!-- http://vcd.vicomtech.org/ontology/automotive#Pole -->
  <owl:Class rdf:about="http://vcd.vicomtech.org/ontology/automotive#Pole">
    <rdfs:label xml:lang="en">Pole</rdfs:label>
    <rdfs:subClassOf rdf:resource="http://vcd.vicomtech.org/ontology/automotive#Support" />
    <dcterms:description xml:lang="en">Thing and elongated, typically vertically oriented poles. Includes poles holding only street lights.</dcterms:description>
  </owl:Class>
  <!-- http://vcd.vicomtech.org/ontology/automotive#Polegroup -->
  <owl:Class rdf:about="http://vcd.vicomtech.org/ontology/automotive#Polegroup">
    <rdfs:label xml:lang="en">Polegroup</rdfs:label>
    <rdfs:subClassOf rdf:resource="http://vcd.vicomtech.org/ontology/automotive#Support" />
    <dcterms:description xml:lang="en">A group of poles.</dcterms:description>
  </owl:Class>
  <!-- http://vcd.vicomtech.org/ontology/automotive#Police -->
  <owl:Class rdf:about="http://vcd.vicomtech.org/ontology/automotive#Police">
    <rdfs:label xml:lang="en">Police</rdfs:label>
    <rdfs:subClassOf rdf:resource="http://vcd.vicomtech.org/ontology/automotive#EmergencyVehicle" />
    <dcterms:description xml:lang="en">A police car is a road vehicle used by police officers for transportation during patrols and to enable them to respond to incidents and chases.</dcterms:description>
  </owl:Class>
  <!-- http://vcd.vicomtech.org/ontology/automotive#PoliceOfficer -->
  <owl:Class rdf:about="http://vcd.vicomtech.org/ontology/automotive#PoliceOfficer">
    <rdfs:label xml:lang="en">Police officer</rdfs:label>
    <rdfs:subClassOf rdf:resource="http://vcd.vicomtech.org/ontology/automotive#Adult" />
    <dcterms:description xml:lang="en">A member of a police force; policeman or policewoman.</dcterms:description>
  </owl:Class>
  <!-- http://vcd.vicomtech.org/ontology/automotive#Pothole -->
  <owl:Class rdf:about="http://vcd.vicomtech.org/ontology/automotive#Pothole">
    <rdfs:label xml:lang="en">Pothole</rdfs:label>
    <rdfs:subClassOf rdf:resource="http://vcd.vicomtech.org/ontology/automotive#RoadsideObject" />
    <dcterms:description xml:lang="en">A depression or hollow in a road caused by wear or subsidence.</dcterms:description>
  </owl:Class>
  <!-- http://vcd.vicomtech.org/ontology/automotive#PushablePullable -->
  <owl:Class rdf:about="http://vcd.vicomtech.org/ontology/automotive#PushablePullable">
    <rdfs:label xml:lang="en">Pushable/Pullable</rdfs:label>
    <rdfs:subClassOf rdf:resource="http://vcd.vicomtech.org/ontology/automotive#MovableObject" />
    <dcterms:description xml:lang="en">An object that can be pushed or pulled.</dcterms:description>
  </owl:Class>
  <!-- http://vcd.vicomtech.org/ontology/automotive#RailTrack -->
  <owl:Class rdf:about="http://vcd.vicomtech.org/ontology/automotive#RailTrack">
    <rdfs:label xml:lang="en">Rail track</rdfs:label>
    <rdfs:subClassOf rdf:resource="http://vcd.vicomtech.org/ontology/automotive#Flat" />
    <dcterms:description xml:lang="en">The parallel steel rails on which a train runs.</dcterms:description>
  </owl:Class>
  <!-- http://vcd.vicomtech.org/ontology/automotive#RailborneVehicle -->
  <owl:Class rdf:about="http://vcd.vicomtech.org/ontology/automotive#RailborneVehicle">
    <rdfs:label xml:lang="en">Railborne vehicle</rdfs:label>
    <rdfs:subClassOf rdf:resource="http://vcd.vicomtech.org/ontology/automotive#Vehicle" />
  </owl:Class>
  <!-- http://vcd.vicomtech.org/ontology/automotive#RainDirt -->
  <owl:Class rdf:about="http://vcd.vicomtech.org/ontology/automotive#RainDirt">
    <rdfs:label xml:lang="en">Rain dirt</rdfs:label>
    <rdfs:subClassOf rdf:resource="http://vcd.vicomtech.org/ontology/automotive#Void" />
    <dcterms:description xml:lang="en">Is a variety of rain which contains enough dust for it to be visible. Also known as rain dust.</dcterms:description>
  </owl:Class>
  <!-- http://vcd.vicomtech.org/ontology/automotive#Rainy -->
  <owl:Class rdf:about="http://vcd.vicomtech.org/ontology/automotive#Rainy">
    <rdfs:label xml:lang="en">Rainy</rdfs:label>
    <rdfs:subClassOf rdf:resource="http://vcd.vicomtech.org/ontology/automotive#Weather" />
    <dcterms:description xml:lang="en">Weather having or characterized by considerable rainfall.</dcterms:description>
  </owl:Class>
  <!-- http://vcd.vicomtech.org/ontology/automotive#RestrictedArea -->
  <owl:Class rdf:about="http://vcd.vicomtech.org/ontology/automotive#RestrictedArea">
    <rdfs:label xml:lang="en">Restricted area</rdfs:label>
    <rdfs:subClassOf rdf:resource="http://vcd.vicomtech.org/ontology/automotive#RoadType" />
    <dcterms:description xml:lang="en">An area which unauthorized people are not allowed to enter or and area with a peed limit for vehicles.</dcterms:description>
  </owl:Class>
  <!-- http://vcd.vicomtech.org/ontology/automotive#Reversing -->
  <owl:Class rdf:about="http://vcd.vicomtech.org/ontology/automotive#Reversing">
    <rdfs:label xml:lang="en">Reversing</rdfs:label>
    <rdfs:subClassOf rdf:resource="http://vcd.vicomtech.org/ontology/automotive#MovingManeuver" />
    <dcterms:description xml:lang="en">Is the process of driving a vehicle in the reverse direction in order to maneuver.</dcterms:description>
  </owl:Class>
  <!-- http://vcd.vicomtech.org/ontology/automotive#Rider -->
  <owl:Class rdf:about="http://vcd.vicomtech.org/ontology/automotive#Rider">
    <rdfs:label xml:lang="en">Rider</rdfs:label>
    <rdfs:subClassOf rdf:resource="http://vcd.vicomtech.org/ontology/automotive#Human" />
    <dcterms:description xml:lang="en">A human who is riding any type of vehicle (horse, bicycle, motorcycle, etc.).</dcterms:description>
  </owl:Class>
  <!-- http://vcd.vicomtech.org/ontology/automotive#Rigid -->
  <owl:Class rdf:about="http://vcd.vicomtech.org/ontology/automotive#Rigid">
    <rdfs:label xml:lang="en">Rigid</rdfs:label>
    <rdfs:subClassOf rdf:resource="http://vcd.vicomtech.org/ontology/automotive#Bus" />
    <dcterms:description xml:lang="en">Is a vehicle  used in public transportation services with a single, rigid chassis.</dcterms:description>
  </owl:Class>
  <!-- http://vcd.vicomtech.org/ontology/automotive#Road -->
  <owl:Class rdf:about="http://vcd.vicomtech.org/ontology/automotive#Road">
    <rdfs:label xml:lang="en">Road</rdfs:label>
    <rdfs:subClassOf rdf:resource="http://vcd.vicomtech.org/ontology/automotive#Flat" />
    <dcterms:description xml:lang="en">A wide way leading from one place to another, especially one with a specially prepared surface which vehicles can use.</dcterms:description>
  </owl:Class>
  <!-- http://vcd.vicomtech.org/ontology/automotive#RoadObstacles -->
  <owl:Class rdf:about="http://vcd.vicomtech.org/ontology/automotive#RoadObstacles">
    <rdfs:label xml:lang="en">Road obstacles</rdfs:label>
    <rdfs:subClassOf rdf:resource="http://vcd.vicomtech.org/ontology/automotive#MovableObject" />
    <dcterms:description xml:lang="en">A thing that blocks one&amp;#39;s way or prevents or hinders progress.</dcterms:description>
  </owl:Class>
  <!-- http://vcd.vicomtech.org/ontology/automotive#RoadType -->
  <owl:Class rdf:about="http://vcd.vicomtech.org/ontology/automotive#RoadType">
    <rdfs:label xml:lang="en">Road type</rdfs:label>
    <rdfs:subClassOf rdf:resource="http://vcd.vicomtech.org/ontology/automotive#Road" />
  </owl:Class>
  <!-- http://vcd.vicomtech.org/ontology/automotive#RoadVehicle -->
  <owl:Class rdf:about="http://vcd.vicomtech.org/ontology/automotive#RoadVehicle">
    <rdfs:label xml:lang="en">Road vehicle</rdfs:label>
    <rdfs:subClassOf rdf:resource="http://vcd.vicomtech.org/ontology/automotive#Vehicle" />
    <dcterms:description xml:lang="en">A vehicle designed to legally carry people or cargo on public roads and highways.</dcterms:description>
  </owl:Class>
  <!-- http://vcd.vicomtech.org/ontology/automotive#Roadblocks -->
  <owl:Class rdf:about="http://vcd.vicomtech.org/ontology/automotive#Roadblocks">
    <rdfs:label xml:lang="en">Roadblocks</rdfs:label>
    <rdfs:subClassOf rdf:resource="http://vcd.vicomtech.org/ontology/automotive#TrafficDevice" />
    <dcterms:description xml:lang="en">An obstruction in a road set up specially by law enforcement officers.</dcterms:description>
  </owl:Class>
  <!-- http://vcd.vicomtech.org/ontology/automotive#RoadsideObject -->
  <owl:Class rdf:about="http://vcd.vicomtech.org/ontology/automotive#RoadsideObject">
    <rdfs:label xml:lang="en">Roadside object</rdfs:label>
    <rdfs:subClassOf rdf:resource="http://vcd.vicomtech.org/ontology/automotive#Static" />
    <dcterms:description xml:lang="en">Fixed objects placed beside a road.</dcterms:description>
  </owl:Class>
  <!-- http://vcd.vicomtech.org/ontology/automotive#Rover -->
  <owl:Class rdf:about="http://vcd.vicomtech.org/ontology/automotive#Rover">
    <rdfs:label xml:lang="en">Rover</rdfs:label>
    <rdfs:subClassOf rdf:resource="http://vcd.vicomtech.org/ontology/automotive#RoadVehicle" />
  </owl:Class>
  <!-- http://vcd.vicomtech.org/ontology/automotive#Running -->
  <owl:Class rdf:about="http://vcd.vicomtech.org/ontology/automotive#Running">
    <rdfs:label xml:lang="en">Running</rdfs:label>
    <rdfs:subClassOf rdf:resource="http://vcd.vicomtech.org/ontology/automotive#MovingManeuver" />
    <dcterms:description xml:lang="en">The action of movement of a runner.</dcterms:description>
  </owl:Class>
  <!-- http://vcd.vicomtech.org/ontology/automotive#SafeStop -->
  <owl:Class rdf:about="http://vcd.vicomtech.org/ontology/automotive#SafeStop">
    <rdfs:label xml:lang="en">Safe stop</rdfs:label>
    <rdfs:subClassOf rdf:resource="http://vcd.vicomtech.org/ontology/automotive#MovingManeuver" />
    <dcterms:description xml:lang="en">The action of deccelerating until stopping safely. For instance, in front of a traffic light or in a traffic jam.</dcterms:description>
  </owl:Class>
  <!-- http://vcd.vicomtech.org/ontology/automotive#Safety -->
  <owl:Class rdf:about="http://vcd.vicomtech.org/ontology/automotive#Safety">
    <rdfs:label xml:lang="en">Safety</rdfs:label>
    <rdfs:subClassOf rdf:resource="http://vcd.vicomtech.org/ontology/automotive#Attribute" />
    <dcterms:description xml:lang="en">Automotive safety is the study and practice of design, construction, equipment and regulation to minimize the occurrence and consequences of traffic collisions involving motor vehicles.</dcterms:description>
  </owl:Class>
  <!-- http://vcd.vicomtech.org/ontology/automotive#Sand -->
  <owl:Class rdf:about="http://vcd.vicomtech.org/ontology/automotive#Sand">
    <rdfs:label xml:lang="en">Sand</rdfs:label>
    <rdfs:subClassOf rdf:resource="http://vcd.vicomtech.org/ontology/automotive#Nature" />
    <dcterms:description xml:lang="en">Includes surfaces consisting of sand or sand heaps, e.g. at construction areas.</dcterms:description>
  </owl:Class>
  <!-- http://vcd.vicomtech.org/ontology/automotive#Security -->
  <owl:Class rdf:about="http://vcd.vicomtech.org/ontology/automotive#Security">
    <rdfs:label xml:lang="en">Security</rdfs:label>
    <rdfs:subClassOf rdf:resource="http://vcd.vicomtech.org/ontology/automotive#Attribute" />
    <dcterms:description xml:lang="en">Automotive security refers to the branch of computer security focused on the cyber risks related to the automotive context.</dcterms:description>
  </owl:Class>
  <!-- http://vcd.vicomtech.org/ontology/automotive#ServiceLane -->
  <owl:Class rdf:about="http://vcd.vicomtech.org/ontology/automotive#ServiceLane">
    <rdfs:label xml:lang="en">Service lane</rdfs:label>
    <rdfs:subClassOf rdf:resource="http://vcd.vicomtech.org/ontology/automotive#Flat" />
    <dcterms:description xml:lang="en">Road shoulders, typically on highways, which offer enough space for a car to drive and stop in emergency cases. Usually on the right side of drivable lanes, but can also be on the left side.</dcterms:description>
  </owl:Class>
  <!-- http://vcd.vicomtech.org/ontology/automotive#Sidebars -->
  <owl:Class rdf:about="http://vcd.vicomtech.org/ontology/automotive#Sidebars">
    <rdfs:label xml:lang="en">Sidebars</rdfs:label>
    <rdfs:subClassOf rdf:resource="http://vcd.vicomtech.org/ontology/automotive#Barrier" />
    <dcterms:description xml:lang="en">An additional or less important thing.</dcterms:description>
  </owl:Class>
  <!-- http://vcd.vicomtech.org/ontology/automotive#Sidewalk -->
  <owl:Class rdf:about="http://vcd.vicomtech.org/ontology/automotive#Sidewalk">
    <rdfs:label xml:lang="en">Sidewalk</rdfs:label>
    <rdfs:subClassOf rdf:resource="http://vcd.vicomtech.org/ontology/automotive#Flat" />
    <dcterms:description xml:lang="en">Horizontal surface designated for pedestrians or cyclist. Delimited from the road by some obstacles or poles, but not only by marking. Often elevated compared to the road and often located at the side of a road. Also includes walkable parts of traffic islands, but not pedestrian areas.</dcterms:description>
  </owl:Class>
  <!-- http://vcd.vicomtech.org/ontology/automotive#Signs -->
  <owl:Class rdf:about="http://vcd.vicomtech.org/ontology/automotive#Signs">
    <rdfs:label xml:lang="en">Signs</rdfs:label>
    <rdfs:subClassOf rdf:resource="http://vcd.vicomtech.org/ontology/automotive#RoadsideObject" />
    <dcterms:description xml:lang="en">An object used to convey information or an instruction.</dcterms:description>
  </owl:Class>
  <!-- http://vcd.vicomtech.org/ontology/automotive#Sitting -->
  <owl:Class rdf:about="http://vcd.vicomtech.org/ontology/automotive#Sitting">
    <rdfs:label xml:lang="en">Sitting</rdfs:label>
    <rdfs:subClassOf rdf:resource="http://vcd.vicomtech.org/ontology/automotive#StationaryManeuver" />
    <dcterms:description xml:lang="en">The action of being resting on a seat or other type of support, with the upper part of the body vertical.</dcterms:description>
  </owl:Class>
  <!-- http://vcd.vicomtech.org/ontology/automotive#SittingOn -->
  <owl:Class rdf:about="http://vcd.vicomtech.org/ontology/automotive#SittingOn">
    <rdfs:label xml:lang="en">Sitting on</rdfs:label>
    <rdfs:subClassOf rdf:resource="http://vcd.vicomtech.org/ontology/automotive#StationaryManeuver" />
    <dcterms:description xml:lang="en">The action of being resting on a seat or other type of support, with the upper part of the body vertical.</dcterms:description>
  </owl:Class>
  <!-- http://vcd.vicomtech.org/ontology/automotive#SkinColor -->
  <owl:Class rdf:about="http://vcd.vicomtech.org/ontology/automotive#SkinColor">
    <rdfs:label xml:lang="en">Skin color</rdfs:label>
    <rdfs:subClassOf rdf:resource="http://vcd.vicomtech.org/ontology/automotive#Attribute" />
  </owl:Class>
  <!-- http://vcd.vicomtech.org/ontology/automotive#Sky -->
  <owl:Class rdf:about="http://vcd.vicomtech.org/ontology/automotive#Sky">
    <rdfs:label xml:lang="en">Sky</rdfs:label>
    <rdfs:subClassOf rdf:resource="http://vcd.vicomtech.org/ontology/automotive#Nature" />
    <dcterms:description xml:lang="en">Sky including fog or heavy precipitation.</dcterms:description>
  </owl:Class>
  <!-- http://vcd.vicomtech.org/ontology/automotive#Sleety -->
  <owl:Class rdf:about="http://vcd.vicomtech.org/ontology/automotive#Sleety">
    <rdfs:label xml:lang="en">Sleety</rdfs:label>
    <rdfs:subClassOf rdf:resource="http://vcd.vicomtech.org/ontology/automotive#Weather" />
    <dcterms:description xml:lang="en">Characterized by rain in the form of ice pellets.</dcterms:description>
  </owl:Class>
  <!-- http://vcd.vicomtech.org/ontology/automotive#SlowDriveArea -->
  <owl:Class rdf:about="http://vcd.vicomtech.org/ontology/automotive#SlowDriveArea">
    <rdfs:label xml:lang="en">Slow drive area</rdfs:label>
    <rdfs:subClassOf rdf:resource="http://vcd.vicomtech.org/ontology/automotive#RoadType" />
    <dcterms:description xml:lang="en">A road with speed limitations.</dcterms:description>
  </owl:Class>
  <!-- http://vcd.vicomtech.org/ontology/automotive#SmallVehicle -->
  <owl:Class rdf:about="http://vcd.vicomtech.org/ontology/automotive#SmallVehicle">
    <rdfs:label xml:lang="en">Small vehicle</rdfs:label>
    <rdfs:subClassOf rdf:resource="http://vcd.vicomtech.org/ontology/automotive#Void" />
    <dcterms:description xml:lang="en">The B-segment is the second smallest of the European segments for passenger cars, which is described as &amp;quot;small cars&amp;quot;.</dcterms:description>
  </owl:Class>
  <!-- http://vcd.vicomtech.org/ontology/automotive#Snow -->
  <owl:Class rdf:about="http://vcd.vicomtech.org/ontology/automotive#Snow">
    <rdfs:label xml:lang="en">Snow</rdfs:label>
    <rdfs:subClassOf rdf:resource="http://vcd.vicomtech.org/ontology/automotive#Nature" />
    <dcterms:description xml:lang="en">Snow covered surface.</dcterms:description>
  </owl:Class>
  <!-- http://vcd.vicomtech.org/ontology/automotive#Snowy -->
  <owl:Class rdf:about="http://vcd.vicomtech.org/ontology/automotive#Snowy">
    <rdfs:label xml:lang="en">Snowy</rdfs:label>
    <rdfs:subClassOf rdf:resource="http://vcd.vicomtech.org/ontology/automotive#Weather" />
    <dcterms:description xml:lang="en">Characterized by snow.</dcterms:description>
  </owl:Class>
  <!-- http://vcd.vicomtech.org/ontology/automotive#SolidBrokenWhite -->
  <owl:Class rdf:about="http://vcd.vicomtech.org/ontology/automotive#SolidBrokenWhite">
    <rdfs:label xml:lang="en">Solid broken white</rdfs:label>
    <rdfs:subClassOf rdf:resource="http://vcd.vicomtech.org/ontology/automotive#WhiteLines" />
    <dcterms:description xml:lang="en">A lane marking formed by a solid and a broken line. If the line nearest to you gets broken it means you may cross the lines to overtake if it is safe.</dcterms:description>
  </owl:Class>
  <!-- http://vcd.vicomtech.org/ontology/automotive#SolidBrokenYellow -->
  <owl:Class rdf:about="http://vcd.vicomtech.org/ontology/automotive#SolidBrokenYellow">
    <rdfs:label xml:lang="en">Solid broken yellow</rdfs:label>
    <rdfs:subClassOf rdf:resource="http://vcd.vicomtech.org/ontology/automotive#YellowLines" />
    <dcterms:description xml:lang="en">A lane marking formed by a solid and a broken line. If the line nearest to you gets broken it means you may cross the lines to overtake if it is safe.</dcterms:description>
  </owl:Class>
  <!-- http://vcd.vicomtech.org/ontology/automotive#SolidChevronWhite -->
  <owl:Class rdf:about="http://vcd.vicomtech.org/ontology/automotive#SolidChevronWhite">
    <rdfs:label xml:lang="en">Solid chevron white</rdfs:label>
    <rdfs:subClassOf rdf:resource="http://vcd.vicomtech.org/ontology/automotive#WhiteLines" />
    <dcterms:description xml:lang="en">Diagonal stripes used to separate traffic lanes or to protect traffic turning right.</dcterms:description>
  </owl:Class>
  <!-- http://vcd.vicomtech.org/ontology/automotive#SolidChevronYellow -->
  <owl:Class rdf:about="http://vcd.vicomtech.org/ontology/automotive#SolidChevronYellow">
    <rdfs:label xml:lang="en">Solid chevron yellow</rdfs:label>
    <rdfs:subClassOf rdf:resource="http://vcd.vicomtech.org/ontology/automotive#YellowLines" />
    <dcterms:description xml:lang="en">Diagonal stripes used to separate traffic lanes or to protect traffic turning right.</dcterms:description>
  </owl:Class>
  <!-- http://vcd.vicomtech.org/ontology/automotive#SolidParking -->
  <owl:Class rdf:about="http://vcd.vicomtech.org/ontology/automotive#SolidParking">
    <rdfs:label xml:lang="en">Solid parking</rdfs:label>
    <rdfs:subClassOf rdf:resource="http://vcd.vicomtech.org/ontology/automotive#WhiteLines" />
  </owl:Class>
  <!-- http://vcd.vicomtech.org/ontology/automotive#SolidWhite -->
  <owl:Class rdf:about="http://vcd.vicomtech.org/ontology/automotive#SolidWhite">
    <rdfs:label xml:lang="en">Solid white</rdfs:label>
    <rdfs:subClassOf rdf:resource="http://vcd.vicomtech.org/ontology/automotive#WhiteLines" />
    <dcterms:description xml:lang="en">Solid line dividing two lanes. Changing lanes is not allowed.</dcterms:description>
  </owl:Class>
  <!-- http://vcd.vicomtech.org/ontology/automotive#SolidYellow -->
  <owl:Class rdf:about="http://vcd.vicomtech.org/ontology/automotive#SolidYellow">
    <rdfs:label xml:lang="en">Solid yellow</rdfs:label>
    <rdfs:subClassOf rdf:resource="http://vcd.vicomtech.org/ontology/automotive#YellowLines" />
    <dcterms:description xml:lang="en">Solid line dividing two lanes. Indicates that changing lanes is not allowed.</dcterms:description>
  </owl:Class>
  <!-- http://vcd.vicomtech.org/ontology/automotive#Speed -->
  <owl:Class rdf:about="http://vcd.vicomtech.org/ontology/automotive#Speed">
    <rdfs:label xml:lang="en">Speed</rdfs:label>
    <rdfs:subClassOf rdf:resource="http://vcd.vicomtech.org/ontology/automotive#Attribute" />
    <dcterms:description xml:lang="en">Rapidity in moving, going, traveling, proceeding, or performing; swiftness; celerity.</dcterms:description>
  </owl:Class>
  <!-- http://vcd.vicomtech.org/ontology/automotive#SpeedBumper -->
  <owl:Class rdf:about="http://vcd.vicomtech.org/ontology/automotive#SpeedBumper">
    <rdfs:label xml:lang="en">Speed bumper</rdfs:label>
    <rdfs:subClassOf rdf:resource="http://vcd.vicomtech.org/ontology/automotive#RoadsideObject" />
    <dcterms:description xml:lang="en">A small raised area built across a road to force people to drive more slowly.</dcterms:description>
  </owl:Class>
  <!-- http://vcd.vicomtech.org/ontology/automotive#Standing -->
  <owl:Class rdf:about="http://vcd.vicomtech.org/ontology/automotive#Standing">
    <rdfs:label xml:lang="en">Standing</rdfs:label>
    <rdfs:subClassOf rdf:resource="http://vcd.vicomtech.org/ontology/automotive#StationaryManeuver" />
    <dcterms:description xml:lang="en">The action of being in a vertical state without moving.</dcterms:description>
  </owl:Class>
  <!-- http://vcd.vicomtech.org/ontology/automotive#StandingOn -->
  <owl:Class rdf:about="http://vcd.vicomtech.org/ontology/automotive#StandingOn">
    <rdfs:label xml:lang="en">Standing on</rdfs:label>
    <rdfs:subClassOf rdf:resource="http://vcd.vicomtech.org/ontology/automotive#StationaryManeuver" />
    <dcterms:description xml:lang="en">The action of being in a vertical state without moving on top of something.</dcterms:description>
  </owl:Class>
  <!-- http://vcd.vicomtech.org/ontology/automotive#Standstill -->
  <owl:Class rdf:about="http://vcd.vicomtech.org/ontology/automotive#Standstill">
    <rdfs:label xml:lang="en">Standstill</rdfs:label>
    <rdfs:subClassOf rdf:resource="http://vcd.vicomtech.org/ontology/automotive#StationaryManeuver" />
    <dcterms:description xml:lang="en">A situation or condition in which there is no movement or activity at all.</dcterms:description>
  </owl:Class>
  <!-- http://vcd.vicomtech.org/ontology/automotive#Static -->
  <owl:Class rdf:about="http://vcd.vicomtech.org/ontology/automotive#Static">
    <rdfs:label xml:lang="en">Static</rdfs:label>
    <rdfs:subClassOf rdf:resource="http://vcd.vicomtech.org/ontology/automotive#Object" />
    <dcterms:description xml:lang="en">Static objects are not able to move or change by themselves.</dcterms:description>
  </owl:Class>
  <!-- http://vcd.vicomtech.org/ontology/automotive#StationaryManeuver -->
  <owl:Class rdf:about="http://vcd.vicomtech.org/ontology/automotive#StationaryManeuver">
    <rdfs:label xml:lang="en">Stationary maneuver</rdfs:label>
    <rdfs:subClassOf rdf:resource="http://vcd.vicomtech.org/ontology/automotive#Action" />
    <dcterms:description xml:lang="en">A static maneuver performed with the aim of maintaining the current state or position of the object.</dcterms:description>
  </owl:Class>
  <!-- http://vcd.vicomtech.org/ontology/automotive#Stopped -->
  <owl:Class rdf:about="http://vcd.vicomtech.org/ontology/automotive#Stopped">
    <rdfs:label xml:lang="en">Stopped</rdfs:label>
    <rdfs:subClassOf rdf:resource="http://vcd.vicomtech.org/ontology/automotive#StationaryManeuver" />
    <dcterms:description xml:lang="en">The action of not moving at all. In the case of a vehicle implies having the engine turned off.</dcterms:description>
  </owl:Class>
  <!-- http://vcd.vicomtech.org/ontology/automotive#StoppedIn -->
  <owl:Class rdf:about="http://vcd.vicomtech.org/ontology/automotive#StoppedIn">
    <rdfs:label xml:lang="en">Stopped in</rdfs:label>
    <rdfs:subClassOf rdf:resource="http://vcd.vicomtech.org/ontology/automotive#StationaryManeuver" />
    <dcterms:description xml:lang="en">The action of not moving at all. In the case of a vehicle implies having the engine turned off.</dcterms:description>
  </owl:Class>
  <!-- http://vcd.vicomtech.org/ontology/automotive#Stormy -->
  <owl:Class rdf:about="http://vcd.vicomtech.org/ontology/automotive#Stormy">
    <rdfs:label xml:lang="en">Stormy</rdfs:label>
    <rdfs:subClassOf rdf:resource="http://vcd.vicomtech.org/ontology/automotive#Weather" />
    <dcterms:description xml:lang="en">Affected by storms; tempestuous.</dcterms:description>
  </owl:Class>
  <!-- http://vcd.vicomtech.org/ontology/automotive#StreetLight -->
  <owl:Class rdf:about="http://vcd.vicomtech.org/ontology/automotive#StreetLight">
    <rdfs:label xml:lang="en">Street light</rdfs:label>
    <rdfs:subClassOf rdf:resource="http://vcd.vicomtech.org/ontology/automotive#RoadsideObject" />
    <dcterms:description xml:lang="en">Lights mounted on poles to illuminate the road or public places.</dcterms:description>
  </owl:Class>
  <!-- http://vcd.vicomtech.org/ontology/automotive#Stroller -->
  <owl:Class rdf:about="http://vcd.vicomtech.org/ontology/automotive#Stroller">
    <rdfs:label xml:lang="en">Stroller</rdfs:label>
    <rdfs:subClassOf rdf:resource="http://vcd.vicomtech.org/ontology/automotive#WheeledSlow" />
    <dcterms:description xml:lang="en">A chair on wheels, typically folding, in which a baby or young child can be pushed along; a pushchair.</dcterms:description>
  </owl:Class>
  <!-- http://vcd.vicomtech.org/ontology/automotive#Structure -->
  <owl:Class rdf:about="http://vcd.vicomtech.org/ontology/automotive#Structure">
    <rdfs:label xml:lang="en">Structure</rdfs:label>
    <rdfs:subClassOf rdf:resource="http://vcd.vicomtech.org/ontology/automotive#Construction" />
    <dcterms:description xml:lang="en">A building or other object constructed from several parts.</dcterms:description>
  </owl:Class>
  <!-- http://vcd.vicomtech.org/ontology/automotive#Sunny -->
  <owl:Class rdf:about="http://vcd.vicomtech.org/ontology/automotive#Sunny">
    <rdfs:label xml:lang="en">Sunny</rdfs:label>
    <rdfs:subClassOf rdf:resource="http://vcd.vicomtech.org/ontology/automotive#Weather" />
    <dcterms:description xml:lang="en">Clear sky and exposed to sunlight.</dcterms:description>
  </owl:Class>
  <!-- http://vcd.vicomtech.org/ontology/automotive#Support -->
  <owl:Class rdf:about="http://vcd.vicomtech.org/ontology/automotive#Support">
    <rdfs:label xml:lang="en">Support</rdfs:label>
    <rdfs:subClassOf rdf:resource="http://vcd.vicomtech.org/ontology/automotive#RoadsideObject" />
    <dcterms:description xml:lang="en">A thing that bears the weight of something or keeps ir upright.</dcterms:description>
  </owl:Class>
  <!-- http://vcd.vicomtech.org/ontology/automotive#SymbolRestricted -->
  <owl:Class rdf:about="http://vcd.vicomtech.org/ontology/automotive#SymbolRestricted">
    <rdfs:label xml:lang="en">Symbol restricted</rdfs:label>
    <rdfs:subClassOf rdf:resource="http://vcd.vicomtech.org/ontology/automotive#Marking" />
  </owl:Class>
  <!-- http://vcd.vicomtech.org/ontology/automotive#Terrain -->
  <owl:Class rdf:about="http://vcd.vicomtech.org/ontology/automotive#Terrain">
    <rdfs:label xml:lang="en">Terrain</rdfs:label>
    <rdfs:subClassOf rdf:resource="http://vcd.vicomtech.org/ontology/automotive#Nature" />
    <dcterms:description xml:lang="en">Grass and all other types of horizontal spreading vegetation, includes soil.</dcterms:description>
  </owl:Class>
  <!-- http://vcd.vicomtech.org/ontology/automotive#Tractor -->
  <owl:Class rdf:about="http://vcd.vicomtech.org/ontology/automotive#Tractor">
    <rdfs:label xml:lang="en">Tractor</rdfs:label>
    <rdfs:subClassOf rdf:resource="http://vcd.vicomtech.org/ontology/automotive#UtilityVehicle" />
    <dcterms:description xml:lang="en">A powerful motor vehicle with large rear wheels, used chiefly on farms for hauling equipment and trailers.</dcterms:description>
  </owl:Class>
  <!-- http://vcd.vicomtech.org/ontology/automotive#TrafficCone -->
  <owl:Class rdf:about="http://vcd.vicomtech.org/ontology/automotive#TrafficCone">
    <rdfs:label xml:lang="en">Traffic cone</rdfs:label>
    <rdfs:subClassOf rdf:resource="http://vcd.vicomtech.org/ontology/automotive#TrafficDevice" />
    <dcterms:description xml:lang="en">A solid or hollow object which tapers from a circular or roughly circular base to a point.</dcterms:description>
  </owl:Class>
  <!-- http://vcd.vicomtech.org/ontology/automotive#TrafficDevice -->
  <owl:Class rdf:about="http://vcd.vicomtech.org/ontology/automotive#TrafficDevice">
    <rdfs:label xml:lang="en">Traffic device</rdfs:label>
    <rdfs:subClassOf rdf:resource="http://vcd.vicomtech.org/ontology/automotive#RoadObstacles" />
    <dcterms:description xml:lang="en">All signs, signals, markings or devices placed for the purpose of regulating, warning or guiding traffic.</dcterms:description>
  </owl:Class>
  <!-- http://vcd.vicomtech.org/ontology/automotive#TrafficLight -->
  <owl:Class rdf:about="http://vcd.vicomtech.org/ontology/automotive#TrafficLight">
    <rdfs:label xml:lang="en">Traffic light</rdfs:label>
    <rdfs:subClassOf rdf:resource="http://vcd.vicomtech.org/ontology/automotive#Signs" />
    <dcterms:description xml:lang="en">Traffic lights without poles in different orientations and for all types or traffic participants.</dcterms:description>
  </owl:Class>
  <!-- http://vcd.vicomtech.org/ontology/automotive#TrafficSign -->
  <owl:Class rdf:about="http://vcd.vicomtech.org/ontology/automotive#TrafficSign">
    <rdfs:label xml:lang="en">Traffic sign</rdfs:label>
    <rdfs:subClassOf rdf:resource="http://vcd.vicomtech.org/ontology/automotive#Signs" />
    <dcterms:description xml:lang="en">Signs with the purpose of conveying information to drivers/cyclistspedestrians.</dcterms:description>
  </owl:Class>
  <!-- http://vcd.vicomtech.org/ontology/automotive#TrafficSignSupport -->
  <owl:Class rdf:about="http://vcd.vicomtech.org/ontology/automotive#TrafficSignSupport">
    <rdfs:label xml:lang="en">Traffic sign support</rdfs:label>
    <rdfs:subClassOf rdf:resource="http://vcd.vicomtech.org/ontology/automotive#Support" />
    <dcterms:description xml:lang="en">Frame construction holding large signs, where frame can be made of round or square poles. Can be typically found on highways.</dcterms:description>
  </owl:Class>
  <!-- http://vcd.vicomtech.org/ontology/automotive#TrafficViolation -->
  <owl:Class rdf:about="http://vcd.vicomtech.org/ontology/automotive#TrafficViolation">
    <rdfs:label xml:lang="en">Traffic violation</rdfs:label>
    <rdfs:subClassOf rdf:resource="http://vcd.vicomtech.org/ontology/automotive#MovingManeuver" />
    <dcterms:description xml:lang="en">Any action that does not respect the traffic laws.</dcterms:description>
  </owl:Class>
  <!-- http://vcd.vicomtech.org/ontology/automotive#Trailer -->
  <owl:Class rdf:about="http://vcd.vicomtech.org/ontology/automotive#Trailer">
    <rdfs:label xml:lang="en">Trailer</rdfs:label>
    <rdfs:subClassOf rdf:resource="http://vcd.vicomtech.org/ontology/automotive#RoadVehicle" />
    <dcterms:description xml:lang="en">An unpowered vehicle towed by another. Excluded trailers attached to trucks, which belongs to class truck.</dcterms:description>
  </owl:Class>
  <!-- http://vcd.vicomtech.org/ontology/automotive#Train -->
  <owl:Class rdf:about="http://vcd.vicomtech.org/ontology/automotive#Train">
    <rdfs:label xml:lang="en">Train</rdfs:label>
    <rdfs:subClassOf rdf:resource="http://vcd.vicomtech.org/ontology/automotive#RailborneVehicle" />
    <dcterms:description xml:lang="en">A series of connected railway carriages or wagons moved by a locomotive or by integral motors.</dcterms:description>
  </owl:Class>
  <!-- http://vcd.vicomtech.org/ontology/automotive#Trash -->
  <owl:Class rdf:about="http://vcd.vicomtech.org/ontology/automotive#Trash">
    <rdfs:label xml:lang="en">Trash</rdfs:label>
    <rdfs:subClassOf rdf:resource="http://vcd.vicomtech.org/ontology/automotive#RoadObstacles" />
    <dcterms:description xml:lang="en">Waste material; refuse.</dcterms:description>
  </owl:Class>
  <!-- http://vcd.vicomtech.org/ontology/automotive#Tricycle -->
  <owl:Class rdf:about="http://vcd.vicomtech.org/ontology/automotive#Tricycle">
    <rdfs:label xml:lang="en">Tricycle</rdfs:label>
    <rdfs:subClassOf rdf:resource="http://vcd.vicomtech.org/ontology/automotive#RoadVehicle" />
    <dcterms:description xml:lang="en">A vehicle similar to a bicycle, but having three wheels, two at the back and one at the front.</dcterms:description>
  </owl:Class>
  <!-- http://vcd.vicomtech.org/ontology/automotive#Truck -->
  <owl:Class rdf:about="http://vcd.vicomtech.org/ontology/automotive#Truck">
    <rdfs:label xml:lang="en">Truck</rdfs:label>
    <rdfs:subClassOf rdf:resource="http://vcd.vicomtech.org/ontology/automotive#RoadVehicle" />
    <dcterms:description xml:lang="en">A large, heavy road vehicle used for carrying goods, materials or troops; a lorry.</dcterms:description>
  </owl:Class>
  <!-- http://vcd.vicomtech.org/ontology/automotive#Tunnel -->
  <owl:Class rdf:about="http://vcd.vicomtech.org/ontology/automotive#Tunnel">
    <rdfs:label xml:lang="en">Tunnel</rdfs:label>
    <rdfs:subClassOf rdf:resource="http://vcd.vicomtech.org/ontology/automotive#Structure" />
    <dcterms:description xml:lang="en">An artificial underground passage, especially one built through a hill or under a building, road, or river.</dcterms:description>
  </owl:Class>
  <!-- http://vcd.vicomtech.org/ontology/automotive#Turn -->
  <owl:Class rdf:about="http://vcd.vicomtech.org/ontology/automotive#Turn">
    <rdfs:label xml:lang="en">Turn</rdfs:label>
    <rdfs:subClassOf rdf:resource="http://vcd.vicomtech.org/ontology/automotive#MovingManeuver" />
    <dcterms:description xml:lang="en">To move in a circular direction wholly or partly round an axis or point.</dcterms:description>
  </owl:Class>
  <!-- http://vcd.vicomtech.org/ontology/automotive#TurningIntoLeft -->
  <owl:Class rdf:about="http://vcd.vicomtech.org/ontology/automotive#TurningIntoLeft">
    <rdfs:label xml:lang="en">Turning into left</rdfs:label>
    <rdfs:subClassOf rdf:resource="http://vcd.vicomtech.org/ontology/automotive#Turn" />
    <dcterms:description xml:lang="en">Making a turn to the left hand side of the road.</dcterms:description>
  </owl:Class>
  <!-- http://vcd.vicomtech.org/ontology/automotive#TurningIntoRight -->
  <owl:Class rdf:about="http://vcd.vicomtech.org/ontology/automotive#TurningIntoRight">
    <rdfs:label xml:lang="en">Turning into right</rdfs:label>
    <rdfs:subClassOf rdf:resource="http://vcd.vicomtech.org/ontology/automotive#Turn" />
    <dcterms:description xml:lang="en">Making a turn to the right hand side of the road.</dcterms:description>
  </owl:Class>
  <!-- http://vcd.vicomtech.org/ontology/automotive#TurningLeft -->
  <owl:Class rdf:about="http://vcd.vicomtech.org/ontology/automotive#TurningLeft">
    <rdfs:label xml:lang="en">Turning left</rdfs:label>
    <rdfs:subClassOf rdf:resource="http://vcd.vicomtech.org/ontology/automotive#Turn" />
    <dcterms:description xml:lang="en">Making a turn to the left hand side of the road.</dcterms:description>
  </owl:Class>
  <!-- http://vcd.vicomtech.org/ontology/automotive#TurningRight -->
  <owl:Class rdf:about="http://vcd.vicomtech.org/ontology/automotive#TurningRight">
    <rdfs:label xml:lang="en">Turning right</rdfs:label>
    <rdfs:subClassOf rdf:resource="http://vcd.vicomtech.org/ontology/automotive#Turn" />
    <dcterms:description xml:lang="en">Making a turn to the right hand side of the road.</dcterms:description>
  </owl:Class>
  <!-- http://vcd.vicomtech.org/ontology/automotive#UTurn -->
  <owl:Class rdf:about="http://vcd.vicomtech.org/ontology/automotive#UTurn">
    <rdfs:label xml:lang="en">uTurn</rdfs:label>
    <rdfs:subClassOf rdf:resource="http://vcd.vicomtech.org/ontology/automotive#MovingManeuver" />
    <dcterms:description xml:lang="en">A U-shaped turn made by a vehicle so as to head in the opposite direction from its original course.</dcterms:description>
  </owl:Class>
  <!-- http://vcd.vicomtech.org/ontology/automotive#Unclassified -->
  <owl:Class rdf:about="http://vcd.vicomtech.org/ontology/automotive#Unclassified">
    <rdfs:label xml:lang="en">Unclassified</rdfs:label>
    <rdfs:subClassOf rdf:resource="http://vcd.vicomtech.org/ontology/automotive#MovingManeuver" />
    <rdfs:subClassOf rdf:resource="http://vcd.vicomtech.org/ontology/automotive#StationaryManeuver" />
    <dcterms:description xml:lang="en">An action that does not fit in any of the defined terms.</dcterms:description>
  </owl:Class>
  <!-- http://vcd.vicomtech.org/ontology/automotive#Unlabeled -->
  <owl:Class rdf:about="http://vcd.vicomtech.org/ontology/automotive#Unlabeled">
    <rdfs:label xml:lang="en">Unlabeled</rdfs:label>
    <rdfs:subClassOf rdf:resource="http://vcd.vicomtech.org/ontology/automotive#Void" />
    <dcterms:description xml:lang="en">An object without a defined class.</dcterms:description>
  </owl:Class>
  <!-- http://vcd.vicomtech.org/ontology/automotive#UtilityPole -->
  <owl:Class rdf:about="http://vcd.vicomtech.org/ontology/automotive#UtilityPole">
    <rdfs:label xml:lang="en">Utility pole</rdfs:label>
    <rdfs:subClassOf rdf:resource="http://vcd.vicomtech.org/ontology/automotive#Support" />
    <dcterms:description xml:lang="en">Utility poles are supposed to carry electrical wires/cables, could be used to mount mobile phone network receivers, and are used in case both, cables and street lights are mounted.</dcterms:description>
  </owl:Class>
  <!-- http://vcd.vicomtech.org/ontology/automotive#UtilityVehicle -->
  <owl:Class rdf:about="http://vcd.vicomtech.org/ontology/automotive#UtilityVehicle">
    <rdfs:label xml:lang="en">Utility vehicle</rdfs:label>
    <rdfs:subClassOf rdf:resource="http://vcd.vicomtech.org/ontology/automotive#RoadVehicle" />
    <dcterms:description xml:lang="en">A truck with low sides designed for carrying small loads.</dcterms:description>
  </owl:Class>
  <!-- http://vcd.vicomtech.org/ontology/automotive#Vansuv -->
  <owl:Class rdf:about="http://vcd.vicomtech.org/ontology/automotive#Vansuv">
    <rdfs:label xml:lang="en">VanSUV</rdfs:label>
    <rdfs:subClassOf rdf:resource="http://vcd.vicomtech.org/ontology/automotive#RoadVehicle" />
  </owl:Class>
  <!-- http://vcd.vicomtech.org/ontology/automotive#Vegetation -->
  <owl:Class rdf:about="http://vcd.vicomtech.org/ontology/automotive#Vegetation">
    <rdfs:label xml:lang="en">Vegetation</rdfs:label>
    <rdfs:subClassOf rdf:resource="http://vcd.vicomtech.org/ontology/automotive#Nature" />
    <dcterms:description xml:lang="en">Trees and other forms of vertical growing vegetation.</dcterms:description>
  </owl:Class>
  <!-- http://vcd.vicomtech.org/ontology/automotive#Vehicle -->
  <owl:Class rdf:about="http://vcd.vicomtech.org/ontology/automotive#Vehicle">
    <rdfs:label xml:lang="en">Vehicle</rdfs:label>
    <rdfs:subClassOf rdf:resource="http://vcd.vicomtech.org/ontology/automotive#Dynamic" />
    <dcterms:description xml:lang="en">A Thing used for transporting people or goods.</dcterms:description>
  </owl:Class>
  <!-- http://vcd.vicomtech.org/ontology/automotive#Void -->
  <owl:Class rdf:about="http://vcd.vicomtech.org/ontology/automotive#Void">
    <rdfs:label xml:lang="en">Void</rdfs:label>
    <rdfs:subClassOf rdf:resource="http://vcd.vicomtech.org/ontology/automotive#Static" />
    <dcterms:description xml:lang="en">Objects that do not fit in the defined categories or too small objects that cannot be recognized.</dcterms:description>
  </owl:Class>
  <!-- http://vcd.vicomtech.org/ontology/automotive#Waiting -->
  <owl:Class rdf:about="http://vcd.vicomtech.org/ontology/automotive#Waiting">
    <rdfs:label xml:lang="en">Waiting</rdfs:label>
    <rdfs:subClassOf rdf:resource="http://vcd.vicomtech.org/ontology/automotive#StationaryManeuver" />
    <dcterms:description xml:lang="en">The action of staying where one is or delaying action until a particular time or event.</dcterms:description>
  </owl:Class>
  <!-- http://vcd.vicomtech.org/ontology/automotive#Walking -->
  <owl:Class rdf:about="http://vcd.vicomtech.org/ontology/automotive#Walking">
    <rdfs:label rdf:datatype="http://www.w3.org/2001/XMLSchema#string">Walking</rdfs:label>
    <rdfs:subClassOf rdf:resource="http://vcd.vicomtech.org/ontology/automotive#MovingManeuver" />
    <dcterms:description rdf:datatype="http://www.w3.org/2001/XMLSchema#string">The action of moving at a regular pace by lifting and setting down each foot in turn.</dcterms:description>
  </owl:Class>
  <!-- http://vcd.vicomtech.org/ontology/automotive#WalkingAlong -->
  <owl:Class rdf:about="http://vcd.vicomtech.org/ontology/automotive#WalkingAlong">
    <rdfs:label xml:lang="en">Walking along</rdfs:label>
    <rdfs:subClassOf rdf:resource="http://vcd.vicomtech.org/ontology/automotive#MovingManeuver" />
    <dcterms:description xml:lang="en">The action of walking following the path.</dcterms:description>
  </owl:Class>
  <!-- http://vcd.vicomtech.org/ontology/automotive#Wall -->
  <owl:Class rdf:about="http://vcd.vicomtech.org/ontology/automotive#Wall">
    <rdfs:label xml:lang="en">Wall</rdfs:label>
    <rdfs:subClassOf rdf:resource="http://vcd.vicomtech.org/ontology/automotive#Barrier" />
    <dcterms:description xml:lang="en">A continuous vertical brick or stone structure that encloses or divides an area of land.d</dcterms:description>
  </owl:Class>
  <!-- http://vcd.vicomtech.org/ontology/automotive#Water -->
  <owl:Class rdf:about="http://vcd.vicomtech.org/ontology/automotive#Water">
    <rdfs:label xml:lang="en">Water</rdfs:label>
    <rdfs:subClassOf rdf:resource="http://vcd.vicomtech.org/ontology/automotive#Nature" />
    <dcterms:description xml:lang="en">Ground surfaces covered by water.</dcterms:description>
  </owl:Class>
  <!-- http://vcd.vicomtech.org/ontology/automotive#WaterVehicle -->
  <owl:Class rdf:about="http://vcd.vicomtech.org/ontology/automotive#WaterVehicle">
    <rdfs:label xml:lang="en">Water vehicle</rdfs:label>
    <rdfs:subClassOf rdf:resource="http://vcd.vicomtech.org/ontology/automotive#Vehicle" />
    <dcterms:description xml:lang="en">Vehicles used in water (Watercraft, water vessels or waterborne vessels).</dcterms:description>
  </owl:Class>
  <!-- http://vcd.vicomtech.org/ontology/automotive#Weather -->
  <owl:Class rdf:about="http://vcd.vicomtech.org/ontology/automotive#Weather">
    <rdfs:label xml:lang="en">Weather</rdfs:label>
    <rdfs:subClassOf rdf:resource="http://vcd.vicomtech.org/ontology/automotive#Static" />
    <dcterms:description xml:lang="en">A state or condition of the atmosphere with respect to wind, temperature, moisture, etc.</dcterms:description>
  </owl:Class>
  <!-- http://vcd.vicomtech.org/ontology/automotive#Wheelchair -->
  <owl:Class rdf:about="http://vcd.vicomtech.org/ontology/automotive#Wheelchair">
    <rdfs:label xml:lang="en">Wheelchair</rdfs:label>
    <rdfs:subClassOf rdf:resource="http://vcd.vicomtech.org/ontology/automotive#WheeledSlow" />
    <dcterms:description xml:lang="en">A chair fitted with wheels for use as a means of transport by a person who is unable to walk as a result of illness, injury, or disability.</dcterms:description>
  </owl:Class>
  <!-- http://vcd.vicomtech.org/ontology/automotive#WheeledSlow -->
  <owl:Class rdf:about="http://vcd.vicomtech.org/ontology/automotive#WheeledSlow">
    <rdfs:label xml:lang="en">Wheeled slow</rdfs:label>
    <rdfs:subClassOf rdf:resource="http://vcd.vicomtech.org/ontology/automotive#RoadVehicle" />
    <dcterms:description xml:lang="en">Covers all slow moving wheeled objects like wheelchairs, mobility scooters, scooters, prams or rickshaw. All of which can potentially have riders sitting on them.</dcterms:description>
  </owl:Class>
  <!-- http://vcd.vicomtech.org/ontology/automotive#WhiteLines -->
  <owl:Class rdf:about="http://vcd.vicomtech.org/ontology/automotive#WhiteLines">
    <rdfs:label xml:lang="en">White lines</rdfs:label>
    <rdfs:subClassOf rdf:resource="http://vcd.vicomtech.org/ontology/automotive#Crosswalk" />
    <rdfs:subClassOf rdf:resource="http://vcd.vicomtech.org/ontology/automotive#LaneMarking" />
    <dcterms:description xml:lang="en">White color lines that delineate the separation of traffic flows in the same direction, or mark the right edge of the pavement.</dcterms:description>
  </owl:Class>
  <!-- http://vcd.vicomtech.org/ontology/automotive#YellowLines -->
  <owl:Class rdf:about="http://vcd.vicomtech.org/ontology/automotive#YellowLines">
    <rdfs:label xml:lang="en">Yellow lines</rdfs:label>
    <rdfs:subClassOf rdf:resource="http://vcd.vicomtech.org/ontology/automotive#LaneMarking" />
    <dcterms:description xml:lang="en">Yellow markings that delineate the separation of traffic flows in opposing directions, or mark the left edge of the pavement of divided highways and one-way roads.</dcterms:description>
  </owl:Class>
</rdf:RDF>
<!--Generated by Cognitum FluentEditor2015, a part of Ontorion(TM) Knowledge Management Framework, (with support of OwlApi)-->