<?xml version="1.0"?>
<rdf:RDF xmlns="http://vcd.vicomtech.org/ontology/automotive#"
     xml:base="http://vcd.vicomtech.org/ontology/automotive"
     xmlns:AGO="http://vcd.vicomtech.org/ontology/automotive#"
     xmlns:owl="http://www.w3.org/2002/07/owl#"
     xmlns:rdf="http://www.w3.org/1999/02/22-rdf-syntax-ns#"
     xmlns:xml="http://www.w3.org/XML/1998/namespace"
     xmlns:xsd="http://www.w3.org/2001/XMLSchema#"
     xmlns:rdfs="http://www.w3.org/2000/01/rdf-schema#"
     xmlns:swrl="http://www.w3.org/2003/11/swrl#"
     xmlns:swrla="http://swrl.stanford.edu/ontologies/3.3/swrla.owl#"
     xmlns:swrlb="http://www.w3.org/2003/11/swrlb#"
     xmlns:terms="http://purl.org/dc/terms#"
     xmlns:dcterms="http://unknown.prefix/dcterms#"
     xmlns:elements="http://purl.org/dc/elements/1.1#">
    <owl:Ontology rdf:about="http://vcd.vicomtech.org/ontology/automotive#">
        <owl:versionIRI rdf:resource="http://vcd.vicomtech.org/ontology/automotive#AGO"/>
        <owl:imports rdf:resource="http://www.semanticweb.org/iurbieta/ontologies/2021/0/untitled-ontology-37"/>
        <elements:creator>Itziar Urbieta</elements:creator>
        <elements:description>This is a global ontology of the main concepts related with the automotive area. The ontology contains the constructs required for annotation and traffic scenario simulation.</elements:description>
        <elements:title>Automotive Global Ontology</elements:title>
        <terms:publisher>Vicomtech</terms:publisher>
        <language>en</language>
        <rdfs:label>automotive</rdfs:label>
        <owl:versionInfo>version 1.0.0</owl:versionInfo>
    </owl:Ontology>
    


    <!-- 
    ///////////////////////////////////////////////////////////////////////////////////////
    //
    // Annotation properties
    //
    ///////////////////////////////////////////////////////////////////////////////////////
     -->

    


    <!-- http://purl.org/dc/elements/1.1#contributor -->

    <owl:AnnotationProperty rdf:about="http://purl.org/dc/elements/1.1#contributor">
        <rdfs:comment>An entity responsible for making contributions to the resource.</rdfs:comment>
        <rdfs:label>Contributor</rdfs:label>
    </owl:AnnotationProperty>
    


    <!-- http://purl.org/dc/elements/1.1#creator -->

    <owl:AnnotationProperty rdf:about="http://purl.org/dc/elements/1.1#creator">
        <rdfs:comment>An entity responsible for making the resource.</rdfs:comment>
        <rdfs:label>Creator</rdfs:label>
    </owl:AnnotationProperty>
    


    <!-- http://purl.org/dc/elements/1.1#description -->

    <owl:AnnotationProperty rdf:about="http://purl.org/dc/elements/1.1#description">
        <rdfs:comment>Description may include but is not limited to: an abstract, a table of contents, a graphical
        representation, or a free-text account of the resource.</rdfs:comment>
        <rdfs:label>Description</rdfs:label>
    </owl:AnnotationProperty>
    


    <!-- http://purl.org/dc/elements/1.1#title -->

    <owl:AnnotationProperty rdf:about="http://purl.org/dc/elements/1.1#title">
        <rdfs:comment>A name given to the resource.</rdfs:comment>
        <rdfs:label>Title</rdfs:label>
    </owl:AnnotationProperty>
    


    <!-- http://purl.org/dc/terms#dateSubmitted -->

    <owl:AnnotationProperty rdf:about="http://purl.org/dc/terms#dateSubmitted">
        <rdfs:comment>Date of submission of the resource.</rdfs:comment>
        <rdfs:label>Date Submitted</rdfs:label>
    </owl:AnnotationProperty>
    


    <!-- http://purl.org/dc/terms#license -->

    <owl:AnnotationProperty rdf:about="http://purl.org/dc/terms#license">
        <rdfs:comment>A legal document giving official permission to do something with the resource.</rdfs:comment>
        <rdfs:label>License</rdfs:label>
    </owl:AnnotationProperty>
    


    <!-- http://purl.org/dc/terms#publisher -->

    <owl:AnnotationProperty rdf:about="http://purl.org/dc/terms#publisher">
        <rdfs:comment>An entity responsible for making the resource available.</rdfs:comment>
        <rdfs:label>Publisher</rdfs:label>
    </owl:AnnotationProperty>
    


    <!-- http://swrl.stanford.edu/ontologies/3.3/swrla.owl#isRuleEnabled -->

    <owl:AnnotationProperty rdf:about="http://swrl.stanford.edu/ontologies/3.3/swrla.owl#isRuleEnabled"/>
    


    <!-- http://vcd.vicomtech.org/ontology/automotive#language -->

    <owl:AnnotationProperty rdf:about="http://vcd.vicomtech.org/ontology/automotive#language">
        <rdfs:comment>A language of the resource.</rdfs:comment>
        <rdfs:label>Language</rdfs:label>
    </owl:AnnotationProperty>
    


    <!-- 
    ///////////////////////////////////////////////////////////////////////////////////////
    //
    // Datatypes
    //
    ///////////////////////////////////////////////////////////////////////////////////////
     -->

    


    <!-- http://vcd.vicomtech.org/ontology/automotive#array -->

    <rdfs:Datatype rdf:about="http://vcd.vicomtech.org/ontology/automotive#array"/>
    


    <!-- 
    ///////////////////////////////////////////////////////////////////////////////////////
    //
    // Object Properties
    //
    ///////////////////////////////////////////////////////////////////////////////////////
     -->

    


    <!-- http://vcd.vicomtech.org/ontology/automotive#before -->

    <owl:ObjectProperty rdf:about="http://vcd.vicomtech.org/ontology/automotive#before">
        <rdfs:subPropertyOf rdf:resource="http://www.w3.org/2002/07/owl#topObjectProperty"/>
        <rdfs:domain rdf:resource="http://vcd.vicomtech.org/ontology/automotive#Action"/>
        <rdfs:domain rdf:resource="http://vcd.vicomtech.org/ontology/automotive#Event"/>
        <rdfs:range rdf:resource="http://vcd.vicomtech.org/ontology/automotive#Action"/>
        <rdfs:range rdf:resource="http://vcd.vicomtech.org/ontology/automotive#Event"/>
    </owl:ObjectProperty>
    


    <!-- http://vcd.vicomtech.org/ontology/automotive#behindOf -->

    <owl:ObjectProperty rdf:about="http://vcd.vicomtech.org/ontology/automotive#behindOf">
        <rdfs:subPropertyOf rdf:resource="http://www.w3.org/2002/07/owl#topObjectProperty"/>
        <owl:inverseOf rdf:resource="http://vcd.vicomtech.org/ontology/automotive#inFrontOf"/>
        <rdfs:domain rdf:resource="http://vcd.vicomtech.org/ontology/automotive#Animal"/>
        <rdfs:domain rdf:resource="http://vcd.vicomtech.org/ontology/automotive#Barrier"/>
        <rdfs:domain rdf:resource="http://vcd.vicomtech.org/ontology/automotive#Flat"/>
        <rdfs:domain rdf:resource="http://vcd.vicomtech.org/ontology/automotive#Human"/>
        <rdfs:domain rdf:resource="http://vcd.vicomtech.org/ontology/automotive#Junction"/>
        <rdfs:domain rdf:resource="http://vcd.vicomtech.org/ontology/automotive#MovableObject"/>
        <rdfs:domain rdf:resource="http://vcd.vicomtech.org/ontology/automotive#RoadVehicle"/>
        <rdfs:domain rdf:resource="http://vcd.vicomtech.org/ontology/automotive#RoadsideObject"/>
        <rdfs:domain rdf:resource="http://vcd.vicomtech.org/ontology/automotive#Structure"/>
        <rdfs:range rdf:resource="http://vcd.vicomtech.org/ontology/automotive#Animal"/>
        <rdfs:range rdf:resource="http://vcd.vicomtech.org/ontology/automotive#Barrier"/>
        <rdfs:range rdf:resource="http://vcd.vicomtech.org/ontology/automotive#Flat"/>
        <rdfs:range rdf:resource="http://vcd.vicomtech.org/ontology/automotive#Human"/>
        <rdfs:range rdf:resource="http://vcd.vicomtech.org/ontology/automotive#Junction"/>
        <rdfs:range rdf:resource="http://vcd.vicomtech.org/ontology/automotive#MovableObject"/>
        <rdfs:range rdf:resource="http://vcd.vicomtech.org/ontology/automotive#RoadVehicle"/>
        <rdfs:range rdf:resource="http://vcd.vicomtech.org/ontology/automotive#RoadsideObject"/>
        <rdfs:range rdf:resource="http://vcd.vicomtech.org/ontology/automotive#Structure"/>
        <rdfs:comment>Indicates that an object is behind another one.</rdfs:comment>
    </owl:ObjectProperty>
    


    <!-- http://vcd.vicomtech.org/ontology/automotive#causes -->

    <owl:ObjectProperty rdf:about="http://vcd.vicomtech.org/ontology/automotive#causes">
        <rdfs:subPropertyOf rdf:resource="http://www.w3.org/2002/07/owl#topObjectProperty"/>
        <rdfs:domain rdf:resource="http://vcd.vicomtech.org/ontology/automotive#Action"/>
        <rdfs:domain rdf:resource="http://vcd.vicomtech.org/ontology/automotive#Event"/>
        <rdfs:range rdf:resource="http://vcd.vicomtech.org/ontology/automotive#Action"/>
        <rdfs:range rdf:resource="http://vcd.vicomtech.org/ontology/automotive#Event"/>
    </owl:ObjectProperty>
    


    <!-- http://vcd.vicomtech.org/ontology/automotive#causes1 -->

    <owl:ObjectProperty rdf:about="http://vcd.vicomtech.org/ontology/automotive#causes1">
        <rdfs:subPropertyOf rdf:resource="http://vcd.vicomtech.org/ontology/automotive#causes"/>
        <rdfs:domain rdf:resource="http://vcd.vicomtech.org/ontology/automotive#ChangeTrafficLightState"/>
        <rdfs:range rdf:resource="http://vcd.vicomtech.org/ontology/automotive#Colliding"/>
        <rdfs:range rdf:resource="http://vcd.vicomtech.org/ontology/automotive#Crossing"/>
        <rdfs:range rdf:resource="http://vcd.vicomtech.org/ontology/automotive#DrivingStraight"/>
        <rdfs:range rdf:resource="http://vcd.vicomtech.org/ontology/automotive#LaneChanging"/>
        <rdfs:range rdf:resource="http://vcd.vicomtech.org/ontology/automotive#Passing"/>
        <rdfs:range rdf:resource="http://vcd.vicomtech.org/ontology/automotive#Running"/>
        <rdfs:range rdf:resource="http://vcd.vicomtech.org/ontology/automotive#Stopping"/>
        <rdfs:range rdf:resource="http://vcd.vicomtech.org/ontology/automotive#Turning"/>
        <rdfs:range rdf:resource="http://vcd.vicomtech.org/ontology/automotive#Walking"/>
    </owl:ObjectProperty>
    


    <!-- http://vcd.vicomtech.org/ontology/automotive#causes10 -->

    <owl:ObjectProperty rdf:about="http://vcd.vicomtech.org/ontology/automotive#causes10">
        <rdfs:subPropertyOf rdf:resource="http://vcd.vicomtech.org/ontology/automotive#causes"/>
        <rdfs:domain rdf:resource="http://vcd.vicomtech.org/ontology/automotive#LossOfControl"/>
        <rdfs:domain rdf:resource="http://vcd.vicomtech.org/ontology/automotive#Swerve"/>
        <rdfs:range rdf:resource="http://vcd.vicomtech.org/ontology/automotive#Colliding"/>
        <rdfs:range rdf:resource="http://vcd.vicomtech.org/ontology/automotive#GlidingOnWheels"/>
        <rdfs:range rdf:resource="http://vcd.vicomtech.org/ontology/automotive#LossingControl"/>
    </owl:ObjectProperty>
    


    <!-- http://vcd.vicomtech.org/ontology/automotive#causes11 -->

    <owl:ObjectProperty rdf:about="http://vcd.vicomtech.org/ontology/automotive#causes11">
        <rdfs:subPropertyOf rdf:resource="http://vcd.vicomtech.org/ontology/automotive#causes"/>
        <rdfs:domain rdf:resource="http://vcd.vicomtech.org/ontology/automotive#SafeStop"/>
        <rdfs:range rdf:resource="http://vcd.vicomtech.org/ontology/automotive#Crossing"/>
        <rdfs:range rdf:resource="http://vcd.vicomtech.org/ontology/automotive#Following"/>
        <rdfs:range rdf:resource="http://vcd.vicomtech.org/ontology/automotive#Passing"/>
        <rdfs:range rdf:resource="http://vcd.vicomtech.org/ontology/automotive#Running"/>
        <rdfs:range rdf:resource="http://vcd.vicomtech.org/ontology/automotive#Walking"/>
    </owl:ObjectProperty>
    


    <!-- http://vcd.vicomtech.org/ontology/automotive#causes12 -->

    <owl:ObjectProperty rdf:about="http://vcd.vicomtech.org/ontology/automotive#causes12">
        <rdfs:subPropertyOf rdf:resource="http://vcd.vicomtech.org/ontology/automotive#causes"/>
        <rdfs:domain rdf:resource="http://vcd.vicomtech.org/ontology/automotive#Failure"/>
        <rdfs:range rdf:resource="http://vcd.vicomtech.org/ontology/automotive#Colliding"/>
        <rdfs:range rdf:resource="http://vcd.vicomtech.org/ontology/automotive#GlidingOnWheels"/>
        <rdfs:range rdf:resource="http://vcd.vicomtech.org/ontology/automotive#LossingControl"/>
        <rdfs:range rdf:resource="http://vcd.vicomtech.org/ontology/automotive#Stopping"/>
        <rdfs:range rdf:resource="http://vcd.vicomtech.org/ontology/automotive#TrafficViolation"/>
    </owl:ObjectProperty>
    


    <!-- http://vcd.vicomtech.org/ontology/automotive#causes13 -->

    <owl:ObjectProperty rdf:about="http://vcd.vicomtech.org/ontology/automotive#causes13">
        <rdfs:subPropertyOf rdf:resource="http://vcd.vicomtech.org/ontology/automotive#causes"/>
        <rdfs:domain rdf:resource="http://vcd.vicomtech.org/ontology/automotive#Reach"/>
        <rdfs:range rdf:resource="http://vcd.vicomtech.org/ontology/automotive#AvoidingCollision"/>
        <rdfs:range rdf:resource="http://vcd.vicomtech.org/ontology/automotive#Colliding"/>
        <rdfs:range rdf:resource="http://vcd.vicomtech.org/ontology/automotive#Crossing"/>
        <rdfs:range rdf:resource="http://vcd.vicomtech.org/ontology/automotive#Decelerating"/>
        <rdfs:range rdf:resource="http://vcd.vicomtech.org/ontology/automotive#LaneChanging"/>
        <rdfs:range rdf:resource="http://vcd.vicomtech.org/ontology/automotive#Overtaking"/>
        <rdfs:range rdf:resource="http://vcd.vicomtech.org/ontology/automotive#Stopping"/>
        <rdfs:range rdf:resource="http://vcd.vicomtech.org/ontology/automotive#Turning"/>
        <rdfs:range rdf:resource="http://vcd.vicomtech.org/ontology/automotive#Waiting"/>
        <rdfs:range rdf:resource="http://vcd.vicomtech.org/ontology/automotive#Walking"/>
    </owl:ObjectProperty>
    


    <!-- http://vcd.vicomtech.org/ontology/automotive#causes2 -->

    <owl:ObjectProperty rdf:about="http://vcd.vicomtech.org/ontology/automotive#causes2">
        <rdfs:subPropertyOf rdf:resource="http://vcd.vicomtech.org/ontology/automotive#causes"/>
        <rdfs:domain rdf:resource="http://vcd.vicomtech.org/ontology/automotive#Collision"/>
        <rdfs:range rdf:resource="http://vcd.vicomtech.org/ontology/automotive#Colliding"/>
        <rdfs:range rdf:resource="http://vcd.vicomtech.org/ontology/automotive#FallingDown"/>
    </owl:ObjectProperty>
    


    <!-- http://vcd.vicomtech.org/ontology/automotive#causes3 -->

    <owl:ObjectProperty rdf:about="http://vcd.vicomtech.org/ontology/automotive#causes3">
        <rdfs:subPropertyOf rdf:resource="http://vcd.vicomtech.org/ontology/automotive#causes"/>
        <rdfs:domain rdf:resource="http://vcd.vicomtech.org/ontology/automotive#Fall"/>
        <rdfs:range rdf:resource="http://vcd.vicomtech.org/ontology/automotive#Rising"/>
    </owl:ObjectProperty>
    


    <!-- http://vcd.vicomtech.org/ontology/automotive#causes4 -->

    <owl:ObjectProperty rdf:about="http://vcd.vicomtech.org/ontology/automotive#causes4">
        <rdfs:subPropertyOf rdf:resource="http://vcd.vicomtech.org/ontology/automotive#causes"/>
        <rdfs:domain rdf:resource="http://vcd.vicomtech.org/ontology/automotive#Rise"/>
        <rdfs:range rdf:resource="http://vcd.vicomtech.org/ontology/automotive#Crossing"/>
        <rdfs:range rdf:resource="http://vcd.vicomtech.org/ontology/automotive#Following"/>
        <rdfs:range rdf:resource="http://vcd.vicomtech.org/ontology/automotive#Running"/>
        <rdfs:range rdf:resource="http://vcd.vicomtech.org/ontology/automotive#Walking"/>
    </owl:ObjectProperty>
    


    <!-- http://vcd.vicomtech.org/ontology/automotive#causes5 -->

    <owl:ObjectProperty rdf:about="http://vcd.vicomtech.org/ontology/automotive#causes5">
        <rdfs:subPropertyOf rdf:resource="http://vcd.vicomtech.org/ontology/automotive#causes"/>
        <rdfs:domain rdf:resource="http://vcd.vicomtech.org/ontology/automotive#Park"/>
        <rdfs:range rdf:resource="http://vcd.vicomtech.org/ontology/automotive#Approaching"/>
        <rdfs:range rdf:resource="http://vcd.vicomtech.org/ontology/automotive#Crossing"/>
        <rdfs:range rdf:resource="http://vcd.vicomtech.org/ontology/automotive#DrivingStraight"/>
        <rdfs:range rdf:resource="http://vcd.vicomtech.org/ontology/automotive#Following"/>
        <rdfs:range rdf:resource="http://vcd.vicomtech.org/ontology/automotive#LaneChanging"/>
        <rdfs:range rdf:resource="http://vcd.vicomtech.org/ontology/automotive#Passing"/>
        <rdfs:range rdf:resource="http://vcd.vicomtech.org/ontology/automotive#Walking"/>
    </owl:ObjectProperty>
    


    <!-- http://vcd.vicomtech.org/ontology/automotive#causes6 -->

    <owl:ObjectProperty rdf:about="http://vcd.vicomtech.org/ontology/automotive#causes6">
        <rdfs:subPropertyOf rdf:resource="http://vcd.vicomtech.org/ontology/automotive#causes"/>
        <rdfs:domain rdf:resource="http://vcd.vicomtech.org/ontology/automotive#LaneChange"/>
        <rdfs:range rdf:resource="http://vcd.vicomtech.org/ontology/automotive#Approaching"/>
        <rdfs:range rdf:resource="http://vcd.vicomtech.org/ontology/automotive#Crossing"/>
        <rdfs:range rdf:resource="http://vcd.vicomtech.org/ontology/automotive#DrivingStraight"/>
        <rdfs:range rdf:resource="http://vcd.vicomtech.org/ontology/automotive#Following"/>
        <rdfs:range rdf:resource="http://vcd.vicomtech.org/ontology/automotive#LaneChanging"/>
        <rdfs:range rdf:resource="http://vcd.vicomtech.org/ontology/automotive#Passing"/>
    </owl:ObjectProperty>
    


    <!-- http://vcd.vicomtech.org/ontology/automotive#causes7 -->

    <owl:ObjectProperty rdf:about="http://vcd.vicomtech.org/ontology/automotive#causes7">
        <rdfs:subPropertyOf rdf:resource="http://vcd.vicomtech.org/ontology/automotive#causes"/>
        <rdfs:domain rdf:resource="http://vcd.vicomtech.org/ontology/automotive#Turn"/>
        <rdfs:range rdf:resource="http://vcd.vicomtech.org/ontology/automotive#Approaching"/>
        <rdfs:range rdf:resource="http://vcd.vicomtech.org/ontology/automotive#Crossing"/>
        <rdfs:range rdf:resource="http://vcd.vicomtech.org/ontology/automotive#DrivingStraight"/>
        <rdfs:range rdf:resource="http://vcd.vicomtech.org/ontology/automotive#Following"/>
        <rdfs:range rdf:resource="http://vcd.vicomtech.org/ontology/automotive#LaneChanging"/>
        <rdfs:range rdf:resource="http://vcd.vicomtech.org/ontology/automotive#Passing"/>
    </owl:ObjectProperty>
    


    <!-- http://vcd.vicomtech.org/ontology/automotive#causes8 -->

    <owl:ObjectProperty rdf:about="http://vcd.vicomtech.org/ontology/automotive#causes8">
        <rdfs:subPropertyOf rdf:resource="http://vcd.vicomtech.org/ontology/automotive#causes"/>
        <rdfs:domain rdf:resource="http://vcd.vicomtech.org/ontology/automotive#Overtake"/>
        <rdfs:range rdf:resource="http://vcd.vicomtech.org/ontology/automotive#Approaching"/>
        <rdfs:range rdf:resource="http://vcd.vicomtech.org/ontology/automotive#Crossing"/>
        <rdfs:range rdf:resource="http://vcd.vicomtech.org/ontology/automotive#DrivingStraight"/>
        <rdfs:range rdf:resource="http://vcd.vicomtech.org/ontology/automotive#FallingBehind"/>
        <rdfs:range rdf:resource="http://vcd.vicomtech.org/ontology/automotive#Following"/>
        <rdfs:range rdf:resource="http://vcd.vicomtech.org/ontology/automotive#LaneChanging"/>
        <rdfs:range rdf:resource="http://vcd.vicomtech.org/ontology/automotive#Passing"/>
    </owl:ObjectProperty>
    


    <!-- http://vcd.vicomtech.org/ontology/automotive#causes9 -->

    <owl:ObjectProperty rdf:about="http://vcd.vicomtech.org/ontology/automotive#causes9">
        <rdfs:subPropertyOf rdf:resource="http://vcd.vicomtech.org/ontology/automotive#causes"/>
        <rdfs:domain rdf:resource="http://vcd.vicomtech.org/ontology/automotive#Pass"/>
        <rdfs:range rdf:resource="http://vcd.vicomtech.org/ontology/automotive#Approaching"/>
        <rdfs:range rdf:resource="http://vcd.vicomtech.org/ontology/automotive#Crossing"/>
        <rdfs:range rdf:resource="http://vcd.vicomtech.org/ontology/automotive#DrivingStraight"/>
        <rdfs:range rdf:resource="http://vcd.vicomtech.org/ontology/automotive#FallingBehind"/>
        <rdfs:range rdf:resource="http://vcd.vicomtech.org/ontology/automotive#Following"/>
        <rdfs:range rdf:resource="http://vcd.vicomtech.org/ontology/automotive#LaneChanging"/>
        <rdfs:range rdf:resource="http://vcd.vicomtech.org/ontology/automotive#Passing"/>
    </owl:ObjectProperty>
    


    <!-- http://vcd.vicomtech.org/ontology/automotive#during -->

    <owl:ObjectProperty rdf:about="http://vcd.vicomtech.org/ontology/automotive#during">
        <rdfs:subPropertyOf rdf:resource="http://www.w3.org/2002/07/owl#topObjectProperty"/>
        <rdfs:domain rdf:resource="http://vcd.vicomtech.org/ontology/automotive#Action"/>
        <rdfs:domain rdf:resource="http://vcd.vicomtech.org/ontology/automotive#Event"/>
        <rdfs:range rdf:resource="http://vcd.vicomtech.org/ontology/automotive#Action"/>
        <rdfs:range rdf:resource="http://vcd.vicomtech.org/ontology/automotive#Event"/>
    </owl:ObjectProperty>
    


    <!-- http://vcd.vicomtech.org/ontology/automotive#equals -->

    <owl:ObjectProperty rdf:about="http://vcd.vicomtech.org/ontology/automotive#equals">
        <rdfs:subPropertyOf rdf:resource="http://www.w3.org/2002/07/owl#topObjectProperty"/>
        <rdfs:domain rdf:resource="http://vcd.vicomtech.org/ontology/automotive#Action"/>
        <rdfs:domain rdf:resource="http://vcd.vicomtech.org/ontology/automotive#Event"/>
        <rdfs:range rdf:resource="http://vcd.vicomtech.org/ontology/automotive#Action"/>
        <rdfs:range rdf:resource="http://vcd.vicomtech.org/ontology/automotive#Event"/>
    </owl:ObjectProperty>
    


    <!-- http://vcd.vicomtech.org/ontology/automotive#finishes -->

    <owl:ObjectProperty rdf:about="http://vcd.vicomtech.org/ontology/automotive#finishes">
        <rdfs:subPropertyOf rdf:resource="http://www.w3.org/2002/07/owl#topObjectProperty"/>
        <owl:inverseOf rdf:resource="http://vcd.vicomtech.org/ontology/automotive#starts"/>
        <rdfs:domain rdf:resource="http://vcd.vicomtech.org/ontology/automotive#Action"/>
        <rdfs:domain rdf:resource="http://vcd.vicomtech.org/ontology/automotive#Event"/>
        <rdfs:range rdf:resource="http://vcd.vicomtech.org/ontology/automotive#Action"/>
        <rdfs:range rdf:resource="http://vcd.vicomtech.org/ontology/automotive#Event"/>
    </owl:ObjectProperty>
    


    <!-- http://vcd.vicomtech.org/ontology/automotive#inFrontOf -->

    <owl:ObjectProperty rdf:about="http://vcd.vicomtech.org/ontology/automotive#inFrontOf">
        <rdfs:subPropertyOf rdf:resource="http://www.w3.org/2002/07/owl#topObjectProperty"/>
        <rdfs:domain rdf:resource="http://vcd.vicomtech.org/ontology/automotive#Animal"/>
        <rdfs:domain rdf:resource="http://vcd.vicomtech.org/ontology/automotive#Barrier"/>
        <rdfs:domain rdf:resource="http://vcd.vicomtech.org/ontology/automotive#Flat"/>
        <rdfs:domain rdf:resource="http://vcd.vicomtech.org/ontology/automotive#Human"/>
        <rdfs:domain rdf:resource="http://vcd.vicomtech.org/ontology/automotive#Junction"/>
        <rdfs:domain rdf:resource="http://vcd.vicomtech.org/ontology/automotive#MovableObject"/>
        <rdfs:domain rdf:resource="http://vcd.vicomtech.org/ontology/automotive#RoadVehicle"/>
        <rdfs:domain rdf:resource="http://vcd.vicomtech.org/ontology/automotive#RoadsideObject"/>
        <rdfs:domain rdf:resource="http://vcd.vicomtech.org/ontology/automotive#Structure"/>
        <rdfs:range rdf:resource="http://vcd.vicomtech.org/ontology/automotive#Animal"/>
        <rdfs:range rdf:resource="http://vcd.vicomtech.org/ontology/automotive#Barrier"/>
        <rdfs:range rdf:resource="http://vcd.vicomtech.org/ontology/automotive#Flat"/>
        <rdfs:range rdf:resource="http://vcd.vicomtech.org/ontology/automotive#Human"/>
        <rdfs:range rdf:resource="http://vcd.vicomtech.org/ontology/automotive#Junction"/>
        <rdfs:range rdf:resource="http://vcd.vicomtech.org/ontology/automotive#MovableObject"/>
        <rdfs:range rdf:resource="http://vcd.vicomtech.org/ontology/automotive#RoadVehicle"/>
        <rdfs:range rdf:resource="http://vcd.vicomtech.org/ontology/automotive#RoadsideObject"/>
        <rdfs:range rdf:resource="http://vcd.vicomtech.org/ontology/automotive#Structure"/>
        <rdfs:comment>Indicates that an object is in front of another one.</rdfs:comment>
    </owl:ObjectProperty>
    


    <!-- http://vcd.vicomtech.org/ontology/automotive#isConnectedTo -->

    <owl:ObjectProperty rdf:about="http://vcd.vicomtech.org/ontology/automotive#isConnectedTo">
        <rdfs:domain rdf:resource="http://vcd.vicomtech.org/ontology/automotive#Construction"/>
        <rdfs:range rdf:resource="http://vcd.vicomtech.org/ontology/automotive#Construction"/>
        <rdfs:comment>Indicates the connection between spatial elements of the road network.</rdfs:comment>
    </owl:ObjectProperty>
    


    <!-- http://vcd.vicomtech.org/ontology/automotive#isObjectOfAction -->

    <owl:ObjectProperty rdf:about="http://vcd.vicomtech.org/ontology/automotive#isObjectOfAction">
        <rdfs:subPropertyOf rdf:resource="http://www.w3.org/2002/07/owl#topObjectProperty"/>
        <rdfs:domain rdf:resource="http://vcd.vicomtech.org/ontology/automotive#Object"/>
        <rdfs:range rdf:resource="http://vcd.vicomtech.org/ontology/automotive#Action"/>
    </owl:ObjectProperty>
    


    <!-- http://vcd.vicomtech.org/ontology/automotive#isObjectOfAction1 -->

    <owl:ObjectProperty rdf:about="http://vcd.vicomtech.org/ontology/automotive#isObjectOfAction1">
        <rdfs:subPropertyOf rdf:resource="http://vcd.vicomtech.org/ontology/automotive#isObjectOfAction"/>
        <rdfs:domain rdf:resource="http://vcd.vicomtech.org/ontology/automotive#AnimalPulled"/>
        <rdfs:domain rdf:resource="http://vcd.vicomtech.org/ontology/automotive#Cycle"/>
        <rdfs:domain rdf:resource="http://vcd.vicomtech.org/ontology/automotive#DrivableVehicle"/>
        <rdfs:domain rdf:resource="http://vcd.vicomtech.org/ontology/automotive#WheeledSlow"/>
        <rdfs:range rdf:resource="http://vcd.vicomtech.org/ontology/automotive#Approaching"/>
        <rdfs:range rdf:resource="http://vcd.vicomtech.org/ontology/automotive#AvoidingCollision"/>
        <rdfs:range rdf:resource="http://vcd.vicomtech.org/ontology/automotive#Colliding"/>
        <rdfs:range rdf:resource="http://vcd.vicomtech.org/ontology/automotive#DrivingInOppositeDirection"/>
        <rdfs:range rdf:resource="http://vcd.vicomtech.org/ontology/automotive#FallingBehind"/>
        <rdfs:range rdf:resource="http://vcd.vicomtech.org/ontology/automotive#Following"/>
        <rdfs:range rdf:resource="http://vcd.vicomtech.org/ontology/automotive#Overtaking"/>
        <rdfs:range rdf:resource="http://vcd.vicomtech.org/ontology/automotive#Passing"/>
        <rdfs:range rdf:resource="http://vcd.vicomtech.org/ontology/automotive#Waiting"/>
    </owl:ObjectProperty>
    


    <!-- http://vcd.vicomtech.org/ontology/automotive#isObjectOfAction10 -->

    <owl:ObjectProperty rdf:about="http://vcd.vicomtech.org/ontology/automotive#isObjectOfAction10">
        <rdfs:subPropertyOf rdf:resource="http://vcd.vicomtech.org/ontology/automotive#isObjectOfAction"/>
        <rdfs:domain rdf:resource="http://vcd.vicomtech.org/ontology/automotive#TrafficLight"/>
        <rdfs:range rdf:resource="http://vcd.vicomtech.org/ontology/automotive#Colliding"/>
        <rdfs:range rdf:resource="http://vcd.vicomtech.org/ontology/automotive#Stopped"/>
        <rdfs:range rdf:resource="http://vcd.vicomtech.org/ontology/automotive#Waiting"/>
    </owl:ObjectProperty>
    


    <!-- http://vcd.vicomtech.org/ontology/automotive#isObjectOfAction11 -->

    <owl:ObjectProperty rdf:about="http://vcd.vicomtech.org/ontology/automotive#isObjectOfAction11">
        <rdfs:subPropertyOf rdf:resource="http://vcd.vicomtech.org/ontology/automotive#isObjectOfAction"/>
        <rdfs:domain rdf:resource="http://vcd.vicomtech.org/ontology/automotive#RailborneVehicle"/>
        <rdfs:range rdf:resource="http://vcd.vicomtech.org/ontology/automotive#DrivingInOppositeDirection"/>
    </owl:ObjectProperty>
    


    <!-- http://vcd.vicomtech.org/ontology/automotive#isObjectOfAction2 -->

    <owl:ObjectProperty rdf:about="http://vcd.vicomtech.org/ontology/automotive#isObjectOfAction2">
        <rdfs:subPropertyOf rdf:resource="http://vcd.vicomtech.org/ontology/automotive#isObjectOfAction"/>
        <rdfs:domain rdf:resource="http://vcd.vicomtech.org/ontology/automotive#Pedestrian"/>
        <rdfs:domain rdf:resource="http://vcd.vicomtech.org/ontology/automotive#PedestrianWithObject"/>
        <rdfs:range rdf:resource="http://vcd.vicomtech.org/ontology/automotive#Approaching"/>
        <rdfs:range rdf:resource="http://vcd.vicomtech.org/ontology/automotive#AvoidingCollision"/>
        <rdfs:range rdf:resource="http://vcd.vicomtech.org/ontology/automotive#Colliding"/>
        <rdfs:range rdf:resource="http://vcd.vicomtech.org/ontology/automotive#DrivingInOppositeDirection"/>
        <rdfs:range rdf:resource="http://vcd.vicomtech.org/ontology/automotive#FallingBehind"/>
        <rdfs:range rdf:resource="http://vcd.vicomtech.org/ontology/automotive#Following"/>
        <rdfs:range rdf:resource="http://vcd.vicomtech.org/ontology/automotive#Overtaking"/>
        <rdfs:range rdf:resource="http://vcd.vicomtech.org/ontology/automotive#Waiting"/>
    </owl:ObjectProperty>
    


    <!-- http://vcd.vicomtech.org/ontology/automotive#isObjectOfAction3 -->

    <owl:ObjectProperty rdf:about="http://vcd.vicomtech.org/ontology/automotive#isObjectOfAction3">
        <rdfs:subPropertyOf rdf:resource="http://vcd.vicomtech.org/ontology/automotive#isObjectOfAction"/>
        <rdfs:domain rdf:resource="http://vcd.vicomtech.org/ontology/automotive#Rider"/>
        <rdfs:range rdf:resource="http://vcd.vicomtech.org/ontology/automotive#Approaching"/>
        <rdfs:range rdf:resource="http://vcd.vicomtech.org/ontology/automotive#AvoidingCollision"/>
        <rdfs:range rdf:resource="http://vcd.vicomtech.org/ontology/automotive#Colliding"/>
        <rdfs:range rdf:resource="http://vcd.vicomtech.org/ontology/automotive#DrivingInOppositeDirection"/>
        <rdfs:range rdf:resource="http://vcd.vicomtech.org/ontology/automotive#FallingBehind"/>
        <rdfs:range rdf:resource="http://vcd.vicomtech.org/ontology/automotive#Following"/>
        <rdfs:range rdf:resource="http://vcd.vicomtech.org/ontology/automotive#Overtaking"/>
        <rdfs:range rdf:resource="http://vcd.vicomtech.org/ontology/automotive#Waiting"/>
    </owl:ObjectProperty>
    


    <!-- http://vcd.vicomtech.org/ontology/automotive#isObjectOfAction4 -->

    <owl:ObjectProperty rdf:about="http://vcd.vicomtech.org/ontology/automotive#isObjectOfAction4">
        <rdfs:subPropertyOf rdf:resource="http://vcd.vicomtech.org/ontology/automotive#isObjectOfAction"/>
        <rdfs:domain rdf:resource="http://vcd.vicomtech.org/ontology/automotive#Road"/>
        <rdfs:range rdf:resource="http://vcd.vicomtech.org/ontology/automotive#Approaching"/>
        <rdfs:range rdf:resource="http://vcd.vicomtech.org/ontology/automotive#Blocking"/>
        <rdfs:range rdf:resource="http://vcd.vicomtech.org/ontology/automotive#Crossing"/>
        <rdfs:range rdf:resource="http://vcd.vicomtech.org/ontology/automotive#Decelerating"/>
        <rdfs:range rdf:resource="http://vcd.vicomtech.org/ontology/automotive#DrivingStraight"/>
        <rdfs:range rdf:resource="http://vcd.vicomtech.org/ontology/automotive#FallingDown"/>
        <rdfs:range rdf:resource="http://vcd.vicomtech.org/ontology/automotive#Following"/>
        <rdfs:range rdf:resource="http://vcd.vicomtech.org/ontology/automotive#GlidingOnWheels"/>
        <rdfs:range rdf:resource="http://vcd.vicomtech.org/ontology/automotive#LossingControl"/>
        <rdfs:range rdf:resource="http://vcd.vicomtech.org/ontology/automotive#Parked"/>
        <rdfs:range rdf:resource="http://vcd.vicomtech.org/ontology/automotive#Parking"/>
        <rdfs:range rdf:resource="http://vcd.vicomtech.org/ontology/automotive#Reversing"/>
        <rdfs:range rdf:resource="http://vcd.vicomtech.org/ontology/automotive#Rising"/>
        <rdfs:range rdf:resource="http://vcd.vicomtech.org/ontology/automotive#Running"/>
        <rdfs:range rdf:resource="http://vcd.vicomtech.org/ontology/automotive#Standing"/>
        <rdfs:range rdf:resource="http://vcd.vicomtech.org/ontology/automotive#Stopped"/>
        <rdfs:range rdf:resource="http://vcd.vicomtech.org/ontology/automotive#Stopping"/>
        <rdfs:range rdf:resource="http://vcd.vicomtech.org/ontology/automotive#Swerving"/>
        <rdfs:range rdf:resource="http://vcd.vicomtech.org/ontology/automotive#Turning"/>
        <rdfs:range rdf:resource="http://vcd.vicomtech.org/ontology/automotive#TurningLeft"/>
        <rdfs:range rdf:resource="http://vcd.vicomtech.org/ontology/automotive#TurningRight"/>
        <rdfs:range rdf:resource="http://vcd.vicomtech.org/ontology/automotive#Waiting"/>
        <rdfs:range rdf:resource="http://vcd.vicomtech.org/ontology/automotive#Walking"/>
    </owl:ObjectProperty>
    


    <!-- http://vcd.vicomtech.org/ontology/automotive#isObjectOfAction5 -->

    <owl:ObjectProperty rdf:about="http://vcd.vicomtech.org/ontology/automotive#isObjectOfAction5">
        <rdfs:subPropertyOf rdf:resource="http://vcd.vicomtech.org/ontology/automotive#isObjectOfAction"/>
        <rdfs:domain rdf:resource="http://vcd.vicomtech.org/ontology/automotive#Lane"/>
        <rdfs:range rdf:resource="http://vcd.vicomtech.org/ontology/automotive#Approaching"/>
        <rdfs:range rdf:resource="http://vcd.vicomtech.org/ontology/automotive#Blocking"/>
        <rdfs:range rdf:resource="http://vcd.vicomtech.org/ontology/automotive#Crossing"/>
        <rdfs:range rdf:resource="http://vcd.vicomtech.org/ontology/automotive#Decelerating"/>
        <rdfs:range rdf:resource="http://vcd.vicomtech.org/ontology/automotive#DrivingStraight"/>
        <rdfs:range rdf:resource="http://vcd.vicomtech.org/ontology/automotive#FallingDown"/>
        <rdfs:range rdf:resource="http://vcd.vicomtech.org/ontology/automotive#Following"/>
        <rdfs:range rdf:resource="http://vcd.vicomtech.org/ontology/automotive#GlidingOnWheels"/>
        <rdfs:range rdf:resource="http://vcd.vicomtech.org/ontology/automotive#LaneChanging"/>
        <rdfs:range rdf:resource="http://vcd.vicomtech.org/ontology/automotive#LaneChangingLeft"/>
        <rdfs:range rdf:resource="http://vcd.vicomtech.org/ontology/automotive#LaneChangingRight"/>
        <rdfs:range rdf:resource="http://vcd.vicomtech.org/ontology/automotive#LossingControl"/>
        <rdfs:range rdf:resource="http://vcd.vicomtech.org/ontology/automotive#Parked"/>
        <rdfs:range rdf:resource="http://vcd.vicomtech.org/ontology/automotive#Parking"/>
        <rdfs:range rdf:resource="http://vcd.vicomtech.org/ontology/automotive#Reversing"/>
        <rdfs:range rdf:resource="http://vcd.vicomtech.org/ontology/automotive#Rising"/>
        <rdfs:range rdf:resource="http://vcd.vicomtech.org/ontology/automotive#Running"/>
        <rdfs:range rdf:resource="http://vcd.vicomtech.org/ontology/automotive#Standing"/>
        <rdfs:range rdf:resource="http://vcd.vicomtech.org/ontology/automotive#Stopped"/>
        <rdfs:range rdf:resource="http://vcd.vicomtech.org/ontology/automotive#Stopping"/>
        <rdfs:range rdf:resource="http://vcd.vicomtech.org/ontology/automotive#Swerving"/>
        <rdfs:range rdf:resource="http://vcd.vicomtech.org/ontology/automotive#Turning"/>
        <rdfs:range rdf:resource="http://vcd.vicomtech.org/ontology/automotive#TurningLeft"/>
        <rdfs:range rdf:resource="http://vcd.vicomtech.org/ontology/automotive#TurningRight"/>
        <rdfs:range rdf:resource="http://vcd.vicomtech.org/ontology/automotive#Waiting"/>
        <rdfs:range rdf:resource="http://vcd.vicomtech.org/ontology/automotive#Walking"/>
    </owl:ObjectProperty>
    


    <!-- http://vcd.vicomtech.org/ontology/automotive#isObjectOfAction6 -->

    <owl:ObjectProperty rdf:about="http://vcd.vicomtech.org/ontology/automotive#isObjectOfAction6">
        <rdfs:subPropertyOf rdf:resource="http://vcd.vicomtech.org/ontology/automotive#isObjectOfAction"/>
        <rdfs:domain rdf:resource="http://vcd.vicomtech.org/ontology/automotive#Junction"/>
        <rdfs:range rdf:resource="http://vcd.vicomtech.org/ontology/automotive#Approaching"/>
        <rdfs:range rdf:resource="http://vcd.vicomtech.org/ontology/automotive#Blocking"/>
        <rdfs:range rdf:resource="http://vcd.vicomtech.org/ontology/automotive#Crossing"/>
        <rdfs:range rdf:resource="http://vcd.vicomtech.org/ontology/automotive#Decelerating"/>
        <rdfs:range rdf:resource="http://vcd.vicomtech.org/ontology/automotive#DrivingStraight"/>
        <rdfs:range rdf:resource="http://vcd.vicomtech.org/ontology/automotive#FallingDown"/>
        <rdfs:range rdf:resource="http://vcd.vicomtech.org/ontology/automotive#GlidingOnWheels"/>
        <rdfs:range rdf:resource="http://vcd.vicomtech.org/ontology/automotive#LossingControl"/>
        <rdfs:range rdf:resource="http://vcd.vicomtech.org/ontology/automotive#Parked"/>
        <rdfs:range rdf:resource="http://vcd.vicomtech.org/ontology/automotive#Reversing"/>
        <rdfs:range rdf:resource="http://vcd.vicomtech.org/ontology/automotive#Rising"/>
        <rdfs:range rdf:resource="http://vcd.vicomtech.org/ontology/automotive#Sitting"/>
        <rdfs:range rdf:resource="http://vcd.vicomtech.org/ontology/automotive#Standing"/>
        <rdfs:range rdf:resource="http://vcd.vicomtech.org/ontology/automotive#Stopped"/>
        <rdfs:range rdf:resource="http://vcd.vicomtech.org/ontology/automotive#Stopping"/>
        <rdfs:range rdf:resource="http://vcd.vicomtech.org/ontology/automotive#Swerving"/>
        <rdfs:range rdf:resource="http://vcd.vicomtech.org/ontology/automotive#Turning"/>
        <rdfs:range rdf:resource="http://vcd.vicomtech.org/ontology/automotive#TurningLeft"/>
        <rdfs:range rdf:resource="http://vcd.vicomtech.org/ontology/automotive#TurningRight"/>
        <rdfs:range rdf:resource="http://vcd.vicomtech.org/ontology/automotive#Waiting"/>
        <rdfs:range rdf:resource="http://vcd.vicomtech.org/ontology/automotive#Walking"/>
    </owl:ObjectProperty>
    


    <!-- http://vcd.vicomtech.org/ontology/automotive#isObjectOfAction7 -->

    <owl:ObjectProperty rdf:about="http://vcd.vicomtech.org/ontology/automotive#isObjectOfAction7">
        <rdfs:subPropertyOf rdf:resource="http://vcd.vicomtech.org/ontology/automotive#isObjectOfAction"/>
        <rdfs:domain rdf:resource="http://vcd.vicomtech.org/ontology/automotive#Footwalk"/>
        <rdfs:domain rdf:resource="http://vcd.vicomtech.org/ontology/automotive#PedestrianArea"/>
        <rdfs:range rdf:resource="http://vcd.vicomtech.org/ontology/automotive#Approaching"/>
        <rdfs:range rdf:resource="http://vcd.vicomtech.org/ontology/automotive#Blocking"/>
        <rdfs:range rdf:resource="http://vcd.vicomtech.org/ontology/automotive#Crossing"/>
        <rdfs:range rdf:resource="http://vcd.vicomtech.org/ontology/automotive#FallingDown"/>
        <rdfs:range rdf:resource="http://vcd.vicomtech.org/ontology/automotive#Following"/>
        <rdfs:range rdf:resource="http://vcd.vicomtech.org/ontology/automotive#Parked"/>
        <rdfs:range rdf:resource="http://vcd.vicomtech.org/ontology/automotive#Parking"/>
        <rdfs:range rdf:resource="http://vcd.vicomtech.org/ontology/automotive#Passing"/>
        <rdfs:range rdf:resource="http://vcd.vicomtech.org/ontology/automotive#Rising"/>
        <rdfs:range rdf:resource="http://vcd.vicomtech.org/ontology/automotive#Running"/>
        <rdfs:range rdf:resource="http://vcd.vicomtech.org/ontology/automotive#Sitting"/>
        <rdfs:range rdf:resource="http://vcd.vicomtech.org/ontology/automotive#Standing"/>
        <rdfs:range rdf:resource="http://vcd.vicomtech.org/ontology/automotive#Stopped"/>
        <rdfs:range rdf:resource="http://vcd.vicomtech.org/ontology/automotive#Stopping"/>
        <rdfs:range rdf:resource="http://vcd.vicomtech.org/ontology/automotive#Waiting"/>
        <rdfs:range rdf:resource="http://vcd.vicomtech.org/ontology/automotive#Walking"/>
    </owl:ObjectProperty>
    


    <!-- http://vcd.vicomtech.org/ontology/automotive#isObjectOfAction8 -->

    <owl:ObjectProperty rdf:about="http://vcd.vicomtech.org/ontology/automotive#isObjectOfAction8">
        <rdfs:subPropertyOf rdf:resource="http://vcd.vicomtech.org/ontology/automotive#isObjectOfAction"/>
        <rdfs:domain rdf:resource="http://vcd.vicomtech.org/ontology/automotive#Bridge"/>
        <rdfs:domain rdf:resource="http://vcd.vicomtech.org/ontology/automotive#Tunnel"/>
        <rdfs:range rdf:resource="http://vcd.vicomtech.org/ontology/automotive#Approaching"/>
        <rdfs:range rdf:resource="http://vcd.vicomtech.org/ontology/automotive#Blocking"/>
        <rdfs:range rdf:resource="http://vcd.vicomtech.org/ontology/automotive#Colliding"/>
        <rdfs:range rdf:resource="http://vcd.vicomtech.org/ontology/automotive#Crossing"/>
        <rdfs:range rdf:resource="http://vcd.vicomtech.org/ontology/automotive#Decelerating"/>
        <rdfs:range rdf:resource="http://vcd.vicomtech.org/ontology/automotive#DrivingStraight"/>
        <rdfs:range rdf:resource="http://vcd.vicomtech.org/ontology/automotive#GlidingOnWheels"/>
        <rdfs:range rdf:resource="http://vcd.vicomtech.org/ontology/automotive#LossingControl"/>
        <rdfs:range rdf:resource="http://vcd.vicomtech.org/ontology/automotive#Parked"/>
        <rdfs:range rdf:resource="http://vcd.vicomtech.org/ontology/automotive#Parking"/>
        <rdfs:range rdf:resource="http://vcd.vicomtech.org/ontology/automotive#Reversing"/>
        <rdfs:range rdf:resource="http://vcd.vicomtech.org/ontology/automotive#Rising"/>
        <rdfs:range rdf:resource="http://vcd.vicomtech.org/ontology/automotive#Running"/>
        <rdfs:range rdf:resource="http://vcd.vicomtech.org/ontology/automotive#Sitting"/>
        <rdfs:range rdf:resource="http://vcd.vicomtech.org/ontology/automotive#Standing"/>
        <rdfs:range rdf:resource="http://vcd.vicomtech.org/ontology/automotive#Stopped"/>
        <rdfs:range rdf:resource="http://vcd.vicomtech.org/ontology/automotive#Stopping"/>
        <rdfs:range rdf:resource="http://vcd.vicomtech.org/ontology/automotive#Swerving"/>
        <rdfs:range rdf:resource="http://vcd.vicomtech.org/ontology/automotive#Turning"/>
        <rdfs:range rdf:resource="http://vcd.vicomtech.org/ontology/automotive#TurningLeft"/>
        <rdfs:range rdf:resource="http://vcd.vicomtech.org/ontology/automotive#TurningRight"/>
        <rdfs:range rdf:resource="http://vcd.vicomtech.org/ontology/automotive#UTurning"/>
        <rdfs:range rdf:resource="http://vcd.vicomtech.org/ontology/automotive#Waiting"/>
        <rdfs:range rdf:resource="http://vcd.vicomtech.org/ontology/automotive#Walking"/>
    </owl:ObjectProperty>
    


    <!-- http://vcd.vicomtech.org/ontology/automotive#isObjectOfAction9 -->

    <owl:ObjectProperty rdf:about="http://vcd.vicomtech.org/ontology/automotive#isObjectOfAction9">
        <rdfs:subPropertyOf rdf:resource="http://vcd.vicomtech.org/ontology/automotive#isObjectOfAction"/>
        <rdfs:domain rdf:resource="http://vcd.vicomtech.org/ontology/automotive#Crosswalk"/>
        <rdfs:range rdf:resource="http://vcd.vicomtech.org/ontology/automotive#Approaching"/>
        <rdfs:range rdf:resource="http://vcd.vicomtech.org/ontology/automotive#Blocking"/>
        <rdfs:range rdf:resource="http://vcd.vicomtech.org/ontology/automotive#Crossing"/>
        <rdfs:range rdf:resource="http://vcd.vicomtech.org/ontology/automotive#FallingDown"/>
        <rdfs:range rdf:resource="http://vcd.vicomtech.org/ontology/automotive#Following"/>
        <rdfs:range rdf:resource="http://vcd.vicomtech.org/ontology/automotive#Parked"/>
        <rdfs:range rdf:resource="http://vcd.vicomtech.org/ontology/automotive#Parking"/>
        <rdfs:range rdf:resource="http://vcd.vicomtech.org/ontology/automotive#Rising"/>
        <rdfs:range rdf:resource="http://vcd.vicomtech.org/ontology/automotive#Running"/>
        <rdfs:range rdf:resource="http://vcd.vicomtech.org/ontology/automotive#Standing"/>
        <rdfs:range rdf:resource="http://vcd.vicomtech.org/ontology/automotive#Stopped"/>
        <rdfs:range rdf:resource="http://vcd.vicomtech.org/ontology/automotive#Stopping"/>
        <rdfs:range rdf:resource="http://vcd.vicomtech.org/ontology/automotive#Waiting"/>
        <rdfs:range rdf:resource="http://vcd.vicomtech.org/ontology/automotive#Walking"/>
    </owl:ObjectProperty>
    


    <!-- http://vcd.vicomtech.org/ontology/automotive#isObjectOfEvent -->

    <owl:ObjectProperty rdf:about="http://vcd.vicomtech.org/ontology/automotive#isObjectOfEvent">
        <rdfs:subPropertyOf rdf:resource="http://www.w3.org/2002/07/owl#topObjectProperty"/>
        <rdfs:domain rdf:resource="http://vcd.vicomtech.org/ontology/automotive#Object"/>
        <rdfs:range rdf:resource="http://vcd.vicomtech.org/ontology/automotive#Event"/>
    </owl:ObjectProperty>
    


    <!-- http://vcd.vicomtech.org/ontology/automotive#isObjectOfEvent1 -->

    <owl:ObjectProperty rdf:about="http://vcd.vicomtech.org/ontology/automotive#isObjectOfEvent1">
        <rdfs:subPropertyOf rdf:resource="http://vcd.vicomtech.org/ontology/automotive#isObjectOfEvent"/>
        <rdfs:domain rdf:resource="http://vcd.vicomtech.org/ontology/automotive#AnimalPulled"/>
        <rdfs:domain rdf:resource="http://vcd.vicomtech.org/ontology/automotive#Cycle"/>
        <rdfs:domain rdf:resource="http://vcd.vicomtech.org/ontology/automotive#DrivableVehicle"/>
        <rdfs:domain rdf:resource="http://vcd.vicomtech.org/ontology/automotive#WheeledSlow"/>
        <rdfs:range rdf:resource="http://vcd.vicomtech.org/ontology/automotive#Overtake"/>
        <rdfs:range rdf:resource="http://vcd.vicomtech.org/ontology/automotive#Pass"/>
    </owl:ObjectProperty>
    


    <!-- http://vcd.vicomtech.org/ontology/automotive#isObjectOfEvent2 -->

    <owl:ObjectProperty rdf:about="http://vcd.vicomtech.org/ontology/automotive#isObjectOfEvent2">
        <rdfs:subPropertyOf rdf:resource="http://vcd.vicomtech.org/ontology/automotive#isObjectOfEvent"/>
        <rdfs:domain rdf:resource="http://vcd.vicomtech.org/ontology/automotive#Junction"/>
        <rdfs:domain rdf:resource="http://vcd.vicomtech.org/ontology/automotive#Lane"/>
        <rdfs:domain rdf:resource="http://vcd.vicomtech.org/ontology/automotive#Road"/>
        <rdfs:domain rdf:resource="http://vcd.vicomtech.org/ontology/automotive#Structure"/>
        <rdfs:range rdf:resource="http://vcd.vicomtech.org/ontology/automotive#LaneChange"/>
        <rdfs:range rdf:resource="http://vcd.vicomtech.org/ontology/automotive#SafeStop"/>
        <rdfs:range rdf:resource="http://vcd.vicomtech.org/ontology/automotive#Swerve"/>
        <rdfs:range rdf:resource="http://vcd.vicomtech.org/ontology/automotive#Turn"/>
    </owl:ObjectProperty>
    


    <!-- http://vcd.vicomtech.org/ontology/automotive#isObjectOfEvent3 -->

    <owl:ObjectProperty rdf:about="http://vcd.vicomtech.org/ontology/automotive#isObjectOfEvent3">
        <rdfs:subPropertyOf rdf:resource="http://vcd.vicomtech.org/ontology/automotive#isObjectOfEvent"/>
        <rdfs:domain rdf:resource="http://vcd.vicomtech.org/ontology/automotive#Animal"/>
        <rdfs:domain rdf:resource="http://vcd.vicomtech.org/ontology/automotive#Barrier"/>
        <rdfs:domain rdf:resource="http://vcd.vicomtech.org/ontology/automotive#Human"/>
        <rdfs:domain rdf:resource="http://vcd.vicomtech.org/ontology/automotive#RoadObstacles"/>
        <rdfs:domain rdf:resource="http://vcd.vicomtech.org/ontology/automotive#RoadsideObject"/>
        <rdfs:domain rdf:resource="http://vcd.vicomtech.org/ontology/automotive#Structure"/>
        <rdfs:range rdf:resource="http://vcd.vicomtech.org/ontology/automotive#Collision"/>
    </owl:ObjectProperty>
    


    <!-- http://vcd.vicomtech.org/ontology/automotive#isObjectOfEvent4 -->

    <owl:ObjectProperty rdf:about="http://vcd.vicomtech.org/ontology/automotive#isObjectOfEvent4">
        <rdfs:subPropertyOf rdf:resource="http://vcd.vicomtech.org/ontology/automotive#isObjectOfEvent"/>
        <rdfs:domain rdf:resource="http://vcd.vicomtech.org/ontology/automotive#ParkingLot"/>
        <rdfs:range rdf:resource="http://vcd.vicomtech.org/ontology/automotive#Park"/>
        <rdfs:range rdf:resource="http://vcd.vicomtech.org/ontology/automotive#SafeStop"/>
    </owl:ObjectProperty>
    


    <!-- http://vcd.vicomtech.org/ontology/automotive#isObjectOfEvent5 -->

    <owl:ObjectProperty rdf:about="http://vcd.vicomtech.org/ontology/automotive#isObjectOfEvent5">
        <rdfs:subPropertyOf rdf:resource="http://vcd.vicomtech.org/ontology/automotive#isObjectOfEvent"/>
        <rdfs:domain rdf:resource="http://vcd.vicomtech.org/ontology/automotive#Animal"/>
        <rdfs:domain rdf:resource="http://vcd.vicomtech.org/ontology/automotive#Construction"/>
        <rdfs:domain rdf:resource="http://vcd.vicomtech.org/ontology/automotive#Human"/>
        <rdfs:domain rdf:resource="http://vcd.vicomtech.org/ontology/automotive#RoadObstacles"/>
        <rdfs:domain rdf:resource="http://vcd.vicomtech.org/ontology/automotive#RoadVehicle"/>
        <rdfs:domain rdf:resource="http://vcd.vicomtech.org/ontology/automotive#RoadsideObject"/>
        <rdfs:range rdf:resource="http://vcd.vicomtech.org/ontology/automotive#Reach"/>
    </owl:ObjectProperty>
    


    <!-- http://vcd.vicomtech.org/ontology/automotive#isObjectOfEvent6 -->

    <owl:ObjectProperty rdf:about="http://vcd.vicomtech.org/ontology/automotive#isObjectOfEvent6">
        <rdfs:subPropertyOf rdf:resource="http://vcd.vicomtech.org/ontology/automotive#isObjectOfEvent"/>
        <rdfs:domain rdf:resource="http://vcd.vicomtech.org/ontology/automotive#Flat"/>
        <rdfs:domain rdf:resource="http://vcd.vicomtech.org/ontology/automotive#Junction"/>
        <rdfs:domain rdf:resource="http://vcd.vicomtech.org/ontology/automotive#Structure"/>
        <rdfs:range rdf:resource="http://vcd.vicomtech.org/ontology/automotive#Fall"/>
        <rdfs:range rdf:resource="http://vcd.vicomtech.org/ontology/automotive#Rise"/>
    </owl:ObjectProperty>
    


    <!-- http://vcd.vicomtech.org/ontology/automotive#isObjectOfEvent7 -->

    <owl:ObjectProperty rdf:about="http://vcd.vicomtech.org/ontology/automotive#isObjectOfEvent7">
        <rdfs:subPropertyOf rdf:resource="http://vcd.vicomtech.org/ontology/automotive#isObjectOfEvent"/>
        <rdfs:domain rdf:resource="http://vcd.vicomtech.org/ontology/automotive#Crosswalk"/>
        <rdfs:domain rdf:resource="http://vcd.vicomtech.org/ontology/automotive#Interchange"/>
        <rdfs:domain rdf:resource="http://vcd.vicomtech.org/ontology/automotive#Intersection"/>
        <rdfs:domain rdf:resource="http://vcd.vicomtech.org/ontology/automotive#Road"/>
        <rdfs:domain rdf:resource="http://vcd.vicomtech.org/ontology/automotive#Structure"/>
        <rdfs:range rdf:resource="http://vcd.vicomtech.org/ontology/automotive#Cross"/>
    </owl:ObjectProperty>
    


    <!-- http://vcd.vicomtech.org/ontology/automotive#isObjectOfEvent8 -->

    <owl:ObjectProperty rdf:about="http://vcd.vicomtech.org/ontology/automotive#isObjectOfEvent8">
        <rdfs:subPropertyOf rdf:resource="http://vcd.vicomtech.org/ontology/automotive#isObjectOfEvent"/>
        <rdfs:domain rdf:resource="http://vcd.vicomtech.org/ontology/automotive#Object"/>
        <rdfs:range rdf:resource="http://vcd.vicomtech.org/ontology/automotive#Detect"/>
    </owl:ObjectProperty>
    


    <!-- http://vcd.vicomtech.org/ontology/automotive#isPartOf -->

    <owl:ObjectProperty rdf:about="http://vcd.vicomtech.org/ontology/automotive#isPartOf">
        <rdfs:subPropertyOf rdf:resource="http://www.w3.org/2002/07/owl#topObjectProperty"/>
        <rdfs:domain rdf:resource="http://vcd.vicomtech.org/ontology/automotive#Object"/>
        <rdfs:range rdf:resource="http://vcd.vicomtech.org/ontology/automotive#Object"/>
        <rdfs:comment>States if an spatial object of the road network is part of another one, so this means that the general term involves all the defined parts.</rdfs:comment>
    </owl:ObjectProperty>
    


    <!-- http://vcd.vicomtech.org/ontology/automotive#isPartOf1 -->

    <owl:ObjectProperty rdf:about="http://vcd.vicomtech.org/ontology/automotive#isPartOf1">
        <rdfs:subPropertyOf rdf:resource="http://vcd.vicomtech.org/ontology/automotive#isPartOf"/>
        <rdfs:domain rdf:resource="http://vcd.vicomtech.org/ontology/automotive#Bridge"/>
        <rdfs:domain rdf:resource="http://vcd.vicomtech.org/ontology/automotive#Building"/>
        <rdfs:domain rdf:resource="http://vcd.vicomtech.org/ontology/automotive#Curve"/>
        <rdfs:domain rdf:resource="http://vcd.vicomtech.org/ontology/automotive#Fence"/>
        <rdfs:domain rdf:resource="http://vcd.vicomtech.org/ontology/automotive#Footwalk"/>
        <rdfs:domain rdf:resource="http://vcd.vicomtech.org/ontology/automotive#GuardRail"/>
        <rdfs:domain rdf:resource="http://vcd.vicomtech.org/ontology/automotive#Interchange"/>
        <rdfs:domain rdf:resource="http://vcd.vicomtech.org/ontology/automotive#Intersection"/>
        <rdfs:domain rdf:resource="http://vcd.vicomtech.org/ontology/automotive#Junction"/>
        <rdfs:domain rdf:resource="http://vcd.vicomtech.org/ontology/automotive#Lane"/>
        <rdfs:domain rdf:resource="http://vcd.vicomtech.org/ontology/automotive#Marking"/>
        <rdfs:domain rdf:resource="http://vcd.vicomtech.org/ontology/automotive#OtherBarrier"/>
        <rdfs:domain rdf:resource="http://vcd.vicomtech.org/ontology/automotive#Overpass"/>
        <rdfs:domain rdf:resource="http://vcd.vicomtech.org/ontology/automotive#ParkingLot"/>
        <rdfs:domain rdf:resource="http://vcd.vicomtech.org/ontology/automotive#RailTrack"/>
        <rdfs:domain rdf:resource="http://vcd.vicomtech.org/ontology/automotive#Roundabout"/>
        <rdfs:domain rdf:resource="http://vcd.vicomtech.org/ontology/automotive#TrafficIsland"/>
        <rdfs:domain rdf:resource="http://vcd.vicomtech.org/ontology/automotive#Tunnel"/>
        <rdfs:domain rdf:resource="http://vcd.vicomtech.org/ontology/automotive#Wall"/>
        <rdfs:range rdf:resource="http://vcd.vicomtech.org/ontology/automotive#Road"/>
    </owl:ObjectProperty>
    


    <!-- http://vcd.vicomtech.org/ontology/automotive#isPartOf2 -->

    <owl:ObjectProperty rdf:about="http://vcd.vicomtech.org/ontology/automotive#isPartOf2">
        <rdfs:subPropertyOf rdf:resource="http://vcd.vicomtech.org/ontology/automotive#isPartOf"/>
        <rdfs:domain rdf:resource="http://vcd.vicomtech.org/ontology/automotive#Bench"/>
        <rdfs:domain rdf:resource="http://vcd.vicomtech.org/ontology/automotive#BikeLane"/>
        <rdfs:domain rdf:resource="http://vcd.vicomtech.org/ontology/automotive#BikeRack"/>
        <rdfs:domain rdf:resource="http://vcd.vicomtech.org/ontology/automotive#Bridge"/>
        <rdfs:domain rdf:resource="http://vcd.vicomtech.org/ontology/automotive#Building"/>
        <rdfs:domain rdf:resource="http://vcd.vicomtech.org/ontology/automotive#CatchBasin"/>
        <rdfs:domain rdf:resource="http://vcd.vicomtech.org/ontology/automotive#CctvCamera"/>
        <rdfs:domain rdf:resource="http://vcd.vicomtech.org/ontology/automotive#CurbCut"/>
        <rdfs:domain rdf:resource="http://vcd.vicomtech.org/ontology/automotive#Curbstone"/>
        <rdfs:domain rdf:resource="http://vcd.vicomtech.org/ontology/automotive#Curve"/>
        <rdfs:domain rdf:resource="http://vcd.vicomtech.org/ontology/automotive#Dustbin"/>
        <rdfs:domain rdf:resource="http://vcd.vicomtech.org/ontology/automotive#Fence"/>
        <rdfs:domain rdf:resource="http://vcd.vicomtech.org/ontology/automotive#FireHydrant"/>
        <rdfs:domain rdf:resource="http://vcd.vicomtech.org/ontology/automotive#LaneDivider"/>
        <rdfs:domain rdf:resource="http://vcd.vicomtech.org/ontology/automotive#Mailbox"/>
        <rdfs:domain rdf:resource="http://vcd.vicomtech.org/ontology/automotive#Manhole"/>
        <rdfs:domain rdf:resource="http://vcd.vicomtech.org/ontology/automotive#Marking"/>
        <rdfs:domain rdf:resource="http://vcd.vicomtech.org/ontology/automotive#Mountain"/>
        <rdfs:domain rdf:resource="http://vcd.vicomtech.org/ontology/automotive#OtherBarrier"/>
        <rdfs:domain rdf:resource="http://vcd.vicomtech.org/ontology/automotive#Overpass"/>
        <rdfs:domain rdf:resource="http://vcd.vicomtech.org/ontology/automotive#PhoneBooth"/>
        <rdfs:domain rdf:resource="http://vcd.vicomtech.org/ontology/automotive#Pole"/>
        <rdfs:domain rdf:resource="http://vcd.vicomtech.org/ontology/automotive#Polegroup"/>
        <rdfs:domain rdf:resource="http://vcd.vicomtech.org/ontology/automotive#Pothole"/>
        <rdfs:domain rdf:resource="http://vcd.vicomtech.org/ontology/automotive#RailTrack"/>
        <rdfs:domain rdf:resource="http://vcd.vicomtech.org/ontology/automotive#Roadblocks"/>
        <rdfs:domain rdf:resource="http://vcd.vicomtech.org/ontology/automotive#Sand"/>
        <rdfs:domain rdf:resource="http://vcd.vicomtech.org/ontology/automotive#Sidewalk"/>
        <rdfs:domain rdf:resource="http://vcd.vicomtech.org/ontology/automotive#Signs"/>
        <rdfs:domain rdf:resource="http://vcd.vicomtech.org/ontology/automotive#Snow"/>
        <rdfs:domain rdf:resource="http://vcd.vicomtech.org/ontology/automotive#StreetLight"/>
        <rdfs:domain rdf:resource="http://vcd.vicomtech.org/ontology/automotive#Terrain"/>
        <rdfs:domain rdf:resource="http://vcd.vicomtech.org/ontology/automotive#TrafficCone"/>
        <rdfs:domain rdf:resource="http://vcd.vicomtech.org/ontology/automotive#Vegetation"/>
        <rdfs:domain rdf:resource="http://vcd.vicomtech.org/ontology/automotive#Wall"/>
        <rdfs:domain rdf:resource="http://vcd.vicomtech.org/ontology/automotive#Water"/>
        <rdfs:range rdf:resource="http://vcd.vicomtech.org/ontology/automotive#Footwalk"/>
    </owl:ObjectProperty>
    


    <!-- http://vcd.vicomtech.org/ontology/automotive#isPartOf3 -->

    <owl:ObjectProperty rdf:about="http://vcd.vicomtech.org/ontology/automotive#isPartOf3">
        <rdfs:subPropertyOf rdf:resource="http://vcd.vicomtech.org/ontology/automotive#isPartOf"/>
        <rdfs:domain rdf:resource="http://vcd.vicomtech.org/ontology/automotive#Banner"/>
        <rdfs:domain rdf:resource="http://vcd.vicomtech.org/ontology/automotive#Billboard"/>
        <rdfs:domain rdf:resource="http://vcd.vicomtech.org/ontology/automotive#IrrelevantSign"/>
        <rdfs:domain rdf:resource="http://vcd.vicomtech.org/ontology/automotive#LaneDivider"/>
        <rdfs:domain rdf:resource="http://vcd.vicomtech.org/ontology/automotive#ParkingSign"/>
        <rdfs:domain rdf:resource="http://vcd.vicomtech.org/ontology/automotive#Signs"/>
        <rdfs:domain rdf:resource="http://vcd.vicomtech.org/ontology/automotive#StreetLight"/>
        <rdfs:domain rdf:resource="http://vcd.vicomtech.org/ontology/automotive#TrafficLight"/>
        <rdfs:domain rdf:resource="http://vcd.vicomtech.org/ontology/automotive#TrafficSign"/>
        <rdfs:range rdf:resource="http://vcd.vicomtech.org/ontology/automotive#Lane"/>
    </owl:ObjectProperty>
    


    <!-- http://vcd.vicomtech.org/ontology/automotive#isPartOf4 -->

    <owl:ObjectProperty rdf:about="http://vcd.vicomtech.org/ontology/automotive#isPartOf4">
        <rdfs:subPropertyOf rdf:resource="http://vcd.vicomtech.org/ontology/automotive#isPartOf"/>
        <rdfs:domain rdf:resource="http://vcd.vicomtech.org/ontology/automotive#Banner"/>
        <rdfs:domain rdf:resource="http://vcd.vicomtech.org/ontology/automotive#Billboard"/>
        <rdfs:domain rdf:resource="http://vcd.vicomtech.org/ontology/automotive#IrrelevantSign"/>
        <rdfs:domain rdf:resource="http://vcd.vicomtech.org/ontology/automotive#ParkingSign"/>
        <rdfs:domain rdf:resource="http://vcd.vicomtech.org/ontology/automotive#Signs"/>
        <rdfs:domain rdf:resource="http://vcd.vicomtech.org/ontology/automotive#StreetLight"/>
        <rdfs:domain rdf:resource="http://vcd.vicomtech.org/ontology/automotive#TrafficLight"/>
        <rdfs:domain rdf:resource="http://vcd.vicomtech.org/ontology/automotive#TrafficSign"/>
        <rdfs:range rdf:resource="http://vcd.vicomtech.org/ontology/automotive#Interchange"/>
        <rdfs:range rdf:resource="http://vcd.vicomtech.org/ontology/automotive#Intersection"/>
        <rdfs:range rdf:resource="http://vcd.vicomtech.org/ontology/automotive#Junction"/>
        <rdfs:range rdf:resource="http://vcd.vicomtech.org/ontology/automotive#Roundabout"/>
    </owl:ObjectProperty>
    


    <!-- http://vcd.vicomtech.org/ontology/automotive#isSubjectOfAction -->

    <owl:ObjectProperty rdf:about="http://vcd.vicomtech.org/ontology/automotive#isSubjectOfAction">
        <rdfs:subPropertyOf rdf:resource="http://www.w3.org/2002/07/owl#topObjectProperty"/>
        <rdfs:domain rdf:resource="http://vcd.vicomtech.org/ontology/automotive#Object"/>
        <rdfs:range rdf:resource="http://vcd.vicomtech.org/ontology/automotive#Action"/>
        <rdfs:comment>States &apos;who&apos; permons an Action by relating the actor and the performed action.</rdfs:comment>
    </owl:ObjectProperty>
    


    <!-- http://vcd.vicomtech.org/ontology/automotive#isSubjectOfAction1 -->

    <owl:ObjectProperty rdf:about="http://vcd.vicomtech.org/ontology/automotive#isSubjectOfAction1">
        <rdfs:subPropertyOf rdf:resource="http://vcd.vicomtech.org/ontology/automotive#isSubjectOfAction"/>
        <rdfs:domain rdf:resource="http://vcd.vicomtech.org/ontology/automotive#AnimalPulled"/>
        <rdfs:domain rdf:resource="http://vcd.vicomtech.org/ontology/automotive#Cycle"/>
        <rdfs:domain rdf:resource="http://vcd.vicomtech.org/ontology/automotive#DrivableVehicle"/>
        <rdfs:domain rdf:resource="http://vcd.vicomtech.org/ontology/automotive#WheeledSlow"/>
        <rdfs:range rdf:resource="http://vcd.vicomtech.org/ontology/automotive#Approaching"/>
        <rdfs:range rdf:resource="http://vcd.vicomtech.org/ontology/automotive#AvoidingCollision"/>
        <rdfs:range rdf:resource="http://vcd.vicomtech.org/ontology/automotive#Blocking"/>
        <rdfs:range rdf:resource="http://vcd.vicomtech.org/ontology/automotive#Colliding"/>
        <rdfs:range rdf:resource="http://vcd.vicomtech.org/ontology/automotive#Crossing"/>
        <rdfs:range rdf:resource="http://vcd.vicomtech.org/ontology/automotive#CuttingIn"/>
        <rdfs:range rdf:resource="http://vcd.vicomtech.org/ontology/automotive#CuttingOut"/>
        <rdfs:range rdf:resource="http://vcd.vicomtech.org/ontology/automotive#Decelerating"/>
        <rdfs:range rdf:resource="http://vcd.vicomtech.org/ontology/automotive#DrivingInOppositeDirection"/>
        <rdfs:range rdf:resource="http://vcd.vicomtech.org/ontology/automotive#DrivingStraight"/>
        <rdfs:range rdf:resource="http://vcd.vicomtech.org/ontology/automotive#FallingBehind"/>
        <rdfs:range rdf:resource="http://vcd.vicomtech.org/ontology/automotive#Following"/>
        <rdfs:range rdf:resource="http://vcd.vicomtech.org/ontology/automotive#GlidingOnWheels"/>
        <rdfs:range rdf:resource="http://vcd.vicomtech.org/ontology/automotive#LaneChanging"/>
        <rdfs:range rdf:resource="http://vcd.vicomtech.org/ontology/automotive#LaneChangingLeft"/>
        <rdfs:range rdf:resource="http://vcd.vicomtech.org/ontology/automotive#LaneChangingRight"/>
        <rdfs:range rdf:resource="http://vcd.vicomtech.org/ontology/automotive#LossingControl"/>
        <rdfs:range rdf:resource="http://vcd.vicomtech.org/ontology/automotive#Overtaking"/>
        <rdfs:range rdf:resource="http://vcd.vicomtech.org/ontology/automotive#Parking"/>
        <rdfs:range rdf:resource="http://vcd.vicomtech.org/ontology/automotive#Passing"/>
        <rdfs:range rdf:resource="http://vcd.vicomtech.org/ontology/automotive#Reversing"/>
        <rdfs:range rdf:resource="http://vcd.vicomtech.org/ontology/automotive#Stopping"/>
        <rdfs:range rdf:resource="http://vcd.vicomtech.org/ontology/automotive#Swerving"/>
        <rdfs:range rdf:resource="http://vcd.vicomtech.org/ontology/automotive#TrafficViolation"/>
        <rdfs:range rdf:resource="http://vcd.vicomtech.org/ontology/automotive#Turning"/>
        <rdfs:range rdf:resource="http://vcd.vicomtech.org/ontology/automotive#TurningLeft"/>
        <rdfs:range rdf:resource="http://vcd.vicomtech.org/ontology/automotive#TurningRight"/>
        <rdfs:range rdf:resource="http://vcd.vicomtech.org/ontology/automotive#UTurning"/>
        <rdfs:range rdf:resource="http://vcd.vicomtech.org/ontology/automotive#Unclassified"/>
        <rdfs:range rdf:resource="http://vcd.vicomtech.org/ontology/automotive#Waiting"/>
    </owl:ObjectProperty>
    


    <!-- http://vcd.vicomtech.org/ontology/automotive#isSubjectOfAction2 -->

    <owl:ObjectProperty rdf:about="http://vcd.vicomtech.org/ontology/automotive#isSubjectOfAction2">
        <rdfs:subPropertyOf rdf:resource="http://vcd.vicomtech.org/ontology/automotive#isSubjectOfAction"/>
        <rdfs:domain rdf:resource="http://vcd.vicomtech.org/ontology/automotive#Pedestrian"/>
        <rdfs:domain rdf:resource="http://vcd.vicomtech.org/ontology/automotive#PedestrianWithObject"/>
        <rdfs:range rdf:resource="http://vcd.vicomtech.org/ontology/automotive#Approaching"/>
        <rdfs:range rdf:resource="http://vcd.vicomtech.org/ontology/automotive#Blocking"/>
        <rdfs:range rdf:resource="http://vcd.vicomtech.org/ontology/automotive#Colliding"/>
        <rdfs:range rdf:resource="http://vcd.vicomtech.org/ontology/automotive#Crossing"/>
        <rdfs:range rdf:resource="http://vcd.vicomtech.org/ontology/automotive#FallingDown"/>
        <rdfs:range rdf:resource="http://vcd.vicomtech.org/ontology/automotive#Following"/>
        <rdfs:range rdf:resource="http://vcd.vicomtech.org/ontology/automotive#Passing"/>
        <rdfs:range rdf:resource="http://vcd.vicomtech.org/ontology/automotive#Rising"/>
        <rdfs:range rdf:resource="http://vcd.vicomtech.org/ontology/automotive#Running"/>
        <rdfs:range rdf:resource="http://vcd.vicomtech.org/ontology/automotive#Sitting"/>
        <rdfs:range rdf:resource="http://vcd.vicomtech.org/ontology/automotive#Standing"/>
        <rdfs:range rdf:resource="http://vcd.vicomtech.org/ontology/automotive#Standstill"/>
        <rdfs:range rdf:resource="http://vcd.vicomtech.org/ontology/automotive#Stopping"/>
        <rdfs:range rdf:resource="http://vcd.vicomtech.org/ontology/automotive#TrafficViolation"/>
        <rdfs:range rdf:resource="http://vcd.vicomtech.org/ontology/automotive#Waiting"/>
        <rdfs:range rdf:resource="http://vcd.vicomtech.org/ontology/automotive#Walking"/>
    </owl:ObjectProperty>
    


    <!-- http://vcd.vicomtech.org/ontology/automotive#isSubjectOfAction3 -->

    <owl:ObjectProperty rdf:about="http://vcd.vicomtech.org/ontology/automotive#isSubjectOfAction3">
        <rdfs:subPropertyOf rdf:resource="http://vcd.vicomtech.org/ontology/automotive#isSubjectOfAction"/>
        <rdfs:domain rdf:resource="http://vcd.vicomtech.org/ontology/automotive#Rider"/>
        <rdfs:range rdf:resource="http://vcd.vicomtech.org/ontology/automotive#Approaching"/>
        <rdfs:range rdf:resource="http://vcd.vicomtech.org/ontology/automotive#AvoidingCollision"/>
        <rdfs:range rdf:resource="http://vcd.vicomtech.org/ontology/automotive#Blocking"/>
        <rdfs:range rdf:resource="http://vcd.vicomtech.org/ontology/automotive#Colliding"/>
        <rdfs:range rdf:resource="http://vcd.vicomtech.org/ontology/automotive#Crossing"/>
        <rdfs:range rdf:resource="http://vcd.vicomtech.org/ontology/automotive#CuttingIn"/>
        <rdfs:range rdf:resource="http://vcd.vicomtech.org/ontology/automotive#CuttingOut"/>
        <rdfs:range rdf:resource="http://vcd.vicomtech.org/ontology/automotive#Decelerating"/>
        <rdfs:range rdf:resource="http://vcd.vicomtech.org/ontology/automotive#DrivingInOppositeDirection"/>
        <rdfs:range rdf:resource="http://vcd.vicomtech.org/ontology/automotive#DrivingStraight"/>
        <rdfs:range rdf:resource="http://vcd.vicomtech.org/ontology/automotive#FallingDown"/>
        <rdfs:range rdf:resource="http://vcd.vicomtech.org/ontology/automotive#Following"/>
        <rdfs:range rdf:resource="http://vcd.vicomtech.org/ontology/automotive#GlidingOnWheels"/>
        <rdfs:range rdf:resource="http://vcd.vicomtech.org/ontology/automotive#LaneChanging"/>
        <rdfs:range rdf:resource="http://vcd.vicomtech.org/ontology/automotive#LaneChangingLeft"/>
        <rdfs:range rdf:resource="http://vcd.vicomtech.org/ontology/automotive#LaneChangingRight"/>
        <rdfs:range rdf:resource="http://vcd.vicomtech.org/ontology/automotive#LossingControl"/>
        <rdfs:range rdf:resource="http://vcd.vicomtech.org/ontology/automotive#Overtaking"/>
        <rdfs:range rdf:resource="http://vcd.vicomtech.org/ontology/automotive#Parked"/>
        <rdfs:range rdf:resource="http://vcd.vicomtech.org/ontology/automotive#Passing"/>
        <rdfs:range rdf:resource="http://vcd.vicomtech.org/ontology/automotive#Reversing"/>
        <rdfs:range rdf:resource="http://vcd.vicomtech.org/ontology/automotive#Rising"/>
        <rdfs:range rdf:resource="http://vcd.vicomtech.org/ontology/automotive#Stopping"/>
        <rdfs:range rdf:resource="http://vcd.vicomtech.org/ontology/automotive#Swerving"/>
        <rdfs:range rdf:resource="http://vcd.vicomtech.org/ontology/automotive#TrafficViolation"/>
        <rdfs:range rdf:resource="http://vcd.vicomtech.org/ontology/automotive#Turning"/>
        <rdfs:range rdf:resource="http://vcd.vicomtech.org/ontology/automotive#TurningLeft"/>
        <rdfs:range rdf:resource="http://vcd.vicomtech.org/ontology/automotive#TurningRight"/>
        <rdfs:range rdf:resource="http://vcd.vicomtech.org/ontology/automotive#UTurning"/>
        <rdfs:range rdf:resource="http://vcd.vicomtech.org/ontology/automotive#Unclassified"/>
        <rdfs:range rdf:resource="http://vcd.vicomtech.org/ontology/automotive#Waiting"/>
    </owl:ObjectProperty>
    


    <!-- http://vcd.vicomtech.org/ontology/automotive#isSubjectOfAction4 -->

    <owl:ObjectProperty rdf:about="http://vcd.vicomtech.org/ontology/automotive#isSubjectOfAction4">
        <rdfs:subPropertyOf rdf:resource="http://vcd.vicomtech.org/ontology/automotive#isSubjectOfAction"/>
        <rdfs:domain rdf:resource="http://vcd.vicomtech.org/ontology/automotive#RailborneVehicle"/>
        <rdfs:range rdf:resource="http://vcd.vicomtech.org/ontology/automotive#Decelerating"/>
        <rdfs:range rdf:resource="http://vcd.vicomtech.org/ontology/automotive#DrivingInOppositeDirection"/>
        <rdfs:range rdf:resource="http://vcd.vicomtech.org/ontology/automotive#Following"/>
        <rdfs:range rdf:resource="http://vcd.vicomtech.org/ontology/automotive#Passing"/>
    </owl:ObjectProperty>
    


    <!-- http://vcd.vicomtech.org/ontology/automotive#isSubjectOfAction5 -->

    <owl:ObjectProperty rdf:about="http://vcd.vicomtech.org/ontology/automotive#isSubjectOfAction5">
        <rdfs:subPropertyOf rdf:resource="http://vcd.vicomtech.org/ontology/automotive#isSubjectOfAction"/>
        <rdfs:domain rdf:resource="http://vcd.vicomtech.org/ontology/automotive#Animal"/>
        <rdfs:domain rdf:resource="http://vcd.vicomtech.org/ontology/automotive#Pet"/>
        <rdfs:domain rdf:resource="http://vcd.vicomtech.org/ontology/automotive#Wildlife"/>
        <rdfs:range rdf:resource="http://vcd.vicomtech.org/ontology/automotive#Approaching"/>
        <rdfs:range rdf:resource="http://vcd.vicomtech.org/ontology/automotive#Blocking"/>
        <rdfs:range rdf:resource="http://vcd.vicomtech.org/ontology/automotive#Colliding"/>
        <rdfs:range rdf:resource="http://vcd.vicomtech.org/ontology/automotive#Crossing"/>
        <rdfs:range rdf:resource="http://vcd.vicomtech.org/ontology/automotive#FallingDown"/>
        <rdfs:range rdf:resource="http://vcd.vicomtech.org/ontology/automotive#Rising"/>
        <rdfs:range rdf:resource="http://vcd.vicomtech.org/ontology/automotive#Running"/>
        <rdfs:range rdf:resource="http://vcd.vicomtech.org/ontology/automotive#Sitting"/>
        <rdfs:range rdf:resource="http://vcd.vicomtech.org/ontology/automotive#Standing"/>
        <rdfs:range rdf:resource="http://vcd.vicomtech.org/ontology/automotive#Stopped"/>
        <rdfs:range rdf:resource="http://vcd.vicomtech.org/ontology/automotive#Stopping"/>
        <rdfs:range rdf:resource="http://vcd.vicomtech.org/ontology/automotive#TrafficViolation"/>
        <rdfs:range rdf:resource="http://vcd.vicomtech.org/ontology/automotive#Unclassified"/>
        <rdfs:range rdf:resource="http://vcd.vicomtech.org/ontology/automotive#Waiting"/>
        <rdfs:range rdf:resource="http://vcd.vicomtech.org/ontology/automotive#Walking"/>
    </owl:ObjectProperty>
    


    <!-- http://vcd.vicomtech.org/ontology/automotive#isSubjectOfEvent -->

    <owl:ObjectProperty rdf:about="http://vcd.vicomtech.org/ontology/automotive#isSubjectOfEvent">
        <rdfs:subPropertyOf rdf:resource="http://www.w3.org/2002/07/owl#topObjectProperty"/>
        <rdfs:domain rdf:resource="http://vcd.vicomtech.org/ontology/automotive#Object"/>
        <rdfs:range rdf:resource="http://vcd.vicomtech.org/ontology/automotive#Event"/>
        <rdfs:comment>States &apos;who&apos; permons an Event by relating the actor and the performed event.</rdfs:comment>
    </owl:ObjectProperty>
    


    <!-- http://vcd.vicomtech.org/ontology/automotive#isSubjectOfEvent1 -->

    <owl:ObjectProperty rdf:about="http://vcd.vicomtech.org/ontology/automotive#isSubjectOfEvent1">
        <rdfs:subPropertyOf rdf:resource="http://vcd.vicomtech.org/ontology/automotive#isSubjectOfEvent"/>
        <rdfs:domain rdf:resource="http://vcd.vicomtech.org/ontology/automotive#AnimalPulled"/>
        <rdfs:domain rdf:resource="http://vcd.vicomtech.org/ontology/automotive#Cycle"/>
        <rdfs:domain rdf:resource="http://vcd.vicomtech.org/ontology/automotive#DrivableVehicle"/>
        <rdfs:domain rdf:resource="http://vcd.vicomtech.org/ontology/automotive#WheeledSlow"/>
        <rdfs:range rdf:resource="http://vcd.vicomtech.org/ontology/automotive#Collision"/>
        <rdfs:range rdf:resource="http://vcd.vicomtech.org/ontology/automotive#LaneChange"/>
        <rdfs:range rdf:resource="http://vcd.vicomtech.org/ontology/automotive#Overtake"/>
        <rdfs:range rdf:resource="http://vcd.vicomtech.org/ontology/automotive#Park"/>
        <rdfs:range rdf:resource="http://vcd.vicomtech.org/ontology/automotive#Pass"/>
        <rdfs:range rdf:resource="http://vcd.vicomtech.org/ontology/automotive#Reach"/>
        <rdfs:range rdf:resource="http://vcd.vicomtech.org/ontology/automotive#SafeStop"/>
        <rdfs:range rdf:resource="http://vcd.vicomtech.org/ontology/automotive#Swerve"/>
        <rdfs:range rdf:resource="http://vcd.vicomtech.org/ontology/automotive#Turn"/>
    </owl:ObjectProperty>
    


    <!-- http://vcd.vicomtech.org/ontology/automotive#isSubjectOfEvent2 -->

    <owl:ObjectProperty rdf:about="http://vcd.vicomtech.org/ontology/automotive#isSubjectOfEvent2">
        <rdfs:subPropertyOf rdf:resource="http://vcd.vicomtech.org/ontology/automotive#isSubjectOfEvent"/>
        <rdfs:domain rdf:resource="http://vcd.vicomtech.org/ontology/automotive#TrafficLight"/>
        <rdfs:range rdf:resource="http://vcd.vicomtech.org/ontology/automotive#ChangeState"/>
        <rdfs:range rdf:resource="http://vcd.vicomtech.org/ontology/automotive#ChangeTrafficLightState"/>
    </owl:ObjectProperty>
    


    <!-- http://vcd.vicomtech.org/ontology/automotive#isSubjectOfEvent3 -->

    <owl:ObjectProperty rdf:about="http://vcd.vicomtech.org/ontology/automotive#isSubjectOfEvent3">
        <rdfs:subPropertyOf rdf:resource="http://vcd.vicomtech.org/ontology/automotive#isSubjectOfEvent"/>
        <rdfs:domain rdf:resource="http://vcd.vicomtech.org/ontology/automotive#Pedestrian"/>
        <rdfs:domain rdf:resource="http://vcd.vicomtech.org/ontology/automotive#PedestrianWithObject"/>
        <rdfs:range rdf:resource="http://vcd.vicomtech.org/ontology/automotive#Collision"/>
        <rdfs:range rdf:resource="http://vcd.vicomtech.org/ontology/automotive#Cross"/>
        <rdfs:range rdf:resource="http://vcd.vicomtech.org/ontology/automotive#Fall"/>
        <rdfs:range rdf:resource="http://vcd.vicomtech.org/ontology/automotive#LaneChange"/>
        <rdfs:range rdf:resource="http://vcd.vicomtech.org/ontology/automotive#Pass"/>
        <rdfs:range rdf:resource="http://vcd.vicomtech.org/ontology/automotive#Reach"/>
        <rdfs:range rdf:resource="http://vcd.vicomtech.org/ontology/automotive#Rise"/>
        <rdfs:range rdf:resource="http://vcd.vicomtech.org/ontology/automotive#Turn"/>
    </owl:ObjectProperty>
    


    <!-- http://vcd.vicomtech.org/ontology/automotive#isSubjectOfEvent4 -->

    <owl:ObjectProperty rdf:about="http://vcd.vicomtech.org/ontology/automotive#isSubjectOfEvent4">
        <rdfs:subPropertyOf rdf:resource="http://vcd.vicomtech.org/ontology/automotive#isSubjectOfEvent"/>
        <rdfs:domain rdf:resource="http://vcd.vicomtech.org/ontology/automotive#InVehicleSystems"/>
        <rdfs:domain rdf:resource="http://vcd.vicomtech.org/ontology/automotive#Sensor"/>
        <rdfs:range rdf:resource="http://vcd.vicomtech.org/ontology/automotive#Detect"/>
    </owl:ObjectProperty>
    


    <!-- http://vcd.vicomtech.org/ontology/automotive#leftOf -->

    <owl:ObjectProperty rdf:about="http://vcd.vicomtech.org/ontology/automotive#leftOf">
        <rdfs:subPropertyOf rdf:resource="http://www.w3.org/2002/07/owl#topObjectProperty"/>
        <owl:inverseOf rdf:resource="http://vcd.vicomtech.org/ontology/automotive#rightOf"/>
        <rdfs:domain rdf:resource="http://vcd.vicomtech.org/ontology/automotive#Animal"/>
        <rdfs:domain rdf:resource="http://vcd.vicomtech.org/ontology/automotive#Barrier"/>
        <rdfs:domain rdf:resource="http://vcd.vicomtech.org/ontology/automotive#Flat"/>
        <rdfs:domain rdf:resource="http://vcd.vicomtech.org/ontology/automotive#Human"/>
        <rdfs:domain rdf:resource="http://vcd.vicomtech.org/ontology/automotive#Junction"/>
        <rdfs:domain rdf:resource="http://vcd.vicomtech.org/ontology/automotive#MovableObject"/>
        <rdfs:domain rdf:resource="http://vcd.vicomtech.org/ontology/automotive#RoadVehicle"/>
        <rdfs:domain rdf:resource="http://vcd.vicomtech.org/ontology/automotive#RoadsideObject"/>
        <rdfs:domain rdf:resource="http://vcd.vicomtech.org/ontology/automotive#Structure"/>
        <rdfs:range rdf:resource="http://vcd.vicomtech.org/ontology/automotive#Animal"/>
        <rdfs:range rdf:resource="http://vcd.vicomtech.org/ontology/automotive#Barrier"/>
        <rdfs:range rdf:resource="http://vcd.vicomtech.org/ontology/automotive#Flat"/>
        <rdfs:range rdf:resource="http://vcd.vicomtech.org/ontology/automotive#Human"/>
        <rdfs:range rdf:resource="http://vcd.vicomtech.org/ontology/automotive#Junction"/>
        <rdfs:range rdf:resource="http://vcd.vicomtech.org/ontology/automotive#MovableObject"/>
        <rdfs:range rdf:resource="http://vcd.vicomtech.org/ontology/automotive#RoadVehicle"/>
        <rdfs:range rdf:resource="http://vcd.vicomtech.org/ontology/automotive#RoadsideObject"/>
        <rdfs:range rdf:resource="http://vcd.vicomtech.org/ontology/automotive#Structure"/>
        <rdfs:comment>Indicates a spatial relation among objects by stating that one of the objects is at the left of the other.</rdfs:comment>
    </owl:ObjectProperty>
    


    <!-- http://vcd.vicomtech.org/ontology/automotive#meets -->

    <owl:ObjectProperty rdf:about="http://vcd.vicomtech.org/ontology/automotive#meets">
        <rdfs:subPropertyOf rdf:resource="http://www.w3.org/2002/07/owl#topObjectProperty"/>
        <rdfs:domain rdf:resource="http://vcd.vicomtech.org/ontology/automotive#Action"/>
        <rdfs:domain rdf:resource="http://vcd.vicomtech.org/ontology/automotive#Event"/>
        <rdfs:range rdf:resource="http://vcd.vicomtech.org/ontology/automotive#Action"/>
        <rdfs:range rdf:resource="http://vcd.vicomtech.org/ontology/automotive#Event"/>
    </owl:ObjectProperty>
    


    <!-- http://vcd.vicomtech.org/ontology/automotive#middleOf -->

    <owl:ObjectProperty rdf:about="http://vcd.vicomtech.org/ontology/automotive#middleOf">
        <rdfs:subPropertyOf rdf:resource="http://www.w3.org/2002/07/owl#topObjectProperty"/>
        <rdfs:domain rdf:resource="http://vcd.vicomtech.org/ontology/automotive#Animal"/>
        <rdfs:domain rdf:resource="http://vcd.vicomtech.org/ontology/automotive#Barrier"/>
        <rdfs:domain rdf:resource="http://vcd.vicomtech.org/ontology/automotive#Flat"/>
        <rdfs:domain rdf:resource="http://vcd.vicomtech.org/ontology/automotive#Human"/>
        <rdfs:domain rdf:resource="http://vcd.vicomtech.org/ontology/automotive#Junction"/>
        <rdfs:domain rdf:resource="http://vcd.vicomtech.org/ontology/automotive#MovableObject"/>
        <rdfs:domain rdf:resource="http://vcd.vicomtech.org/ontology/automotive#RoadVehicle"/>
        <rdfs:domain rdf:resource="http://vcd.vicomtech.org/ontology/automotive#RoadsideObject"/>
        <rdfs:domain rdf:resource="http://vcd.vicomtech.org/ontology/automotive#Structure"/>
        <rdfs:range rdf:resource="http://vcd.vicomtech.org/ontology/automotive#Animal"/>
        <rdfs:range rdf:resource="http://vcd.vicomtech.org/ontology/automotive#Barrier"/>
        <rdfs:range rdf:resource="http://vcd.vicomtech.org/ontology/automotive#Flat"/>
        <rdfs:range rdf:resource="http://vcd.vicomtech.org/ontology/automotive#Human"/>
        <rdfs:range rdf:resource="http://vcd.vicomtech.org/ontology/automotive#Junction"/>
        <rdfs:range rdf:resource="http://vcd.vicomtech.org/ontology/automotive#MovableObject"/>
        <rdfs:range rdf:resource="http://vcd.vicomtech.org/ontology/automotive#RoadVehicle"/>
        <rdfs:range rdf:resource="http://vcd.vicomtech.org/ontology/automotive#RoadsideObject"/>
        <rdfs:range rdf:resource="http://vcd.vicomtech.org/ontology/automotive#Structure"/>
        <rdfs:comment>Indicates a spatial relation among objects by stating that one of the objects is in the middle of the other.</rdfs:comment>
    </owl:ObjectProperty>
    


    <!-- http://vcd.vicomtech.org/ontology/automotive#overlaps -->

    <owl:ObjectProperty rdf:about="http://vcd.vicomtech.org/ontology/automotive#overlaps">
        <rdfs:subPropertyOf rdf:resource="http://www.w3.org/2002/07/owl#topObjectProperty"/>
        <rdfs:domain rdf:resource="http://vcd.vicomtech.org/ontology/automotive#Action"/>
        <rdfs:domain rdf:resource="http://vcd.vicomtech.org/ontology/automotive#Event"/>
        <rdfs:range rdf:resource="http://vcd.vicomtech.org/ontology/automotive#Action"/>
        <rdfs:range rdf:resource="http://vcd.vicomtech.org/ontology/automotive#Event"/>
    </owl:ObjectProperty>
    


    <!-- http://vcd.vicomtech.org/ontology/automotive#rightOf -->

    <owl:ObjectProperty rdf:about="http://vcd.vicomtech.org/ontology/automotive#rightOf">
        <rdfs:subPropertyOf rdf:resource="http://www.w3.org/2002/07/owl#topObjectProperty"/>
        <rdfs:domain rdf:resource="http://vcd.vicomtech.org/ontology/automotive#Animal"/>
        <rdfs:domain rdf:resource="http://vcd.vicomtech.org/ontology/automotive#Barrier"/>
        <rdfs:domain rdf:resource="http://vcd.vicomtech.org/ontology/automotive#Flat"/>
        <rdfs:domain rdf:resource="http://vcd.vicomtech.org/ontology/automotive#Human"/>
        <rdfs:domain rdf:resource="http://vcd.vicomtech.org/ontology/automotive#Junction"/>
        <rdfs:domain rdf:resource="http://vcd.vicomtech.org/ontology/automotive#MovableObject"/>
        <rdfs:domain rdf:resource="http://vcd.vicomtech.org/ontology/automotive#RoadVehicle"/>
        <rdfs:domain rdf:resource="http://vcd.vicomtech.org/ontology/automotive#RoadsideObject"/>
        <rdfs:domain rdf:resource="http://vcd.vicomtech.org/ontology/automotive#Structure"/>
        <rdfs:range rdf:resource="http://vcd.vicomtech.org/ontology/automotive#Animal"/>
        <rdfs:range rdf:resource="http://vcd.vicomtech.org/ontology/automotive#Barrier"/>
        <rdfs:range rdf:resource="http://vcd.vicomtech.org/ontology/automotive#Flat"/>
        <rdfs:range rdf:resource="http://vcd.vicomtech.org/ontology/automotive#Human"/>
        <rdfs:range rdf:resource="http://vcd.vicomtech.org/ontology/automotive#Junction"/>
        <rdfs:range rdf:resource="http://vcd.vicomtech.org/ontology/automotive#MovableObject"/>
        <rdfs:range rdf:resource="http://vcd.vicomtech.org/ontology/automotive#RoadVehicle"/>
        <rdfs:range rdf:resource="http://vcd.vicomtech.org/ontology/automotive#RoadsideObject"/>
        <rdfs:range rdf:resource="http://vcd.vicomtech.org/ontology/automotive#Structure"/>
        <rdfs:comment>Indicates a spatial relation among objects by stating that one of the objects is at the right of the other.</rdfs:comment>
    </owl:ObjectProperty>
    


    <!-- http://vcd.vicomtech.org/ontology/automotive#starts -->

    <owl:ObjectProperty rdf:about="http://vcd.vicomtech.org/ontology/automotive#starts">
        <rdfs:subPropertyOf rdf:resource="http://www.w3.org/2002/07/owl#topObjectProperty"/>
        <rdfs:domain rdf:resource="http://vcd.vicomtech.org/ontology/automotive#Action"/>
        <rdfs:domain rdf:resource="http://vcd.vicomtech.org/ontology/automotive#Event"/>
        <rdfs:range rdf:resource="http://vcd.vicomtech.org/ontology/automotive#Action"/>
        <rdfs:range rdf:resource="http://vcd.vicomtech.org/ontology/automotive#Event"/>
    </owl:ObjectProperty>
    


    <!-- 
    ///////////////////////////////////////////////////////////////////////////////////////
    //
    // Data properties
    //
    ///////////////////////////////////////////////////////////////////////////////////////
     -->

    


    <!-- http://vcd.vicomtech.org/ontology/automotive#hasAcceleration -->

    <owl:DatatypeProperty rdf:about="http://vcd.vicomtech.org/ontology/automotive#hasAcceleration">
        <rdfs:subPropertyOf rdf:resource="http://www.w3.org/2002/07/owl#topDataProperty"/>
        <rdfs:domain rdf:resource="http://vcd.vicomtech.org/ontology/automotive#Animal"/>
        <rdfs:domain rdf:resource="http://vcd.vicomtech.org/ontology/automotive#Human"/>
        <rdfs:domain rdf:resource="http://vcd.vicomtech.org/ontology/automotive#RoadVehicle"/>
        <rdfs:domain rdf:resource="http://vcd.vicomtech.org/ontology/automotive#Train"/>
        <rdfs:range rdf:resource="http://www.w3.org/2001/XMLSchema#int"/>
        <rdfs:comment>Acceleration is the rate of change of velocity as a function of time.</rdfs:comment>
    </owl:DatatypeProperty>
    


    <!-- http://vcd.vicomtech.org/ontology/automotive#hasCapacity -->

    <owl:DatatypeProperty rdf:about="http://vcd.vicomtech.org/ontology/automotive#hasCapacity">
        <owl:equivalentProperty rdf:resource="http://vcd.vicomtech.org/ontology/automotive#hasVehicleDensity"/>
        <rdfs:subPropertyOf rdf:resource="http://www.w3.org/2002/07/owl#topDataProperty"/>
        <rdfs:domain rdf:resource="http://vcd.vicomtech.org/ontology/automotive#Lane"/>
        <rdfs:domain rdf:resource="http://vcd.vicomtech.org/ontology/automotive#ParkingLot"/>
        <rdfs:domain rdf:resource="http://vcd.vicomtech.org/ontology/automotive#Road"/>
        <rdfs:range rdf:resource="http://www.w3.org/2001/XMLSchema#int"/>
        <rdfs:comment>The maximum traffic flow obtainable on a given roadway using all available lanes; usually expressed in vehicles per hour or vehicles per day.</rdfs:comment>
    </owl:DatatypeProperty>
    


    <!-- http://vcd.vicomtech.org/ontology/automotive#hasColor -->

    <owl:DatatypeProperty rdf:about="http://vcd.vicomtech.org/ontology/automotive#hasColor">
        <rdfs:subPropertyOf rdf:resource="http://www.w3.org/2002/07/owl#topDataProperty"/>
        <rdfs:domain rdf:resource="http://vcd.vicomtech.org/ontology/automotive#Marking"/>
        <rdfs:domain rdf:resource="http://vcd.vicomtech.org/ontology/automotive#Vehicle"/>
        <rdfs:range rdf:resource="http://www.w3.org/2001/XMLSchema#string"/>
        <rdfs:comment>Color is defined as the quality of an object or substance with respect to light reflected by the object, usually determined visually by measurement of hue, saturation or chroma.</rdfs:comment>
    </owl:DatatypeProperty>
    


    <!-- http://vcd.vicomtech.org/ontology/automotive#hasController -->

    <owl:DatatypeProperty rdf:about="http://vcd.vicomtech.org/ontology/automotive#hasController">
        <rdfs:subPropertyOf rdf:resource="http://www.w3.org/2002/07/owl#topDataProperty"/>
        <rdfs:domain rdf:resource="http://vcd.vicomtech.org/ontology/automotive#Animal"/>
        <rdfs:domain rdf:resource="http://vcd.vicomtech.org/ontology/automotive#Human"/>
        <rdfs:domain rdf:resource="http://vcd.vicomtech.org/ontology/automotive#Vehicle"/>
        <rdfs:range rdf:resource="http://www.w3.org/2001/XMLSchema#string"/>
        <rdfs:comment>Controller are elements of the simulation core that control the motion of ScenarioObject (OpenSCENARIO context).</rdfs:comment>
    </owl:DatatypeProperty>
    


    <!-- http://vcd.vicomtech.org/ontology/automotive#hasCoordinateSystem -->

    <owl:DatatypeProperty rdf:about="http://vcd.vicomtech.org/ontology/automotive#hasCoordinateSystem">
        <rdfs:subPropertyOf rdf:resource="http://www.w3.org/2002/07/owl#topDataProperty"/>
        <rdfs:domain rdf:resource="http://vcd.vicomtech.org/ontology/automotive#Action"/>
        <rdfs:domain rdf:resource="http://vcd.vicomtech.org/ontology/automotive#Context"/>
        <rdfs:domain rdf:resource="http://vcd.vicomtech.org/ontology/automotive#Event"/>
        <rdfs:domain rdf:resource="http://vcd.vicomtech.org/ontology/automotive#Object"/>
        <rdfs:range rdf:resource="http://vcd.vicomtech.org/ontology/automotive#array"/>
        <rdfs:comment>In geometry, a coordinate system is a system that uses one or more numbers, or coordinates, to uniquely determine the position of the points or other geometric elements on a manifold such as Euclidean space.</rdfs:comment>
    </owl:DatatypeProperty>
    


    <!-- http://vcd.vicomtech.org/ontology/automotive#hasCurvature -->

    <owl:DatatypeProperty rdf:about="http://vcd.vicomtech.org/ontology/automotive#hasCurvature">
        <rdfs:subPropertyOf rdf:resource="http://www.w3.org/2002/07/owl#topDataProperty"/>
        <rdfs:domain rdf:resource="http://vcd.vicomtech.org/ontology/automotive#Curve"/>
        <rdfs:domain rdf:resource="http://vcd.vicomtech.org/ontology/automotive#Lane"/>
        <rdfs:domain rdf:resource="http://vcd.vicomtech.org/ontology/automotive#RailTrack"/>
        <rdfs:domain rdf:resource="http://vcd.vicomtech.org/ontology/automotive#Road"/>
        <rdfs:range rdf:resource="http://www.w3.org/2001/XMLSchema#int"/>
        <rdfs:comment>The fact of being curved or the degree to which something is curved.</rdfs:comment>
    </owl:DatatypeProperty>
    


    <!-- http://vcd.vicomtech.org/ontology/automotive#hasDeceleration -->

    <owl:DatatypeProperty rdf:about="http://vcd.vicomtech.org/ontology/automotive#hasDeceleration">
        <rdfs:subPropertyOf rdf:resource="http://www.w3.org/2002/07/owl#topDataProperty"/>
        <rdfs:domain rdf:resource="http://vcd.vicomtech.org/ontology/automotive#Animal"/>
        <rdfs:domain rdf:resource="http://vcd.vicomtech.org/ontology/automotive#Human"/>
        <rdfs:domain rdf:resource="http://vcd.vicomtech.org/ontology/automotive#RoadVehicle"/>
        <rdfs:domain rdf:resource="http://vcd.vicomtech.org/ontology/automotive#Train"/>
        <rdfs:range rdf:resource="http://www.w3.org/2001/XMLSchema#int"/>
        <rdfs:comment>Reduction in speed or rate.</rdfs:comment>
    </owl:DatatypeProperty>
    


    <!-- http://vcd.vicomtech.org/ontology/automotive#hasDegree -->

    <owl:DatatypeProperty rdf:about="http://vcd.vicomtech.org/ontology/automotive#hasDegree">
        <rdfs:subPropertyOf rdf:resource="http://www.w3.org/2002/07/owl#topDataProperty"/>
        <rdfs:domain rdf:resource="http://vcd.vicomtech.org/ontology/automotive#Temperature"/>
        <rdfs:range rdf:resource="http://www.w3.org/2001/XMLSchema#int"/>
        <rdfs:comment>The amount, level, or extent to which something happens or is present.</rdfs:comment>
    </owl:DatatypeProperty>
    


    <!-- http://vcd.vicomtech.org/ontology/automotive#hasDetectionRange -->

    <owl:DatatypeProperty rdf:about="http://vcd.vicomtech.org/ontology/automotive#hasDetectionRange">
        <rdfs:subPropertyOf rdf:resource="http://www.w3.org/2002/07/owl#topDataProperty"/>
        <rdfs:domain rdf:resource="http://vcd.vicomtech.org/ontology/automotive#InVehicleSystems"/>
        <rdfs:range rdf:resource="http://www.w3.org/2001/XMLSchema#int"/>
        <rdfs:comment>&quot;Detection range&quot; of the sensing system is the distance at which the system can reliably recognise a target, taking account of the deterioration of components of the sensing system due to time and usage throughout the lifetime of the vehicle and generate a control signal.</rdfs:comment>
    </owl:DatatypeProperty>
    


    <!-- http://vcd.vicomtech.org/ontology/automotive#hasFailure -->

    <owl:DatatypeProperty rdf:about="http://vcd.vicomtech.org/ontology/automotive#hasFailure">
        <rdfs:subPropertyOf rdf:resource="http://www.w3.org/2002/07/owl#topDataProperty"/>
        <rdfs:domain rdf:resource="http://vcd.vicomtech.org/ontology/automotive#ALKS"/>
        <rdfs:domain rdf:resource="http://vcd.vicomtech.org/ontology/automotive#InVehicleSystems"/>
        <rdfs:domain rdf:resource="http://vcd.vicomtech.org/ontology/automotive#Sensor"/>
        <rdfs:range rdf:resource="http://www.w3.org/2001/XMLSchema#boolean"/>
        <rdfs:comment>Is any single failure specific to the operation of the system (e.g. single sensor failure, loss of necessary calculation data for the driving path of the vehicle).</rdfs:comment>
    </owl:DatatypeProperty>
    


    <!-- http://vcd.vicomtech.org/ontology/automotive#hasFrameIntervals -->

    <owl:DatatypeProperty rdf:about="http://vcd.vicomtech.org/ontology/automotive#hasFrameIntervals">
        <rdfs:subPropertyOf rdf:resource="http://www.w3.org/2002/07/owl#topDataProperty"/>
        <rdfs:domain rdf:resource="http://vcd.vicomtech.org/ontology/automotive#Action"/>
        <rdfs:domain rdf:resource="http://vcd.vicomtech.org/ontology/automotive#Context"/>
        <rdfs:domain rdf:resource="http://vcd.vicomtech.org/ontology/automotive#Event"/>
        <rdfs:domain rdf:resource="http://vcd.vicomtech.org/ontology/automotive#Object"/>
        <rdfs:range rdf:resource="http://vcd.vicomtech.org/ontology/automotive#array"/>
        <rdfs:comment>The number of partial frames that occur between full frames in the video stream.</rdfs:comment>
    </owl:DatatypeProperty>
    


    <!-- http://vcd.vicomtech.org/ontology/automotive#hasFrictionCoefficient -->

    <owl:DatatypeProperty rdf:about="http://vcd.vicomtech.org/ontology/automotive#hasFrictionCoefficient">
        <rdfs:subPropertyOf rdf:resource="http://www.w3.org/2002/07/owl#topDataProperty"/>
        <rdfs:domain rdf:resource="http://vcd.vicomtech.org/ontology/automotive#Road"/>
        <rdfs:range rdf:resource="http://www.w3.org/2001/XMLSchema#int"/>
        <rdfs:comment>Is defined as the ratio of the force required to move tow sliding surfaces over each other, and the force holding them together.</rdfs:comment>
    </owl:DatatypeProperty>
    


    <!-- http://vcd.vicomtech.org/ontology/automotive#hasGender -->

    <owl:DatatypeProperty rdf:about="http://vcd.vicomtech.org/ontology/automotive#hasGender">
        <rdfs:subPropertyOf rdf:resource="http://www.w3.org/2002/07/owl#topDataProperty"/>
        <rdfs:domain rdf:resource="http://vcd.vicomtech.org/ontology/automotive#Human"/>
        <rdfs:range rdf:resource="http://www.w3.org/2001/XMLSchema#string"/>
        <rdfs:comment>Either of the two sexes (male and female), especially when considered with reference to social and cultural differences rather than biological ones. The term is also used more broadly to denote a range of identities that do not correspond to established ideas of male and female.</rdfs:comment>
    </owl:DatatypeProperty>
    


    <!-- http://vcd.vicomtech.org/ontology/automotive#hasGeometry -->

    <owl:DatatypeProperty rdf:about="http://vcd.vicomtech.org/ontology/automotive#hasGeometry">
        <rdfs:subPropertyOf rdf:resource="http://www.w3.org/2002/07/owl#topDataProperty"/>
        <rdfs:domain rdf:resource="http://vcd.vicomtech.org/ontology/automotive#Road"/>
        <rdfs:range rdf:resource="http://www.w3.org/2001/XMLSchema#string"/>
        <rdfs:comment>The shape and realtive arrangement of the parts of something. In the automotive context usually the road.</rdfs:comment>
    </owl:DatatypeProperty>
    


    <!-- http://vcd.vicomtech.org/ontology/automotive#hasHeading -->

    <owl:DatatypeProperty rdf:about="http://vcd.vicomtech.org/ontology/automotive#hasHeading">
        <rdfs:subPropertyOf rdf:resource="http://www.w3.org/2002/07/owl#topDataProperty"/>
        <rdfs:domain rdf:resource="http://vcd.vicomtech.org/ontology/automotive#Animal"/>
        <rdfs:domain rdf:resource="http://vcd.vicomtech.org/ontology/automotive#Human"/>
        <rdfs:domain rdf:resource="http://vcd.vicomtech.org/ontology/automotive#Vehicle"/>
        <rdfs:range rdf:resource="http://www.w3.org/2001/XMLSchema#int"/>
        <rdfs:comment>A direction or bearing an object is following.</rdfs:comment>
    </owl:DatatypeProperty>
    


    <!-- http://vcd.vicomtech.org/ontology/automotive#hasHeadway -->

    <owl:DatatypeProperty rdf:about="http://vcd.vicomtech.org/ontology/automotive#hasHeadway">
        <rdfs:subPropertyOf rdf:resource="http://www.w3.org/2002/07/owl#topDataProperty"/>
        <rdfs:domain rdf:resource="http://vcd.vicomtech.org/ontology/automotive#Following"/>
        <rdfs:range rdf:resource="http://www.w3.org/2001/XMLSchema#int"/>
        <rdfs:comment>Is the distance between vehicles in a transit system measured in time or space.</rdfs:comment>
    </owl:DatatypeProperty>
    


    <!-- http://vcd.vicomtech.org/ontology/automotive#hasIntensity -->

    <owl:DatatypeProperty rdf:about="http://vcd.vicomtech.org/ontology/automotive#hasIntensity">
        <rdfs:subPropertyOf rdf:resource="http://www.w3.org/2002/07/owl#topDataProperty"/>
        <rdfs:domain rdf:resource="http://vcd.vicomtech.org/ontology/automotive#Lighting"/>
        <rdfs:range rdf:resource="http://www.w3.org/2001/XMLSchema#int"/>
        <rdfs:comment>The measurable amount of a property, such as force, brightness, or a magnetic field.</rdfs:comment>
    </owl:DatatypeProperty>
    


    <!-- http://vcd.vicomtech.org/ontology/automotive#hasLaneId -->

    <owl:DatatypeProperty rdf:about="http://vcd.vicomtech.org/ontology/automotive#hasLaneId">
        <rdfs:subPropertyOf rdf:resource="http://www.w3.org/2002/07/owl#topDataProperty"/>
        <rdfs:domain rdf:resource="http://vcd.vicomtech.org/ontology/automotive#Lane"/>
        <rdfs:range rdf:resource="http://www.w3.org/2001/XMLSchema#int"/>
        <rdfs:comment>Unique id of the lanes as defined in OpenSCENARIO (OSC).</rdfs:comment>
    </owl:DatatypeProperty>
    


    <!-- http://vcd.vicomtech.org/ontology/automotive#hasLanePosition -->

    <owl:DatatypeProperty rdf:about="http://vcd.vicomtech.org/ontology/automotive#hasLanePosition">
        <rdfs:subPropertyOf rdf:resource="http://www.w3.org/2002/07/owl#topDataProperty"/>
        <rdfs:domain rdf:resource="http://vcd.vicomtech.org/ontology/automotive#Lane"/>
        <rdfs:range rdf:resource="http://www.w3.org/2001/XMLSchema#string"/>
        <rdfs:range>
            <rdfs:Datatype>
                <owl:oneOf>
                    <rdf:Description>
                        <rdf:type rdf:resource="http://www.w3.org/1999/02/22-rdf-syntax-ns#List"/>
                        <rdf:first>Left</rdf:first>
                        <rdf:rest>
                            <rdf:Description>
                                <rdf:type rdf:resource="http://www.w3.org/1999/02/22-rdf-syntax-ns#List"/>
                                <rdf:first>Middle</rdf:first>
                                <rdf:rest>
                                    <rdf:Description>
                                        <rdf:type rdf:resource="http://www.w3.org/1999/02/22-rdf-syntax-ns#List"/>
                                        <rdf:first>Right</rdf:first>
                                        <rdf:rest rdf:resource="http://www.w3.org/1999/02/22-rdf-syntax-ns#nil"/>
                                    </rdf:Description>
                                </rdf:rest>
                            </rdf:Description>
                        </rdf:rest>
                    </rdf:Description>
                </owl:oneOf>
            </rdfs:Datatype>
        </rdfs:range>
        <rdfs:comment>Refers to the relative position of an object in the lane: left, middle, right. Could be defined according to the lateral distance.</rdfs:comment>
    </owl:DatatypeProperty>
    


    <!-- http://vcd.vicomtech.org/ontology/automotive#hasLateralDistance -->

    <owl:DatatypeProperty rdf:about="http://vcd.vicomtech.org/ontology/automotive#hasLateralDistance">
        <rdfs:subPropertyOf rdf:resource="http://www.w3.org/2002/07/owl#topDataProperty"/>
        <rdfs:domain rdf:resource="http://vcd.vicomtech.org/ontology/automotive#Animal"/>
        <rdfs:domain rdf:resource="http://vcd.vicomtech.org/ontology/automotive#Human"/>
        <rdfs:domain rdf:resource="http://vcd.vicomtech.org/ontology/automotive#RoadVehicle"/>
        <rdfs:range rdf:resource="http://www.w3.org/2001/XMLSchema#int"/>
        <rdfs:comment>Defines the horizontal distance between consecutive objects. Could be also refered in reference to the reference line of the road.</rdfs:comment>
    </owl:DatatypeProperty>
    


    <!-- http://vcd.vicomtech.org/ontology/automotive#hasLateralSpeed -->

    <owl:DatatypeProperty rdf:about="http://vcd.vicomtech.org/ontology/automotive#hasLateralSpeed">
        <rdfs:subPropertyOf rdf:resource="http://www.w3.org/2002/07/owl#topDataProperty"/>
        <rdfs:domain rdf:resource="http://vcd.vicomtech.org/ontology/automotive#Animal"/>
        <rdfs:domain rdf:resource="http://vcd.vicomtech.org/ontology/automotive#Human"/>
        <rdfs:domain rdf:resource="http://vcd.vicomtech.org/ontology/automotive#RoadVehicle"/>
        <rdfs:domain rdf:resource="http://vcd.vicomtech.org/ontology/automotive#Train"/>
        <rdfs:range rdf:resource="http://www.w3.org/2001/XMLSchema#int"/>
        <rdfs:comment>The lateral velocity is the component of velocity moving perpendicular to forwards.</rdfs:comment>
    </owl:DatatypeProperty>
    


    <!-- http://vcd.vicomtech.org/ontology/automotive#hasLength -->

    <owl:DatatypeProperty rdf:about="http://vcd.vicomtech.org/ontology/automotive#hasLength">
        <rdfs:subPropertyOf rdf:resource="http://www.w3.org/2002/07/owl#topDataProperty"/>
        <rdfs:domain rdf:resource="http://vcd.vicomtech.org/ontology/automotive#DrivableVehicle"/>
        <rdfs:domain rdf:resource="http://vcd.vicomtech.org/ontology/automotive#Road"/>
        <rdfs:range rdf:resource="http://www.w3.org/2001/XMLSchema#int"/>
        <rdfs:comment>The measurement or extent of something from end to end; the greater of two or the greatest of three dimensions of an object.</rdfs:comment>
    </owl:DatatypeProperty>
    


    <!-- http://vcd.vicomtech.org/ontology/automotive#hasLongitudinalDistance -->

    <owl:DatatypeProperty rdf:about="http://vcd.vicomtech.org/ontology/automotive#hasLongitudinalDistance">
        <owl:equivalentProperty rdf:resource="http://vcd.vicomtech.org/ontology/automotive#hasS"/>
        <rdfs:subPropertyOf rdf:resource="http://www.w3.org/2002/07/owl#topDataProperty"/>
        <rdfs:domain rdf:resource="http://vcd.vicomtech.org/ontology/automotive#Animal"/>
        <rdfs:domain rdf:resource="http://vcd.vicomtech.org/ontology/automotive#Human"/>
        <rdfs:domain rdf:resource="http://vcd.vicomtech.org/ontology/automotive#RoadVehicle"/>
        <rdfs:range rdf:resource="http://www.w3.org/2001/XMLSchema#int"/>
        <rdfs:comment>The perpendicular distance from a vehicle to the leading vehicle.</rdfs:comment>
    </owl:DatatypeProperty>
    


    <!-- http://vcd.vicomtech.org/ontology/automotive#hasLongitudinalSpeed -->

    <owl:DatatypeProperty rdf:about="http://vcd.vicomtech.org/ontology/automotive#hasLongitudinalSpeed">
        <rdfs:subPropertyOf rdf:resource="http://www.w3.org/2002/07/owl#topDataProperty"/>
        <rdfs:domain rdf:resource="http://vcd.vicomtech.org/ontology/automotive#Animal"/>
        <rdfs:domain rdf:resource="http://vcd.vicomtech.org/ontology/automotive#Human"/>
        <rdfs:domain rdf:resource="http://vcd.vicomtech.org/ontology/automotive#RoadVehicle"/>
        <rdfs:domain rdf:resource="http://vcd.vicomtech.org/ontology/automotive#Train"/>
        <rdfs:range rdf:resource="http://www.w3.org/2001/XMLSchema#int"/>
    </owl:DatatypeProperty>
    


    <!-- http://vcd.vicomtech.org/ontology/automotive#hasManufacturer -->

    <owl:DatatypeProperty rdf:about="http://vcd.vicomtech.org/ontology/automotive#hasManufacturer">
        <rdfs:subPropertyOf rdf:resource="http://www.w3.org/2002/07/owl#topDataProperty"/>
        <rdfs:domain rdf:resource="http://vcd.vicomtech.org/ontology/automotive#RoadVehicle"/>
        <rdfs:range rdf:resource="http://www.w3.org/2001/XMLSchema#string"/>
        <rdfs:comment>The person or company that makes an object for sale. In this context refering to vehicle manufacturers.</rdfs:comment>
    </owl:DatatypeProperty>
    


    <!-- http://vcd.vicomtech.org/ontology/automotive#hasMaximumDeceleration -->

    <owl:DatatypeProperty rdf:about="http://vcd.vicomtech.org/ontology/automotive#hasMaximumDeceleration">
        <rdfs:subPropertyOf rdf:resource="http://www.w3.org/2002/07/owl#topDataProperty"/>
        <rdfs:domain rdf:resource="http://vcd.vicomtech.org/ontology/automotive#Animal"/>
        <rdfs:domain rdf:resource="http://vcd.vicomtech.org/ontology/automotive#Human"/>
        <rdfs:domain rdf:resource="http://vcd.vicomtech.org/ontology/automotive#RoadVehicle"/>
        <rdfs:domain rdf:resource="http://vcd.vicomtech.org/ontology/automotive#Train"/>
        <rdfs:range rdf:resource="http://www.w3.org/2001/XMLSchema#int"/>
        <rdfs:comment>Maximum braking depends on vehicle weight and tire traction, width and diameter.</rdfs:comment>
    </owl:DatatypeProperty>
    


    <!-- http://vcd.vicomtech.org/ontology/automotive#hasMaximumOperationalSpeed -->

    <owl:DatatypeProperty rdf:about="http://vcd.vicomtech.org/ontology/automotive#hasMaximumOperationalSpeed">
        <rdfs:subPropertyOf rdf:resource="http://www.w3.org/2002/07/owl#topDataProperty"/>
        <rdfs:domain rdf:resource="http://vcd.vicomtech.org/ontology/automotive#RoadVehicle"/>
        <rdfs:range rdf:resource="http://www.w3.org/2001/XMLSchema#int"/>
        <rdfs:comment>Is the speed selected by the system up to which the system operates under current environmental and sensor conditions. It is the maximum vehicle speed at which the system may be active and shall be determined by the capability of the sensing system as well as the environmental conditions.</rdfs:comment>
    </owl:DatatypeProperty>
    


    <!-- http://vcd.vicomtech.org/ontology/automotive#hasMaximumSpeed -->

    <owl:DatatypeProperty rdf:about="http://vcd.vicomtech.org/ontology/automotive#hasMaximumSpeed">
        <rdfs:subPropertyOf rdf:resource="http://www.w3.org/2002/07/owl#topDataProperty"/>
        <rdfs:domain rdf:resource="http://vcd.vicomtech.org/ontology/automotive#Animal"/>
        <rdfs:domain rdf:resource="http://vcd.vicomtech.org/ontology/automotive#Human"/>
        <rdfs:domain rdf:resource="http://vcd.vicomtech.org/ontology/automotive#RoadVehicle"/>
        <rdfs:domain rdf:resource="http://vcd.vicomtech.org/ontology/automotive#Train"/>
        <rdfs:range rdf:resource="http://www.w3.org/2001/XMLSchema#int"/>
        <rdfs:comment>Is the highest rate of speed an object can attain.</rdfs:comment>
    </owl:DatatypeProperty>
    


    <!-- http://vcd.vicomtech.org/ontology/automotive#hasModel -->

    <owl:DatatypeProperty rdf:about="http://vcd.vicomtech.org/ontology/automotive#hasModel">
        <rdfs:subPropertyOf rdf:resource="http://www.w3.org/2002/07/owl#topDataProperty"/>
        <rdfs:domain rdf:resource="http://vcd.vicomtech.org/ontology/automotive#RoadVehicle"/>
        <rdfs:range rdf:resource="http://www.w3.org/2001/XMLSchema#string"/>
        <rdfs:comment>A particular design or version of a product.</rdfs:comment>
    </owl:DatatypeProperty>
    


    <!-- http://vcd.vicomtech.org/ontology/automotive#hasNumberOfLanes -->

    <owl:DatatypeProperty rdf:about="http://vcd.vicomtech.org/ontology/automotive#hasNumberOfLanes">
        <rdfs:subPropertyOf rdf:resource="http://www.w3.org/2002/07/owl#topDataProperty"/>
        <rdfs:domain rdf:resource="http://vcd.vicomtech.org/ontology/automotive#Road"/>
        <rdfs:range rdf:resource="http://www.w3.org/2001/XMLSchema#int"/>
        <rdfs:comment>The total number of lanes that constitute a road.</rdfs:comment>
    </owl:DatatypeProperty>
    


    <!-- http://vcd.vicomtech.org/ontology/automotive#hasOccludedSide -->

    <owl:DatatypeProperty rdf:about="http://vcd.vicomtech.org/ontology/automotive#hasOccludedSide">
        <rdfs:subPropertyOf rdf:resource="http://www.w3.org/2002/07/owl#topDataProperty"/>
        <rdfs:domain rdf:resource="http://vcd.vicomtech.org/ontology/automotive#Signs"/>
        <rdfs:range rdf:resource="http://www.w3.org/2001/XMLSchema#string"/>
        <rdfs:comment>Determines that an object is partially visible and defines which is the side that can not be seen.</rdfs:comment>
    </owl:DatatypeProperty>
    


    <!-- http://vcd.vicomtech.org/ontology/automotive#hasOffset -->

    <owl:DatatypeProperty rdf:about="http://vcd.vicomtech.org/ontology/automotive#hasOffset">
        <rdfs:subPropertyOf rdf:resource="http://www.w3.org/2002/07/owl#topDataProperty"/>
        <rdfs:domain rdf:resource="http://vcd.vicomtech.org/ontology/automotive#Vehicle"/>
        <rdfs:range rdf:resource="http://www.w3.org/2001/XMLSchema#int"/>
        <rdfs:comment>Means the distance between the vehicle’s and the respective target’s longitudinal median plane in driving direction, measured on the ground, normalized by the half the vehicle width excluding devices for indirect vision and corrected by adding 50 per cent.</rdfs:comment>
    </owl:DatatypeProperty>
    


    <!-- http://vcd.vicomtech.org/ontology/automotive#hasOrientation -->

    <owl:DatatypeProperty rdf:about="http://vcd.vicomtech.org/ontology/automotive#hasOrientation">
        <rdfs:subPropertyOf rdf:resource="http://www.w3.org/2002/07/owl#topDataProperty"/>
        <rdfs:domain rdf:resource="http://vcd.vicomtech.org/ontology/automotive#Animal"/>
        <rdfs:domain rdf:resource="http://vcd.vicomtech.org/ontology/automotive#Human"/>
        <rdfs:domain rdf:resource="http://vcd.vicomtech.org/ontology/automotive#Vehicle"/>
        <rdfs:range rdf:resource="http://www.w3.org/2001/XMLSchema#int"/>
        <rdfs:comment>The orientation, angular position or direction of an object is part of the description of how it is placed in the space it occupies. More specifically, it refers to the imaginary rotation that is needed to move the object from a reference placement to its current placement.</rdfs:comment>
    </owl:DatatypeProperty>
    


    <!-- http://vcd.vicomtech.org/ontology/automotive#hasPosition -->

    <owl:DatatypeProperty rdf:about="http://vcd.vicomtech.org/ontology/automotive#hasPosition">
        <rdfs:subPropertyOf rdf:resource="http://www.w3.org/2002/07/owl#topDataProperty"/>
        <rdfs:domain rdf:resource="http://vcd.vicomtech.org/ontology/automotive#Animal"/>
        <rdfs:domain rdf:resource="http://vcd.vicomtech.org/ontology/automotive#Barrier"/>
        <rdfs:domain rdf:resource="http://vcd.vicomtech.org/ontology/automotive#Human"/>
        <rdfs:domain rdf:resource="http://vcd.vicomtech.org/ontology/automotive#Junction"/>
        <rdfs:domain rdf:resource="http://vcd.vicomtech.org/ontology/automotive#RailborneVehicle"/>
        <rdfs:domain rdf:resource="http://vcd.vicomtech.org/ontology/automotive#RoadObstacles"/>
        <rdfs:domain rdf:resource="http://vcd.vicomtech.org/ontology/automotive#RoadVehicle"/>
        <rdfs:domain rdf:resource="http://vcd.vicomtech.org/ontology/automotive#RoadsideObject"/>
        <rdfs:domain rdf:resource="http://vcd.vicomtech.org/ontology/automotive#Structure"/>
        <rdfs:domain rdf:resource="http://vcd.vicomtech.org/ontology/automotive#Vehicle"/>
        <rdfs:range rdf:resource="http://vcd.vicomtech.org/ontology/automotive#array"/>
        <rdfs:comment>A place where someone or something is located according to the geographic coordinate system: latitude and longitude [lat, lon].</rdfs:comment>
    </owl:DatatypeProperty>
    


    <!-- http://vcd.vicomtech.org/ontology/automotive#hasRelativePosition -->

    <owl:DatatypeProperty rdf:about="http://vcd.vicomtech.org/ontology/automotive#hasRelativePosition">
        <rdfs:subPropertyOf rdf:resource="http://www.w3.org/2002/07/owl#topDataProperty"/>
        <rdfs:domain rdf:resource="http://vcd.vicomtech.org/ontology/automotive#Animal"/>
        <rdfs:domain rdf:resource="http://vcd.vicomtech.org/ontology/automotive#Barrier"/>
        <rdfs:domain rdf:resource="http://vcd.vicomtech.org/ontology/automotive#CurbCut"/>
        <rdfs:domain rdf:resource="http://vcd.vicomtech.org/ontology/automotive#Footwalk"/>
        <rdfs:domain rdf:resource="http://vcd.vicomtech.org/ontology/automotive#Human"/>
        <rdfs:domain rdf:resource="http://vcd.vicomtech.org/ontology/automotive#Junction"/>
        <rdfs:domain rdf:resource="http://vcd.vicomtech.org/ontology/automotive#Lane"/>
        <rdfs:domain rdf:resource="http://vcd.vicomtech.org/ontology/automotive#PedestrianArea"/>
        <rdfs:domain rdf:resource="http://vcd.vicomtech.org/ontology/automotive#RailTrack"/>
        <rdfs:domain rdf:resource="http://vcd.vicomtech.org/ontology/automotive#RailborneVehicle"/>
        <rdfs:domain rdf:resource="http://vcd.vicomtech.org/ontology/automotive#RoadObstacles"/>
        <rdfs:domain rdf:resource="http://vcd.vicomtech.org/ontology/automotive#RoadVehicle"/>
        <rdfs:domain rdf:resource="http://vcd.vicomtech.org/ontology/automotive#RoadsideObject"/>
        <rdfs:domain rdf:resource="http://vcd.vicomtech.org/ontology/automotive#Structure"/>
        <rdfs:domain rdf:resource="http://vcd.vicomtech.org/ontology/automotive#TrafficIsland"/>
        <rdfs:domain rdf:resource="http://vcd.vicomtech.org/ontology/automotive#Vehicle"/>
        <rdfs:range rdf:resource="http://www.w3.org/2001/XMLSchema#string"/>
        <rdfs:comment>The change in position of one object compared to another object.</rdfs:comment>
    </owl:DatatypeProperty>
    


    <!-- http://vcd.vicomtech.org/ontology/automotive#hasRelativeSpeed -->

    <owl:DatatypeProperty rdf:about="http://vcd.vicomtech.org/ontology/automotive#hasRelativeSpeed">
        <rdfs:subPropertyOf rdf:resource="http://www.w3.org/2002/07/owl#topDataProperty"/>
        <rdfs:domain rdf:resource="http://vcd.vicomtech.org/ontology/automotive#Animal"/>
        <rdfs:domain rdf:resource="http://vcd.vicomtech.org/ontology/automotive#Human"/>
        <rdfs:domain rdf:resource="http://vcd.vicomtech.org/ontology/automotive#RoadVehicle"/>
        <rdfs:domain rdf:resource="http://vcd.vicomtech.org/ontology/automotive#Train"/>
        <rdfs:range rdf:resource="http://www.w3.org/2001/XMLSchema#int"/>
        <rdfs:comment>The change in velocity of one object compared to another object.</rdfs:comment>
    </owl:DatatypeProperty>
    


    <!-- http://vcd.vicomtech.org/ontology/automotive#hasRoadCondition -->

    <owl:DatatypeProperty rdf:about="http://vcd.vicomtech.org/ontology/automotive#hasRoadCondition">
        <rdfs:subPropertyOf rdf:resource="http://www.w3.org/2002/07/owl#topDataProperty"/>
        <rdfs:domain rdf:resource="http://vcd.vicomtech.org/ontology/automotive#Road"/>
        <rdfs:range rdf:resource="http://www.w3.org/2001/XMLSchema#string"/>
        <rdfs:comment>The circumstances or factors affecting the state of the road with regard to its appearance or quality.</rdfs:comment>
    </owl:DatatypeProperty>
    


    <!-- http://vcd.vicomtech.org/ontology/automotive#hasRoadDirection -->

    <owl:DatatypeProperty rdf:about="http://vcd.vicomtech.org/ontology/automotive#hasRoadDirection">
        <rdfs:subPropertyOf rdf:resource="http://www.w3.org/2002/07/owl#topDataProperty"/>
        <rdfs:domain rdf:resource="http://vcd.vicomtech.org/ontology/automotive#Road"/>
        <rdfs:range rdf:resource="http://www.w3.org/2001/XMLSchema#string"/>
        <rdfs:range>
            <rdfs:Datatype>
                <owl:oneOf>
                    <rdf:Description>
                        <rdf:type rdf:resource="http://www.w3.org/1999/02/22-rdf-syntax-ns#List"/>
                        <rdf:first>Single-way</rdf:first>
                        <rdf:rest>
                            <rdf:Description>
                                <rdf:type rdf:resource="http://www.w3.org/1999/02/22-rdf-syntax-ns#List"/>
                                <rdf:first>Two-way</rdf:first>
                                <rdf:rest rdf:resource="http://www.w3.org/1999/02/22-rdf-syntax-ns#nil"/>
                            </rdf:Description>
                        </rdf:rest>
                    </rdf:Description>
                </owl:oneOf>
            </rdfs:Datatype>
        </rdfs:range>
        <rdfs:comment>Determines in which direction the vehicles can move: single-way or two-way.</rdfs:comment>
    </owl:DatatypeProperty>
    


    <!-- http://vcd.vicomtech.org/ontology/automotive#hasS -->

    <owl:DatatypeProperty rdf:about="http://vcd.vicomtech.org/ontology/automotive#hasS">
        <rdfs:subPropertyOf rdf:resource="http://www.w3.org/2002/07/owl#topDataProperty"/>
        <rdfs:domain rdf:resource="http://vcd.vicomtech.org/ontology/automotive#Animal"/>
        <rdfs:domain rdf:resource="http://vcd.vicomtech.org/ontology/automotive#Human"/>
        <rdfs:domain rdf:resource="http://vcd.vicomtech.org/ontology/automotive#RoadVehicle"/>
        <rdfs:range rdf:resource="http://www.w3.org/2001/XMLSchema#int"/>
        <rdfs:comment>Determines the longitudinal position along the road (OpenSCENARIO context).</rdfs:comment>
    </owl:DatatypeProperty>
    


    <!-- http://vcd.vicomtech.org/ontology/automotive#hasSlope -->

    <owl:DatatypeProperty rdf:about="http://vcd.vicomtech.org/ontology/automotive#hasSlope">
        <rdfs:subPropertyOf rdf:resource="http://www.w3.org/2002/07/owl#topDataProperty"/>
        <rdfs:domain rdf:resource="http://vcd.vicomtech.org/ontology/automotive#Road"/>
        <rdfs:range rdf:resource="http://www.w3.org/2001/XMLSchema#int"/>
        <rdfs:comment>The inclination of a surface.</rdfs:comment>
    </owl:DatatypeProperty>
    


    <!-- http://vcd.vicomtech.org/ontology/automotive#hasSpecifiedMaximumSpeed -->

    <owl:DatatypeProperty rdf:about="http://vcd.vicomtech.org/ontology/automotive#hasSpecifiedMaximumSpeed">
        <rdfs:subPropertyOf rdf:resource="http://www.w3.org/2002/07/owl#topDataProperty"/>
        <rdfs:domain rdf:resource="http://vcd.vicomtech.org/ontology/automotive#RoadVehicle"/>
        <rdfs:range rdf:resource="http://www.w3.org/2001/XMLSchema#int"/>
        <rdfs:comment>Is the speed declared by the manufacturer up to which the system operates under optimum conditions.</rdfs:comment>
    </owl:DatatypeProperty>
    


    <!-- http://vcd.vicomtech.org/ontology/automotive#hasSpeed -->

    <owl:DatatypeProperty rdf:about="http://vcd.vicomtech.org/ontology/automotive#hasSpeed">
        <rdfs:subPropertyOf rdf:resource="http://www.w3.org/2002/07/owl#topDataProperty"/>
        <rdfs:domain rdf:resource="http://vcd.vicomtech.org/ontology/automotive#Animal"/>
        <rdfs:domain rdf:resource="http://vcd.vicomtech.org/ontology/automotive#Human"/>
        <rdfs:domain rdf:resource="http://vcd.vicomtech.org/ontology/automotive#RoadVehicle"/>
        <rdfs:domain rdf:resource="http://vcd.vicomtech.org/ontology/automotive#Train"/>
        <rdfs:range rdf:resource="http://www.w3.org/2001/XMLSchema#int"/>
        <rdfs:comment>Speed is defined as. The rate of change of position of an object in any direction. Speed is measured as the ratio of distance to the time in which the distance was covered. Speed is a scalar quantity as it has only direction and no magnitude.</rdfs:comment>
    </owl:DatatypeProperty>
    


    <!-- http://vcd.vicomtech.org/ontology/automotive#hasState -->

    <owl:DatatypeProperty rdf:about="http://vcd.vicomtech.org/ontology/automotive#hasState">
        <rdfs:subPropertyOf rdf:resource="http://www.w3.org/2002/07/owl#topDataProperty"/>
        <rdfs:domain rdf:resource="http://vcd.vicomtech.org/ontology/automotive#TrafficLight"/>
        <rdfs:range rdf:resource="http://www.w3.org/2001/XMLSchema#string"/>
        <rdfs:range>
            <rdfs:Datatype>
                <owl:oneOf>
                    <rdf:Description>
                        <rdf:type rdf:resource="http://www.w3.org/1999/02/22-rdf-syntax-ns#List"/>
                        <rdf:first>Amber</rdf:first>
                        <rdf:rest>
                            <rdf:Description>
                                <rdf:type rdf:resource="http://www.w3.org/1999/02/22-rdf-syntax-ns#List"/>
                                <rdf:first>Red</rdf:first>
                                <rdf:rest>
                                    <rdf:Description>
                                        <rdf:type rdf:resource="http://www.w3.org/1999/02/22-rdf-syntax-ns#List"/>
                                        <rdf:first>Yellow</rdf:first>
                                        <rdf:rest rdf:resource="http://www.w3.org/1999/02/22-rdf-syntax-ns#nil"/>
                                    </rdf:Description>
                                </rdf:rest>
                            </rdf:Description>
                        </rdf:rest>
                    </rdf:Description>
                </owl:oneOf>
            </rdfs:Datatype>
        </rdfs:range>
        <rdfs:comment>Current condition of an object.</rdfs:comment>
    </owl:DatatypeProperty>
    


    <!-- http://vcd.vicomtech.org/ontology/automotive#hasTTC -->

    <owl:DatatypeProperty rdf:about="http://vcd.vicomtech.org/ontology/automotive#hasTTC">
        <rdfs:subPropertyOf rdf:resource="http://www.w3.org/2002/07/owl#topDataProperty"/>
        <rdfs:domain rdf:resource="http://vcd.vicomtech.org/ontology/automotive#Vehicle"/>
        <rdfs:range rdf:resource="http://www.w3.org/2001/XMLSchema#int"/>
        <rdfs:comment>&quot;Time to Collision&quot; (TTC) means the value of time obtained by dividing the
longitudinal distance (in the direction of travel of the subject vehicle) between the subject vehicle and the target by the longitudinal relative speed of the subject vehicle and the target, at any instant in time</rdfs:comment>
    </owl:DatatypeProperty>
    


    <!-- http://vcd.vicomtech.org/ontology/automotive#hasTargetLane -->

    <owl:DatatypeProperty rdf:about="http://vcd.vicomtech.org/ontology/automotive#hasTargetLane">
        <rdfs:subPropertyOf rdf:resource="http://www.w3.org/2002/07/owl#topDataProperty"/>
        <rdfs:domain rdf:resource="http://vcd.vicomtech.org/ontology/automotive#LaneChanging"/>
        <rdfs:domain rdf:resource="http://vcd.vicomtech.org/ontology/automotive#LaneChangingLeft"/>
        <rdfs:domain rdf:resource="http://vcd.vicomtech.org/ontology/automotive#LaneChangingRight"/>
        <rdfs:range rdf:resource="http://www.w3.org/2001/XMLSchema#string"/>
        <rdfs:comment>The lane to be reached.</rdfs:comment>
    </owl:DatatypeProperty>
    


    <!-- http://vcd.vicomtech.org/ontology/automotive#hasTemporalDuration -->

    <owl:DatatypeProperty rdf:about="http://vcd.vicomtech.org/ontology/automotive#hasTemporalDuration">
        <rdfs:subPropertyOf rdf:resource="http://www.w3.org/2002/07/owl#topDataProperty"/>
        <rdfs:domain rdf:resource="http://vcd.vicomtech.org/ontology/automotive#Action"/>
        <rdfs:range rdf:resource="http://www.w3.org/2001/XMLSchema#int"/>
        <rdfs:comment>The duration of tge length of time that something will last.</rdfs:comment>
    </owl:DatatypeProperty>
    


    <!-- http://vcd.vicomtech.org/ontology/automotive#hasTrigger -->

    <owl:DatatypeProperty rdf:about="http://vcd.vicomtech.org/ontology/automotive#hasTrigger">
        <rdfs:domain rdf:resource="http://vcd.vicomtech.org/ontology/automotive#Action"/>
        <rdfs:range rdf:resource="http://www.w3.org/2000/01/rdf-schema#Literal"/>
        <rdfs:comment>A happening that causes the starting of an action.</rdfs:comment>
    </owl:DatatypeProperty>
    


    <!-- http://vcd.vicomtech.org/ontology/automotive#hasVehicleDensity -->

    <owl:DatatypeProperty rdf:about="http://vcd.vicomtech.org/ontology/automotive#hasVehicleDensity">
        <rdfs:subPropertyOf rdf:resource="http://www.w3.org/2002/07/owl#topDataProperty"/>
        <rdfs:domain rdf:resource="http://vcd.vicomtech.org/ontology/automotive#Lane"/>
        <rdfs:domain rdf:resource="http://vcd.vicomtech.org/ontology/automotive#ParkingLot"/>
        <rdfs:domain rdf:resource="http://vcd.vicomtech.org/ontology/automotive#Road"/>
        <rdfs:range rdf:resource="http://www.w3.org/2001/XMLSchema#int"/>
    </owl:DatatypeProperty>
    


    <!-- http://vcd.vicomtech.org/ontology/automotive#hasVisibleSide -->

    <owl:DatatypeProperty rdf:about="http://vcd.vicomtech.org/ontology/automotive#hasVisibleSide">
        <rdfs:subPropertyOf rdf:resource="http://www.w3.org/2002/07/owl#topDataProperty"/>
        <rdfs:domain rdf:resource="http://vcd.vicomtech.org/ontology/automotive#Marking"/>
        <rdfs:domain rdf:resource="http://vcd.vicomtech.org/ontology/automotive#Signs"/>
        <rdfs:range rdf:resource="http://www.w3.org/2001/XMLSchema#string"/>
        <rdfs:comment>Determines that an object is partially occluded and defines which is the side that can be seen.</rdfs:comment>
    </owl:DatatypeProperty>
    


    <!-- http://vcd.vicomtech.org/ontology/automotive#hasWidth -->

    <owl:DatatypeProperty rdf:about="http://vcd.vicomtech.org/ontology/automotive#hasWidth">
        <rdfs:subPropertyOf rdf:resource="http://www.w3.org/2002/07/owl#topDataProperty"/>
        <rdfs:domain rdf:resource="http://vcd.vicomtech.org/ontology/automotive#DrivableVehicle"/>
        <rdfs:domain rdf:resource="http://vcd.vicomtech.org/ontology/automotive#Lane"/>
        <rdfs:domain rdf:resource="http://vcd.vicomtech.org/ontology/automotive#Road"/>
        <rdfs:range rdf:resource="http://www.w3.org/2001/XMLSchema#int"/>
        <rdfs:comment>The measurement or extent of something from side to side; the lesser of two or the least of three dimensions of a body.</rdfs:comment>
    </owl:DatatypeProperty>
    


    <!-- http://vcd.vicomtech.org/ontology/automotive#hasYawRate -->

    <owl:DatatypeProperty rdf:about="http://vcd.vicomtech.org/ontology/automotive#hasYawRate">
        <rdfs:subPropertyOf rdf:resource="http://www.w3.org/2002/07/owl#topDataProperty"/>
        <rdfs:domain rdf:resource="http://vcd.vicomtech.org/ontology/automotive#Vehicle"/>
        <rdfs:range rdf:resource="http://www.w3.org/2001/XMLSchema#int"/>
        <rdfs:comment>The yaw rate or yaw velocity of a car, aircraft, projectile or other rigid body is the angular velocity of this rotation, or rate of change of the heading angle when the aircraft is horizontal. It is commonly measured in degrees per second or radians per second.</rdfs:comment>
    </owl:DatatypeProperty>
    


    <!-- http://vcd.vicomtech.org/ontology/automotive#isActivated -->

    <owl:DatatypeProperty rdf:about="http://vcd.vicomtech.org/ontology/automotive#isActivated">
        <rdfs:subPropertyOf rdf:resource="http://www.w3.org/2002/07/owl#topDataProperty"/>
        <rdfs:domain rdf:resource="http://vcd.vicomtech.org/ontology/automotive#InVehicleSystems"/>
        <rdfs:range rdf:resource="http://www.w3.org/2001/XMLSchema#boolean"/>
        <rdfs:comment>Determines if a systen is operative (on/off).</rdfs:comment>
    </owl:DatatypeProperty>
    


    <!-- http://vcd.vicomtech.org/ontology/automotive#isCarryingObject -->

    <owl:DatatypeProperty rdf:about="http://vcd.vicomtech.org/ontology/automotive#isCarryingObject">
        <rdfs:subPropertyOf rdf:resource="http://www.w3.org/2002/07/owl#topDataProperty"/>
        <rdfs:comment>States that an object is holding or moving another object from one place to another.</rdfs:comment>
    </owl:DatatypeProperty>
    


    <!-- http://vcd.vicomtech.org/ontology/automotive#isCarryingObject1 -->

    <owl:DatatypeProperty rdf:about="http://vcd.vicomtech.org/ontology/automotive#isCarryingObject1">
        <rdfs:subPropertyOf rdf:resource="http://vcd.vicomtech.org/ontology/automotive#isCarryingObject"/>
        <rdfs:domain rdf:resource="http://vcd.vicomtech.org/ontology/automotive#AdultWithObject"/>
        <rdfs:range rdf:resource="http://www.w3.org/2001/XMLSchema#string"/>
        <rdfs:comment>States that an adult is holding or moving another object from one place to another.</rdfs:comment>
    </owl:DatatypeProperty>
    


    <!-- http://vcd.vicomtech.org/ontology/automotive#isCarryingObject2 -->

    <owl:DatatypeProperty rdf:about="http://vcd.vicomtech.org/ontology/automotive#isCarryingObject2">
        <rdfs:subPropertyOf rdf:resource="http://vcd.vicomtech.org/ontology/automotive#isCarryingObject"/>
        <rdfs:domain rdf:resource="http://vcd.vicomtech.org/ontology/automotive#ChildWithObject"/>
        <rdfs:range rdf:resource="http://www.w3.org/2001/XMLSchema#string"/>
        <rdfs:comment>States that a child is holding or moving another object from one place to another.</rdfs:comment>
    </owl:DatatypeProperty>
    


    <!-- http://vcd.vicomtech.org/ontology/automotive#isEquippedWith -->

    <owl:DatatypeProperty rdf:about="http://vcd.vicomtech.org/ontology/automotive#isEquippedWith">
        <rdfs:subPropertyOf rdf:resource="http://www.w3.org/2002/07/owl#topDataProperty"/>
        <rdfs:domain rdf:resource="http://vcd.vicomtech.org/ontology/automotive#Vehicle"/>
        <rdfs:range rdf:resource="http://www.w3.org/2001/XMLSchema#string"/>
        <rdfs:comment>To define which in-vehicle systems or sensor are installed in the vehicle.</rdfs:comment>
    </owl:DatatypeProperty>
    


    <!-- http://vcd.vicomtech.org/ontology/automotive#isVisible -->

    <owl:DatatypeProperty rdf:about="http://vcd.vicomtech.org/ontology/automotive#isVisible">
        <rdfs:subPropertyOf rdf:resource="http://www.w3.org/2002/07/owl#topDataProperty"/>
        <rdfs:domain rdf:resource="http://vcd.vicomtech.org/ontology/automotive#Animal"/>
        <rdfs:domain rdf:resource="http://vcd.vicomtech.org/ontology/automotive#Construction"/>
        <rdfs:domain rdf:resource="http://vcd.vicomtech.org/ontology/automotive#Human"/>
        <rdfs:domain rdf:resource="http://vcd.vicomtech.org/ontology/automotive#MovableObject"/>
        <rdfs:domain rdf:resource="http://vcd.vicomtech.org/ontology/automotive#RoadsideObject"/>
        <rdfs:domain rdf:resource="http://vcd.vicomtech.org/ontology/automotive#Vehicle"/>
        <rdfs:range rdf:resource="http://www.w3.org/2001/XMLSchema#boolean"/>
        <rdfs:comment>Determines whether the object can be seen according to the light and weather conditions or is occluded.</rdfs:comment>
    </owl:DatatypeProperty>
    


    <!-- 
    ///////////////////////////////////////////////////////////////////////////////////////
    //
    // Classes
    //
    ///////////////////////////////////////////////////////////////////////////////////////
     -->

    


    <!-- http://vcd.vicomtech.org/ontology/automotive#ALKS -->

    <owl:Class rdf:about="http://vcd.vicomtech.org/ontology/automotive#ALKS">
        <rdfs:subClassOf rdf:resource="http://vcd.vicomtech.org/ontology/automotive#InVehicleSystems"/>
        <rdfs:comment>Automated Lane Keeping Systems (ALKS) for low speed application is a system which is activated by the driver and which keeps the vehicle within its lane for travelling speed of 60 km/h or less by controlling the lateral and longitudinal movements of the vehicle for extended periods without the need for further driver input.</rdfs:comment>
        <rdfs:label>ALKS</rdfs:label>
    </owl:Class>
    


    <!-- http://vcd.vicomtech.org/ontology/automotive#ATV -->

    <owl:Class rdf:about="http://vcd.vicomtech.org/ontology/automotive#ATV">
        <rdfs:subClassOf rdf:resource="http://vcd.vicomtech.org/ontology/automotive#Cycle"/>
        <rdfs:comment>A small vehicle with one seat and usually 4 wheels fitted with large tires, designed for use on rough ground. Propelled by a motor and steered with a handlebar linked to the front axle.</rdfs:comment>
        <rdfs:label>ATV</rdfs:label>
    </owl:Class>
    


    <!-- http://vcd.vicomtech.org/ontology/automotive#Accident -->

    <owl:Class rdf:about="http://vcd.vicomtech.org/ontology/automotive#Accident">
        <rdfs:subClassOf rdf:resource="http://vcd.vicomtech.org/ontology/automotive#Event"/>
        <rdfs:comment>Accidents are situations in which one or more vehicles lose control and do not recover.  They include collisions between vehicle(s) or other network user(s), between vehicle(s) and fixed obstacle(s), or they result from a vehicle running off the network infrastructure. This concept and description are a generalised version of the DATEX II concept accident.</rdfs:comment>
        <rdfs:label>Accident</rdfs:label>
    </owl:Class>
    


    <!-- http://vcd.vicomtech.org/ontology/automotive#Action -->

    <owl:Class rdf:about="http://vcd.vicomtech.org/ontology/automotive#Action">
        <rdfs:subClassOf rdf:resource="http://www.w3.org/2002/07/owl#Thing"/>
        <rdfs:comment>Traffic maneuvers performed by any of the possible subjects of the scenario.</rdfs:comment>
        <rdfs:label>Action</rdfs:label>
    </owl:Class>
    


    <!-- http://vcd.vicomtech.org/ontology/automotive#Adult -->

    <owl:Class rdf:about="http://vcd.vicomtech.org/ontology/automotive#Adult">
        <rdfs:subClassOf rdf:resource="http://vcd.vicomtech.org/ontology/automotive#Pedestrian"/>
        <owl:disjointWith rdf:resource="http://vcd.vicomtech.org/ontology/automotive#Child"/>
        <rdfs:comment>A human who is fully grown or developed.</rdfs:comment>
        <rdfs:label>Adult</rdfs:label>
    </owl:Class>
    


    <!-- http://vcd.vicomtech.org/ontology/automotive#AdultWithObject -->

    <owl:Class rdf:about="http://vcd.vicomtech.org/ontology/automotive#AdultWithObject">
        <rdfs:subClassOf rdf:resource="http://vcd.vicomtech.org/ontology/automotive#PedestrianWithObject"/>
        <owl:disjointWith rdf:resource="http://vcd.vicomtech.org/ontology/automotive#ChildWithObject"/>
        <rdfs:comment>Any person about older than 8 years that is carrying an object while acting as a pedestrian in the surroundings of the vehicle.</rdfs:comment>
        <rdfs:label>Adult with Object</rdfs:label>
    </owl:Class>
    


    <!-- http://vcd.vicomtech.org/ontology/automotive#AgriculturalVehicle -->

    <owl:Class rdf:about="http://vcd.vicomtech.org/ontology/automotive#AgriculturalVehicle">
        <rdfs:subClassOf rdf:resource="http://vcd.vicomtech.org/ontology/automotive#DrivableVehicle"/>
        <rdfs:comment>A vehicle which is substantially designed, equipped, or materially altered from its original construction for the purpose of agricultural use. Usually have large, heavily treaded tires and are used to pulling farm implements or machinery.</rdfs:comment>
        <rdfs:label>Agricultural vehicle</rdfs:label>
    </owl:Class>
    


    <!-- http://vcd.vicomtech.org/ontology/automotive#Air -->

    <owl:Class rdf:about="http://vcd.vicomtech.org/ontology/automotive#Air">
        <rdfs:subClassOf rdf:resource="http://vcd.vicomtech.org/ontology/automotive#Element"/>
        <rdfs:comment>The invisible gaseous substance surrounding the earth, a mixture mainly of oxygen and nitrogen.</rdfs:comment>
        <rdfs:label>Air</rdfs:label>
    </owl:Class>
    


    <!-- http://vcd.vicomtech.org/ontology/automotive#Aircraft -->

    <owl:Class rdf:about="http://vcd.vicomtech.org/ontology/automotive#Aircraft">
        <rdfs:subClassOf rdf:resource="http://vcd.vicomtech.org/ontology/automotive#Vehicle"/>
        <rdfs:comment>An aeroplane, helicopter or other machine capable of flight.</rdfs:comment>
        <rdfs:label>Aircraft</rdfs:label>
    </owl:Class>
    


    <!-- http://vcd.vicomtech.org/ontology/automotive#Ambulance -->

    <owl:Class rdf:about="http://vcd.vicomtech.org/ontology/automotive#Ambulance">
        <rdfs:subClassOf rdf:resource="http://vcd.vicomtech.org/ontology/automotive#EmergencyVehicle"/>
        <rdfs:comment>A road vehicle equipped for taking sick or injured people to and from hospital, especially in emergencies.</rdfs:comment>
        <rdfs:label>Ambulance</rdfs:label>
    </owl:Class>
    


    <!-- http://vcd.vicomtech.org/ontology/automotive#AmbulanceBicycle -->

    <owl:Class rdf:about="http://vcd.vicomtech.org/ontology/automotive#AmbulanceBicycle">
        <rdfs:subClassOf rdf:resource="http://vcd.vicomtech.org/ontology/automotive#EmergencyBicycle"/>
        <rdfs:label>Ambulance Bicycle</rdfs:label>
    </owl:Class>
    


    <!-- http://vcd.vicomtech.org/ontology/automotive#AmbulanceMotorcycle -->

    <owl:Class rdf:about="http://vcd.vicomtech.org/ontology/automotive#AmbulanceMotorcycle">
        <rdfs:subClassOf rdf:resource="http://vcd.vicomtech.org/ontology/automotive#EmergencyMotorcycle"/>
        <rdfs:label>Ambulance Motorcycle</rdfs:label>
    </owl:Class>
    


    <!-- http://vcd.vicomtech.org/ontology/automotive#AmbulanceOperator -->

    <owl:Class rdf:about="http://vcd.vicomtech.org/ontology/automotive#AmbulanceOperator">
        <rdfs:subClassOf rdf:resource="http://vcd.vicomtech.org/ontology/automotive#FirstResponder"/>
        <rdfs:comment>Ambulance operators belong to organizations whose primary goal is to carry out the tasks of Medical Doctors and provide health/medical services in situations of emergency. Usually wear a particular uniform that explicits this role.</rdfs:comment>
        <rdfs:label>Ambulance operator</rdfs:label>
    </owl:Class>
    


    <!-- http://vcd.vicomtech.org/ontology/automotive#AmbulanceTruck -->

    <owl:Class rdf:about="http://vcd.vicomtech.org/ontology/automotive#AmbulanceTruck">
        <rdfs:subClassOf rdf:resource="http://vcd.vicomtech.org/ontology/automotive#LargeEmergencyVehicle"/>
        <rdfs:comment>Trucks or Heavy-duty vehicles adopted by Ambulance.</rdfs:comment>
        <rdfs:label>Ambulance truck</rdfs:label>
    </owl:Class>
    


    <!-- http://vcd.vicomtech.org/ontology/automotive#Animal -->

    <owl:Class rdf:about="http://vcd.vicomtech.org/ontology/automotive#Animal">
        <rdfs:subClassOf rdf:resource="http://vcd.vicomtech.org/ontology/automotive#Dynamic"/>
        <rdfs:comment>A living organism that feeds on organic matter, typically having specialized sense organs and nervous system and able to respond rapidly to stimuli.</rdfs:comment>
        <rdfs:label>Animal</rdfs:label>
    </owl:Class>
    


    <!-- http://vcd.vicomtech.org/ontology/automotive#AnimalPulled -->

    <owl:Class rdf:about="http://vcd.vicomtech.org/ontology/automotive#AnimalPulled">
        <rdfs:subClassOf rdf:resource="http://vcd.vicomtech.org/ontology/automotive#RoadVehicle"/>
        <rdfs:comment>Any vehicle carried by animals or group of animals. The vehicle can be both ridden or driven (according to the definitions below) as long as it is being pulled by animals.</rdfs:comment>
        <rdfs:label>Animal-pulled vehicle</rdfs:label>
    </owl:Class>
    


    <!-- http://vcd.vicomtech.org/ontology/automotive#Approaching -->

    <owl:Class rdf:about="http://vcd.vicomtech.org/ontology/automotive#Approaching">
        <rdfs:subClassOf rdf:resource="http://vcd.vicomtech.org/ontology/automotive#MovingManeuver"/>
        <rdfs:comment>The action of getting closer to a junction, crosswalk or other object.</rdfs:comment>
        <rdfs:label>Approaching</rdfs:label>
    </owl:Class>
    


    <!-- http://vcd.vicomtech.org/ontology/automotive#Arrow -->

    <owl:Class rdf:about="http://vcd.vicomtech.org/ontology/automotive#Arrow">
        <rdfs:subClassOf rdf:resource="http://vcd.vicomtech.org/ontology/automotive#Marking"/>
        <rdfs:comment>Direction arrows used on the approach to busy multi-lane junctions to give drivers advance indication of the correct lane.</rdfs:comment>
        <rdfs:label>Arrow</rdfs:label>
    </owl:Class>
    


    <!-- http://vcd.vicomtech.org/ontology/automotive#ArrowLeftTurn -->

    <owl:Class rdf:about="http://vcd.vicomtech.org/ontology/automotive#ArrowLeftTurn">
        <rdfs:subClassOf rdf:resource="http://vcd.vicomtech.org/ontology/automotive#Arrow"/>
        <rdfs:comment>Arrow indicating a left turn.</rdfs:comment>
        <rdfs:label>Arrow left turn</rdfs:label>
    </owl:Class>
    


    <!-- http://vcd.vicomtech.org/ontology/automotive#ArrowLeftrightTurn -->

    <owl:Class rdf:about="http://vcd.vicomtech.org/ontology/automotive#ArrowLeftrightTurn">
        <rdfs:subClassOf rdf:resource="http://vcd.vicomtech.org/ontology/automotive#Arrow"/>
        <rdfs:comment>A two headed arrow indicating a left and right turn.</rdfs:comment>
        <rdfs:label>Arrow leftright turn</rdfs:label>
    </owl:Class>
    


    <!-- http://vcd.vicomtech.org/ontology/automotive#ArrowRightTurn -->

    <owl:Class rdf:about="http://vcd.vicomtech.org/ontology/automotive#ArrowRightTurn">
        <rdfs:subClassOf rdf:resource="http://vcd.vicomtech.org/ontology/automotive#Arrow"/>
        <rdfs:comment>Arrow indicating a right turn.</rdfs:comment>
        <rdfs:label>Arrow right turn</rdfs:label>
    </owl:Class>
    


    <!-- http://vcd.vicomtech.org/ontology/automotive#ArrowThru -->

    <owl:Class rdf:about="http://vcd.vicomtech.org/ontology/automotive#ArrowThru">
        <rdfs:subClassOf rdf:resource="http://vcd.vicomtech.org/ontology/automotive#Arrow"/>
        <rdfs:comment>Arrow marking pointing straight ahead.</rdfs:comment>
        <rdfs:label>Arrow thru</rdfs:label>
    </owl:Class>
    


    <!-- http://vcd.vicomtech.org/ontology/automotive#ArrowThruleftTurn -->

    <owl:Class rdf:about="http://vcd.vicomtech.org/ontology/automotive#ArrowThruleftTurn">
        <rdfs:subClassOf rdf:resource="http://vcd.vicomtech.org/ontology/automotive#Arrow"/>
        <rdfs:comment>A two-headed arrow with one head pointing straight ahead and the other pointing to the left.</rdfs:comment>
        <rdfs:label>Arrow thruleft turn</rdfs:label>
    </owl:Class>
    


    <!-- http://vcd.vicomtech.org/ontology/automotive#ArrowThrurightTurn -->

    <owl:Class rdf:about="http://vcd.vicomtech.org/ontology/automotive#ArrowThrurightTurn">
        <rdfs:subClassOf rdf:resource="http://vcd.vicomtech.org/ontology/automotive#Arrow"/>
        <rdfs:comment>A two-headed arrow with one head pointing straight ahead and the other pointing to the right.</rdfs:comment>
        <rdfs:label>Arrow thruright turn</rdfs:label>
    </owl:Class>
    


    <!-- http://vcd.vicomtech.org/ontology/automotive#ArrowUturn -->

    <owl:Class rdf:about="http://vcd.vicomtech.org/ontology/automotive#ArrowUturn">
        <rdfs:subClassOf rdf:resource="http://vcd.vicomtech.org/ontology/automotive#Arrow"/>
        <rdfs:comment>U-shaped arrow indicating that a change of direction can be done.</rdfs:comment>
        <rdfs:label>U turn arrow</rdfs:label>
    </owl:Class>
    


    <!-- http://vcd.vicomtech.org/ontology/automotive#ArtificialLighting -->

    <owl:Class rdf:about="http://vcd.vicomtech.org/ontology/automotive#ArtificialLighting">
        <rdfs:subClassOf rdf:resource="http://vcd.vicomtech.org/ontology/automotive#Lighting"/>
        <rdfs:comment>Refers to the opposed to natural light, this is, any light source that is produced by electrical means.</rdfs:comment>
        <rdfs:label>Artificial lighting</rdfs:label>
    </owl:Class>
    


    <!-- http://vcd.vicomtech.org/ontology/automotive#AvoidingCollision -->

    <owl:Class rdf:about="http://vcd.vicomtech.org/ontology/automotive#AvoidingCollision">
        <rdfs:subClassOf rdf:resource="http://vcd.vicomtech.org/ontology/automotive#MovingManeuver"/>
        <rdfs:comment>An instance of one moving object or person when it avoids striking violently against another or any other object of the scene.</rdfs:comment>
        <rdfs:label>Avoiding collision</rdfs:label>
    </owl:Class>
    


    <!-- http://vcd.vicomtech.org/ontology/automotive#Banner -->

    <owl:Class rdf:about="http://vcd.vicomtech.org/ontology/automotive#Banner">
        <rdfs:subClassOf rdf:resource="http://vcd.vicomtech.org/ontology/automotive#Signs"/>
        <rdfs:comment>Typically a flag, made of textile or plastic.</rdfs:comment>
        <rdfs:label>Banner</rdfs:label>
    </owl:Class>
    


    <!-- http://vcd.vicomtech.org/ontology/automotive#Barrier -->

    <owl:Class rdf:about="http://vcd.vicomtech.org/ontology/automotive#Barrier">
        <rdfs:subClassOf rdf:resource="http://vcd.vicomtech.org/ontology/automotive#Construction"/>
        <rdfs:comment>A fence or other obstacle that prevents movement or access.</rdfs:comment>
        <rdfs:label>Barrier</rdfs:label>
    </owl:Class>
    


    <!-- http://vcd.vicomtech.org/ontology/automotive#BasketweaveInterchange -->

    <owl:Class rdf:about="http://vcd.vicomtech.org/ontology/automotive#BasketweaveInterchange">
        <rdfs:subClassOf rdf:resource="http://vcd.vicomtech.org/ontology/automotive#TwoWayInterchange"/>
        <rdfs:comment>A basketweave interchange is commonly found on highways using a collector/express system or long collector/distributor lanes. In a basketweave one highway is able to interchange with itself, allowing traffic traveling in the same direction to switch between carriageways through the use of flyover/under ramps created between two carriageways without causing weaving. These interchanges usually involve left exits and entry for the outer carriageway (right in left-hand drive) but can be configured to meet on the right.</rdfs:comment>
        <rdfs:label>Basketweave interchange</rdfs:label>
    </owl:Class>
    


    <!-- http://vcd.vicomtech.org/ontology/automotive#BeaconLights -->

    <owl:Class rdf:about="http://vcd.vicomtech.org/ontology/automotive#BeaconLights">
        <rdfs:subClassOf rdf:resource="http://vcd.vicomtech.org/ontology/automotive#ArtificialLighting"/>
        <rdfs:comment>Beacon lights are positioned at the intersection of two roads to aid in navigation.</rdfs:comment>
        <rdfs:label>Beacon lights</rdfs:label>
    </owl:Class>
    


    <!-- http://vcd.vicomtech.org/ontology/automotive#Bear -->

    <owl:Class rdf:about="http://vcd.vicomtech.org/ontology/automotive#Bear">
        <rdfs:subClassOf rdf:resource="http://vcd.vicomtech.org/ontology/automotive#GroundAnimal"/>
        <rdfs:comment>A large, heavy mammal that walks on the soles of its feet, having thick fur and a very short tail. Bears are related to the dog family but most species are omnivorous.</rdfs:comment>
        <rdfs:label>Bear</rdfs:label>
    </owl:Class>
    


    <!-- http://vcd.vicomtech.org/ontology/automotive#Bench -->

    <owl:Class rdf:about="http://vcd.vicomtech.org/ontology/automotive#Bench">
        <rdfs:subClassOf rdf:resource="http://vcd.vicomtech.org/ontology/automotive#RoadsideObject"/>
        <rdfs:comment>A place to sit down.</rdfs:comment>
        <rdfs:label>Bench</rdfs:label>
    </owl:Class>
    


    <!-- http://vcd.vicomtech.org/ontology/automotive#Bendy -->

    <owl:Class rdf:about="http://vcd.vicomtech.org/ontology/automotive#Bendy">
        <rdfs:subClassOf rdf:resource="http://vcd.vicomtech.org/ontology/automotive#Bus"/>
        <rdfs:comment>An articulated vehicle used in public transportation. It is usually a single-decker, and comprises two or more rigid sections linked by a pivoting joint (articulation) enclosed by protectuve bellows inside and outside and a cover plate on the floor.</rdfs:comment>
        <rdfs:label>Bendy</rdfs:label>
    </owl:Class>
    


    <!-- http://vcd.vicomtech.org/ontology/automotive#Bicycle -->

    <owl:Class rdf:about="http://vcd.vicomtech.org/ontology/automotive#Bicycle">
        <rdfs:subClassOf rdf:resource="http://vcd.vicomtech.org/ontology/automotive#Cycle"/>
        <rdfs:comment>A vehicle consisting of two wheels held in a frame one behind the other, propelled by pedals and steered with handlebars attached to the front wheel.</rdfs:comment>
        <rdfs:label>Bicycle</rdfs:label>
    </owl:Class>
    


    <!-- http://vcd.vicomtech.org/ontology/automotive#BicycleTrailer -->

    <owl:Class rdf:about="http://vcd.vicomtech.org/ontology/automotive#BicycleTrailer">
        <rdfs:subClassOf rdf:resource="http://vcd.vicomtech.org/ontology/automotive#PushablePullable"/>
        <rdfs:comment>A trailer very similar to a cart usually designed to transport goods and or children and attached to a bicycle.</rdfs:comment>
        <rdfs:label>Bicycle trailer</rdfs:label>
    </owl:Class>
    


    <!-- http://vcd.vicomtech.org/ontology/automotive#BikeLane -->

    <owl:Class rdf:about="http://vcd.vicomtech.org/ontology/automotive#BikeLane">
        <rdfs:subClassOf rdf:resource="http://vcd.vicomtech.org/ontology/automotive#Lane"/>
        <rdfs:comment>Paved areas intended for bicycle use only. Contains only regions or ground specifically designated for cyclists where pedestrians and cars should not enter.</rdfs:comment>
        <rdfs:label>Bike lane</rdfs:label>
    </owl:Class>
    


    <!-- http://vcd.vicomtech.org/ontology/automotive#BikeRack -->

    <owl:Class rdf:about="http://vcd.vicomtech.org/ontology/automotive#BikeRack">
        <rdfs:subClassOf rdf:resource="http://vcd.vicomtech.org/ontology/automotive#RoadsideObject"/>
        <rdfs:comment>A construction to place and lock a bike.</rdfs:comment>
        <rdfs:label>Bike rack</rdfs:label>
    </owl:Class>
    


    <!-- http://vcd.vicomtech.org/ontology/automotive#Billboard -->

    <owl:Class rdf:about="http://vcd.vicomtech.org/ontology/automotive#Billboard">
        <rdfs:subClassOf rdf:resource="http://vcd.vicomtech.org/ontology/automotive#Signs"/>
        <rdfs:comment>Advertisements placed in public space and also those mounted on buildings.</rdfs:comment>
        <rdfs:label>Billboard</rdfs:label>
    </owl:Class>
    


    <!-- http://vcd.vicomtech.org/ontology/automotive#Bird -->

    <owl:Class rdf:about="http://vcd.vicomtech.org/ontology/automotive#Bird">
        <rdfs:subClassOf rdf:resource="http://vcd.vicomtech.org/ontology/automotive#Wildlife"/>
        <rdfs:comment>A creature (animal) with feathers and wings, usually able to fly. Includes birds on the ground.</rdfs:comment>
        <rdfs:label>Bird</rdfs:label>
    </owl:Class>
    


    <!-- http://vcd.vicomtech.org/ontology/automotive#Blocking -->

    <owl:Class rdf:about="http://vcd.vicomtech.org/ontology/automotive#Blocking">
        <rdfs:subClassOf rdf:resource="http://vcd.vicomtech.org/ontology/automotive#MovingManeuver"/>
        <rdfs:comment>The action or fact of blocking or obstructing someone or something.</rdfs:comment>
        <rdfs:label>Blocking</rdfs:label>
    </owl:Class>
    


    <!-- http://vcd.vicomtech.org/ontology/automotive#BlurredArea -->

    <owl:Class rdf:about="http://vcd.vicomtech.org/ontology/automotive#BlurredArea">
        <rdfs:subClassOf rdf:resource="http://vcd.vicomtech.org/ontology/automotive#Void"/>
        <rdfs:comment>An indistinct area.</rdfs:comment>
        <rdfs:label>Blurred area</rdfs:label>
    </owl:Class>
    


    <!-- http://vcd.vicomtech.org/ontology/automotive#Boat -->

    <owl:Class rdf:about="http://vcd.vicomtech.org/ontology/automotive#Boat">
        <rdfs:subClassOf rdf:resource="http://vcd.vicomtech.org/ontology/automotive#WaterVehicle"/>
        <rdfs:comment>Vehicle suitable for riding/sailing on water. Propelled by oars, sails or an engine.</rdfs:comment>
        <rdfs:label>Boat</rdfs:label>
    </owl:Class>
    


    <!-- http://vcd.vicomtech.org/ontology/automotive#BoxJunction -->

    <owl:Class rdf:about="http://vcd.vicomtech.org/ontology/automotive#BoxJunction">
        <rdfs:subClassOf rdf:resource="http://vcd.vicomtech.org/ontology/automotive#Marking"/>
        <rdfs:comment>A box junction is a road traffic control measure designed to prevent congestion and gridlock at junctions. The surface of the junction is typically marked with a yellow criss-cross grid of diagonal painted lines (or only two lines crossing each other in the box), and vehicles may not enter the area so marked unless their exit from the junction is clear, or they are intending to turn and are prevented from doing so by oncoming traffic, or other vehicles on the box waiting to turn.</rdfs:comment>
        <rdfs:label>Box junction</rdfs:label>
    </owl:Class>
    


    <!-- http://vcd.vicomtech.org/ontology/automotive#Bridge -->

    <owl:Class rdf:about="http://vcd.vicomtech.org/ontology/automotive#Bridge">
        <rdfs:subClassOf rdf:resource="http://vcd.vicomtech.org/ontology/automotive#Structure"/>
        <rdfs:comment>A structure carrying a road, path, railway, etc. across a river, road, or other obstacle.</rdfs:comment>
        <rdfs:label>Bridge</rdfs:label>
    </owl:Class>
    


    <!-- http://vcd.vicomtech.org/ontology/automotive#BrokenStop -->

    <owl:Class rdf:about="http://vcd.vicomtech.org/ontology/automotive#BrokenStop">
        <rdfs:subClassOf rdf:resource="http://vcd.vicomtech.org/ontology/automotive#WhiteLines"/>
        <rdfs:label>Broken stop</rdfs:label>
    </owl:Class>
    


    <!-- http://vcd.vicomtech.org/ontology/automotive#Building -->

    <owl:Class rdf:about="http://vcd.vicomtech.org/ontology/automotive#Building">
        <rdfs:subClassOf rdf:resource="http://vcd.vicomtech.org/ontology/automotive#Structure"/>
        <rdfs:comment>A structure with a roof and walls, such as a house or factory.</rdfs:comment>
        <rdfs:label>Building</rdfs:label>
    </owl:Class>
    


    <!-- http://vcd.vicomtech.org/ontology/automotive#Bump -->

    <owl:Class rdf:about="http://vcd.vicomtech.org/ontology/automotive#Bump">
        <rdfs:subClassOf rdf:resource="http://vcd.vicomtech.org/ontology/automotive#Marking"/>
        <rdfs:comment>A marking indicating speed reduction.</rdfs:comment>
        <rdfs:label>Bump</rdfs:label>
    </owl:Class>
    


    <!-- http://vcd.vicomtech.org/ontology/automotive#Bus -->

    <owl:Class rdf:about="http://vcd.vicomtech.org/ontology/automotive#Bus">
        <rdfs:subClassOf rdf:resource="http://vcd.vicomtech.org/ontology/automotive#LargeVehicle"/>
        <rdfs:comment>A large motor vehicle, having a long body, equipped with seats or benches for passengers, usually operating as part of a scheduled service; omnibus.</rdfs:comment>
        <rdfs:label>Bus</rdfs:label>
    </owl:Class>
    


    <!-- http://vcd.vicomtech.org/ontology/automotive#Bush -->

    <owl:Class rdf:about="http://vcd.vicomtech.org/ontology/automotive#Bush">
        <rdfs:subClassOf rdf:resource="http://vcd.vicomtech.org/ontology/automotive#Vegetation"/>
        <rdfs:comment>A shrub or clump of shrubs with stems of moderate length.</rdfs:comment>
        <rdfs:label>Bush</rdfs:label>
    </owl:Class>
    


    <!-- http://vcd.vicomtech.org/ontology/automotive#CamperVan -->

    <owl:Class rdf:about="http://vcd.vicomtech.org/ontology/automotive#CamperVan">
        <rdfs:subClassOf rdf:resource="http://vcd.vicomtech.org/ontology/automotive#DrivableVehicle"/>
        <rdfs:comment>A large motor vehicle with living accommodation.</rdfs:comment>
        <rdfs:label>Camper van</rdfs:label>
    </owl:Class>
    


    <!-- http://vcd.vicomtech.org/ontology/automotive#Car -->

    <owl:Class rdf:about="http://vcd.vicomtech.org/ontology/automotive#Car">
        <rdfs:subClassOf rdf:resource="http://vcd.vicomtech.org/ontology/automotive#SmallVehicle"/>
        <rdfs:comment>A road vehicle with an engine, four wheels, and seats for a small number of people.</rdfs:comment>
        <rdfs:label>Car</rdfs:label>
    </owl:Class>
    


    <!-- http://vcd.vicomtech.org/ontology/automotive#CarMount -->

    <owl:Class rdf:about="http://vcd.vicomtech.org/ontology/automotive#CarMount">
        <rdfs:subClassOf rdf:resource="http://vcd.vicomtech.org/ontology/automotive#Void"/>
        <rdfs:comment>Mount used to hold the camera while capturing.</rdfs:comment>
        <rdfs:label>Car mount</rdfs:label>
    </owl:Class>
    


    <!-- http://vcd.vicomtech.org/ontology/automotive#Caravan -->

    <owl:Class rdf:about="http://vcd.vicomtech.org/ontology/automotive#Caravan">
        <rdfs:subClassOf rdf:resource="http://vcd.vicomtech.org/ontology/automotive#Trailer"/>
        <rdfs:comment>A road vehicle equipped for living in, typically towed by a car and used for holidays.</rdfs:comment>
        <rdfs:label>Caravan</rdfs:label>
    </owl:Class>
    


    <!-- http://vcd.vicomtech.org/ontology/automotive#Cargo -->

    <owl:Class rdf:about="http://vcd.vicomtech.org/ontology/automotive#Cargo">
        <rdfs:subClassOf rdf:resource="http://vcd.vicomtech.org/ontology/automotive#Trailer"/>
        <rdfs:comment>A (usually big) non-motorized vehicle designed to carry goods/animals and other vehicles (almost always without passengers) which is generally pulled by a motorized vehicle</rdfs:comment>
        <rdfs:label>Cargo</rdfs:label>
    </owl:Class>
    


    <!-- http://vcd.vicomtech.org/ontology/automotive#Cart -->

    <owl:Class rdf:about="http://vcd.vicomtech.org/ontology/automotive#Cart">
        <rdfs:subClassOf rdf:resource="http://vcd.vicomtech.org/ontology/automotive#PushablePullable"/>
        <rdfs:comment>A basket or board on wheels used for carrying goods and objects and be pushed or pulled by humans.</rdfs:comment>
        <rdfs:label>Cart</rdfs:label>
    </owl:Class>
    


    <!-- http://vcd.vicomtech.org/ontology/automotive#Cat -->

    <owl:Class rdf:about="http://vcd.vicomtech.org/ontology/automotive#Cat">
        <rdfs:subClassOf rdf:resource="http://vcd.vicomtech.org/ontology/automotive#Pet"/>
        <rdfs:comment>Cats are considered pets</rdfs:comment>
        <rdfs:label>Cat</rdfs:label>
    </owl:Class>
    


    <!-- http://vcd.vicomtech.org/ontology/automotive#CatchBasin -->

    <owl:Class rdf:about="http://vcd.vicomtech.org/ontology/automotive#CatchBasin">
        <rdfs:subClassOf rdf:resource="http://vcd.vicomtech.org/ontology/automotive#RoadsideObject"/>
        <rdfs:comment>Sewage water draigane, typically with a grid on top or inlet of a curb.</rdfs:comment>
        <rdfs:label>Catch basin</rdfs:label>
    </owl:Class>
    


    <!-- http://vcd.vicomtech.org/ontology/automotive#CctvCamera -->

    <owl:Class rdf:about="http://vcd.vicomtech.org/ontology/automotive#CctvCamera">
        <rdfs:subClassOf rdf:resource="http://vcd.vicomtech.org/ontology/automotive#RoadsideObject"/>
        <rdfs:comment>Surveillance camera mounted in public space.</rdfs:comment>
        <rdfs:label>CCTV camera</rdfs:label>
    </owl:Class>
    


    <!-- http://vcd.vicomtech.org/ontology/automotive#ChangeState -->

    <owl:Class rdf:about="http://vcd.vicomtech.org/ontology/automotive#ChangeState">
        <rdfs:subClassOf rdf:resource="http://vcd.vicomtech.org/ontology/automotive#Event"/>
        <rdfs:label>Change state</rdfs:label>
    </owl:Class>
    


    <!-- http://vcd.vicomtech.org/ontology/automotive#ChangeTrafficLightState -->

    <owl:Class rdf:about="http://vcd.vicomtech.org/ontology/automotive#ChangeTrafficLightState">
        <rdfs:subClassOf rdf:resource="http://vcd.vicomtech.org/ontology/automotive#ChangeState"/>
        <rdfs:comment>When a traffic light changes its color.</rdfs:comment>
        <rdfs:label>Change traffic light state</rdfs:label>
    </owl:Class>
    


    <!-- http://vcd.vicomtech.org/ontology/automotive#Child -->

    <owl:Class rdf:about="http://vcd.vicomtech.org/ontology/automotive#Child">
        <rdfs:subClassOf rdf:resource="http://vcd.vicomtech.org/ontology/automotive#Pedestrian"/>
        <rdfs:comment>A young human being below the age of puberty or below the legal age of majority.</rdfs:comment>
        <rdfs:label>Child</rdfs:label>
    </owl:Class>
    


    <!-- http://vcd.vicomtech.org/ontology/automotive#ChildRider -->

    <owl:Class rdf:about="http://vcd.vicomtech.org/ontology/automotive#ChildRider">
        <rdfs:subClassOf rdf:resource="http://vcd.vicomtech.org/ontology/automotive#Rider"/>
        <rdfs:comment>Any person about younger than 8 that is riding a ridable vehicle.</rdfs:comment>
        <rdfs:label>Child rider</rdfs:label>
    </owl:Class>
    


    <!-- http://vcd.vicomtech.org/ontology/automotive#ChildWithObject -->

    <owl:Class rdf:about="http://vcd.vicomtech.org/ontology/automotive#ChildWithObject">
        <rdfs:subClassOf rdf:resource="http://vcd.vicomtech.org/ontology/automotive#PedestrianWithObject"/>
        <rdfs:comment>Any person about younger than 8 years that is carrying an object while acting as a pedestrian in the surroundings of the vehicle.</rdfs:comment>
        <rdfs:label>Child with Object</rdfs:label>
    </owl:Class>
    


    <!-- http://vcd.vicomtech.org/ontology/automotive#City -->

    <owl:Class rdf:about="http://vcd.vicomtech.org/ontology/automotive#City">
        <rdfs:subClassOf rdf:resource="http://vcd.vicomtech.org/ontology/automotive#Environment"/>
        <rdfs:comment>A city is an area in which a large number of people live fairly close together.</rdfs:comment>
        <rdfs:label>City</rdfs:label>
    </owl:Class>
    


    <!-- http://vcd.vicomtech.org/ontology/automotive#Cloud -->

    <owl:Class rdf:about="http://vcd.vicomtech.org/ontology/automotive#Cloud">
        <rdfs:subClassOf rdf:resource="http://vcd.vicomtech.org/ontology/automotive#Weather"/>
        <rdfs:comment>Full of or overcast by clouds which causes having little or no sunshine.</rdfs:comment>
        <rdfs:label>Cloud</rdfs:label>
    </owl:Class>
    


    <!-- http://vcd.vicomtech.org/ontology/automotive#Cloudy -->

    <owl:Class rdf:about="http://vcd.vicomtech.org/ontology/automotive#Cloudy">
        <rdfs:subClassOf rdf:resource="http://vcd.vicomtech.org/ontology/automotive#DiffusedSunlight"/>
        <rdfs:comment>When the sunlight is blocked by clouds.</rdfs:comment>
        <rdfs:label>Cloudy</rdfs:label>
    </owl:Class>
    


    <!-- http://vcd.vicomtech.org/ontology/automotive#CloverleafInterchange -->

    <owl:Class rdf:about="http://vcd.vicomtech.org/ontology/automotive#CloverleafInterchange">
        <rdfs:subClassOf rdf:resource="http://vcd.vicomtech.org/ontology/automotive#FourWayInterchange"/>
        <rdfs:comment>A cloverleaf interchange is typically a two-level, four-way interchange where all turns across opposing traffic are handled by non-directional loop ramps. Assuming right-handed traffic, to go left vehicles first cross over or under the target route, then bear right onto a sharply curved ramp that turns roughly 270 degrees, merging onto the target route from the right, and crossing the route just departed. These loop ramps produce the namesake cloverleaf shape.</rdfs:comment>
        <rdfs:label>Cloverleaf interchange</rdfs:label>
    </owl:Class>
    


    <!-- http://vcd.vicomtech.org/ontology/automotive#CloverstackInterchange -->

    <owl:Class rdf:about="http://vcd.vicomtech.org/ontology/automotive#CloverstackInterchange">
        <rdfs:subClassOf rdf:resource="http://vcd.vicomtech.org/ontology/automotive#FourWayInterchange"/>
        <rdfs:comment>Cloverstack interchanges are hybrid interchanges, using loop ramps like cloverleafs to serve slower or less occupied traffic flow and flyover ramps like stack interchanges to serve faster and higher occupied traffic flow. If local and express ways serving the same directions and each roadway is connected righthand to the interchange, extra ramps are installed.</rdfs:comment>
        <rdfs:label>Cloverstack interchange</rdfs:label>
    </owl:Class>
    


    <!-- http://vcd.vicomtech.org/ontology/automotive#Coach -->

    <owl:Class rdf:about="http://vcd.vicomtech.org/ontology/automotive#Coach">
        <rdfs:subClassOf rdf:resource="http://vcd.vicomtech.org/ontology/automotive#LargeVehicle"/>
        <rdfs:comment>Coach is similar to a bus: a large vehicle destined to transportation of passengers, but it is designed for extraurban long distance journey. Coaches have usually smaller doors than urban buses and accomodate only for seated passengers. Coaches usually travel on highway and does not have the typical stop and go behavior of urban buses within urban environments.</rdfs:comment>
        <rdfs:label>Coach</rdfs:label>
    </owl:Class>
    


    <!-- http://vcd.vicomtech.org/ontology/automotive#Colliding -->

    <owl:Class rdf:about="http://vcd.vicomtech.org/ontology/automotive#Colliding">
        <rdfs:subClassOf rdf:resource="http://vcd.vicomtech.org/ontology/automotive#MovingManeuver"/>
        <rdfs:comment>An instance of one moving object or person striking violently against another or any other object of the scene.</rdfs:comment>
        <rdfs:label>Colliding</rdfs:label>
    </owl:Class>
    


    <!-- http://vcd.vicomtech.org/ontology/automotive#Collision -->

    <owl:Class rdf:about="http://vcd.vicomtech.org/ontology/automotive#Collision">
        <rdfs:subClassOf rdf:resource="http://vcd.vicomtech.org/ontology/automotive#Event"/>
        <rdfs:comment>An instance of one moving object or person striking violently against another or any other object of the scene.</rdfs:comment>
        <rdfs:label>Collision</rdfs:label>
    </owl:Class>
    


    <!-- http://vcd.vicomtech.org/ontology/automotive#Construction -->

    <owl:Class rdf:about="http://vcd.vicomtech.org/ontology/automotive#Construction">
        <rdfs:subClassOf rdf:resource="http://vcd.vicomtech.org/ontology/automotive#Static"/>
        <rdfs:comment>A building or other structure.</rdfs:comment>
        <rdfs:label>Construction</rdfs:label>
    </owl:Class>
    


    <!-- http://vcd.vicomtech.org/ontology/automotive#ConstructionSign -->

    <owl:Class rdf:about="http://vcd.vicomtech.org/ontology/automotive#ConstructionSign">
        <rdfs:subClassOf rdf:resource="http://vcd.vicomtech.org/ontology/automotive#TrafficDevice"/>
        <rdfs:comment>Construction sign shall mean any temporary on premise sign located upon a site where construction or landscaping is in progress and relating specifically to the project which is under construction.</rdfs:comment>
        <rdfs:label>Construction sign</rdfs:label>
    </owl:Class>
    


    <!-- http://vcd.vicomtech.org/ontology/automotive#ConstructionVehicle -->

    <owl:Class rdf:about="http://vcd.vicomtech.org/ontology/automotive#ConstructionVehicle">
        <rdfs:subClassOf rdf:resource="http://vcd.vicomtech.org/ontology/automotive#DrivableVehicle"/>
        <rdfs:comment>Refers to heavy-duty vehicles, specially designed for executing construction tasks.</rdfs:comment>
        <rdfs:label>Construction vehicle</rdfs:label>
    </owl:Class>
    


    <!-- http://vcd.vicomtech.org/ontology/automotive#ConstructionWorker -->

    <owl:Class rdf:about="http://vcd.vicomtech.org/ontology/automotive#ConstructionWorker">
        <rdfs:subClassOf rdf:resource="http://vcd.vicomtech.org/ontology/automotive#Adult"/>
        <rdfs:comment>A person (Human) who works in the construction industry.</rdfs:comment>
        <rdfs:label>Construction worker</rdfs:label>
    </owl:Class>
    


    <!-- http://vcd.vicomtech.org/ontology/automotive#Context -->

    <owl:Class rdf:about="http://vcd.vicomtech.org/ontology/automotive#Context">
        <rdfs:subClassOf rdf:resource="http://www.w3.org/2002/07/owl#Thing"/>
        <rdfs:comment>Context is any information that can be used to characterise the sit-uation of an entity. An entity is a person, place, or object that isconsidered relevant in an Scenario.</rdfs:comment>
        <rdfs:label>Context</rdfs:label>
    </owl:Class>
    


    <!-- http://vcd.vicomtech.org/ontology/automotive#Convertible -->

    <owl:Class rdf:about="http://vcd.vicomtech.org/ontology/automotive#Convertible">
        <rdfs:subClassOf rdf:resource="http://vcd.vicomtech.org/ontology/automotive#Car"/>
        <rdfs:comment>A convertible, cabriolet or spyder/spider is a passenger car that can be driven with or without a roof in place. The methods of retracting and storing the roof vary between models. A convertible allows an open-air driving experience, with the ability to provide a roof when required. Usually can accomodate 2 passengers comfortably. Most Convertibles are designed for 4/5 passengers though.</rdfs:comment>
        <rdfs:label>Convertible</rdfs:label>
    </owl:Class>
    


    <!-- http://vcd.vicomtech.org/ontology/automotive#Country -->

    <owl:Class rdf:about="http://vcd.vicomtech.org/ontology/automotive#Country">
        <rdfs:subClassOf rdf:resource="http://vcd.vicomtech.org/ontology/automotive#Context"/>
        <rdfs:comment>The recognized boundaries of a formal sub-division of a country.</rdfs:comment>
        <rdfs:label>Country</rdfs:label>
    </owl:Class>
    


    <!-- http://vcd.vicomtech.org/ontology/automotive#Cross -->

    <owl:Class rdf:about="http://vcd.vicomtech.org/ontology/automotive#Cross">
        <rdfs:subClassOf rdf:resource="http://vcd.vicomtech.org/ontology/automotive#Event"/>
        <rdfs:comment>To move from one side to the other of either a juntion or a crosswalk.</rdfs:comment>
        <rdfs:label>Cross</rdfs:label>
    </owl:Class>
    


    <!-- http://vcd.vicomtech.org/ontology/automotive#Crossing -->

    <owl:Class rdf:about="http://vcd.vicomtech.org/ontology/automotive#Crossing">
        <rdfs:subClassOf rdf:resource="http://vcd.vicomtech.org/ontology/automotive#MovingManeuver"/>
        <rdfs:comment>The action of crossing either a juntion or a crosswalk.</rdfs:comment>
        <rdfs:label>Crossing</rdfs:label>
    </owl:Class>
    


    <!-- http://vcd.vicomtech.org/ontology/automotive#Crosswalk -->

    <owl:Class rdf:about="http://vcd.vicomtech.org/ontology/automotive#Crosswalk">
        <rdfs:subClassOf rdf:resource="http://vcd.vicomtech.org/ontology/automotive#Marking"/>
        <rdfs:comment>A marked part of a road where pedestrians have right of way to cross; a pedestrian crossing.</rdfs:comment>
        <rdfs:label>Crosswalk</rdfs:label>
    </owl:Class>
    


    <!-- http://vcd.vicomtech.org/ontology/automotive#CrosswalkPlain -->

    <owl:Class rdf:about="http://vcd.vicomtech.org/ontology/automotive#CrosswalkPlain">
        <rdfs:subClassOf rdf:resource="http://vcd.vicomtech.org/ontology/automotive#Crosswalk"/>
        <rdfs:comment>Region of a road which is meant to cross the street but not marked with a zebra pattern, instead two parallel lines indicate the crosswalk. The road surface is marked as plain crosswalk, the two lines indicating the border are marked as general markings.</rdfs:comment>
        <rdfs:label>Crosswalk plain</rdfs:label>
    </owl:Class>
    


    <!-- http://vcd.vicomtech.org/ontology/automotive#CrosswalkZebra -->

    <owl:Class rdf:about="http://vcd.vicomtech.org/ontology/automotive#CrosswalkZebra">
        <rdfs:subClassOf rdf:resource="http://vcd.vicomtech.org/ontology/automotive#Crosswalk"/>
        <rdfs:comment>Crosswalk indicated by a zebra pattern.</rdfs:comment>
        <rdfs:label>Crosswalk zebra</rdfs:label>
    </owl:Class>
    


    <!-- http://vcd.vicomtech.org/ontology/automotive#CurbCut -->

    <owl:Class rdf:about="http://vcd.vicomtech.org/ontology/automotive#CurbCut">
        <rdfs:subClassOf rdf:resource="http://vcd.vicomtech.org/ontology/automotive#Flat"/>
        <rdfs:comment>Lowered curbs or curb cuts which can be driven over.</rdfs:comment>
        <rdfs:label>Curb cut</rdfs:label>
    </owl:Class>
    


    <!-- http://vcd.vicomtech.org/ontology/automotive#Curbstone -->

    <owl:Class rdf:about="http://vcd.vicomtech.org/ontology/automotive#Curbstone">
        <rdfs:subClassOf rdf:resource="http://vcd.vicomtech.org/ontology/automotive#RoadsideObject"/>
        <rdfs:comment>A long, narrow stone or concrete block, laid end to end with others to form a kerb.  variant spelling of kerbstone.</rdfs:comment>
        <rdfs:label>Curbstone</rdfs:label>
    </owl:Class>
    


    <!-- http://vcd.vicomtech.org/ontology/automotive#Curve -->

    <owl:Class rdf:about="http://vcd.vicomtech.org/ontology/automotive#Curve">
        <rdfs:subClassOf rdf:resource="http://vcd.vicomtech.org/ontology/automotive#Barrier"/>
        <rdfs:subClassOf rdf:resource="http://vcd.vicomtech.org/ontology/automotive#Junction"/>
        <rdfs:comment>Is the edge where a raised sidewalk or road median/central reservation meets a street or other roadway.</rdfs:comment>
        <rdfs:label>Curve</rdfs:label>
    </owl:Class>
    


    <!-- http://vcd.vicomtech.org/ontology/automotive#CuttingIn -->

    <owl:Class rdf:about="http://vcd.vicomtech.org/ontology/automotive#CuttingIn">
        <rdfs:subClassOf rdf:resource="http://vcd.vicomtech.org/ontology/automotive#MovingManeuver"/>
        <rdfs:comment>Is a lane change maneuver where the target vehicle moves into the space ahead of a relatively closely following vehicle in the adjacent lane.</rdfs:comment>
        <rdfs:label>Cutting-in</rdfs:label>
    </owl:Class>
    


    <!-- http://vcd.vicomtech.org/ontology/automotive#CuttingOut -->

    <owl:Class rdf:about="http://vcd.vicomtech.org/ontology/automotive#CuttingOut">
        <rdfs:subClassOf rdf:resource="http://vcd.vicomtech.org/ontology/automotive#MovingManeuver"/>
        <rdfs:comment>When a vehicle in the middle of the platoon decides to leave and the following one has to cover the cut-out vehicle gap.</rdfs:comment>
        <rdfs:label>Cutting-out</rdfs:label>
    </owl:Class>
    


    <!-- http://vcd.vicomtech.org/ontology/automotive#Cycle -->

    <owl:Class rdf:about="http://vcd.vicomtech.org/ontology/automotive#Cycle">
        <rdfs:subClassOf rdf:resource="http://vcd.vicomtech.org/ontology/automotive#RoadVehicle"/>
        <rdfs:comment>A ridable vehicle, this is, any vehicle that, in order to be controlled, requires the rider to take a sitting position and use not only designated control devices such as handlebars or steering wheels, but also bodyweight as an effective mean of exerting control. Moreover, Ridable vehicles do not offer any (or barely any) structural protection to the rider and passengers. Ridable vehicles most often have 2 wheels, occasionally more.</rdfs:comment>
        <rdfs:label>Cycle</rdfs:label>
    </owl:Class>
    


    <!-- http://vcd.vicomtech.org/ontology/automotive#Cyclist -->

    <owl:Class rdf:about="http://vcd.vicomtech.org/ontology/automotive#Cyclist">
        <rdfs:subClassOf rdf:resource="http://vcd.vicomtech.org/ontology/automotive#Rider"/>
        <rdfs:comment>A person who rides a bicycle. Dows not include the bicycle or persons moving a bike while walking.</rdfs:comment>
        <rdfs:label>Cyclist</rdfs:label>
    </owl:Class>
    


    <!-- http://vcd.vicomtech.org/ontology/automotive#Daylight -->

    <owl:Class rdf:about="http://vcd.vicomtech.org/ontology/automotive#Daylight">
        <rdfs:subClassOf rdf:resource="http://vcd.vicomtech.org/ontology/automotive#Lighting"/>
        <rdfs:comment>The natural light being the main source of light during daytime.</rdfs:comment>
        <rdfs:label>Daylight</rdfs:label>
    </owl:Class>
    


    <!-- http://vcd.vicomtech.org/ontology/automotive#Daytime -->

    <owl:Class rdf:about="http://vcd.vicomtech.org/ontology/automotive#Daytime">
        <rdfs:subClassOf rdf:resource="http://vcd.vicomtech.org/ontology/automotive#TimeOfDay"/>
        <rdfs:comment>Daytime is from sunrise to sunset.</rdfs:comment>
        <rdfs:label>Daytime</rdfs:label>
    </owl:Class>
    


    <!-- http://vcd.vicomtech.org/ontology/automotive#Debris -->

    <owl:Class rdf:about="http://vcd.vicomtech.org/ontology/automotive#Debris">
        <rdfs:subClassOf rdf:resource="http://vcd.vicomtech.org/ontology/automotive#MovableObject"/>
        <rdfs:comment>Scattered pieces of rubbish or remains. Loose natural material consisting especially of broken pieces of rock.</rdfs:comment>
        <rdfs:label>Debris</rdfs:label>
    </owl:Class>
    


    <!-- http://vcd.vicomtech.org/ontology/automotive#Decelerating -->

    <owl:Class rdf:about="http://vcd.vicomtech.org/ontology/automotive#Decelerating">
        <rdfs:subClassOf rdf:resource="http://vcd.vicomtech.org/ontology/automotive#MovingManeuver"/>
        <rdfs:comment>To reduce the speed that a vehicle is travelling at.</rdfs:comment>
        <rdfs:label>Decelerating</rdfs:label>
    </owl:Class>
    


    <!-- http://vcd.vicomtech.org/ontology/automotive#Deer -->

    <owl:Class rdf:about="http://vcd.vicomtech.org/ontology/automotive#Deer">
        <rdfs:subClassOf rdf:resource="http://vcd.vicomtech.org/ontology/automotive#GroundAnimal"/>
        <rdfs:comment>A hoofed grazing or browsing animal, with branched bony antlers that are shed annually and typically borne only by the male.</rdfs:comment>
        <rdfs:label>Deer</rdfs:label>
    </owl:Class>
    


    <!-- http://vcd.vicomtech.org/ontology/automotive#Detect -->

    <owl:Class rdf:about="http://vcd.vicomtech.org/ontology/automotive#Detect">
        <rdfs:subClassOf rdf:resource="http://vcd.vicomtech.org/ontology/automotive#Event"/>
        <rdfs:comment>When a sensor discovers or identifies the presence or existence of an object.</rdfs:comment>
        <rdfs:label>Detect</rdfs:label>
    </owl:Class>
    


    <!-- http://vcd.vicomtech.org/ontology/automotive#DiamondInterchange -->

    <owl:Class rdf:about="http://vcd.vicomtech.org/ontology/automotive#DiamondInterchange">
        <rdfs:subClassOf rdf:resource="http://vcd.vicomtech.org/ontology/automotive#ServiceInterchange"/>
        <rdfs:comment>A diamond interchange is a common type of road junction, used where a controlled-access highway crosses a minor road.</rdfs:comment>
        <rdfs:label>Diamond interchange</rdfs:label>
    </owl:Class>
    


    <!-- http://vcd.vicomtech.org/ontology/automotive#DiffusedSunlight -->

    <owl:Class rdf:about="http://vcd.vicomtech.org/ontology/automotive#DiffusedSunlight">
        <rdfs:subClassOf rdf:resource="http://vcd.vicomtech.org/ontology/automotive#Daylight"/>
        <rdfs:comment>Sunlight that is scattered in the atmosphere is &quot;diffused daylight&quot;. Sunlight reflected off walls and the ground also contributes to daylight.</rdfs:comment>
        <rdfs:label>Diffused sunlight</rdfs:label>
    </owl:Class>
    


    <!-- http://vcd.vicomtech.org/ontology/automotive#DirectSunlight -->

    <owl:Class rdf:about="http://vcd.vicomtech.org/ontology/automotive#DirectSunlight">
        <rdfs:subClassOf rdf:resource="http://vcd.vicomtech.org/ontology/automotive#Daylight"/>
        <rdfs:comment>&quot;Direct sunlight&quot; reaches a site without being scattered within Earth&apos;s atmosphere.</rdfs:comment>
        <rdfs:label>Direct sunlight</rdfs:label>
    </owl:Class>
    


    <!-- http://vcd.vicomtech.org/ontology/automotive#DivergingDiamongInterchange -->

    <owl:Class rdf:about="http://vcd.vicomtech.org/ontology/automotive#DivergingDiamongInterchange">
        <rdfs:subClassOf rdf:resource="http://vcd.vicomtech.org/ontology/automotive#ServiceInterchange"/>
        <rdfs:comment>In a diverging diamond interchange (DDI) or (DCD), the two directions of traffic on the non-freeway road cross to the opposite side on both sides of the bridge at the freeway to save the third traffic signal phase.</rdfs:comment>
        <rdfs:label>Diverging diamond interchange</rdfs:label>
    </owl:Class>
    


    <!-- http://vcd.vicomtech.org/ontology/automotive#Dog -->

    <owl:Class rdf:about="http://vcd.vicomtech.org/ontology/automotive#Dog">
        <rdfs:subClassOf rdf:resource="http://vcd.vicomtech.org/ontology/automotive#Pet"/>
        <rdfs:comment>Dogs are considered pets</rdfs:comment>
        <rdfs:label>Dog</rdfs:label>
    </owl:Class>
    


    <!-- http://vcd.vicomtech.org/ontology/automotive#DogboneInterchange -->

    <owl:Class rdf:about="http://vcd.vicomtech.org/ontology/automotive#DogboneInterchange">
        <rdfs:subClassOf rdf:resource="http://vcd.vicomtech.org/ontology/automotive#DiamondInterchange"/>
        <rdfs:comment>A variation of the dumbbell interchange, occurs when the roundabouts do not form a complete circle but instead have a &quot;raindrop&quot; or &quot;teardrop&quot; shape. These two raindrop roundabouts are fused together, forming a single &quot;squashed&quot; roundabout. This configuration reduces conflicts between vehicles entering the raindrop roundabouts from the ramps, reducing queueing and delays, compared with the dumbbell interchange. Direct U-turns are not possible, although the movement can be made by circulating around both raindrop roundabouts.</rdfs:comment>
        <rdfs:label>Dogbone interchange</rdfs:label>
    </owl:Class>
    


    <!-- http://vcd.vicomtech.org/ontology/automotive#DonkeyCarriage -->

    <owl:Class rdf:about="http://vcd.vicomtech.org/ontology/automotive#DonkeyCarriage">
        <rdfs:subClassOf rdf:resource="http://vcd.vicomtech.org/ontology/automotive#AnimalPulled"/>
        <rdfs:comment>Any vehicle carried by a donkey or a group of donkeys.</rdfs:comment>
        <rdfs:label>Donkey-carriage</rdfs:label>
    </owl:Class>
    


    <!-- http://vcd.vicomtech.org/ontology/automotive#DontCare -->

    <owl:Class rdf:about="http://vcd.vicomtech.org/ontology/automotive#DontCare">
        <rdfs:subClassOf rdf:resource="http://vcd.vicomtech.org/ontology/automotive#Object"/>
        <rdfs:label>Dont care</rdfs:label>
    </owl:Class>
    


    <!-- http://vcd.vicomtech.org/ontology/automotive#DoubleBrokenWhite -->

    <owl:Class rdf:about="http://vcd.vicomtech.org/ontology/automotive#DoubleBrokenWhite">
        <rdfs:subClassOf rdf:resource="http://vcd.vicomtech.org/ontology/automotive#WhiteLines"/>
        <rdfs:comment>A double row of thicker short broken lines can be seen on a major road indicating that you need to give way they can also be used at mini-roundabouts.</rdfs:comment>
        <rdfs:label>Double broken white</rdfs:label>
    </owl:Class>
    


    <!-- http://vcd.vicomtech.org/ontology/automotive#DoubleBrokenYellow -->

    <owl:Class rdf:about="http://vcd.vicomtech.org/ontology/automotive#DoubleBrokenYellow">
        <rdfs:subClassOf rdf:resource="http://vcd.vicomtech.org/ontology/automotive#YellowLines"/>
        <rdfs:comment>A double row of thicker short broken lines can be seen on a major road indicating that you need to give way they can also be used at mini-roundabouts.</rdfs:comment>
        <rdfs:label>Double broken yellow</rdfs:label>
    </owl:Class>
    


    <!-- http://vcd.vicomtech.org/ontology/automotive#DoubleSolidWhite -->

    <owl:Class rdf:about="http://vcd.vicomtech.org/ontology/automotive#DoubleSolidWhite">
        <rdfs:subClassOf rdf:resource="http://vcd.vicomtech.org/ontology/automotive#WhiteLines"/>
        <rdfs:comment>Two solid lines that indicate a lane barrier between a regular use and a preferential use lane, such as a carpool/HOV. Never change lanes while in these lanes.</rdfs:comment>
        <rdfs:label>Double solid white</rdfs:label>
    </owl:Class>
    


    <!-- http://vcd.vicomtech.org/ontology/automotive#DoubleSolidYellow -->

    <owl:Class rdf:about="http://vcd.vicomtech.org/ontology/automotive#DoubleSolidYellow">
        <rdfs:subClassOf rdf:resource="http://vcd.vicomtech.org/ontology/automotive#YellowLines"/>
        <rdfs:comment>Two solid lines that indicate a lane barrier between a regular use and a preferential use lane, such as a carpool/HOV. Never change lanes while in these lanes.</rdfs:comment>
        <rdfs:label>Double solid yellow</rdfs:label>
    </owl:Class>
    


    <!-- http://vcd.vicomtech.org/ontology/automotive#DrivableCobblestone -->

    <owl:Class rdf:about="http://vcd.vicomtech.org/ontology/automotive#DrivableCobblestone">
        <rdfs:subClassOf rdf:resource="http://vcd.vicomtech.org/ontology/automotive#RoadSurface"/>
        <rdfs:comment>A road with a surface formed by naturally rounded stones.</rdfs:comment>
        <rdfs:label>Drivable cobblestone</rdfs:label>
    </owl:Class>
    


    <!-- http://vcd.vicomtech.org/ontology/automotive#DrivableVehicle -->

    <owl:Class rdf:about="http://vcd.vicomtech.org/ontology/automotive#DrivableVehicle">
        <rdfs:subClassOf rdf:resource="http://vcd.vicomtech.org/ontology/automotive#RoadVehicle"/>
        <rdfs:comment>It is considered a drivable vehicle any vehicle that offers significant structural protection to the driver and the other occupants. It is composed by a chassis and a body structure closed on all four sides. 
in order to be controlled, it usually requires the driver to adopt a sitting position and act on pedals and a steering wheel. Drivable vehicles have usually 4 or more wheels and motorized propulsion.</rdfs:comment>
        <rdfs:label>Drivable vehicle</rdfs:label>
    </owl:Class>
    


    <!-- http://vcd.vicomtech.org/ontology/automotive#Driveaway -->

    <owl:Class rdf:about="http://vcd.vicomtech.org/ontology/automotive#Driveaway">
        <rdfs:subClassOf rdf:resource="http://vcd.vicomtech.org/ontology/automotive#Event"/>
        <rdfs:comment>The action perforned when a vehicle starts moving.</rdfs:comment>
        <rdfs:label>Driveaway</rdfs:label>
    </owl:Class>
    


    <!-- http://vcd.vicomtech.org/ontology/automotive#DrivingInOppositeDirection -->

    <owl:Class rdf:about="http://vcd.vicomtech.org/ontology/automotive#DrivingInOppositeDirection">
        <rdfs:subClassOf rdf:resource="http://vcd.vicomtech.org/ontology/automotive#MovingManeuver"/>
        <rdfs:comment>To move in the opposite direction with reference to the ego-vehicle.</rdfs:comment>
        <rdfs:label>Driving in opposite direction</rdfs:label>
    </owl:Class>
    


    <!-- http://vcd.vicomtech.org/ontology/automotive#DrivingStraight -->

    <owl:Class rdf:about="http://vcd.vicomtech.org/ontology/automotive#DrivingStraight">
        <rdfs:subClassOf rdf:resource="http://vcd.vicomtech.org/ontology/automotive#MovingManeuver"/>
        <rdfs:comment>The action of driving following the current road path.</rdfs:comment>
        <rdfs:label>Driving straight</rdfs:label>
    </owl:Class>
    


    <!-- http://vcd.vicomtech.org/ontology/automotive#Duck -->

    <owl:Class rdf:about="http://vcd.vicomtech.org/ontology/automotive#Duck">
        <rdfs:subClassOf rdf:resource="http://vcd.vicomtech.org/ontology/automotive#Bird"/>
        <rdfs:comment>A waterbird with a broad blunt bill, short legs, webbed feet, and a waddling gait.</rdfs:comment>
        <rdfs:label>Duck</rdfs:label>
    </owl:Class>
    


    <!-- http://vcd.vicomtech.org/ontology/automotive#DumbbellInterchange -->

    <owl:Class rdf:about="http://vcd.vicomtech.org/ontology/automotive#DumbbellInterchange">
        <rdfs:subClassOf rdf:resource="http://vcd.vicomtech.org/ontology/automotive#DiamondInterchange"/>
        <rdfs:comment>Sometimes called a double roundabout interchange. This configuration allows other roads to form approach legs to the roundabouts and also allows easy U-turns.</rdfs:comment>
        <rdfs:label>Dumbbell interchange</rdfs:label>
    </owl:Class>
    


    <!-- http://vcd.vicomtech.org/ontology/automotive#Dust -->

    <owl:Class rdf:about="http://vcd.vicomtech.org/ontology/automotive#Dust">
        <rdfs:subClassOf rdf:resource="http://vcd.vicomtech.org/ontology/automotive#Air"/>
        <rdfs:comment>Fine, dry powder consisting of tiny particles of earth or waste matter lying on the ground or on surfaces or carried in the air.</rdfs:comment>
        <rdfs:label>Dust</rdfs:label>
    </owl:Class>
    


    <!-- http://vcd.vicomtech.org/ontology/automotive#Dustbin -->

    <owl:Class rdf:about="http://vcd.vicomtech.org/ontology/automotive#Dustbin">
        <rdfs:subClassOf rdf:resource="http://vcd.vicomtech.org/ontology/automotive#RoadObstacles"/>
        <rdfs:comment>A container for household refuse, especially one kept outside.</rdfs:comment>
        <rdfs:label>Dustbin</rdfs:label>
    </owl:Class>
    


    <!-- http://vcd.vicomtech.org/ontology/automotive#Dynamic -->

    <owl:Class rdf:about="http://vcd.vicomtech.org/ontology/automotive#Dynamic">
        <rdfs:subClassOf rdf:resource="http://vcd.vicomtech.org/ontology/automotive#Object"/>
        <rdfs:comment>Dynamic objects are characterized by the hability to perform an activity, change their state or move.</rdfs:comment>
        <rdfs:label>Dynamic</rdfs:label>
    </owl:Class>
    


    <!-- http://vcd.vicomtech.org/ontology/automotive#EgoVehicle -->

    <owl:Class rdf:about="http://vcd.vicomtech.org/ontology/automotive#EgoVehicle">
        <rdfs:subClassOf rdf:resource="http://vcd.vicomtech.org/ontology/automotive#DrivableVehicle"/>
        <rdfs:comment>A vehicle with sensors and other detection systems. The vehicle under test.</rdfs:comment>
    </owl:Class>
    


    <!-- http://vcd.vicomtech.org/ontology/automotive#ElectronicTraffic -->

    <owl:Class rdf:about="http://vcd.vicomtech.org/ontology/automotive#ElectronicTraffic">
        <rdfs:subClassOf rdf:resource="http://vcd.vicomtech.org/ontology/automotive#Void"/>
        <rdfs:comment>Traffic enhanced with electronic equipment.</rdfs:comment>
        <rdfs:label>Electronic traffic</rdfs:label>
    </owl:Class>
    


    <!-- http://vcd.vicomtech.org/ontology/automotive#Element -->

    <owl:Class rdf:about="http://vcd.vicomtech.org/ontology/automotive#Element">
        <rdfs:subClassOf rdf:resource="http://vcd.vicomtech.org/ontology/automotive#Nature"/>
        <rdfs:comment>Natural elements are those elements than have been produced by nature, without the intervention of man.</rdfs:comment>
        <rdfs:label>Element</rdfs:label>
    </owl:Class>
    


    <!-- http://vcd.vicomtech.org/ontology/automotive#EmergencyBicycle -->

    <owl:Class rdf:about="http://vcd.vicomtech.org/ontology/automotive#EmergencyBicycle">
        <rdfs:subClassOf rdf:resource="http://vcd.vicomtech.org/ontology/automotive#Cycle"/>
        <rdfs:comment>Bicycles aimed to respond to emergency calls.</rdfs:comment>
        <rdfs:label>Emergency Bicycle</rdfs:label>
    </owl:Class>
    


    <!-- http://vcd.vicomtech.org/ontology/automotive#EmergencyManoeuvre -->

    <owl:Class rdf:about="http://vcd.vicomtech.org/ontology/automotive#EmergencyManoeuvre">
        <rdfs:subClassOf rdf:resource="http://vcd.vicomtech.org/ontology/automotive#Event"/>
        <rdfs:comment>Emergency Manoeuvre (EM) is a manoeuvre performed by the system in case of an event in which the vehicle is at imminent collision risk and has the purpose of avoiding or mitigating a collision.</rdfs:comment>
        <rdfs:label>Emergency manoeuvre</rdfs:label>
    </owl:Class>
    


    <!-- http://vcd.vicomtech.org/ontology/automotive#EmergencyMotorcycle -->

    <owl:Class rdf:about="http://vcd.vicomtech.org/ontology/automotive#EmergencyMotorcycle">
        <rdfs:subClassOf rdf:resource="http://vcd.vicomtech.org/ontology/automotive#Cycle"/>
        <rdfs:comment>A motorcycle aimed to respond to emergency calls.</rdfs:comment>
        <rdfs:label>Emergency Motocycle</rdfs:label>
    </owl:Class>
    


    <!-- http://vcd.vicomtech.org/ontology/automotive#EmergencyVehicle -->

    <owl:Class rdf:about="http://vcd.vicomtech.org/ontology/automotive#EmergencyVehicle">
        <rdfs:subClassOf rdf:resource="http://vcd.vicomtech.org/ontology/automotive#DrivableVehicle"/>
        <rdfs:comment>Any vehicle that is designated and authorized to respond to an emergency in a life-threatening situation.</rdfs:comment>
        <rdfs:label>Emergency vehicle</rdfs:label>
    </owl:Class>
    


    <!-- http://vcd.vicomtech.org/ontology/automotive#Empty -->

    <owl:Class rdf:about="http://vcd.vicomtech.org/ontology/automotive#Empty">
        <rdfs:subClassOf rdf:resource="http://vcd.vicomtech.org/ontology/automotive#Trailer"/>
        <rdfs:comment>Any trailer structure/chassis which is not carrying any type of load but it is nevertheless towed by another motorized vehicle.</rdfs:comment>
        <rdfs:label>Empty</rdfs:label>
    </owl:Class>
    


    <!-- http://vcd.vicomtech.org/ontology/automotive#Environment -->

    <owl:Class rdf:about="http://vcd.vicomtech.org/ontology/automotive#Environment">
        <rdfs:subClassOf rdf:resource="http://vcd.vicomtech.org/ontology/automotive#Context"/>
        <rdfs:comment>The general conditions by which the scenario is surrounded.</rdfs:comment>
        <rdfs:label>Environment</rdfs:label>
    </owl:Class>
    


    <!-- http://vcd.vicomtech.org/ontology/automotive#Event -->

    <owl:Class rdf:about="http://vcd.vicomtech.org/ontology/automotive#Event">
        <rdfs:subClassOf rdf:resource="http://www.w3.org/2002/07/owl#Thing"/>
        <rdfs:comment>A thing that happens or takes place in a concrete instant of time and is relevant for the description of the scenario. It usually causes other events  or actions.</rdfs:comment>
        <rdfs:label>Event</rdfs:label>
    </owl:Class>
    


    <!-- http://vcd.vicomtech.org/ontology/automotive#Exceptional -->

    <owl:Class rdf:about="http://vcd.vicomtech.org/ontology/automotive#Exceptional">
        <rdfs:subClassOf rdf:resource="http://vcd.vicomtech.org/ontology/automotive#LargeVehicle"/>
        <rdfs:comment>An Exceptional convoy is transportation of a piece of cargo that cannot be loaded on a normal truck since dimensions do not fit the road profile. In such cases the cargo requires a modified custom vehicle to be transported. Exceptional convoys are usually made of a truck tractor cab and a trailer with the exceptional load. This configuration, though, can vary.</rdfs:comment>
        <rdfs:label>Exceptional transport</rdfs:label>
    </owl:Class>
    


    <!-- http://vcd.vicomtech.org/ontology/automotive#Exhaust -->

    <owl:Class rdf:about="http://vcd.vicomtech.org/ontology/automotive#Exhaust">
        <rdfs:subClassOf rdf:resource="http://vcd.vicomtech.org/ontology/automotive#Air"/>
        <rdfs:comment>Air that is deliberately removed from the building envelope and rejected to the environment is referred to as exhaust air. Building ventilation systems are equipped with exhaust fans that work to draw air out of the buildings from strategic locations where low quality, moist or polluted air is likely to accumulate.</rdfs:comment>
        <rdfs:label>Exhaust</rdfs:label>
    </owl:Class>
    


    <!-- http://vcd.vicomtech.org/ontology/automotive#Failure -->

    <owl:Class rdf:about="http://vcd.vicomtech.org/ontology/automotive#Failure">
        <rdfs:subClassOf rdf:resource="http://vcd.vicomtech.org/ontology/automotive#Event"/>
        <rdfs:comment>The action or state of not functioning.</rdfs:comment>
        <rdfs:label>Failure</rdfs:label>
    </owl:Class>
    


    <!-- http://vcd.vicomtech.org/ontology/automotive#Fall -->

    <owl:Class rdf:about="http://vcd.vicomtech.org/ontology/automotive#Fall">
        <rdfs:subClassOf rdf:resource="http://vcd.vicomtech.org/ontology/automotive#Event"/>
        <rdfs:label>Fall</rdfs:label>
    </owl:Class>
    


    <!-- http://vcd.vicomtech.org/ontology/automotive#FallBehind -->

    <owl:Class rdf:about="http://vcd.vicomtech.org/ontology/automotive#FallBehind">
        <rdfs:subClassOf rdf:resource="http://vcd.vicomtech.org/ontology/automotive#Event"/>
        <rdfs:comment>Occurs when the ego-vehicle is driving slower than the leading vehicle or is decelerating.</rdfs:comment>
        <rdfs:label>Fall behind</rdfs:label>
    </owl:Class>
    


    <!-- http://vcd.vicomtech.org/ontology/automotive#FallingBehind -->

    <owl:Class rdf:about="http://vcd.vicomtech.org/ontology/automotive#FallingBehind">
        <rdfs:subClassOf rdf:resource="http://vcd.vicomtech.org/ontology/automotive#MovingManeuver"/>
        <rdfs:comment>The action of driving slower than its lead vehicle and is also decelerating.</rdfs:comment>
        <rdfs:label>Falling behind</rdfs:label>
    </owl:Class>
    


    <!-- http://vcd.vicomtech.org/ontology/automotive#FallingDown -->

    <owl:Class rdf:about="http://vcd.vicomtech.org/ontology/automotive#FallingDown">
        <rdfs:subClassOf rdf:resource="http://vcd.vicomtech.org/ontology/automotive#MovingManeuver"/>
        <rdfs:comment>Occurs when a person or object loses balance and collapses to the ground.</rdfs:comment>
        <rdfs:label>Falling down</rdfs:label>
    </owl:Class>
    


    <!-- http://vcd.vicomtech.org/ontology/automotive#Fence -->

    <owl:Class rdf:about="http://vcd.vicomtech.org/ontology/automotive#Fence">
        <rdfs:subClassOf rdf:resource="http://vcd.vicomtech.org/ontology/automotive#Barrier"/>
        <rdfs:comment>A barrier, railing, or other upright structure, typically of wood or wire, enclosing an area of ground to prevent or control access or escape.</rdfs:comment>
        <rdfs:label>Fence</rdfs:label>
    </owl:Class>
    


    <!-- http://vcd.vicomtech.org/ontology/automotive#FireHydrant -->

    <owl:Class rdf:about="http://vcd.vicomtech.org/ontology/automotive#FireHydrant">
        <rdfs:subClassOf rdf:resource="http://vcd.vicomtech.org/ontology/automotive#RoadsideObject"/>
        <rdfs:comment>Water outlet typically used by fire-fighters.</rdfs:comment>
        <rdfs:label>Fire hydrant</rdfs:label>
    </owl:Class>
    


    <!-- http://vcd.vicomtech.org/ontology/automotive#FireTruck -->

    <owl:Class rdf:about="http://vcd.vicomtech.org/ontology/automotive#FireTruck">
        <rdfs:subClassOf rdf:resource="http://vcd.vicomtech.org/ontology/automotive#LargeEmergencyVehicle"/>
        <rdfs:comment>Trucks or Heavy-duty vehicles adopted by Firefighters.</rdfs:comment>
        <rdfs:label>Fire truck</rdfs:label>
    </owl:Class>
    


    <!-- http://vcd.vicomtech.org/ontology/automotive#Firefighters -->

    <owl:Class rdf:about="http://vcd.vicomtech.org/ontology/automotive#Firefighters">
        <rdfs:subClassOf rdf:resource="http://vcd.vicomtech.org/ontology/automotive#EmergencyVehicle"/>
        <rdfs:comment>Passenger cars or Vans adopted by Firefighters.</rdfs:comment>
        <rdfs:label>Firefighters</rdfs:label>
    </owl:Class>
    


    <!-- http://vcd.vicomtech.org/ontology/automotive#FirefightersBicycle -->

    <owl:Class rdf:about="http://vcd.vicomtech.org/ontology/automotive#FirefightersBicycle">
        <rdfs:subClassOf rdf:resource="http://vcd.vicomtech.org/ontology/automotive#EmergencyBicycle"/>
        <rdfs:label>Firefighters Bicycle</rdfs:label>
    </owl:Class>
    


    <!-- http://vcd.vicomtech.org/ontology/automotive#FirefightersMotorcycle -->

    <owl:Class rdf:about="http://vcd.vicomtech.org/ontology/automotive#FirefightersMotorcycle">
        <rdfs:subClassOf rdf:resource="http://vcd.vicomtech.org/ontology/automotive#EmergencyMotorcycle"/>
        <rdfs:label>Firefighters Motorcycle</rdfs:label>
    </owl:Class>
    


    <!-- http://vcd.vicomtech.org/ontology/automotive#Fireman -->

    <owl:Class rdf:about="http://vcd.vicomtech.org/ontology/automotive#Fireman">
        <rdfs:subClassOf rdf:resource="http://vcd.vicomtech.org/ontology/automotive#FirstResponder"/>
        <rdfs:comment>Fireman belongs to organizations whose primary goal is to extinguish fire, or intervene as rescuers in any other catastrophic situation such as earthquakes, floods etc. Usually wear a particular uniform that explicits this role.</rdfs:comment>
        <rdfs:label>Fireman</rdfs:label>
    </owl:Class>
    


    <!-- http://vcd.vicomtech.org/ontology/automotive#FirstResponder -->

    <owl:Class rdf:about="http://vcd.vicomtech.org/ontology/automotive#FirstResponder">
        <rdfs:subClassOf rdf:resource="http://vcd.vicomtech.org/ontology/automotive#Adult"/>
        <rdfs:comment>A person who&apos;s task is to arrive first and provide assistance in the scene of an emergency. Usually wear particular uniforms that explicits this role.</rdfs:comment>
        <rdfs:label>First responder</rdfs:label>
    </owl:Class>
    


    <!-- http://vcd.vicomtech.org/ontology/automotive#Flat -->

    <owl:Class rdf:about="http://vcd.vicomtech.org/ontology/automotive#Flat">
        <rdfs:subClassOf rdf:resource="http://vcd.vicomtech.org/ontology/automotive#Construction"/>
        <rdfs:comment>Objects or areas without raised areas or indentations.</rdfs:comment>
        <rdfs:label>Flat</rdfs:label>
    </owl:Class>
    


    <!-- http://vcd.vicomtech.org/ontology/automotive#Floodlights -->

    <owl:Class rdf:about="http://vcd.vicomtech.org/ontology/automotive#Floodlights">
        <rdfs:subClassOf rdf:resource="http://vcd.vicomtech.org/ontology/automotive#ArtificialLighting"/>
        <rdfs:comment>Floodlights can be used to illuminate work zones or outdoor playing fields during nighttime hours.</rdfs:comment>
        <rdfs:label>Floodlights</rdfs:label>
    </owl:Class>
    


    <!-- http://vcd.vicomtech.org/ontology/automotive#Fog -->

    <owl:Class rdf:about="http://vcd.vicomtech.org/ontology/automotive#Fog">
        <rdfs:subClassOf rdf:resource="http://vcd.vicomtech.org/ontology/automotive#Element"/>
        <rdfs:subClassOf rdf:resource="http://vcd.vicomtech.org/ontology/automotive#Weather"/>
        <rdfs:comment>A thick cloud of tiny water droplets suspended in the atmosphere at or near the earth&apos;s surface which obscures or restricts visibility (to a greater extent than mist; strictly, reducing visibility to below 1 km).</rdfs:comment>
        <rdfs:label>Fog</rdfs:label>
    </owl:Class>
    


    <!-- http://vcd.vicomtech.org/ontology/automotive#Foggy -->

    <owl:Class rdf:about="http://vcd.vicomtech.org/ontology/automotive#Foggy">
        <rdfs:subClassOf rdf:resource="http://vcd.vicomtech.org/ontology/automotive#DiffusedSunlight"/>
        <rdfs:comment>Full of or characterized by fog.</rdfs:comment>
        <rdfs:label>Foggy</rdfs:label>
    </owl:Class>
    


    <!-- http://vcd.vicomtech.org/ontology/automotive#Following -->

    <owl:Class rdf:about="http://vcd.vicomtech.org/ontology/automotive#Following">
        <rdfs:subClassOf rdf:resource="http://vcd.vicomtech.org/ontology/automotive#MovingManeuver"/>
        <rdfs:comment>When the vehicle is driving with the same velocity as the vehicle in front.</rdfs:comment>
        <rdfs:label>Following</rdfs:label>
    </owl:Class>
    


    <!-- http://vcd.vicomtech.org/ontology/automotive#Footwalk -->

    <owl:Class rdf:about="http://vcd.vicomtech.org/ontology/automotive#Footwalk">
        <rdfs:subClassOf rdf:resource="http://vcd.vicomtech.org/ontology/automotive#Flat"/>
        <rdfs:comment>A surface paved or constructed for walking along often with a handrail (as on a bridge or on a parapet).</rdfs:comment>
        <rdfs:label>Footwalk</rdfs:label>
    </owl:Class>
    


    <!-- http://vcd.vicomtech.org/ontology/automotive#FourWayInterchange -->

    <owl:Class rdf:about="http://vcd.vicomtech.org/ontology/automotive#FourWayInterchange">
        <rdfs:subClassOf rdf:resource="http://vcd.vicomtech.org/ontology/automotive#SystemInterchange"/>
        <rdfs:label>Four-way interchange</rdfs:label>
    </owl:Class>
    


    <!-- http://vcd.vicomtech.org/ontology/automotive#FourWayIntersection -->

    <owl:Class rdf:about="http://vcd.vicomtech.org/ontology/automotive#FourWayIntersection">
        <rdfs:subClassOf rdf:resource="http://vcd.vicomtech.org/ontology/automotive#RoadSegments"/>
        <rdfs:comment>A four-way intersection, or crossroads, usually involves a crossing over of two streets or roads. In areas where there are blocks and in some other cases, the crossing streets or roads are perpendicular to each other. However, two roads may cross at a different angle. In a few cases, the junction of two road segments may be offset from each when reaching an intersection, even though both ends may be considered the same street.</rdfs:comment>
        <rdfs:label>Four-way intersection</rdfs:label>
    </owl:Class>
    


    <!-- http://vcd.vicomtech.org/ontology/automotive#Garage -->

    <owl:Class rdf:about="http://vcd.vicomtech.org/ontology/automotive#Garage">
        <rdfs:subClassOf rdf:resource="http://vcd.vicomtech.org/ontology/automotive#Barrier"/>
        <rdfs:comment>A building for housing a motor vehicle or vehicles.</rdfs:comment>
        <rdfs:label>Garage</rdfs:label>
    </owl:Class>
    


    <!-- http://vcd.vicomtech.org/ontology/automotive#GlidingOnWheels -->

    <owl:Class rdf:about="http://vcd.vicomtech.org/ontology/automotive#GlidingOnWheels">
        <rdfs:subClassOf rdf:resource="http://vcd.vicomtech.org/ontology/automotive#MovingManeuver"/>
        <rdfs:comment>Gliding is an energy-efficient driving mode achieved by turning off the internal combustion engine while the vehicle is still moving in order to save fuel.</rdfs:comment>
        <rdfs:label>Gliding on wheels</rdfs:label>
    </owl:Class>
    


    <!-- http://vcd.vicomtech.org/ontology/automotive#Grass -->

    <owl:Class rdf:about="http://vcd.vicomtech.org/ontology/automotive#Grass">
        <rdfs:subClassOf rdf:resource="http://vcd.vicomtech.org/ontology/automotive#Vegetation"/>
        <rdfs:comment>Vegetation consisting of typically short plants with long, narrow leaves, growing wild or cultivated on lawns and pasture, and as a fodder crop.</rdfs:comment>
        <rdfs:label>Grass</rdfs:label>
    </owl:Class>
    


    <!-- http://vcd.vicomtech.org/ontology/automotive#GroundAnimal -->

    <owl:Class rdf:about="http://vcd.vicomtech.org/ontology/automotive#GroundAnimal">
        <rdfs:subClassOf rdf:resource="http://vcd.vicomtech.org/ontology/automotive#Wildlife"/>
        <rdfs:comment>Animals which move on the ground.</rdfs:comment>
        <rdfs:label>Ground animal</rdfs:label>
    </owl:Class>
    


    <!-- http://vcd.vicomtech.org/ontology/automotive#GuardRail -->

    <owl:Class rdf:about="http://vcd.vicomtech.org/ontology/automotive#GuardRail">
        <rdfs:subClassOf rdf:resource="http://vcd.vicomtech.org/ontology/automotive#Barrier"/>
        <rdfs:comment>A strong fence at the side of a road or in the middle of an expressway, intended to reduce the risk of serious accidents; a crash barrier.</rdfs:comment>
        <rdfs:label>Guard rail</rdfs:label>
    </owl:Class>
    


    <!-- http://vcd.vicomtech.org/ontology/automotive#HOV -->

    <owl:Class rdf:about="http://vcd.vicomtech.org/ontology/automotive#HOV">
        <rdfs:subClassOf rdf:resource="http://vcd.vicomtech.org/ontology/automotive#Lane"/>
        <rdfs:comment>A high-occupancy vehicle lane (also known as an HOV lane, carpool lane, diamond lane, 2+ lane, and transit lane or T2 or T3 lanes) is a restricted traffic lane reserved for the exclusive use of vehicles with a driver and one or more passengers, including carpools, vanpools, and transit buses. The normal minimum occupancy level is 2 or 3 occupants.</rdfs:comment>
        <rdfs:label>HOV lane</rdfs:label>
    </owl:Class>
    


    <!-- http://vcd.vicomtech.org/ontology/automotive#Hail -->

    <owl:Class rdf:about="http://vcd.vicomtech.org/ontology/automotive#Hail">
        <rdfs:subClassOf rdf:resource="http://vcd.vicomtech.org/ontology/automotive#Weather"/>
        <rdfs:comment>Pellets of frozen rain which fall in showers from cumulonimbus clouds.</rdfs:comment>
        <rdfs:label>Hail</rdfs:label>
    </owl:Class>
    


    <!-- http://vcd.vicomtech.org/ontology/automotive#HalfCloverInterchange -->

    <owl:Class rdf:about="http://vcd.vicomtech.org/ontology/automotive#HalfCloverInterchange">
        <rdfs:subClassOf rdf:resource="http://vcd.vicomtech.org/ontology/automotive#HybridInterchange"/>
        <rdfs:comment>A half-clover interchange is essentially half a cloverleaf interchange, constructed to connect in just three directions instead of four. These are rarely used due to the traffic weaving that they cause and the large amount of land that they consume, but they can be built in areas where the connecting ramp along the loop of a trumpet interchange is not feasible due to building developments or physical limitations.</rdfs:comment>
        <rdfs:label>Half-clover interchange</rdfs:label>
    </owl:Class>
    


    <!-- http://vcd.vicomtech.org/ontology/automotive#HalfTrumpetInterchange -->

    <owl:Class rdf:about="http://vcd.vicomtech.org/ontology/automotive#HalfTrumpetInterchange">
        <rdfs:subClassOf rdf:resource="http://vcd.vicomtech.org/ontology/automotive#TwoWayInterchange"/>
        <rdfs:comment>A half-trumpet interchange is essentially a trumpet interchange with either its loop ramp or the outer connecting ramp (but not both), and only one of its directional ramps, instead of two, designed to meet the continuous highway in one direction, usually on a 90-degree or semi-perpendicular angle.</rdfs:comment>
        <rdfs:label>Half-trumpet interchange</rdfs:label>
    </owl:Class>
    


    <!-- http://vcd.vicomtech.org/ontology/automotive#Halt -->

    <owl:Class rdf:about="http://vcd.vicomtech.org/ontology/automotive#Halt">
        <rdfs:subClassOf rdf:resource="http://vcd.vicomtech.org/ontology/automotive#Event"/>
        <rdfs:comment>The action of braking till coming to a halt.</rdfs:comment>
        <rdfs:label>Halt</rdfs:label>
    </owl:Class>
    


    <!-- http://vcd.vicomtech.org/ontology/automotive#Horse -->

    <owl:Class rdf:about="http://vcd.vicomtech.org/ontology/automotive#Horse">
        <rdfs:subClassOf rdf:resource="http://vcd.vicomtech.org/ontology/automotive#Pet"/>
        <rdfs:comment>Horses are considered pets</rdfs:comment>
        <rdfs:label>Horse</rdfs:label>
    </owl:Class>
    


    <!-- http://vcd.vicomtech.org/ontology/automotive#HorseCarriage -->

    <owl:Class rdf:about="http://vcd.vicomtech.org/ontology/automotive#HorseCarriage">
        <rdfs:subClassOf rdf:resource="http://vcd.vicomtech.org/ontology/automotive#AnimalPulled"/>
        <rdfs:comment>Any vehicle carried by a horse or a group of horses.</rdfs:comment>
        <rdfs:label>Horse-carriage</rdfs:label>
    </owl:Class>
    


    <!-- http://vcd.vicomtech.org/ontology/automotive#Human -->

    <owl:Class rdf:about="http://vcd.vicomtech.org/ontology/automotive#Human">
        <rdfs:subClassOf rdf:resource="http://vcd.vicomtech.org/ontology/automotive#Dynamic"/>
        <rdfs:comment>A bipedal primate mammal (Homo sapiens). A person.</rdfs:comment>
        <rdfs:label>Human</rdfs:label>
    </owl:Class>
    


    <!-- http://vcd.vicomtech.org/ontology/automotive#HybridFourWayInterchange -->

    <owl:Class rdf:about="http://vcd.vicomtech.org/ontology/automotive#HybridFourWayInterchange">
        <rdfs:subClassOf rdf:resource="http://vcd.vicomtech.org/ontology/automotive#FourWayInterchange"/>
        <rdfs:comment>Hybrid interchanges use a mixture of interchange types and are not uncommon. Their construction can consist of multiple interchange designs such as loop ramps, flyovers and roundabouts.</rdfs:comment>
        <rdfs:label>Hybrid four-way interchange</rdfs:label>
    </owl:Class>
    


    <!-- http://vcd.vicomtech.org/ontology/automotive#HybridInterchange -->

    <owl:Class rdf:about="http://vcd.vicomtech.org/ontology/automotive#HybridInterchange">
        <rdfs:subClassOf rdf:resource="http://vcd.vicomtech.org/ontology/automotive#ThreeWayInterchange"/>
        <rdfs:comment>Hybrid interchanges use a mixture of interchange types and are not uncommon. Their construction can consist of multiple interchange designs such as loop ramps and flyovers.</rdfs:comment>
        <rdfs:label>Hybrid interchange</rdfs:label>
    </owl:Class>
    


    <!-- http://vcd.vicomtech.org/ontology/automotive#HybridServiceInterchange -->

    <owl:Class rdf:about="http://vcd.vicomtech.org/ontology/automotive#HybridServiceInterchange">
        <rdfs:subClassOf rdf:resource="http://vcd.vicomtech.org/ontology/automotive#ServiceInterchange"/>
        <rdfs:comment>Highway/non-highway hybrid interchanges consist of diamond and partial cloverleaf elements. Their construction can consist of multiple interchange designs such as loop ramps, flyovers, and roundabouts.</rdfs:comment>
        <rdfs:label>Hybrid service interchange</rdfs:label>
    </owl:Class>
    


    <!-- http://vcd.vicomtech.org/ontology/automotive#InVehicleSystems -->

    <owl:Class rdf:about="http://vcd.vicomtech.org/ontology/automotive#InVehicleSystems">
        <rdfs:subClassOf rdf:resource="http://vcd.vicomtech.org/ontology/automotive#Static"/>
        <rdfs:comment>In-vehicle information systems can improve safety, improve driver’s situational awareness and reduce anxiety, but they may also increase mental workload and distraction.</rdfs:comment>
        <rdfs:label>In-vehicle systems</rdfs:label>
    </owl:Class>
    


    <!-- http://vcd.vicomtech.org/ontology/automotive#Interchange -->

    <owl:Class rdf:about="http://vcd.vicomtech.org/ontology/automotive#Interchange">
        <rdfs:subClassOf rdf:resource="http://vcd.vicomtech.org/ontology/automotive#Junction"/>
        <rdfs:comment>At interchanges, roads pass above or below each other, using grade separation and slip roads. The terms motorway junction and highway junction typically refer to this layout.</rdfs:comment>
        <rdfs:label>Interchange</rdfs:label>
    </owl:Class>
    


    <!-- http://vcd.vicomtech.org/ontology/automotive#Intersection -->

    <owl:Class rdf:about="http://vcd.vicomtech.org/ontology/automotive#Intersection">
        <rdfs:subClassOf rdf:resource="http://vcd.vicomtech.org/ontology/automotive#Junction"/>
        <rdfs:comment>An intersection is an at-grade junction where two or more roads or streets meet or cross.</rdfs:comment>
        <rdfs:label>Intersection</rdfs:label>
    </owl:Class>
    


    <!-- http://vcd.vicomtech.org/ontology/automotive#IrrelevantSign -->

    <owl:Class rdf:about="http://vcd.vicomtech.org/ontology/automotive#IrrelevantSign">
        <rdfs:subClassOf rdf:resource="http://vcd.vicomtech.org/ontology/automotive#Signs"/>
        <rdfs:comment>A sign that is not relevant in a traffic scenario, that is, it is not designated to inform the traffic participants.</rdfs:comment>
        <rdfs:label>Irrelevant sign</rdfs:label>
    </owl:Class>
    


    <!-- http://vcd.vicomtech.org/ontology/automotive#Junction -->

    <owl:Class rdf:about="http://vcd.vicomtech.org/ontology/automotive#Junction">
        <rdfs:subClassOf rdf:resource="http://vcd.vicomtech.org/ontology/automotive#Construction"/>
        <rdfs:comment>A point where two or more roads meet.</rdfs:comment>
        <rdfs:label>Junction</rdfs:label>
    </owl:Class>
    


    <!-- http://vcd.vicomtech.org/ontology/automotive#Lake -->

    <owl:Class rdf:about="http://vcd.vicomtech.org/ontology/automotive#Lake">
        <rdfs:subClassOf rdf:resource="http://vcd.vicomtech.org/ontology/automotive#Water"/>
        <rdfs:comment>A large area of water surrounded by land.</rdfs:comment>
        <rdfs:label>Lake</rdfs:label>
    </owl:Class>
    


    <!-- http://vcd.vicomtech.org/ontology/automotive#Lane -->

    <owl:Class rdf:about="http://vcd.vicomtech.org/ontology/automotive#Lane">
        <rdfs:subClassOf rdf:resource="http://vcd.vicomtech.org/ontology/automotive#Flat"/>
        <rdfs:comment>A division of a road marked off with painted lines and intended to separate single lines of traffic according to speed or direction.</rdfs:comment>
        <rdfs:label>Lane</rdfs:label>
    </owl:Class>
    


    <!-- http://vcd.vicomtech.org/ontology/automotive#LaneChange -->

    <owl:Class rdf:about="http://vcd.vicomtech.org/ontology/automotive#LaneChange">
        <rdfs:subClassOf rdf:resource="http://vcd.vicomtech.org/ontology/automotive#Event"/>
        <rdfs:comment>The vehicle moves from one lane to another where both lanes have the same direction of travel. The lane change ends when  he vehicle position in the adjacent lane normalizes.</rdfs:comment>
        <rdfs:label>Lane change</rdfs:label>
    </owl:Class>
    


    <!-- http://vcd.vicomtech.org/ontology/automotive#LaneChanging -->

    <owl:Class rdf:about="http://vcd.vicomtech.org/ontology/automotive#LaneChanging">
        <rdfs:subClassOf rdf:resource="http://vcd.vicomtech.org/ontology/automotive#MovingManeuver"/>
        <rdfs:comment>Is a driving maneuver that moves a vehicle from one lane to another where both lanes have the same direction of travel.</rdfs:comment>
        <rdfs:label>Lane changing</rdfs:label>
    </owl:Class>
    


    <!-- http://vcd.vicomtech.org/ontology/automotive#LaneChangingLeft -->

    <owl:Class rdf:about="http://vcd.vicomtech.org/ontology/automotive#LaneChangingLeft">
        <rdfs:subClassOf rdf:resource="http://vcd.vicomtech.org/ontology/automotive#LaneChanging"/>
        <rdfs:comment>Is a driving maneuver that moves a vehicle from one lane to the one on the left where both lanes have the same direction of travel.</rdfs:comment>
        <rdfs:label>Lane changing left</rdfs:label>
    </owl:Class>
    


    <!-- http://vcd.vicomtech.org/ontology/automotive#LaneChangingRight -->

    <owl:Class rdf:about="http://vcd.vicomtech.org/ontology/automotive#LaneChangingRight">
        <rdfs:subClassOf rdf:resource="http://vcd.vicomtech.org/ontology/automotive#LaneChanging"/>
        <rdfs:comment>Is a driving maneuver that moves a vehicle from one lane to the one on the right where both lanes have the same direction of travel.</rdfs:comment>
        <rdfs:label>Lane changing right</rdfs:label>
    </owl:Class>
    


    <!-- http://vcd.vicomtech.org/ontology/automotive#LaneDivider -->

    <owl:Class rdf:about="http://vcd.vicomtech.org/ontology/automotive#LaneDivider">
        <rdfs:subClassOf rdf:resource="http://vcd.vicomtech.org/ontology/automotive#RoadsideObject"/>
        <rdfs:comment>A barrier placed between the lanes of a highway to divide the traffic moving in opposite directions.</rdfs:comment>
        <rdfs:label>Lane divider</rdfs:label>
    </owl:Class>
    


    <!-- http://vcd.vicomtech.org/ontology/automotive#LaneMarking -->

    <owl:Class rdf:about="http://vcd.vicomtech.org/ontology/automotive#LaneMarking">
        <rdfs:subClassOf rdf:resource="http://vcd.vicomtech.org/ontology/automotive#Marking"/>
        <rdfs:comment>Markings delimiting the lanes along the road.</rdfs:comment>
        <rdfs:label>Lane marking</rdfs:label>
    </owl:Class>
    


    <!-- http://vcd.vicomtech.org/ontology/automotive#LargeEmergencyVehicle -->

    <owl:Class rdf:about="http://vcd.vicomtech.org/ontology/automotive#LargeEmergencyVehicle">
        <rdfs:subClassOf rdf:resource="http://vcd.vicomtech.org/ontology/automotive#LargeVehicle"/>
        <rdfs:comment>An emergency vehicle is any vehicle that is designated and authorized to respond to an emergency in a life-threatening situation. These vehicles are usually operated by designated agencies, often part of the government, but also run by charities, non-governmental organizations and some commercial companies. Often emergency vehicles are permitted by law to break conventional road rules in order to reach their destinations in the fastest possible time, such as driving through an intersection when the traffic light is red, or exceeding the speed limit. Large emergency vehicles are Emergency vehicles of the kind described in thee Large Vehicles subclasses.</rdfs:comment>
        <rdfs:label>Large Emergency Vehicle</rdfs:label>
    </owl:Class>
    


    <!-- http://vcd.vicomtech.org/ontology/automotive#LargeVehicle -->

    <owl:Class rdf:about="http://vcd.vicomtech.org/ontology/automotive#LargeVehicle">
        <rdfs:subClassOf rdf:resource="http://vcd.vicomtech.org/ontology/automotive#DrivableVehicle"/>
        <rdfs:comment>A Large vehicle is any drivable vehicle whose weight and dimensions significantly exceed those of a regular passenger car.</rdfs:comment>
        <rdfs:label>Large Vehicle</rdfs:label>
    </owl:Class>
    


    <!-- http://vcd.vicomtech.org/ontology/automotive#Lighting -->

    <owl:Class rdf:about="http://vcd.vicomtech.org/ontology/automotive#Lighting">
        <rdfs:subClassOf rdf:resource="http://vcd.vicomtech.org/ontology/automotive#Context"/>
        <rdfs:comment>Lighting or illumination is the deliberate use of light to achieve practical or aesthetic effects. Lighting includes the use of both artificial light sources like lamps and light fixtures, as well as natural illumination by capturing daylight.</rdfs:comment>
        <rdfs:label>Lighting</rdfs:label>
    </owl:Class>
    


    <!-- http://vcd.vicomtech.org/ontology/automotive#Limo -->

    <owl:Class rdf:about="http://vcd.vicomtech.org/ontology/automotive#Limo">
        <rdfs:subClassOf rdf:resource="http://vcd.vicomtech.org/ontology/automotive#LargeVehicle"/>
        <rdfs:comment>A large, luxurious car longer than regular cars, designed to transport passengers.</rdfs:comment>
        <rdfs:label>Limo</rdfs:label>
    </owl:Class>
    


    <!-- http://vcd.vicomtech.org/ontology/automotive#LossOfControl -->

    <owl:Class rdf:about="http://vcd.vicomtech.org/ontology/automotive#LossOfControl">
        <rdfs:subClassOf rdf:resource="http://vcd.vicomtech.org/ontology/automotive#Event"/>
        <rdfs:comment>The action of losing the control of the vehicle which usually leads to an incident.</rdfs:comment>
        <rdfs:label>Loss of control</rdfs:label>
    </owl:Class>
    


    <!-- http://vcd.vicomtech.org/ontology/automotive#LossingControl -->

    <owl:Class rdf:about="http://vcd.vicomtech.org/ontology/automotive#LossingControl">
        <rdfs:subClassOf rdf:resource="http://vcd.vicomtech.org/ontology/automotive#MovingManeuver"/>
        <rdfs:comment>The action of losing the control of the vehicle which usually leads to an incident.</rdfs:comment>
        <rdfs:label>Lossing control</rdfs:label>
    </owl:Class>
    


    <!-- http://vcd.vicomtech.org/ontology/automotive#Mailbox -->

    <owl:Class rdf:about="http://vcd.vicomtech.org/ontology/automotive#Mailbox">
        <rdfs:subClassOf rdf:resource="http://vcd.vicomtech.org/ontology/automotive#RoadsideObject"/>
        <rdfs:comment>A box to put mail into.</rdfs:comment>
        <rdfs:label>Mailbox</rdfs:label>
    </owl:Class>
    


    <!-- http://vcd.vicomtech.org/ontology/automotive#Manhole -->

    <owl:Class rdf:about="http://vcd.vicomtech.org/ontology/automotive#Manhole">
        <rdfs:subClassOf rdf:resource="http://vcd.vicomtech.org/ontology/automotive#RoadsideObject"/>
        <rdfs:comment>Opening in road to access canal system. Has to be big enough to fit a person and includes squared ones.</rdfs:comment>
        <rdfs:label>Manhole</rdfs:label>
    </owl:Class>
    


    <!-- http://vcd.vicomtech.org/ontology/automotive#Marking -->

    <owl:Class rdf:about="http://vcd.vicomtech.org/ontology/automotive#Marking">
        <rdfs:subClassOf rdf:resource="http://vcd.vicomtech.org/ontology/automotive#Flat"/>
        <rdfs:comment>A mark or patten of marks delimiting a concrete area of the road.</rdfs:comment>
        <rdfs:label>Marking</rdfs:label>
    </owl:Class>
    


    <!-- http://vcd.vicomtech.org/ontology/automotive#Meteorology -->

    <owl:Class rdf:about="http://vcd.vicomtech.org/ontology/automotive#Meteorology">
        <rdfs:subClassOf rdf:resource="http://vcd.vicomtech.org/ontology/automotive#Context"/>
        <rdfs:label>Meteorology</rdfs:label>
        <rdfs:label>The climate and weather of a region.</rdfs:label>
    </owl:Class>
    


    <!-- http://vcd.vicomtech.org/ontology/automotive#MilitaryTruck -->

    <owl:Class rdf:about="http://vcd.vicomtech.org/ontology/automotive#MilitaryTruck">
        <rdfs:subClassOf rdf:resource="http://vcd.vicomtech.org/ontology/automotive#LargeEmergencyVehicle"/>
        <rdfs:comment>Trucks or Heavy-duty vehicles adopted by Military.</rdfs:comment>
        <rdfs:label>Military truck</rdfs:label>
    </owl:Class>
    


    <!-- http://vcd.vicomtech.org/ontology/automotive#MiniVan -->

    <owl:Class rdf:about="http://vcd.vicomtech.org/ontology/automotive#MiniVan">
        <rdfs:subClassOf rdf:resource="http://vcd.vicomtech.org/ontology/automotive#Car"/>
        <rdfs:comment>Minivans are regular passenger cars designed to transport more than 5 passengers, usually 7 or even 9. Differently from Vans, MiniVans usually do not have &quot;wardrobe-like&quot; opening doors in the trunk, and have windows looking like any other passenger car along the whole body.</rdfs:comment>
        <rdfs:label>Mini-van</rdfs:label>
    </owl:Class>
    


    <!-- http://vcd.vicomtech.org/ontology/automotive#MinimumRiskManoeuvre -->

    <owl:Class rdf:about="http://vcd.vicomtech.org/ontology/automotive#MinimumRiskManoeuvre">
        <rdfs:subClassOf rdf:resource="http://vcd.vicomtech.org/ontology/automotive#Event"/>
        <rdfs:comment>Minimum Risk Manoeuvre (MRM) means a procedure aimed at minimising risks in traffic, which is automatically performed by the system after a transition demand without driver response or in the case of a severe ALKS or vehicle failure.</rdfs:comment>
        <rdfs:label>Minimum risk manoeuvre</rdfs:label>
    </owl:Class>
    


    <!-- http://vcd.vicomtech.org/ontology/automotive#Misc -->

    <owl:Class rdf:about="http://vcd.vicomtech.org/ontology/automotive#Misc">
        <rdfs:subClassOf rdf:resource="http://vcd.vicomtech.org/ontology/automotive#RoadVehicle"/>
        <rdfs:comment>Miscellaneous; Objects of various types or from different sources.</rdfs:comment>
        <rdfs:label>Misc</rdfs:label>
    </owl:Class>
    


    <!-- http://vcd.vicomtech.org/ontology/automotive#Motorcycle -->

    <owl:Class rdf:about="http://vcd.vicomtech.org/ontology/automotive#Motorcycle">
        <rdfs:subClassOf rdf:resource="http://vcd.vicomtech.org/ontology/automotive#Cycle"/>
        <rdfs:comment>A two-wheeled vehicle that is powered by a motor and has no pedals.</rdfs:comment>
        <rdfs:label>Motorcycle</rdfs:label>
    </owl:Class>
    


    <!-- http://vcd.vicomtech.org/ontology/automotive#Motorcyclist -->

    <owl:Class rdf:about="http://vcd.vicomtech.org/ontology/automotive#Motorcyclist">
        <rdfs:subClassOf rdf:resource="http://vcd.vicomtech.org/ontology/automotive#Rider"/>
        <rdfs:comment>A person who rides a motorcycle. Includes passengers.</rdfs:comment>
        <rdfs:label>Motorcyclist</rdfs:label>
    </owl:Class>
    


    <!-- http://vcd.vicomtech.org/ontology/automotive#Mountain -->

    <owl:Class rdf:about="http://vcd.vicomtech.org/ontology/automotive#Mountain">
        <rdfs:subClassOf rdf:resource="http://vcd.vicomtech.org/ontology/automotive#Nature"/>
        <rdfs:comment>Distant elevations of the ground.</rdfs:comment>
        <rdfs:label>Mountain</rdfs:label>
    </owl:Class>
    


    <!-- http://vcd.vicomtech.org/ontology/automotive#MovableObject -->

    <owl:Class rdf:about="http://vcd.vicomtech.org/ontology/automotive#MovableObject">
        <rdfs:subClassOf rdf:resource="http://vcd.vicomtech.org/ontology/automotive#Static"/>
        <rdfs:comment>An object capable of being moved.</rdfs:comment>
        <rdfs:label>Movable object</rdfs:label>
    </owl:Class>
    


    <!-- http://vcd.vicomtech.org/ontology/automotive#MovingManeuver -->

    <owl:Class rdf:about="http://vcd.vicomtech.org/ontology/automotive#MovingManeuver">
        <rdfs:subClassOf rdf:resource="http://vcd.vicomtech.org/ontology/automotive#Action"/>
        <owl:disjointWith rdf:resource="http://vcd.vicomtech.org/ontology/automotive#StationaryManeuver"/>
        <rdfs:comment>A maneuver performed to change the initial state of the object.</rdfs:comment>
        <rdfs:label>Moving maneuver</rdfs:label>
    </owl:Class>
    


    <!-- http://vcd.vicomtech.org/ontology/automotive#Nature -->

    <owl:Class rdf:about="http://vcd.vicomtech.org/ontology/automotive#Nature">
        <rdfs:subClassOf rdf:resource="http://vcd.vicomtech.org/ontology/automotive#Static"/>
        <rdfs:comment>The phenomena of the physical world collectively, including plants, animals, the landscape, and other features and products of the earth, as opposed to humans or human creations.</rdfs:comment>
        <rdfs:label>Nature</rdfs:label>
    </owl:Class>
    


    <!-- http://vcd.vicomtech.org/ontology/automotive#Nighttime -->

    <owl:Class rdf:about="http://vcd.vicomtech.org/ontology/automotive#Nighttime">
        <rdfs:subClassOf rdf:resource="http://vcd.vicomtech.org/ontology/automotive#TimeOfDay"/>
        <rdfs:comment>The night-time is from sunset to sunrise.</rdfs:comment>
        <rdfs:label>Nighttime</rdfs:label>
    </owl:Class>
    


    <!-- http://vcd.vicomtech.org/ontology/automotive#NonDrivableStreet -->

    <owl:Class rdf:about="http://vcd.vicomtech.org/ontology/automotive#NonDrivableStreet">
        <rdfs:subClassOf rdf:resource="http://vcd.vicomtech.org/ontology/automotive#RoadSurface"/>
        <rdfs:comment>A road where is not allowed to drive any king of vehicle.</rdfs:comment>
        <rdfs:label>Non drivable street</rdfs:label>
    </owl:Class>
    


    <!-- http://vcd.vicomtech.org/ontology/automotive#NormalStreet -->

    <owl:Class rdf:about="http://vcd.vicomtech.org/ontology/automotive#NormalStreet">
        <rdfs:subClassOf rdf:resource="http://vcd.vicomtech.org/ontology/automotive#RoadSurface"/>
        <rdfs:comment>Street with no restriction.</rdfs:comment>
        <rdfs:label>Normal street</rdfs:label>
    </owl:Class>
    


    <!-- http://vcd.vicomtech.org/ontology/automotive#Object -->

    <owl:Class rdf:about="http://vcd.vicomtech.org/ontology/automotive#Object">
        <rdfs:subClassOf rdf:resource="http://www.w3.org/2002/07/owl#Thing"/>
        <rdfs:comment>An object is any material thing that can be seen and touched.</rdfs:comment>
        <rdfs:label>Object</rdfs:label>
    </owl:Class>
    


    <!-- http://vcd.vicomtech.org/ontology/automotive#OfficialSignaler -->

    <owl:Class rdf:about="http://vcd.vicomtech.org/ontology/automotive#OfficialSignaler">
        <rdfs:subClassOf rdf:resource="http://vcd.vicomtech.org/ontology/automotive#TrafficSignaler"/>
        <rdfs:comment>A person with authority, such as police, or other first responders and/or construction workers who is actively managing traffic through signaling, wearing particular clothes or uniforms that explicit his official role</rdfs:comment>
        <rdfs:label>Official Traffic signaler</rdfs:label>
    </owl:Class>
    


    <!-- http://vcd.vicomtech.org/ontology/automotive#OldMarkingWhite -->

    <owl:Class rdf:about="http://vcd.vicomtech.org/ontology/automotive#OldMarkingWhite">
        <rdfs:subClassOf rdf:resource="http://vcd.vicomtech.org/ontology/automotive#WhiteLines"/>
        <rdfs:comment>An old marking that is still visible.</rdfs:comment>
        <rdfs:label>Old marking white</rdfs:label>
    </owl:Class>
    


    <!-- http://vcd.vicomtech.org/ontology/automotive#OldMarkingYellow -->

    <owl:Class rdf:about="http://vcd.vicomtech.org/ontology/automotive#OldMarkingYellow">
        <rdfs:subClassOf rdf:resource="http://vcd.vicomtech.org/ontology/automotive#YellowLines"/>
        <rdfs:comment>An old marking that is still visible.</rdfs:comment>
        <rdfs:label>Old marking yellow</rdfs:label>
    </owl:Class>
    


    <!-- http://vcd.vicomtech.org/ontology/automotive#OtherAir -->

    <owl:Class rdf:about="http://vcd.vicomtech.org/ontology/automotive#OtherAir">
        <rdfs:subClassOf rdf:resource="http://vcd.vicomtech.org/ontology/automotive#Air"/>
        <rdfs:label>Other air</rdfs:label>
    </owl:Class>
    


    <!-- http://vcd.vicomtech.org/ontology/automotive#OtherBarrier -->

    <owl:Class rdf:about="http://vcd.vicomtech.org/ontology/automotive#OtherBarrier">
        <rdfs:subClassOf rdf:resource="http://vcd.vicomtech.org/ontology/automotive#Barrier"/>
        <rdfs:label>Other barrier</rdfs:label>
    </owl:Class>
    


    <!-- http://vcd.vicomtech.org/ontology/automotive#OtherRider -->

    <owl:Class rdf:about="http://vcd.vicomtech.org/ontology/automotive#OtherRider">
        <rdfs:subClassOf rdf:resource="http://vcd.vicomtech.org/ontology/automotive#Rider"/>
        <rdfs:comment>A person who rides a vehicle other than a motorcycle or a bicycle. For examples, vehicles like ricksaw, wheeled char, scooter, mobility-scooter, etc.</rdfs:comment>
        <rdfs:label>Other rider</rdfs:label>
    </owl:Class>
    


    <!-- http://vcd.vicomtech.org/ontology/automotive#Overpass -->

    <owl:Class rdf:about="http://vcd.vicomtech.org/ontology/automotive#Overpass">
        <rdfs:subClassOf rdf:resource="http://vcd.vicomtech.org/ontology/automotive#Barrier"/>
        <rdfs:comment>A crossing of two highways or of a highway and pedestrian path or railroad at different levels where clearance to traffic on the lower level is obtained by elevating the higher level also : the upper level of such a crossing.</rdfs:comment>
        <rdfs:label>Overpass</rdfs:label>
    </owl:Class>
    


    <!-- http://vcd.vicomtech.org/ontology/automotive#Overtake -->

    <owl:Class rdf:about="http://vcd.vicomtech.org/ontology/automotive#Overtake">
        <rdfs:subClassOf rdf:resource="http://vcd.vicomtech.org/ontology/automotive#Event"/>
        <rdfs:comment>To go past another vehicle that is travelling in the same direction.</rdfs:comment>
        <rdfs:label>Overtake</rdfs:label>
    </owl:Class>
    


    <!-- http://vcd.vicomtech.org/ontology/automotive#Overtaking -->

    <owl:Class rdf:about="http://vcd.vicomtech.org/ontology/automotive#Overtaking">
        <rdfs:subClassOf rdf:resource="http://vcd.vicomtech.org/ontology/automotive#MovingManeuver"/>
        <rdfs:comment>To go past another vehicle that is travelling in the same direction.</rdfs:comment>
        <rdfs:label>Overtaking</rdfs:label>
    </owl:Class>
    


    <!-- http://vcd.vicomtech.org/ontology/automotive#PTW -->

    <owl:Class rdf:about="http://vcd.vicomtech.org/ontology/automotive#PTW">
        <rdfs:subClassOf rdf:resource="http://vcd.vicomtech.org/ontology/automotive#Cycle"/>
        <rdfs:comment>Powered Two-Wheeler Target (PTW) means a combination of a motorcycle and motorcyclist.</rdfs:comment>
        <rdfs:label>PTW</rdfs:label>
    </owl:Class>
    


    <!-- http://vcd.vicomtech.org/ontology/automotive#ParcelDelivery -->

    <owl:Class rdf:about="http://vcd.vicomtech.org/ontology/automotive#ParcelDelivery">
        <rdfs:subClassOf rdf:resource="http://vcd.vicomtech.org/ontology/automotive#StreetOperationsVehicle"/>
        <rdfs:comment>A type of van suited for delivery goods, parcels and packages to houses, offices and factories. Usually branded with logistic company logo. Characterized by stop-and-go behavior and often by a human operator (sometimes the driver himself) jumping on and off to carry out the delivery task.</rdfs:comment>
        <rdfs:label>Parcel delivery van</rdfs:label>
    </owl:Class>
    


    <!-- http://vcd.vicomtech.org/ontology/automotive#ParcloInterchange -->

    <owl:Class rdf:about="http://vcd.vicomtech.org/ontology/automotive#ParcloInterchange">
        <rdfs:subClassOf rdf:resource="http://vcd.vicomtech.org/ontology/automotive#ServiceInterchange"/>
        <rdfs:comment>A parclo (partial cloverleaf) interchange is an interchange usually involving four to six ramps, two of which are loop ramps, which connect to the non-highway.</rdfs:comment>
        <rdfs:label>Parclo interchange</rdfs:label>
    </owl:Class>
    


    <!-- http://vcd.vicomtech.org/ontology/automotive#Park -->

    <owl:Class rdf:about="http://vcd.vicomtech.org/ontology/automotive#Park">
        <rdfs:subClassOf rdf:resource="http://vcd.vicomtech.org/ontology/automotive#Event"/>
        <rdfs:comment>Ending the parking action.</rdfs:comment>
        <rdfs:label>Park</rdfs:label>
    </owl:Class>
    


    <!-- http://vcd.vicomtech.org/ontology/automotive#Parked -->

    <owl:Class rdf:about="http://vcd.vicomtech.org/ontology/automotive#Parked">
        <rdfs:subClassOf rdf:resource="http://vcd.vicomtech.org/ontology/automotive#StationaryManeuver"/>
        <rdfs:comment>The action of being stopped an leaving the vehicle temporarily in that spot.</rdfs:comment>
        <rdfs:label>Parked</rdfs:label>
    </owl:Class>
    


    <!-- http://vcd.vicomtech.org/ontology/automotive#Parking -->

    <owl:Class rdf:about="http://vcd.vicomtech.org/ontology/automotive#Parking">
        <rdfs:subClassOf rdf:resource="http://vcd.vicomtech.org/ontology/automotive#MovingManeuver"/>
        <rdfs:comment>The act of bringing (a vehicle that one is driving) to a halt and leave it temporarily, typically in a car park or by the side of the road.</rdfs:comment>
        <rdfs:label>Parking</rdfs:label>
    </owl:Class>
    


    <!-- http://vcd.vicomtech.org/ontology/automotive#ParkingLot -->

    <owl:Class rdf:about="http://vcd.vicomtech.org/ontology/automotive#ParkingLot">
        <rdfs:subClassOf rdf:resource="http://vcd.vicomtech.org/ontology/automotive#Flat"/>
        <rdfs:comment>A building, or an area under a building, where cars can be parked.</rdfs:comment>
        <rdfs:label>Parking lot</rdfs:label>
    </owl:Class>
    


    <!-- http://vcd.vicomtech.org/ontology/automotive#ParkingMeter -->

    <owl:Class rdf:about="http://vcd.vicomtech.org/ontology/automotive#ParkingMeter">
        <rdfs:subClassOf rdf:resource="http://vcd.vicomtech.org/ontology/automotive#RoadsideObject"/>
        <rdfs:comment>A machine next to a parking space in a street, into which the driver puts money so as to be authorized to park the vehicle for a particular length of time.</rdfs:comment>
        <rdfs:label>Parking meter</rdfs:label>
    </owl:Class>
    


    <!-- http://vcd.vicomtech.org/ontology/automotive#ParkingSign -->

    <owl:Class rdf:about="http://vcd.vicomtech.org/ontology/automotive#ParkingSign">
        <rdfs:subClassOf rdf:resource="http://vcd.vicomtech.org/ontology/automotive#Signs"/>
        <rdfs:comment>A sign that gives information about a parking space.</rdfs:comment>
        <rdfs:label>Parking sign</rdfs:label>
    </owl:Class>
    


    <!-- http://vcd.vicomtech.org/ontology/automotive#PartialYInterchange -->

    <owl:Class rdf:about="http://vcd.vicomtech.org/ontology/automotive#PartialYInterchange">
        <rdfs:subClassOf rdf:resource="http://vcd.vicomtech.org/ontology/automotive#TwoWayInterchange"/>
        <rdfs:comment>A partial-Y interchange is used where one highway terminates at another highway with the same general directional alignment (usually a maximum of sixty degrees). The trunk of the terminating highway merges with the trunk of the continuous highway; vehicles traveling into the interchange may only exit traveling in the same direction. This type of interchange is often used for bypass routes, and is named for the shape the two highways&apos; confluence makes when drawn on a map, creating a lower-case &quot;y&quot;.</rdfs:comment>
        <rdfs:label>Partial-Y interchange</rdfs:label>
    </owl:Class>
    


    <!-- http://vcd.vicomtech.org/ontology/automotive#Pass -->

    <owl:Class rdf:about="http://vcd.vicomtech.org/ontology/automotive#Pass">
        <rdfs:subClassOf rdf:resource="http://vcd.vicomtech.org/ontology/automotive#Event"/>
        <rdfs:comment>When a vehicle drives past another vehicle in a neighboring lane.</rdfs:comment>
        <rdfs:label>Pass</rdfs:label>
    </owl:Class>
    


    <!-- http://vcd.vicomtech.org/ontology/automotive#PassengerCar -->

    <owl:Class rdf:about="http://vcd.vicomtech.org/ontology/automotive#PassengerCar">
        <rdfs:subClassOf rdf:resource="http://vcd.vicomtech.org/ontology/automotive#Car"/>
        <rdfs:comment>A passenger car is a road motor vehicle, other than a motor cycle, intended for the carriage of passengers and designed to seat no more than nine persons (including the driver).</rdfs:comment>
        <rdfs:label>Passenger car</rdfs:label>
    </owl:Class>
    


    <!-- http://vcd.vicomtech.org/ontology/automotive#Passing -->

    <owl:Class rdf:about="http://vcd.vicomtech.org/ontology/automotive#Passing">
        <rdfs:subClassOf rdf:resource="http://vcd.vicomtech.org/ontology/automotive#MovingManeuver"/>
        <rdfs:comment>When a vehicle is driving past another vehicle in a neighboring lane.</rdfs:comment>
        <rdfs:label>Passing</rdfs:label>
    </owl:Class>
    


    <!-- http://vcd.vicomtech.org/ontology/automotive#Pedestrian -->

    <owl:Class rdf:about="http://vcd.vicomtech.org/ontology/automotive#Pedestrian">
        <rdfs:subClassOf rdf:resource="http://vcd.vicomtech.org/ontology/automotive#Human"/>
        <rdfs:comment>Persons moving by their own legs, sitting or in any unusual pose but not meant to drive a vehicle.</rdfs:comment>
        <rdfs:label>Pedestrian</rdfs:label>
    </owl:Class>
    


    <!-- http://vcd.vicomtech.org/ontology/automotive#PedestrianArea -->

    <owl:Class rdf:about="http://vcd.vicomtech.org/ontology/automotive#PedestrianArea">
        <rdfs:subClassOf rdf:resource="http://vcd.vicomtech.org/ontology/automotive#Flat"/>
        <rdfs:comment>Areas solely to be used by pedestrians. E.g. inner city areas, parks, shopping zones, etc.</rdfs:comment>
        <rdfs:label>Pedestrian area</rdfs:label>
    </owl:Class>
    


    <!-- http://vcd.vicomtech.org/ontology/automotive#PedestrianWithObject -->

    <owl:Class rdf:about="http://vcd.vicomtech.org/ontology/automotive#PedestrianWithObject">
        <rdfs:subClassOf rdf:resource="http://vcd.vicomtech.org/ontology/automotive#Human"/>
        <rdfs:comment>Any person that is carrying an object while acting as a pedestrian in the surroundings of the vehicle.</rdfs:comment>
        <rdfs:label>Pedestrian with Object</rdfs:label>
    </owl:Class>
    


    <!-- http://vcd.vicomtech.org/ontology/automotive#PersonalMobilityDevice -->

    <owl:Class rdf:about="http://vcd.vicomtech.org/ontology/automotive#PersonalMobilityDevice">
        <rdfs:subClassOf rdf:resource="http://vcd.vicomtech.org/ontology/automotive#WheeledSlow"/>
        <rdfs:comment>Personal mobility Personal mobility devices are small vehicles, motorized or not, that are designed for agile mobility of a single person normally. They are not considered ridable or drivable vehicles due to their low weight ( &lt;15 kg ) and small dimensions and due to the fact that they do not offer any structural protection to the rider, nor have any articulated systems designed to control such vehicles ( steering wheels, pedals etc.). The rider is completely exposed, usually standing on the device.</rdfs:comment>
        <rdfs:label>Personal Mobility device</rdfs:label>
    </owl:Class>
    


    <!-- http://vcd.vicomtech.org/ontology/automotive#Pet -->

    <owl:Class rdf:about="http://vcd.vicomtech.org/ontology/automotive#Pet">
        <rdfs:subClassOf rdf:resource="http://vcd.vicomtech.org/ontology/automotive#Animal"/>
        <rdfs:comment>Animal usually adopted by humans, grown and taken care of by a person. Horses, dog, cats fall under this category.</rdfs:comment>
        <rdfs:label>Pet</rdfs:label>
    </owl:Class>
    


    <!-- http://vcd.vicomtech.org/ontology/automotive#PhoneBooth -->

    <owl:Class rdf:about="http://vcd.vicomtech.org/ontology/automotive#PhoneBooth">
        <rdfs:subClassOf rdf:resource="http://vcd.vicomtech.org/ontology/automotive#RoadsideObject"/>
        <rdfs:comment>A public call box typically equipped with a payphone.</rdfs:comment>
        <rdfs:label>Phone booth</rdfs:label>
    </owl:Class>
    


    <!-- http://vcd.vicomtech.org/ontology/automotive#Pickup -->

    <owl:Class rdf:about="http://vcd.vicomtech.org/ontology/automotive#Pickup">
        <rdfs:subClassOf rdf:resource="http://vcd.vicomtech.org/ontology/automotive#Car"/>
        <rdfs:comment>A pickup truck or pickup is a light-duty truck having an enclosed cab and an open cargo area with low sides and tailgate. It can be used as a regular private passenger vehicle or for working/construction purposes.</rdfs:comment>
        <rdfs:label>Pickup-truck</rdfs:label>
    </owl:Class>
    


    <!-- http://vcd.vicomtech.org/ontology/automotive#Pig -->

    <owl:Class rdf:about="http://vcd.vicomtech.org/ontology/automotive#Pig">
        <rdfs:subClassOf rdf:resource="http://vcd.vicomtech.org/ontology/automotive#GroundAnimal"/>
        <rdfs:comment>An omnivorous domesticated hoofed mammal with sparse bristly hair and a flat snout for rooting in the soil, kept for its meat.</rdfs:comment>
        <rdfs:label>Pig</rdfs:label>
    </owl:Class>
    


    <!-- http://vcd.vicomtech.org/ontology/automotive#Pole -->

    <owl:Class rdf:about="http://vcd.vicomtech.org/ontology/automotive#Pole">
        <rdfs:subClassOf rdf:resource="http://vcd.vicomtech.org/ontology/automotive#Support"/>
        <rdfs:comment>Thing and elongated, typically vertically oriented poles. Includes poles holding only street lights.</rdfs:comment>
        <rdfs:label>Pole</rdfs:label>
    </owl:Class>
    


    <!-- http://vcd.vicomtech.org/ontology/automotive#Polegroup -->

    <owl:Class rdf:about="http://vcd.vicomtech.org/ontology/automotive#Polegroup">
        <rdfs:subClassOf rdf:resource="http://vcd.vicomtech.org/ontology/automotive#Support"/>
        <rdfs:comment>A group of poles.</rdfs:comment>
        <rdfs:label>Polegroup</rdfs:label>
    </owl:Class>
    


    <!-- http://vcd.vicomtech.org/ontology/automotive#Police -->

    <owl:Class rdf:about="http://vcd.vicomtech.org/ontology/automotive#Police">
        <rdfs:subClassOf rdf:resource="http://vcd.vicomtech.org/ontology/automotive#EmergencyVehicle"/>
        <rdfs:comment>A police car is a road vehicle used by police officers for transportation during patrols and to enable them to respond to incidents and chases.</rdfs:comment>
        <rdfs:label>Police car</rdfs:label>
    </owl:Class>
    


    <!-- http://vcd.vicomtech.org/ontology/automotive#PoliceBicycle -->

    <owl:Class rdf:about="http://vcd.vicomtech.org/ontology/automotive#PoliceBicycle">
        <rdfs:subClassOf rdf:resource="http://vcd.vicomtech.org/ontology/automotive#EmergencyBicycle"/>
        <rdfs:label>Police Bicycle</rdfs:label>
    </owl:Class>
    


    <!-- http://vcd.vicomtech.org/ontology/automotive#PoliceMotorcycle -->

    <owl:Class rdf:about="http://vcd.vicomtech.org/ontology/automotive#PoliceMotorcycle">
        <rdfs:subClassOf rdf:resource="http://vcd.vicomtech.org/ontology/automotive#EmergencyMotorcycle"/>
        <rdfs:label>Police Motorcycle</rdfs:label>
    </owl:Class>
    


    <!-- http://vcd.vicomtech.org/ontology/automotive#PoliceOfficer -->

    <owl:Class rdf:about="http://vcd.vicomtech.org/ontology/automotive#PoliceOfficer">
        <rdfs:subClassOf rdf:resource="http://vcd.vicomtech.org/ontology/automotive#FirstResponder"/>
        <rdfs:comment>Police officers belongs to organizations whose primary goal is the prevention and detection of crime. Usually wear a particular uniform that explicits this role. A member of a police force; policeman or policewoman.</rdfs:comment>
        <rdfs:label>Police officer</rdfs:label>
    </owl:Class>
    


    <!-- http://vcd.vicomtech.org/ontology/automotive#PoliceTruck -->

    <owl:Class rdf:about="http://vcd.vicomtech.org/ontology/automotive#PoliceTruck">
        <rdfs:subClassOf rdf:resource="http://vcd.vicomtech.org/ontology/automotive#LargeEmergencyVehicle"/>
        <rdfs:comment>Trucks or Heavy-duty vehicles adopted by Police.</rdfs:comment>
        <rdfs:label>Police truck</rdfs:label>
    </owl:Class>
    


    <!-- http://vcd.vicomtech.org/ontology/automotive#Pothole -->

    <owl:Class rdf:about="http://vcd.vicomtech.org/ontology/automotive#Pothole">
        <rdfs:subClassOf rdf:resource="http://vcd.vicomtech.org/ontology/automotive#Water"/>
        <rdfs:comment>A depression or hollow in a road caused by wear or subsidence.</rdfs:comment>
        <rdfs:label>Pothole</rdfs:label>
    </owl:Class>
    


    <!-- http://vcd.vicomtech.org/ontology/automotive#PushablePullable -->

    <owl:Class rdf:about="http://vcd.vicomtech.org/ontology/automotive#PushablePullable">
        <rdfs:subClassOf rdf:resource="http://vcd.vicomtech.org/ontology/automotive#RoadVehicle"/>
        <rdfs:comment>An object that can be pushed or pulled.</rdfs:comment>
        <rdfs:label>Pushable/Pullable</rdfs:label>
    </owl:Class>
    


    <!-- http://vcd.vicomtech.org/ontology/automotive#RV -->

    <owl:Class rdf:about="http://vcd.vicomtech.org/ontology/automotive#RV">
        <rdfs:subClassOf rdf:resource="http://vcd.vicomtech.org/ontology/automotive#Trailer"/>
        <rdfs:comment>An RV is a trailed vehicle which is designed to be used as a moving house for people, usually equipped with things such as beed and cooking equipment. Dimensions can largely vary and it can have one or more axles.</rdfs:comment>
        <rdfs:label>RV</rdfs:label>
    </owl:Class>
    


    <!-- http://vcd.vicomtech.org/ontology/automotive#RailTrack -->

    <owl:Class rdf:about="http://vcd.vicomtech.org/ontology/automotive#RailTrack">
        <rdfs:subClassOf rdf:resource="http://vcd.vicomtech.org/ontology/automotive#Flat"/>
        <rdfs:comment>The parallel steel rails on which a train runs.</rdfs:comment>
        <rdfs:label>Rail track</rdfs:label>
    </owl:Class>
    


    <!-- http://vcd.vicomtech.org/ontology/automotive#RailborneVehicle -->

    <owl:Class rdf:about="http://vcd.vicomtech.org/ontology/automotive#RailborneVehicle">
        <rdfs:subClassOf rdf:resource="http://vcd.vicomtech.org/ontology/automotive#Vehicle"/>
        <rdfs:comment>A vehicle formed by one or more wagons that moves along a railway.</rdfs:comment>
        <rdfs:label>Railborne vehicle</rdfs:label>
    </owl:Class>
    


    <!-- http://vcd.vicomtech.org/ontology/automotive#Rain -->

    <owl:Class rdf:about="http://vcd.vicomtech.org/ontology/automotive#Rain">
        <rdfs:subClassOf rdf:resource="http://vcd.vicomtech.org/ontology/automotive#Element"/>
        <rdfs:subClassOf rdf:resource="http://vcd.vicomtech.org/ontology/automotive#Weather"/>
        <rdfs:comment>Having or characterized by considerable rainfall.</rdfs:comment>
        <rdfs:label>Rain</rdfs:label>
    </owl:Class>
    


    <!-- http://vcd.vicomtech.org/ontology/automotive#RainDirt -->

    <owl:Class rdf:about="http://vcd.vicomtech.org/ontology/automotive#RainDirt">
        <rdfs:subClassOf rdf:resource="http://vcd.vicomtech.org/ontology/automotive#Rain"/>
        <rdfs:comment>Is a variety of rain which contains enough dust for it to be visible. Also known as rain dust.</rdfs:comment>
        <rdfs:label>Rain dirt</rdfs:label>
    </owl:Class>
    


    <!-- http://vcd.vicomtech.org/ontology/automotive#Ramp -->

    <owl:Class rdf:about="http://vcd.vicomtech.org/ontology/automotive#Ramp">
        <rdfs:subClassOf rdf:resource="http://vcd.vicomtech.org/ontology/automotive#RoadObstacles"/>
        <rdfs:comment>A sloping surface joining two different levels.</rdfs:comment>
        <rdfs:label>Ramp</rdfs:label>
    </owl:Class>
    


    <!-- http://vcd.vicomtech.org/ontology/automotive#Reach -->

    <owl:Class rdf:about="http://vcd.vicomtech.org/ontology/automotive#Reach">
        <rdfs:subClassOf rdf:resource="http://vcd.vicomtech.org/ontology/automotive#Event"/>
        <rdfs:comment>To arrive at a certain point in distance.</rdfs:comment>
        <rdfs:label>Reach</rdfs:label>
    </owl:Class>
    


    <!-- http://vcd.vicomtech.org/ontology/automotive#ReflectionPoint -->

    <owl:Class rdf:about="http://vcd.vicomtech.org/ontology/automotive#ReflectionPoint">
        <rdfs:subClassOf rdf:resource="http://vcd.vicomtech.org/ontology/automotive#Void"/>
        <rdfs:comment>A transformation where a point appears an equal distance on the other. side of a given line - the line of reflection.</rdfs:comment>
        <rdfs:label>Reflection point</rdfs:label>
    </owl:Class>
    


    <!-- http://vcd.vicomtech.org/ontology/automotive#RestrictedArea -->

    <owl:Class rdf:about="http://vcd.vicomtech.org/ontology/automotive#RestrictedArea">
        <rdfs:subClassOf rdf:resource="http://vcd.vicomtech.org/ontology/automotive#RoadSurface"/>
        <rdfs:comment>An area which unauthorized people are not allowed to enter or and area with a peed limit for vehicles.</rdfs:comment>
        <rdfs:label>Restricted area</rdfs:label>
    </owl:Class>
    


    <!-- http://vcd.vicomtech.org/ontology/automotive#Reversing -->

    <owl:Class rdf:about="http://vcd.vicomtech.org/ontology/automotive#Reversing">
        <rdfs:subClassOf rdf:resource="http://vcd.vicomtech.org/ontology/automotive#MovingManeuver"/>
        <rdfs:comment>Is the process of driving a vehicle in the reverse direction in order to maneuver.</rdfs:comment>
        <rdfs:label>Reversing</rdfs:label>
    </owl:Class>
    


    <!-- http://vcd.vicomtech.org/ontology/automotive#Rider -->

    <owl:Class rdf:about="http://vcd.vicomtech.org/ontology/automotive#Rider">
        <rdfs:subClassOf rdf:resource="http://vcd.vicomtech.org/ontology/automotive#Human"/>
        <rdfs:comment>A human who is riding any type of vehicle (horse, bicycle, motorcycle, etc.).</rdfs:comment>
        <rdfs:label>Rider</rdfs:label>
    </owl:Class>
    


    <!-- http://vcd.vicomtech.org/ontology/automotive#Rigid -->

    <owl:Class rdf:about="http://vcd.vicomtech.org/ontology/automotive#Rigid">
        <rdfs:subClassOf rdf:resource="http://vcd.vicomtech.org/ontology/automotive#Bus"/>
        <rdfs:comment>Is a vehicle  used in public transportation services with a single, rigid chassis.</rdfs:comment>
        <rdfs:label>Rigid</rdfs:label>
    </owl:Class>
    


    <!-- http://vcd.vicomtech.org/ontology/automotive#Rise -->

    <owl:Class rdf:about="http://vcd.vicomtech.org/ontology/automotive#Rise">
        <rdfs:subClassOf rdf:resource="http://vcd.vicomtech.org/ontology/automotive#Event"/>
        <rdfs:comment>To get up from lying, sitting, or kneeling.</rdfs:comment>
        <rdfs:label>Rise</rdfs:label>
    </owl:Class>
    


    <!-- http://vcd.vicomtech.org/ontology/automotive#Rising -->

    <owl:Class rdf:about="http://vcd.vicomtech.org/ontology/automotive#Rising">
        <rdfs:subClassOf rdf:resource="http://vcd.vicomtech.org/ontology/automotive#MovingManeuver"/>
        <rdfs:comment>When a person stands up.</rdfs:comment>
        <rdfs:label>Rising</rdfs:label>
    </owl:Class>
    


    <!-- http://vcd.vicomtech.org/ontology/automotive#River -->

    <owl:Class rdf:about="http://vcd.vicomtech.org/ontology/automotive#River">
        <rdfs:subClassOf rdf:resource="http://vcd.vicomtech.org/ontology/automotive#Water"/>
        <rdfs:comment>A large natural stream of water flowing in a channel to the sea, a lake, or another river.</rdfs:comment>
        <rdfs:label>River</rdfs:label>
    </owl:Class>
    


    <!-- http://vcd.vicomtech.org/ontology/automotive#Road -->

    <owl:Class rdf:about="http://vcd.vicomtech.org/ontology/automotive#Road">
        <rdfs:subClassOf rdf:resource="http://vcd.vicomtech.org/ontology/automotive#Flat"/>
        <rdfs:comment>A wide way leading from one place to another, especially one with a specially prepared surface which vehicles can use.</rdfs:comment>
        <rdfs:label>Road</rdfs:label>
    </owl:Class>
    


    <!-- http://vcd.vicomtech.org/ontology/automotive#RoadObstacles -->

    <owl:Class rdf:about="http://vcd.vicomtech.org/ontology/automotive#RoadObstacles">
        <rdfs:subClassOf rdf:resource="http://vcd.vicomtech.org/ontology/automotive#MovableObject"/>
        <rdfs:comment>A thing that blocks one way or prevents or hinders progress.</rdfs:comment>
        <rdfs:label>Road obstacles</rdfs:label>
    </owl:Class>
    


    <!-- http://vcd.vicomtech.org/ontology/automotive#RoadSection -->

    <owl:Class rdf:about="http://vcd.vicomtech.org/ontology/automotive#RoadSection">
        <rdfs:subClassOf rdf:resource="http://vcd.vicomtech.org/ontology/automotive#Road"/>
        <rdfs:comment>A distinct part of the road.</rdfs:comment>
        <rdfs:label>Road section</rdfs:label>
    </owl:Class>
    


    <!-- http://vcd.vicomtech.org/ontology/automotive#RoadSegments -->

    <owl:Class rdf:about="http://vcd.vicomtech.org/ontology/automotive#RoadSegments">
        <rdfs:subClassOf rdf:resource="http://vcd.vicomtech.org/ontology/automotive#Intersection"/>
        <rdfs:comment>One way to classify intersections is by the number of road segments (arms) that are involved.</rdfs:comment>
        <rdfs:label>Road segments</rdfs:label>
    </owl:Class>
    


    <!-- http://vcd.vicomtech.org/ontology/automotive#RoadSurface -->

    <owl:Class rdf:about="http://vcd.vicomtech.org/ontology/automotive#RoadSurface">
        <rdfs:subClassOf rdf:resource="http://vcd.vicomtech.org/ontology/automotive#Road"/>
        <rdfs:comment>A road surface or pavement, is the durable surface material laid down on an area intended to sustain vehicular or foot traffic, such as a road or walkway.</rdfs:comment>
        <rdfs:label>Road surface</rdfs:label>
    </owl:Class>
    


    <!-- http://vcd.vicomtech.org/ontology/automotive#RoadVehicle -->

    <owl:Class rdf:about="http://vcd.vicomtech.org/ontology/automotive#RoadVehicle">
        <rdfs:subClassOf rdf:resource="http://vcd.vicomtech.org/ontology/automotive#Vehicle"/>
        <rdfs:comment>A vehicle designed to legally carry people or cargo on public roads and highways.</rdfs:comment>
        <rdfs:label>Road vehicle</rdfs:label>
    </owl:Class>
    


    <!-- http://vcd.vicomtech.org/ontology/automotive#Roadblocks -->

    <owl:Class rdf:about="http://vcd.vicomtech.org/ontology/automotive#Roadblocks">
        <rdfs:subClassOf rdf:resource="http://vcd.vicomtech.org/ontology/automotive#TrafficDevice"/>
        <rdfs:comment>An obstruction in a road set up specially by law enforcement officers.</rdfs:comment>
        <rdfs:label>Roadblocks</rdfs:label>
    </owl:Class>
    


    <!-- http://vcd.vicomtech.org/ontology/automotive#RoadsideObject -->

    <owl:Class rdf:about="http://vcd.vicomtech.org/ontology/automotive#RoadsideObject">
        <rdfs:subClassOf rdf:resource="http://vcd.vicomtech.org/ontology/automotive#Static"/>
        <rdfs:comment>Fixed objects placed beside a road.</rdfs:comment>
        <rdfs:label>Roadside object</rdfs:label>
    </owl:Class>
    


    <!-- http://vcd.vicomtech.org/ontology/automotive#Roundabout -->

    <owl:Class rdf:about="http://vcd.vicomtech.org/ontology/automotive#Roundabout">
        <rdfs:subClassOf rdf:resource="http://vcd.vicomtech.org/ontology/automotive#Junction"/>
        <rdfs:comment>A road junction at which traffic moves in one direction round a central island to reach one of the roads converging on it.</rdfs:comment>
        <rdfs:label>Roundabout</rdfs:label>
    </owl:Class>
    


    <!-- http://vcd.vicomtech.org/ontology/automotive#RoundaboutInterchange -->

    <owl:Class rdf:about="http://vcd.vicomtech.org/ontology/automotive#RoundaboutInterchange">
        <rdfs:subClassOf rdf:resource="http://vcd.vicomtech.org/ontology/automotive#FourWayInterchange"/>
        <rdfs:comment>A further alternative found often is called a roundabout interchange. This is a normal roundabout except one (two-level) or both (three-level) mainlines pass under or over the whole interchange. The ramps of the interchanging highways meet at a roundabout, or rotary, on a separated level above, below, or in the middle of the two highways.</rdfs:comment>
        <rdfs:label>Roundabout interchange</rdfs:label>
    </owl:Class>
    


    <!-- http://vcd.vicomtech.org/ontology/automotive#Rover -->

    <owl:Class rdf:about="http://vcd.vicomtech.org/ontology/automotive#Rover">
        <rdfs:subClassOf rdf:resource="http://vcd.vicomtech.org/ontology/automotive#Car"/>
        <rdfs:comment>Rover is a British automotive marque that was used for over a century. The rights to the marque are currently part of Jaguar Land Rover.</rdfs:comment>
        <rdfs:label>Rover</rdfs:label>
    </owl:Class>
    


    <!-- http://vcd.vicomtech.org/ontology/automotive#Running -->

    <owl:Class rdf:about="http://vcd.vicomtech.org/ontology/automotive#Running">
        <rdfs:subClassOf rdf:resource="http://vcd.vicomtech.org/ontology/automotive#MovingManeuver"/>
        <rdfs:comment>The action of movement of a runner.</rdfs:comment>
        <rdfs:label>Running</rdfs:label>
    </owl:Class>
    


    <!-- http://vcd.vicomtech.org/ontology/automotive#SUV -->

    <owl:Class rdf:about="http://vcd.vicomtech.org/ontology/automotive#SUV">
        <rdfs:subClassOf rdf:resource="http://vcd.vicomtech.org/ontology/automotive#Car"/>
        <rdfs:comment>An SUV is a powerful vehicle with four-wheel drive that can be driven over rough ground. SUV is an abbreviation for &apos;sport utility vehicle&apos;. SUVs combine elements of road-going passenger cars with features from off-road vehicles, such as raised ground clearance and four-wheel drive.</rdfs:comment>
        <rdfs:label>SUV</rdfs:label>
    </owl:Class>
    


    <!-- http://vcd.vicomtech.org/ontology/automotive#SafeStop -->

    <owl:Class rdf:about="http://vcd.vicomtech.org/ontology/automotive#SafeStop">
        <rdfs:subClassOf rdf:resource="http://vcd.vicomtech.org/ontology/automotive#Event"/>
        <rdfs:comment>The action of deccelerating until stopping safely. For instance, in front of a traffic light or in a traffic jam.</rdfs:comment>
        <rdfs:label>Safe stop</rdfs:label>
    </owl:Class>
    


    <!-- http://vcd.vicomtech.org/ontology/automotive#Sand -->

    <owl:Class rdf:about="http://vcd.vicomtech.org/ontology/automotive#Sand">
        <rdfs:subClassOf rdf:resource="http://vcd.vicomtech.org/ontology/automotive#Nature"/>
        <rdfs:comment>Includes surfaces consisting of sand or sand heaps, e.g. at construction areas.</rdfs:comment>
        <rdfs:label>Sand</rdfs:label>
    </owl:Class>
    


    <!-- http://vcd.vicomtech.org/ontology/automotive#Scooter -->

    <owl:Class rdf:about="http://vcd.vicomtech.org/ontology/automotive#Scooter">
        <rdfs:subClassOf rdf:resource="http://vcd.vicomtech.org/ontology/automotive#PersonalMobilityDevice"/>
        <rdfs:comment>A Scooter is a small, light usually 2 wheeled personal mobility device consisting of a footboards mounted on two wheels and a long steering handle. Scooters can be propelled by resting one foot on the footboards and pushing the other against the ground or they can be motorized withe electrical actuators.</rdfs:comment>
        <rdfs:label>Scooter</rdfs:label>
    </owl:Class>
    


    <!-- http://vcd.vicomtech.org/ontology/automotive#SecurityLighting -->

    <owl:Class rdf:about="http://vcd.vicomtech.org/ontology/automotive#SecurityLighting">
        <rdfs:subClassOf rdf:resource="http://vcd.vicomtech.org/ontology/automotive#ArtificialLighting"/>
        <rdfs:comment>Security lighting can be used along roadways in urban areas, or behind homes or commercial facilities. These are extremely bright lights used to deter crime. Security lights may include floodlights and be activated with PIR switches that detect moving heat sources in darkness.</rdfs:comment>
        <rdfs:label>Security lighting</rdfs:label>
    </owl:Class>
    


    <!-- http://vcd.vicomtech.org/ontology/automotive#Sedan -->

    <owl:Class rdf:about="http://vcd.vicomtech.org/ontology/automotive#Sedan">
        <rdfs:subClassOf rdf:resource="http://vcd.vicomtech.org/ontology/automotive#Car"/>
        <rdfs:comment>A sedan is the most common form of a passenger car, with a three box configuration for separate compartments of engine, passenger and cargo. Small and sub-compacts cars falls under this class as well.</rdfs:comment>
        <rdfs:label>Sedan</rdfs:label>
    </owl:Class>
    


    <!-- http://vcd.vicomtech.org/ontology/automotive#SemiDirectionalTInterchange -->

    <owl:Class rdf:about="http://vcd.vicomtech.org/ontology/automotive#SemiDirectionalTInterchange">
        <rdfs:subClassOf rdf:resource="http://vcd.vicomtech.org/ontology/automotive#ThreeWayInterchange"/>
        <rdfs:comment>Like a directional T interchange, a semi-directional T interchange uses flyover (overpass) or underpass ramps in all directions at a three-way interchange. However, in a semi-directional T some of the splits and merges are switched to avoid ramps to and from the passing lane. Semi-directional T interchanges are built as two or three-level junctions, with three-level interchanges typically being used in urban or suburban areas where land is more expensive.</rdfs:comment>
        <rdfs:label>Semi-directional T interchange</rdfs:label>
    </owl:Class>
    


    <!-- http://vcd.vicomtech.org/ontology/automotive#Sensor -->

    <owl:Class rdf:about="http://vcd.vicomtech.org/ontology/automotive#Sensor">
        <rdfs:subClassOf rdf:resource="http://vcd.vicomtech.org/ontology/automotive#InVehicleSystems"/>
        <rdfs:comment>Automobile sensors are intelligent sensors which can be used to control and process the pressure of oil, temperature, level of emission, coolant levels, etc.</rdfs:comment>
        <rdfs:label>Sensor</rdfs:label>
    </owl:Class>
    


    <!-- http://vcd.vicomtech.org/ontology/automotive#ServiceInterchange -->

    <owl:Class rdf:about="http://vcd.vicomtech.org/ontology/automotive#ServiceInterchange">
        <rdfs:subClassOf rdf:resource="http://vcd.vicomtech.org/ontology/automotive#Interchange"/>
        <rdfs:label>Service interchange</rdfs:label>
    </owl:Class>
    


    <!-- http://vcd.vicomtech.org/ontology/automotive#ServiceLane -->

    <owl:Class rdf:about="http://vcd.vicomtech.org/ontology/automotive#ServiceLane">
        <rdfs:subClassOf rdf:resource="http://vcd.vicomtech.org/ontology/automotive#Lane"/>
        <rdfs:comment>Road shoulders, typically on highways, which offer enough space for a car to drive and stop in emergency cases. Usually on the right side of drivable lanes, but can also be on the left side.</rdfs:comment>
        <rdfs:label>Service lane</rdfs:label>
    </owl:Class>
    


    <!-- http://vcd.vicomtech.org/ontology/automotive#ShopingCart -->

    <owl:Class rdf:about="http://vcd.vicomtech.org/ontology/automotive#ShopingCart">
        <rdfs:subClassOf rdf:resource="http://vcd.vicomtech.org/ontology/automotive#PushablePullable"/>
        <rdfs:comment>A bag or basket on wheels for carrying shopping purchases, in particular one on wheels provided for the use of supermarket customers; a shopping trolley.</rdfs:comment>
        <rdfs:label>Shopping cart</rdfs:label>
    </owl:Class>
    


    <!-- http://vcd.vicomtech.org/ontology/automotive#Sidebars -->

    <owl:Class rdf:about="http://vcd.vicomtech.org/ontology/automotive#Sidebars">
        <rdfs:subClassOf rdf:resource="http://vcd.vicomtech.org/ontology/automotive#Barrier"/>
        <rdfs:comment>An additional or less important thing.</rdfs:comment>
        <rdfs:label>Sidebars</rdfs:label>
    </owl:Class>
    


    <!-- http://vcd.vicomtech.org/ontology/automotive#Sidewalk -->

    <owl:Class rdf:about="http://vcd.vicomtech.org/ontology/automotive#Sidewalk">
        <rdfs:subClassOf rdf:resource="http://vcd.vicomtech.org/ontology/automotive#Lane"/>
        <rdfs:comment>Horizontal surface designated for pedestrians or cyclist. Delimited from the road by some obstacles or poles, but not only by marking. Often elevated compared to the road and often located at the side of a road. Also includes walkable parts of traffic islands, but not pedestrian areas.</rdfs:comment>
        <rdfs:label>Sidewalk</rdfs:label>
    </owl:Class>
    


    <!-- http://vcd.vicomtech.org/ontology/automotive#Signs -->

    <owl:Class rdf:about="http://vcd.vicomtech.org/ontology/automotive#Signs">
        <rdfs:subClassOf rdf:resource="http://vcd.vicomtech.org/ontology/automotive#RoadsideObject"/>
        <rdfs:comment>An object used to convey information or an instruction.</rdfs:comment>
        <rdfs:label>Signs</rdfs:label>
    </owl:Class>
    


    <!-- http://vcd.vicomtech.org/ontology/automotive#SinglePointUrbanInterchange -->

    <owl:Class rdf:about="http://vcd.vicomtech.org/ontology/automotive#SinglePointUrbanInterchange">
        <rdfs:subClassOf rdf:resource="http://vcd.vicomtech.org/ontology/automotive#ServiceInterchange"/>
        <rdfs:comment>Is built with a large over- or clear underpass providing space for a single traffic signal controlled intersection with the ramps and the cross street.</rdfs:comment>
        <rdfs:label>Single-point urban interchange</rdfs:label>
    </owl:Class>
    


    <!-- http://vcd.vicomtech.org/ontology/automotive#Sitting -->

    <owl:Class rdf:about="http://vcd.vicomtech.org/ontology/automotive#Sitting">
        <rdfs:subClassOf rdf:resource="http://vcd.vicomtech.org/ontology/automotive#StationaryManeuver"/>
        <rdfs:comment>The action of being resting on a seat or other type of support, with the upper part of the body vertical.</rdfs:comment>
        <rdfs:label>Sitting</rdfs:label>
    </owl:Class>
    


    <!-- http://vcd.vicomtech.org/ontology/automotive#SixWayItersection -->

    <owl:Class rdf:about="http://vcd.vicomtech.org/ontology/automotive#SixWayItersection">
        <rdfs:subClassOf rdf:resource="http://vcd.vicomtech.org/ontology/automotive#RoadSegments"/>
        <rdfs:comment>Six-way intersections usually involve a crossing of three streets at one junction; for example, a crossing of two perpendicular streets and a diagonal street is a rather common type of 6-way intersection.</rdfs:comment>
        <rdfs:label>Six-way intersection</rdfs:label>
    </owl:Class>
    


    <!-- http://vcd.vicomtech.org/ontology/automotive#Skateboard -->

    <owl:Class rdf:about="http://vcd.vicomtech.org/ontology/automotive#Skateboard">
        <rdfs:subClassOf rdf:resource="http://vcd.vicomtech.org/ontology/automotive#PersonalMobilityDevice"/>
        <rdfs:comment>A skatboards is a short and narrow boards with usually two pairs of wheels fixed at the bottom of either end, on which a person can ride in a standing or crouching position, propelling themselves by occasionally pushing one foot against the ground. Today&apos;s skateboards can have electrical actuators as propellers, usually controlled by a joystick-like device hold in the hand of the rider. They also fall in this cathegory</rdfs:comment>
        <rdfs:label>Skateboard</rdfs:label>
    </owl:Class>
    


    <!-- http://vcd.vicomtech.org/ontology/automotive#Sky -->

    <owl:Class rdf:about="http://vcd.vicomtech.org/ontology/automotive#Sky">
        <rdfs:subClassOf rdf:resource="http://vcd.vicomtech.org/ontology/automotive#Nature"/>
        <rdfs:comment>Sky including fog or heavy precipitation.</rdfs:comment>
        <rdfs:label>Sky</rdfs:label>
    </owl:Class>
    


    <!-- http://vcd.vicomtech.org/ontology/automotive#Sleet -->

    <owl:Class rdf:about="http://vcd.vicomtech.org/ontology/automotive#Sleet">
        <rdfs:subClassOf rdf:resource="http://vcd.vicomtech.org/ontology/automotive#Weather"/>
        <rdfs:comment>Rain containing some ice, as when snow melts as it falls.</rdfs:comment>
        <rdfs:label>Sleet</rdfs:label>
    </owl:Class>
    


    <!-- http://vcd.vicomtech.org/ontology/automotive#SlowDriveArea -->

    <owl:Class rdf:about="http://vcd.vicomtech.org/ontology/automotive#SlowDriveArea">
        <rdfs:subClassOf rdf:resource="http://vcd.vicomtech.org/ontology/automotive#RoadSurface"/>
        <rdfs:comment>A road with speed limitations.</rdfs:comment>
        <rdfs:label>Slow drive area</rdfs:label>
    </owl:Class>
    


    <!-- http://vcd.vicomtech.org/ontology/automotive#SmallVehicle -->

    <owl:Class rdf:about="http://vcd.vicomtech.org/ontology/automotive#SmallVehicle">
        <rdfs:subClassOf rdf:resource="http://vcd.vicomtech.org/ontology/automotive#DrivableVehicle"/>
        <rdfs:comment>The B-segment is the second smallest of the European segments for passenger cars, which is described as &quot;small cars&quot;.</rdfs:comment>
        <rdfs:label>Small vehicle</rdfs:label>
    </owl:Class>
    


    <!-- http://vcd.vicomtech.org/ontology/automotive#Snow -->

    <owl:Class rdf:about="http://vcd.vicomtech.org/ontology/automotive#Snow">
        <rdfs:subClassOf rdf:resource="http://vcd.vicomtech.org/ontology/automotive#Element"/>
        <rdfs:subClassOf rdf:resource="http://vcd.vicomtech.org/ontology/automotive#Weather"/>
        <rdfs:comment>Snow covered surface.</rdfs:comment>
        <rdfs:label>Snow</rdfs:label>
    </owl:Class>
    


    <!-- http://vcd.vicomtech.org/ontology/automotive#SnowPlow -->

    <owl:Class rdf:about="http://vcd.vicomtech.org/ontology/automotive#SnowPlow">
        <rdfs:subClassOf rdf:resource="http://vcd.vicomtech.org/ontology/automotive#StreetOperationsVehicle"/>
        <rdfs:comment>An implement or vehicle for clearing roads of thick snow by pushing it aside.</rdfs:comment>
        <rdfs:label>Snow plow</rdfs:label>
    </owl:Class>
    


    <!-- http://vcd.vicomtech.org/ontology/automotive#SolidBrokenWhite -->

    <owl:Class rdf:about="http://vcd.vicomtech.org/ontology/automotive#SolidBrokenWhite">
        <rdfs:subClassOf rdf:resource="http://vcd.vicomtech.org/ontology/automotive#WhiteLines"/>
        <rdfs:comment>A lane marking formed by a solid and a broken line. If the line nearest to you gets broken it means you may cross the lines to overtake if it is safe.</rdfs:comment>
        <rdfs:label>Solid broken white</rdfs:label>
    </owl:Class>
    


    <!-- http://vcd.vicomtech.org/ontology/automotive#SolidBrokenYellow -->

    <owl:Class rdf:about="http://vcd.vicomtech.org/ontology/automotive#SolidBrokenYellow">
        <rdfs:subClassOf rdf:resource="http://vcd.vicomtech.org/ontology/automotive#YellowLines"/>
        <rdfs:comment>A lane marking formed by a solid and a broken line. If the line nearest to you gets broken it means you may cross the lines to overtake if it is safe.</rdfs:comment>
        <rdfs:label>Solid broken yellow</rdfs:label>
    </owl:Class>
    


    <!-- http://vcd.vicomtech.org/ontology/automotive#SolidChevronWhite -->

    <owl:Class rdf:about="http://vcd.vicomtech.org/ontology/automotive#SolidChevronWhite">
        <rdfs:subClassOf rdf:resource="http://vcd.vicomtech.org/ontology/automotive#WhiteLines"/>
        <rdfs:comment>Diagonal stripes used to separate traffic lanes or to protect traffic turning right.</rdfs:comment>
        <rdfs:label>Solid chevron white</rdfs:label>
    </owl:Class>
    


    <!-- http://vcd.vicomtech.org/ontology/automotive#SolidChevronYellow -->

    <owl:Class rdf:about="http://vcd.vicomtech.org/ontology/automotive#SolidChevronYellow">
        <rdfs:subClassOf rdf:resource="http://vcd.vicomtech.org/ontology/automotive#YellowLines"/>
        <rdfs:comment>Diagonal stripes used to separate traffic lanes or to protect traffic turning right.</rdfs:comment>
        <rdfs:label>Solid chevron yellow</rdfs:label>
    </owl:Class>
    


    <!-- http://vcd.vicomtech.org/ontology/automotive#SolidParking -->

    <owl:Class rdf:about="http://vcd.vicomtech.org/ontology/automotive#SolidParking">
        <rdfs:subClassOf rdf:resource="http://vcd.vicomtech.org/ontology/automotive#WhiteLines"/>
        <rdfs:label>Solid parking</rdfs:label>
    </owl:Class>
    


    <!-- http://vcd.vicomtech.org/ontology/automotive#SolidWhite -->

    <owl:Class rdf:about="http://vcd.vicomtech.org/ontology/automotive#SolidWhite">
        <rdfs:subClassOf rdf:resource="http://vcd.vicomtech.org/ontology/automotive#WhiteLines"/>
        <rdfs:comment>Solid line dividing two lanes. Changing lanes is not allowed.</rdfs:comment>
        <rdfs:label>Solid white</rdfs:label>
    </owl:Class>
    


    <!-- http://vcd.vicomtech.org/ontology/automotive#SolidYellow -->

    <owl:Class rdf:about="http://vcd.vicomtech.org/ontology/automotive#SolidYellow">
        <rdfs:subClassOf rdf:resource="http://vcd.vicomtech.org/ontology/automotive#YellowLines"/>
        <rdfs:comment>Solid line dividing two lanes. Indicates that changing lanes is not allowed.</rdfs:comment>
        <rdfs:label>Solid yellow</rdfs:label>
    </owl:Class>
    


    <!-- http://vcd.vicomtech.org/ontology/automotive#SpeedBumper -->

    <owl:Class rdf:about="http://vcd.vicomtech.org/ontology/automotive#SpeedBumper">
        <rdfs:subClassOf rdf:resource="http://vcd.vicomtech.org/ontology/automotive#RoadsideObject"/>
        <rdfs:comment>A small raised area built across a road to force people to drive more slowly.</rdfs:comment>
        <rdfs:label>Speed bumper</rdfs:label>
    </owl:Class>
    


    <!-- http://vcd.vicomtech.org/ontology/automotive#SplitDiamondInterchange -->

    <owl:Class rdf:about="http://vcd.vicomtech.org/ontology/automotive#SplitDiamondInterchange">
        <rdfs:subClassOf rdf:resource="http://vcd.vicomtech.org/ontology/automotive#ServiceInterchange"/>
        <rdfs:comment>A split diamond interchange has its ramps &quot;split&quot; between two crossroads, typically with an exit ramp/entrance ramp pair serving each of the crossroads. The crossroads themselves may be one-way or two-way, and are most often connected by frontage roads, usually one-way.</rdfs:comment>
        <rdfs:label>Split diamond interchange</rdfs:label>
    </owl:Class>
    


    <!-- http://vcd.vicomtech.org/ontology/automotive#SportsCar -->

    <owl:Class rdf:about="http://vcd.vicomtech.org/ontology/automotive#SportsCar">
        <rdfs:subClassOf rdf:resource="http://vcd.vicomtech.org/ontology/automotive#Car"/>
        <rdfs:comment>A sports car is designed to emphasise handling, performance or thrill of driving. Usually designed for 2 people, these car are more powerful and fast than average.</rdfs:comment>
        <rdfs:label>Sports car</rdfs:label>
    </owl:Class>
    


    <!-- http://vcd.vicomtech.org/ontology/automotive#Spray -->

    <owl:Class rdf:about="http://vcd.vicomtech.org/ontology/automotive#Spray">
        <rdfs:subClassOf rdf:resource="http://vcd.vicomtech.org/ontology/automotive#Air"/>
        <rdfs:comment>A colloidal dispersion of solid or liquid particles in a gas; smoke or fog</rdfs:comment>
        <rdfs:label>Spray</rdfs:label>
    </owl:Class>
    


    <!-- http://vcd.vicomtech.org/ontology/automotive#StackInterchange -->

    <owl:Class rdf:about="http://vcd.vicomtech.org/ontology/automotive#StackInterchange">
        <rdfs:subClassOf rdf:resource="http://vcd.vicomtech.org/ontology/automotive#FourWayInterchange"/>
        <rdfs:comment>A stack interchange is a four-way interchange whereby a semi-directional left turn and a directional right turn are both available. Usually access to both turns is provided simultaneously by a single offramp. Assuming right-handed driving, in order to cross over incoming traffic and go left, vehicles first exit onto an off-ramp from the rightmost lane. After demerging from right-turning traffic, they complete their left turn by crossing both highways on a flyover ramp or underpass. The penultimate step is a merge with the right-turn on-ramp traffic from the opposite quadrant of the interchange. Finally an onramp merges both streams of incoming traffic into the left-bound highway.</rdfs:comment>
        <rdfs:label>Stack interchange</rdfs:label>
    </owl:Class>
    


    <!-- http://vcd.vicomtech.org/ontology/automotive#Standing -->

    <owl:Class rdf:about="http://vcd.vicomtech.org/ontology/automotive#Standing">
        <rdfs:subClassOf rdf:resource="http://vcd.vicomtech.org/ontology/automotive#StationaryManeuver"/>
        <rdfs:comment>The action of being in a vertical state without moving.</rdfs:comment>
        <rdfs:label>Standing</rdfs:label>
    </owl:Class>
    


    <!-- http://vcd.vicomtech.org/ontology/automotive#Standstill -->

    <owl:Class rdf:about="http://vcd.vicomtech.org/ontology/automotive#Standstill">
        <rdfs:subClassOf rdf:resource="http://vcd.vicomtech.org/ontology/automotive#StationaryManeuver"/>
        <rdfs:comment>A situation or condition in which there is no movement or activity at all.</rdfs:comment>
        <rdfs:label>Standstill</rdfs:label>
    </owl:Class>
    


    <!-- http://vcd.vicomtech.org/ontology/automotive#Static -->

    <owl:Class rdf:about="http://vcd.vicomtech.org/ontology/automotive#Static">
        <rdfs:subClassOf rdf:resource="http://vcd.vicomtech.org/ontology/automotive#Object"/>
        <rdfs:comment>Static objects are not able to move or change by themselves.</rdfs:comment>
        <rdfs:label>Static</rdfs:label>
    </owl:Class>
    


    <!-- http://vcd.vicomtech.org/ontology/automotive#StationaryManeuver -->

    <owl:Class rdf:about="http://vcd.vicomtech.org/ontology/automotive#StationaryManeuver">
        <rdfs:subClassOf rdf:resource="http://vcd.vicomtech.org/ontology/automotive#Action"/>
        <rdfs:comment>A static maneuver performed with the aim of maintaining the current state or position of the object.</rdfs:comment>
        <rdfs:label>Stationary maneuver</rdfs:label>
    </owl:Class>
    


    <!-- http://vcd.vicomtech.org/ontology/automotive#Stopped -->

    <owl:Class rdf:about="http://vcd.vicomtech.org/ontology/automotive#Stopped">
        <rdfs:subClassOf rdf:resource="http://vcd.vicomtech.org/ontology/automotive#StationaryManeuver"/>
        <rdfs:comment>The action of not moving at all. In the case of a vehicle implies having the engine turned off.</rdfs:comment>
        <rdfs:label>Stopped</rdfs:label>
    </owl:Class>
    


    <!-- http://vcd.vicomtech.org/ontology/automotive#Stopping -->

    <owl:Class rdf:about="http://vcd.vicomtech.org/ontology/automotive#Stopping">
        <rdfs:subClassOf rdf:resource="http://vcd.vicomtech.org/ontology/automotive#MovingManeuver"/>
        <rdfs:comment>The act of stopping occurs when a subject starts deccelerating until being stationary.</rdfs:comment>
        <rdfs:label>Stopping</rdfs:label>
    </owl:Class>
    


    <!-- http://vcd.vicomtech.org/ontology/automotive#Storm -->

    <owl:Class rdf:about="http://vcd.vicomtech.org/ontology/automotive#Storm">
        <rdfs:subClassOf rdf:resource="http://vcd.vicomtech.org/ontology/automotive#Weather"/>
        <rdfs:comment>Characterized by strong winds and usually rain, thunder, lightning, or snow.</rdfs:comment>
        <rdfs:label>Storm</rdfs:label>
    </owl:Class>
    


    <!-- http://vcd.vicomtech.org/ontology/automotive#StreetLight -->

    <owl:Class rdf:about="http://vcd.vicomtech.org/ontology/automotive#StreetLight">
        <rdfs:subClassOf rdf:resource="http://vcd.vicomtech.org/ontology/automotive#RoadsideObject"/>
        <rdfs:comment>Lights mounted on poles to illuminate the road or public places.</rdfs:comment>
        <rdfs:label>Street light</rdfs:label>
    </owl:Class>
    


    <!-- http://vcd.vicomtech.org/ontology/automotive#StreetLights -->

    <owl:Class rdf:about="http://vcd.vicomtech.org/ontology/automotive#StreetLights">
        <rdfs:subClassOf rdf:resource="http://vcd.vicomtech.org/ontology/automotive#ArtificialLighting"/>
        <rdfs:comment>Street Lights are used to light roadways and walkways at night.</rdfs:comment>
        <rdfs:label>Street lights</rdfs:label>
    </owl:Class>
    


    <!-- http://vcd.vicomtech.org/ontology/automotive#StreetOperationsVehicle -->

    <owl:Class rdf:about="http://vcd.vicomtech.org/ontology/automotive#StreetOperationsVehicle">
        <rdfs:subClassOf rdf:resource="http://vcd.vicomtech.org/ontology/automotive#DrivableVehicle"/>
        <rdfs:comment>Street operations vehicles are vehicles, usually larger than regular passenger cars, whose primary function is to carry out tasks related to road maintenance (non cosntruction), postal and trash services. These vehicles are normally characterized by a stop-and-go behavior and can have people operators jumping on and off to carry out tasks in the proximity of the vehicle.</rdfs:comment>
        <rdfs:label>Street operations vehicle</rdfs:label>
    </owl:Class>
    


    <!-- http://vcd.vicomtech.org/ontology/automotive#StreetSweeper -->

    <owl:Class rdf:about="http://vcd.vicomtech.org/ontology/automotive#StreetSweeper">
        <rdfs:subClassOf rdf:resource="http://vcd.vicomtech.org/ontology/automotive#StreetOperationsVehicle"/>
        <rdfs:comment>A vehicle designed to clean streets, usually equipped with big rotating brushes and other cleaning equipment. Characterized by low speed when in active operations and proximity to sidewalks.</rdfs:comment>
        <rdfs:label>Street sweeper</rdfs:label>
    </owl:Class>
    


    <!-- http://vcd.vicomtech.org/ontology/automotive#Stroller -->

    <owl:Class rdf:about="http://vcd.vicomtech.org/ontology/automotive#Stroller">
        <rdfs:subClassOf rdf:resource="http://vcd.vicomtech.org/ontology/automotive#PushablePullable"/>
        <rdfs:comment>A chair on wheels, typically folding, in which a baby or young child can be pushed along; a pushchair.</rdfs:comment>
        <rdfs:label>Stroller</rdfs:label>
    </owl:Class>
    


    <!-- http://vcd.vicomtech.org/ontology/automotive#Structure -->

    <owl:Class rdf:about="http://vcd.vicomtech.org/ontology/automotive#Structure">
        <rdfs:subClassOf rdf:resource="http://vcd.vicomtech.org/ontology/automotive#Construction"/>
        <rdfs:comment>A building or other object constructed from several parts.</rdfs:comment>
        <rdfs:label>Structure</rdfs:label>
    </owl:Class>
    


    <!-- http://vcd.vicomtech.org/ontology/automotive#Subway -->

    <owl:Class rdf:about="http://vcd.vicomtech.org/ontology/automotive#Subway">
        <rdfs:subClassOf rdf:resource="http://vcd.vicomtech.org/ontology/automotive#RailborneVehicle"/>
        <rdfs:comment>A passenger vehicle powered by electricity conveyed by overhead cables, or additional power track, and running on rails laid underground.</rdfs:comment>
        <rdfs:label>Subway</rdfs:label>
    </owl:Class>
    


    <!-- http://vcd.vicomtech.org/ontology/automotive#Sun -->

    <owl:Class rdf:about="http://vcd.vicomtech.org/ontology/automotive#Sun">
        <rdfs:subClassOf rdf:resource="http://vcd.vicomtech.org/ontology/automotive#Weather"/>
        <rdfs:comment>Bright with sunlight.</rdfs:comment>
        <rdfs:label>Sun</rdfs:label>
    </owl:Class>
    


    <!-- http://vcd.vicomtech.org/ontology/automotive#Sunny -->

    <owl:Class rdf:about="http://vcd.vicomtech.org/ontology/automotive#Sunny">
        <rdfs:subClassOf rdf:resource="http://vcd.vicomtech.org/ontology/automotive#DirectSunlight"/>
        <rdfs:subClassOf rdf:resource="http://vcd.vicomtech.org/ontology/automotive#Weather"/>
        <rdfs:comment>Bright with sunlight.</rdfs:comment>
        <rdfs:label>Sunny</rdfs:label>
    </owl:Class>
    


    <!-- http://vcd.vicomtech.org/ontology/automotive#Support -->

    <owl:Class rdf:about="http://vcd.vicomtech.org/ontology/automotive#Support">
        <rdfs:subClassOf rdf:resource="http://vcd.vicomtech.org/ontology/automotive#RoadsideObject"/>
        <rdfs:comment>A thing that bears the weight of something or keeps ir upright.</rdfs:comment>
        <rdfs:label>Support</rdfs:label>
    </owl:Class>
    


    <!-- http://vcd.vicomtech.org/ontology/automotive#Swerve -->

    <owl:Class rdf:about="http://vcd.vicomtech.org/ontology/automotive#Swerve">
        <rdfs:subClassOf rdf:resource="http://vcd.vicomtech.org/ontology/automotive#Event"/>
        <rdfs:comment>To suddenly change direction.</rdfs:comment>
        <rdfs:label>Swerve</rdfs:label>
    </owl:Class>
    


    <!-- http://vcd.vicomtech.org/ontology/automotive#Swerving -->

    <owl:Class rdf:about="http://vcd.vicomtech.org/ontology/automotive#Swerving">
        <rdfs:subClassOf rdf:resource="http://vcd.vicomtech.org/ontology/automotive#MovingManeuver"/>
        <rdfs:comment>When a vehicle changes direction, especially suddenly.</rdfs:comment>
        <rdfs:label>Swerving</rdfs:label>
    </owl:Class>
    


    <!-- http://vcd.vicomtech.org/ontology/automotive#SymbolRestricted -->

    <owl:Class rdf:about="http://vcd.vicomtech.org/ontology/automotive#SymbolRestricted">
        <rdfs:subClassOf rdf:resource="http://vcd.vicomtech.org/ontology/automotive#Marking"/>
        <rdfs:label>Symbol restricted</rdfs:label>
    </owl:Class>
    


    <!-- http://vcd.vicomtech.org/ontology/automotive#SystemInterchange -->

    <owl:Class rdf:about="http://vcd.vicomtech.org/ontology/automotive#SystemInterchange">
        <rdfs:subClassOf rdf:resource="http://vcd.vicomtech.org/ontology/automotive#Interchange"/>
        <rdfs:comment>These interchanges are between two roads with access control.</rdfs:comment>
        <rdfs:label>System interchange</rdfs:label>
    </owl:Class>
    


    <!-- http://vcd.vicomtech.org/ontology/automotive#TBoneInterchange -->

    <owl:Class rdf:about="http://vcd.vicomtech.org/ontology/automotive#TBoneInterchange">
        <rdfs:subClassOf rdf:resource="http://vcd.vicomtech.org/ontology/automotive#HybridInterchange"/>
        <rdfs:comment>A T-bone interchange is essentially a compacted directional T interchange with sharper turns and a lower capacity, built when there is insufficient land or funds to build a directional T. Its two flyover/flyunder ramps contract together after passing over the through highway, but then they split into two segments, resembling the bone in a T-bone steak.</rdfs:comment>
        <rdfs:label>T-bone interchange</rdfs:label>
    </owl:Class>
    


    <!-- http://vcd.vicomtech.org/ontology/automotive#Temperature -->

    <owl:Class rdf:about="http://vcd.vicomtech.org/ontology/automotive#Temperature">
        <rdfs:subClassOf rdf:resource="http://vcd.vicomtech.org/ontology/automotive#Meteorology"/>
        <rdfs:comment>The degree or intensity of heat present in a substance or object, especially as expressed according to a comparative scale and shown by a thermometer or perceived by touch.</rdfs:comment>
        <rdfs:label>Temperature</rdfs:label>
    </owl:Class>
    


    <!-- http://vcd.vicomtech.org/ontology/automotive#Terrain -->

    <owl:Class rdf:about="http://vcd.vicomtech.org/ontology/automotive#Terrain">
        <rdfs:subClassOf rdf:resource="http://vcd.vicomtech.org/ontology/automotive#Nature"/>
        <rdfs:comment>Grass and all other types of horizontal spreading vegetation, includes soil.</rdfs:comment>
        <rdfs:label>Terrain</rdfs:label>
    </owl:Class>
    


    <!-- http://vcd.vicomtech.org/ontology/automotive#ThreeLevelDiamondInterchange -->

    <owl:Class rdf:about="http://vcd.vicomtech.org/ontology/automotive#ThreeLevelDiamondInterchange">
        <rdfs:subClassOf rdf:resource="http://vcd.vicomtech.org/ontology/automotive#HybridServiceInterchange"/>
        <rdfs:comment>In a three-level diamond interchange, the cross street is built in a third level with free flowing traffic as a second arterial road. The intersection is split up into four intersections, handling just two conflicting directions each.</rdfs:comment>
        <rdfs:label>Three-level diamond interchange</rdfs:label>
    </owl:Class>
    


    <!-- http://vcd.vicomtech.org/ontology/automotive#ThreeWayInterchange -->

    <owl:Class rdf:about="http://vcd.vicomtech.org/ontology/automotive#ThreeWayInterchange">
        <rdfs:subClassOf rdf:resource="http://vcd.vicomtech.org/ontology/automotive#SystemInterchange"/>
        <rdfs:comment>These interchanges can also be used to make a &quot;linking road&quot; to the destination for a service interchange, or the creation of a new basic road as a service interchange.</rdfs:comment>
        <rdfs:label>Three-way interchange</rdfs:label>
    </owl:Class>
    


    <!-- http://vcd.vicomtech.org/ontology/automotive#ThreeWayIntersection -->

    <owl:Class rdf:about="http://vcd.vicomtech.org/ontology/automotive#ThreeWayIntersection">
        <rdfs:subClassOf rdf:resource="http://vcd.vicomtech.org/ontology/automotive#RoadSegments"/>
        <rdfs:comment>Is a junction between three road segments (arms): a T junction when two arms form one road, or a Y junction, the latter also known as a fork if approached from the stem of the Y.</rdfs:comment>
        <rdfs:label>Three-way intersection</rdfs:label>
    </owl:Class>
    


    <!-- http://vcd.vicomtech.org/ontology/automotive#TightDiamondInterchange -->

    <owl:Class rdf:about="http://vcd.vicomtech.org/ontology/automotive#TightDiamondInterchange">
        <rdfs:subClassOf rdf:resource="http://vcd.vicomtech.org/ontology/automotive#ServiceInterchange"/>
        <rdfs:comment>Also known as a compressed diamond interchange or a tight urban diamond interchange (TUDI), is sometimes used in areas where there is insufficient right-of-way for a standard diamond interchange. The pair of intersections where the ramps meet the minor road are closely spaced. This spacing forces the turn lanes for each direction to run beside each other, causing the minor road to be wider than it would be if it were a standard diamond.</rdfs:comment>
        <rdfs:label>Tight diamond interchange</rdfs:label>
    </owl:Class>
    


    <!-- http://vcd.vicomtech.org/ontology/automotive#TimeOfDay -->

    <owl:Class rdf:about="http://vcd.vicomtech.org/ontology/automotive#TimeOfDay">
        <rdfs:subClassOf rdf:resource="http://vcd.vicomtech.org/ontology/automotive#Context"/>
        <rdfs:comment>A loosely specified period of time, minutes or hours in duration, especially daytime, or point in time.</rdfs:comment>
        <rdfs:label>Time-of-day</rdfs:label>
    </owl:Class>
    


    <!-- http://vcd.vicomtech.org/ontology/automotive#TowTruck -->

    <owl:Class rdf:about="http://vcd.vicomtech.org/ontology/automotive#TowTruck">
        <rdfs:subClassOf rdf:resource="http://vcd.vicomtech.org/ontology/automotive#LargeVehicle"/>
        <rdfs:comment>A motor vehicle equipped for towing away wrecked or disabled cars.</rdfs:comment>
        <rdfs:label>Tow Truck</rdfs:label>
    </owl:Class>
    


    <!-- http://vcd.vicomtech.org/ontology/automotive#TowedVehicle -->

    <owl:Class rdf:about="http://vcd.vicomtech.org/ontology/automotive#TowedVehicle">
        <rdfs:subClassOf rdf:resource="http://vcd.vicomtech.org/ontology/automotive#Trailer"/>
        <rdfs:comment>Any vehicle that is not self-propelled but instead is being towed by another motorized vehicle.</rdfs:comment>
        <rdfs:label>Towed Vehicle</rdfs:label>
    </owl:Class>
    


    <!-- http://vcd.vicomtech.org/ontology/automotive#Town -->

    <owl:Class rdf:about="http://vcd.vicomtech.org/ontology/automotive#Town">
        <rdfs:subClassOf rdf:resource="http://vcd.vicomtech.org/ontology/automotive#Environment"/>
        <rdfs:comment>A built-up area with a name, defined boundaries, and local government, that is larger than a village and generally smaller than a city.</rdfs:comment>
        <rdfs:label>Town</rdfs:label>
    </owl:Class>
    


    <!-- http://vcd.vicomtech.org/ontology/automotive#Tractor -->

    <owl:Class rdf:about="http://vcd.vicomtech.org/ontology/automotive#Tractor">
        <rdfs:subClassOf rdf:resource="http://vcd.vicomtech.org/ontology/automotive#AgriculturalVehicle"/>
        <rdfs:comment>A powerful motor vehicle with large rear wheels, used chiefly on farms for hauling equipment and trailers.</rdfs:comment>
        <rdfs:label>Tractor</rdfs:label>
    </owl:Class>
    


    <!-- http://vcd.vicomtech.org/ontology/automotive#TrafficCone -->

    <owl:Class rdf:about="http://vcd.vicomtech.org/ontology/automotive#TrafficCone">
        <rdfs:subClassOf rdf:resource="http://vcd.vicomtech.org/ontology/automotive#TrafficDevice"/>
        <rdfs:comment>A solid or hollow object which tapers from a circular or roughly circular base to a point.</rdfs:comment>
        <rdfs:label>Traffic cone</rdfs:label>
    </owl:Class>
    


    <!-- http://vcd.vicomtech.org/ontology/automotive#TrafficControls -->

    <owl:Class rdf:about="http://vcd.vicomtech.org/ontology/automotive#TrafficControls">
        <rdfs:subClassOf rdf:resource="http://vcd.vicomtech.org/ontology/automotive#Intersection"/>
        <rdfs:label>Traffic controls</rdfs:label>
    </owl:Class>
    


    <!-- http://vcd.vicomtech.org/ontology/automotive#TrafficDevice -->

    <owl:Class rdf:about="http://vcd.vicomtech.org/ontology/automotive#TrafficDevice">
        <rdfs:subClassOf rdf:resource="http://vcd.vicomtech.org/ontology/automotive#RoadObstacles"/>
        <rdfs:comment>All signs, signals, markings or devices placed for the purpose of regulating, warning or guiding traffic.</rdfs:comment>
        <rdfs:label>Traffic device</rdfs:label>
    </owl:Class>
    


    <!-- http://vcd.vicomtech.org/ontology/automotive#TrafficIsland -->

    <owl:Class rdf:about="http://vcd.vicomtech.org/ontology/automotive#TrafficIsland">
        <rdfs:subClassOf rdf:resource="http://vcd.vicomtech.org/ontology/automotive#Flat"/>
        <rdfs:comment>A small raised area in the middle of a road which provides a safe place for pedestrians to stand and marks a division between two opposing streams of traffic.</rdfs:comment>
        <rdfs:label>Traffic island</rdfs:label>
    </owl:Class>
    


    <!-- http://vcd.vicomtech.org/ontology/automotive#TrafficLane -->

    <owl:Class rdf:about="http://vcd.vicomtech.org/ontology/automotive#TrafficLane">
        <rdfs:subClassOf rdf:resource="http://vcd.vicomtech.org/ontology/automotive#Lane"/>
        <rdfs:comment>Traffic stream marked off on a road.</rdfs:comment>
        <rdfs:label>Traffic lane</rdfs:label>
    </owl:Class>
    


    <!-- http://vcd.vicomtech.org/ontology/automotive#TrafficLight -->

    <owl:Class rdf:about="http://vcd.vicomtech.org/ontology/automotive#TrafficLight">
        <rdfs:subClassOf rdf:resource="http://vcd.vicomtech.org/ontology/automotive#Signs"/>
        <rdfs:comment>Traffic lights without poles in different orientations and for all types or traffic participants.</rdfs:comment>
        <rdfs:label>Traffic light</rdfs:label>
    </owl:Class>
    


    <!-- http://vcd.vicomtech.org/ontology/automotive#TrafficSign -->

    <owl:Class rdf:about="http://vcd.vicomtech.org/ontology/automotive#TrafficSign">
        <rdfs:subClassOf rdf:resource="http://vcd.vicomtech.org/ontology/automotive#Signs"/>
        <rdfs:comment>Signs with the purpose of conveying information to drivers/cyclistspedestrians.</rdfs:comment>
        <rdfs:label>Traffic sign</rdfs:label>
    </owl:Class>
    


    <!-- http://vcd.vicomtech.org/ontology/automotive#TrafficSignSupport -->

    <owl:Class rdf:about="http://vcd.vicomtech.org/ontology/automotive#TrafficSignSupport">
        <rdfs:subClassOf rdf:resource="http://vcd.vicomtech.org/ontology/automotive#Support"/>
        <rdfs:comment>Frame construction holding large signs, where frame can be made of round or square poles. Can be typically found on highways.</rdfs:comment>
        <rdfs:label>Traffic sign support</rdfs:label>
    </owl:Class>
    


    <!-- http://vcd.vicomtech.org/ontology/automotive#TrafficSignaler -->

    <owl:Class rdf:about="http://vcd.vicomtech.org/ontology/automotive#TrafficSignaler">
        <rdfs:subClassOf rdf:resource="http://vcd.vicomtech.org/ontology/automotive#Adult"/>
        <rdfs:comment>A person who is actively managing traffic through signaling and nothing can be said about his/her legitimacy in doing so</rdfs:comment>
        <rdfs:label>Traffic signaler</rdfs:label>
    </owl:Class>
    


    <!-- http://vcd.vicomtech.org/ontology/automotive#TrafficViolation -->

    <owl:Class rdf:about="http://vcd.vicomtech.org/ontology/automotive#TrafficViolation">
        <rdfs:subClassOf rdf:resource="http://vcd.vicomtech.org/ontology/automotive#MovingManeuver"/>
        <rdfs:comment>Any action that does not respect the traffic laws.</rdfs:comment>
        <rdfs:label>Traffic violation</rdfs:label>
    </owl:Class>
    


    <!-- http://vcd.vicomtech.org/ontology/automotive#Trailer -->

    <owl:Class rdf:about="http://vcd.vicomtech.org/ontology/automotive#Trailer">
        <rdfs:subClassOf rdf:resource="http://vcd.vicomtech.org/ontology/automotive#RoadVehicle"/>
        <rdfs:comment>An unpowered vehicle towed by another. Excluded trailers attached to trucks, which belongs to class truck.</rdfs:comment>
        <rdfs:label>Trailer</rdfs:label>
    </owl:Class>
    


    <!-- http://vcd.vicomtech.org/ontology/automotive#Train -->

    <owl:Class rdf:about="http://vcd.vicomtech.org/ontology/automotive#Train">
        <rdfs:subClassOf rdf:resource="http://vcd.vicomtech.org/ontology/automotive#RailborneVehicle"/>
        <rdfs:comment>A series of connected railway carriages or wagons moved by a locomotive or by integral motors.</rdfs:comment>
        <rdfs:label>Train</rdfs:label>
    </owl:Class>
    


    <!-- http://vcd.vicomtech.org/ontology/automotive#Tram -->

    <owl:Class rdf:about="http://vcd.vicomtech.org/ontology/automotive#Tram">
        <rdfs:subClassOf rdf:resource="http://vcd.vicomtech.org/ontology/automotive#RailborneVehicle"/>
        <rdfs:comment>A passenger vehicle powered by electricity conveyed by overhead cables, or additional power track, and running on rails laid in a public road. Usually consists of more than one wagons.</rdfs:comment>
        <rdfs:label>Tram</rdfs:label>
    </owl:Class>
    


    <!-- http://vcd.vicomtech.org/ontology/automotive#Trash -->

    <owl:Class rdf:about="http://vcd.vicomtech.org/ontology/automotive#Trash">
        <rdfs:subClassOf rdf:resource="http://vcd.vicomtech.org/ontology/automotive#RoadObstacles"/>
        <rdfs:comment>Waste material; refuse.</rdfs:comment>
        <rdfs:label>Trash</rdfs:label>
    </owl:Class>
    


    <!-- http://vcd.vicomtech.org/ontology/automotive#TrashTruck -->

    <owl:Class rdf:about="http://vcd.vicomtech.org/ontology/automotive#TrashTruck">
        <rdfs:subClassOf rdf:resource="http://vcd.vicomtech.org/ontology/automotive#StreetOperationsVehicle"/>
        <rdfs:comment>A garbage truck is a truck specially designed to collect municipal solid waste and transport it to a solid waste treatment facility, such as a landfill or transfer station. Usually have one or more human operators carrying out frequent on-offloading tasks in the proximity of the vehicle.</rdfs:comment>
        <rdfs:label>Trash Truck</rdfs:label>
    </owl:Class>
    


    <!-- http://vcd.vicomtech.org/ontology/automotive#Tree -->

    <owl:Class rdf:about="http://vcd.vicomtech.org/ontology/automotive#Tree">
        <rdfs:subClassOf rdf:resource="http://vcd.vicomtech.org/ontology/automotive#Vegetation"/>
        <rdfs:comment>A woody perennial plant, typically having a single stem or trunk growing to a considerable height and bearing lateral branches at some distance from the ground.</rdfs:comment>
        <rdfs:label>Tree</rdfs:label>
    </owl:Class>
    


    <!-- http://vcd.vicomtech.org/ontology/automotive#Tricycle -->

    <owl:Class rdf:about="http://vcd.vicomtech.org/ontology/automotive#Tricycle">
        <rdfs:subClassOf rdf:resource="http://vcd.vicomtech.org/ontology/automotive#Cycle"/>
        <rdfs:comment>A vehicle similar to a bicycle, but having three wheels, two at the back and one at the front.</rdfs:comment>
        <rdfs:label>Tricycle</rdfs:label>
    </owl:Class>
    


    <!-- http://vcd.vicomtech.org/ontology/automotive#Trike -->

    <owl:Class rdf:about="http://vcd.vicomtech.org/ontology/automotive#Trike">
        <rdfs:subClassOf rdf:resource="http://vcd.vicomtech.org/ontology/automotive#Cycle"/>
        <rdfs:comment>A modified version of a motorcycle that shares majority of design and appearance characteristics but has 2 wheels in the back and one in the front.</rdfs:comment>
        <rdfs:label>Trike</rdfs:label>
    </owl:Class>
    


    <!-- http://vcd.vicomtech.org/ontology/automotive#Truck -->

    <owl:Class rdf:about="http://vcd.vicomtech.org/ontology/automotive#Truck">
        <rdfs:subClassOf rdf:resource="http://vcd.vicomtech.org/ontology/automotive#LargeVehicle"/>
        <rdfs:comment>A large, heavy road vehicle used for carrying goods, materials or troops; a lorry.</rdfs:comment>
        <rdfs:label>Truck</rdfs:label>
    </owl:Class>
    


    <!-- http://vcd.vicomtech.org/ontology/automotive#TrumpetInterchange -->

    <owl:Class rdf:about="http://vcd.vicomtech.org/ontology/automotive#TrumpetInterchange">
        <rdfs:subClassOf rdf:resource="http://vcd.vicomtech.org/ontology/automotive#ThreeWayInterchange"/>
        <rdfs:comment>Trumpet interchanges have been used where one highway terminates at another highway. These involve at least one loop ramp connecting traffic either entering or leaving the terminating expressway with the far lanes of the continuous highway.</rdfs:comment>
        <rdfs:label>Trumpet interchange</rdfs:label>
    </owl:Class>
    


    <!-- http://vcd.vicomtech.org/ontology/automotive#Tunnel -->

    <owl:Class rdf:about="http://vcd.vicomtech.org/ontology/automotive#Tunnel">
        <rdfs:subClassOf rdf:resource="http://vcd.vicomtech.org/ontology/automotive#Structure"/>
        <rdfs:comment>An artificial underground passage, especially one built through a hill or under a building, road, or river.</rdfs:comment>
        <rdfs:label>Tunnel</rdfs:label>
    </owl:Class>
    


    <!-- http://vcd.vicomtech.org/ontology/automotive#TurbineInterchange -->

    <owl:Class rdf:about="http://vcd.vicomtech.org/ontology/automotive#TurbineInterchange">
        <rdfs:subClassOf rdf:resource="http://vcd.vicomtech.org/ontology/automotive#FourWayInterchange"/>
        <rdfs:comment>Another alternative to the four-level stack interchange is the turbine interchange (also known as a whirlpool). The turbine/whirlpool interchange requires fewer levels (usually two or three) while retaining semi-directional ramps throughout, and has its left-turning ramps sweep around the center of the interchange in a spiral pattern in right-hand traffic.</rdfs:comment>
        <rdfs:label>Turbine interchange</rdfs:label>
    </owl:Class>
    


    <!-- http://vcd.vicomtech.org/ontology/automotive#Turn -->

    <owl:Class rdf:about="http://vcd.vicomtech.org/ontology/automotive#Turn">
        <rdfs:subClassOf rdf:resource="http://vcd.vicomtech.org/ontology/automotive#Event"/>
        <rdfs:comment>To move in a circular direction wholly or partly round an axis or point so that it is in a different position in relation to its surroundings or its previous position.</rdfs:comment>
        <rdfs:label>Turn</rdfs:label>
    </owl:Class>
    


    <!-- http://vcd.vicomtech.org/ontology/automotive#Turning -->

    <owl:Class rdf:about="http://vcd.vicomtech.org/ontology/automotive#Turning">
        <rdfs:subClassOf rdf:resource="http://vcd.vicomtech.org/ontology/automotive#MovingManeuver"/>
        <rdfs:comment>To move in a circular direction wholly or partly round an axis or point.</rdfs:comment>
        <rdfs:label>Turning</rdfs:label>
    </owl:Class>
    


    <!-- http://vcd.vicomtech.org/ontology/automotive#TurningLeft -->

    <owl:Class rdf:about="http://vcd.vicomtech.org/ontology/automotive#TurningLeft">
        <rdfs:subClassOf rdf:resource="http://vcd.vicomtech.org/ontology/automotive#Turning"/>
        <rdfs:comment>To move in a circular direction wholly or partly round an axis or point to the left.</rdfs:comment>
        <rdfs:label>Turning left</rdfs:label>
    </owl:Class>
    


    <!-- http://vcd.vicomtech.org/ontology/automotive#TurningRight -->

    <owl:Class rdf:about="http://vcd.vicomtech.org/ontology/automotive#TurningRight">
        <rdfs:subClassOf rdf:resource="http://vcd.vicomtech.org/ontology/automotive#Turning"/>
        <rdfs:comment>To move in a circular direction wholly or partly round an axis or point to the right.</rdfs:comment>
        <rdfs:label>Turning right</rdfs:label>
    </owl:Class>
    


    <!-- http://vcd.vicomtech.org/ontology/automotive#TwoWayInterchange -->

    <owl:Class rdf:about="http://vcd.vicomtech.org/ontology/automotive#TwoWayInterchange">
        <rdfs:subClassOf rdf:resource="http://vcd.vicomtech.org/ontology/automotive#SystemInterchange"/>
        <rdfs:label>Two-way interchange</rdfs:label>
    </owl:Class>
    


    <!-- http://vcd.vicomtech.org/ontology/automotive#UTurning -->

    <owl:Class rdf:about="http://vcd.vicomtech.org/ontology/automotive#UTurning">
        <rdfs:subClassOf rdf:resource="http://vcd.vicomtech.org/ontology/automotive#Turning"/>
        <rdfs:comment>A U-shaped turn made by a vehicle so as to head in the opposite direction from its original course.</rdfs:comment>
        <rdfs:label>uTurning</rdfs:label>
    </owl:Class>
    


    <!-- http://vcd.vicomtech.org/ontology/automotive#Unclassified -->

    <owl:Class rdf:about="http://vcd.vicomtech.org/ontology/automotive#Unclassified">
        <rdfs:subClassOf rdf:resource="http://vcd.vicomtech.org/ontology/automotive#MovingManeuver"/>
        <rdfs:subClassOf rdf:resource="http://vcd.vicomtech.org/ontology/automotive#StationaryManeuver"/>
        <rdfs:comment>An action that does not fit in any of the defined terms.</rdfs:comment>
        <rdfs:label>Unclassified</rdfs:label>
    </owl:Class>
    


    <!-- http://vcd.vicomtech.org/ontology/automotive#Unlabeled -->

    <owl:Class rdf:about="http://vcd.vicomtech.org/ontology/automotive#Unlabeled">
        <rdfs:subClassOf rdf:resource="http://vcd.vicomtech.org/ontology/automotive#Void"/>
        <rdfs:comment>An object without a defined class.</rdfs:comment>
        <rdfs:label>Unlabeled</rdfs:label>
    </owl:Class>
    


    <!-- http://vcd.vicomtech.org/ontology/automotive#UnofficialSignaler -->

    <owl:Class rdf:about="http://vcd.vicomtech.org/ontology/automotive#UnofficialSignaler">
        <rdfs:subClassOf rdf:resource="http://vcd.vicomtech.org/ontology/automotive#TrafficSignaler"/>
        <rdfs:comment>An ordinary civilian who is actively managing traffic through signaling, not wearing particular clothes or uniforms that explicit his official role</rdfs:comment>
        <rdfs:label>Unofficial Traffic signaler</rdfs:label>
    </owl:Class>
    


    <!-- http://vcd.vicomtech.org/ontology/automotive#UtilityPole -->

    <owl:Class rdf:about="http://vcd.vicomtech.org/ontology/automotive#UtilityPole">
        <rdfs:subClassOf rdf:resource="http://vcd.vicomtech.org/ontology/automotive#Support"/>
        <rdfs:comment>Utility poles are supposed to carry electrical wires/cables, could be used to mount mobile phone network receivers, and are used in case both, cables and street lights are mounted.</rdfs:comment>
        <rdfs:label>Utility pole</rdfs:label>
    </owl:Class>
    


    <!-- http://vcd.vicomtech.org/ontology/automotive#UtilityVehicle -->

    <owl:Class rdf:about="http://vcd.vicomtech.org/ontology/automotive#UtilityVehicle">
        <rdfs:subClassOf rdf:resource="http://vcd.vicomtech.org/ontology/automotive#DrivableVehicle"/>
        <rdfs:comment>A truck with low sides designed for carrying small loads.</rdfs:comment>
        <rdfs:label>Utility vehicle</rdfs:label>
    </owl:Class>
    


    <!-- http://vcd.vicomtech.org/ontology/automotive#Van -->

    <owl:Class rdf:about="http://vcd.vicomtech.org/ontology/automotive#Van">
        <rdfs:subClassOf rdf:resource="http://vcd.vicomtech.org/ontology/automotive#DrivableVehicle"/>
        <rdfs:comment>Four-wheeled motor vehicle designed for the transport of goods, with two side doors and one or two doors at the rear.</rdfs:comment>
        <rdfs:label>Van</rdfs:label>
    </owl:Class>
    


    <!-- http://vcd.vicomtech.org/ontology/automotive#Vegetation -->

    <owl:Class rdf:about="http://vcd.vicomtech.org/ontology/automotive#Vegetation">
        <rdfs:subClassOf rdf:resource="http://vcd.vicomtech.org/ontology/automotive#Nature"/>
        <rdfs:comment>Trees and other forms of vertical growing vegetation.</rdfs:comment>
        <rdfs:label>Vegetation</rdfs:label>
    </owl:Class>
    


    <!-- http://vcd.vicomtech.org/ontology/automotive#Vehicle -->

    <owl:Class rdf:about="http://vcd.vicomtech.org/ontology/automotive#Vehicle">
        <rdfs:subClassOf rdf:resource="http://vcd.vicomtech.org/ontology/automotive#Dynamic"/>
        <rdfs:comment>A Thing used for transporting people or goods.</rdfs:comment>
        <rdfs:label>Vehicle</rdfs:label>
    </owl:Class>
    


    <!-- http://vcd.vicomtech.org/ontology/automotive#Void -->

    <owl:Class rdf:about="http://vcd.vicomtech.org/ontology/automotive#Void">
        <rdfs:subClassOf rdf:resource="http://vcd.vicomtech.org/ontology/automotive#Static"/>
        <rdfs:comment>Objects that do not fit in the defined categories or too small objects that cannot be recognized.</rdfs:comment>
        <rdfs:label>Void</rdfs:label>
    </owl:Class>
    


    <!-- http://vcd.vicomtech.org/ontology/automotive#Waiting -->

    <owl:Class rdf:about="http://vcd.vicomtech.org/ontology/automotive#Waiting">
        <rdfs:subClassOf rdf:resource="http://vcd.vicomtech.org/ontology/automotive#StationaryManeuver"/>
        <rdfs:comment>The action of staying where one is or delaying action until a particular time or event.</rdfs:comment>
        <rdfs:label>Waiting</rdfs:label>
    </owl:Class>
    


    <!-- http://vcd.vicomtech.org/ontology/automotive#Walking -->

    <owl:Class rdf:about="http://vcd.vicomtech.org/ontology/automotive#Walking">
        <rdfs:subClassOf rdf:resource="http://vcd.vicomtech.org/ontology/automotive#MovingManeuver"/>
        <rdfs:comment>The action of moving at a regular pace by lifting and setting down each foot in turn.</rdfs:comment>
        <rdfs:label>Walking</rdfs:label>
    </owl:Class>
    


    <!-- http://vcd.vicomtech.org/ontology/automotive#Wall -->

    <owl:Class rdf:about="http://vcd.vicomtech.org/ontology/automotive#Wall">
        <rdfs:subClassOf rdf:resource="http://vcd.vicomtech.org/ontology/automotive#Barrier"/>
        <rdfs:comment>A continuous vertical brick or stone structure that encloses or divides an area of land.d</rdfs:comment>
        <rdfs:label>Wall</rdfs:label>
    </owl:Class>
    


    <!-- http://vcd.vicomtech.org/ontology/automotive#Water -->

    <owl:Class rdf:about="http://vcd.vicomtech.org/ontology/automotive#Water">
        <rdfs:subClassOf rdf:resource="http://vcd.vicomtech.org/ontology/automotive#Nature"/>
        <rdfs:comment>Ground surfaces covered by water.</rdfs:comment>
        <rdfs:label>Water</rdfs:label>
    </owl:Class>
    


    <!-- http://vcd.vicomtech.org/ontology/automotive#WaterVehicle -->

    <owl:Class rdf:about="http://vcd.vicomtech.org/ontology/automotive#WaterVehicle">
        <rdfs:subClassOf rdf:resource="http://vcd.vicomtech.org/ontology/automotive#Vehicle"/>
        <rdfs:comment>Vehicles used in water (Watercraft, water vessels or waterborne vessels).</rdfs:comment>
        <rdfs:label>Water vehicle</rdfs:label>
    </owl:Class>
    


    <!-- http://vcd.vicomtech.org/ontology/automotive#Weather -->

    <owl:Class rdf:about="http://vcd.vicomtech.org/ontology/automotive#Weather">
        <rdfs:subClassOf rdf:resource="http://vcd.vicomtech.org/ontology/automotive#Meteorology"/>
        <rdfs:comment>The state of the atmosphere at a particular place and time as regards heat, cloudiness, dryness, sunshine, wind, rain, etc.</rdfs:comment>
        <rdfs:label>Weather</rdfs:label>
    </owl:Class>
    


    <!-- http://vcd.vicomtech.org/ontology/automotive#Wheelchair -->

    <owl:Class rdf:about="http://vcd.vicomtech.org/ontology/automotive#Wheelchair">
        <rdfs:subClassOf rdf:resource="http://vcd.vicomtech.org/ontology/automotive#PersonalMobilityDevice"/>
        <rdfs:comment>A chair fitted with wheels for use as a means of transport by a person who is unable to walk as a result of illness, injury, or disability.</rdfs:comment>
        <rdfs:label>Wheelchair</rdfs:label>
    </owl:Class>
    


    <!-- http://vcd.vicomtech.org/ontology/automotive#WheeledSlow -->

    <owl:Class rdf:about="http://vcd.vicomtech.org/ontology/automotive#WheeledSlow">
        <rdfs:subClassOf rdf:resource="http://vcd.vicomtech.org/ontology/automotive#RoadVehicle"/>
        <rdfs:comment>Covers all slow moving wheeled objects like wheelchairs, mobility scooters, scooters, prams or rickshaw. All of which can potentially have riders sitting on them.</rdfs:comment>
        <rdfs:label>Wheeled slow</rdfs:label>
    </owl:Class>
    


    <!-- http://vcd.vicomtech.org/ontology/automotive#WhiteLines -->

    <owl:Class rdf:about="http://vcd.vicomtech.org/ontology/automotive#WhiteLines">
        <rdfs:subClassOf rdf:resource="http://vcd.vicomtech.org/ontology/automotive#LaneMarking"/>
        <rdfs:comment>White color lines that delineate the separation of traffic flows in the same direction, or mark the right edge of the pavement.</rdfs:comment>
        <rdfs:label>White lines</rdfs:label>
    </owl:Class>
    


    <!-- http://vcd.vicomtech.org/ontology/automotive#Wildlife -->

    <owl:Class rdf:about="http://vcd.vicomtech.org/ontology/automotive#Wildlife">
        <rdfs:subClassOf rdf:resource="http://vcd.vicomtech.org/ontology/automotive#Animal"/>
        <rdfs:comment>Animals that are conducting a life on their own without having an owner-pet relationship with humans. Pigs, ducks, bears, deers etc. fall under this category</rdfs:comment>
        <rdfs:label>Wildlife</rdfs:label>
    </owl:Class>
    


    <!-- http://vcd.vicomtech.org/ontology/automotive#Wind -->

    <owl:Class rdf:about="http://vcd.vicomtech.org/ontology/automotive#Wind">
        <rdfs:subClassOf rdf:resource="http://vcd.vicomtech.org/ontology/automotive#Weather"/>
        <rdfs:comment>Characterized by or exposed to strong winds.</rdfs:comment>
        <rdfs:label>Wind</rdfs:label>
    </owl:Class>
    


    <!-- http://vcd.vicomtech.org/ontology/automotive#WindmillInterchange -->

    <owl:Class rdf:about="http://vcd.vicomtech.org/ontology/automotive#WindmillInterchange">
        <rdfs:subClassOf rdf:resource="http://vcd.vicomtech.org/ontology/automotive#FourWayInterchange"/>
        <rdfs:comment>A windmill interchange is similar to a turbine interchange, but it has much sharper turns, reducing its size and capacity. The interchange is named for its similar overhead appearance to the blades of a windmill.</rdfs:comment>
        <rdfs:label>Windmill interchange</rdfs:label>
    </owl:Class>
    


    <!-- http://vcd.vicomtech.org/ontology/automotive#YInterchange -->

    <owl:Class rdf:about="http://vcd.vicomtech.org/ontology/automotive#YInterchange">
        <rdfs:subClassOf rdf:resource="http://vcd.vicomtech.org/ontology/automotive#ThreeWayInterchange"/>
        <rdfs:comment>A full Y-interchange (also known as a directional T interchange) is typically used when a three-way interchange is required for two or three highways interchanging in semi-parallel/perpendicular directions, but it can also be used in right-angle case as well. Their connecting ramps can spur from either the right or left side of the highway, depending on the direction of travel and the angle.</rdfs:comment>
        <rdfs:label>Y interchange</rdfs:label>
    </owl:Class>
    


    <!-- http://vcd.vicomtech.org/ontology/automotive#YellowLines -->

    <owl:Class rdf:about="http://vcd.vicomtech.org/ontology/automotive#YellowLines">
        <rdfs:subClassOf rdf:resource="http://vcd.vicomtech.org/ontology/automotive#LaneMarking"/>
        <rdfs:comment>Yellow markings that delineate the separation of traffic flows in opposing directions, or mark the left edge of the pavement of divided highways and one-way roads.</rdfs:comment>
        <rdfs:label>Yellow lines</rdfs:label>
    </owl:Class>
    


    <!-- http://vcd.vicomtech.org/ontology/automotive#ZigZag -->

    <owl:Class rdf:about="http://vcd.vicomtech.org/ontology/automotive#ZigZag">
        <rdfs:subClassOf rdf:resource="http://vcd.vicomtech.org/ontology/automotive#Marking"/>
        <rdfs:label>Zig-zag</rdfs:label>
    </owl:Class>
    <rdf:Description>
        <owl:topDataProperty rdf:datatype="http://www.w3.org/2001/XMLSchema#double"></owl:topDataProperty>
    </rdf:Description>
    


    <!-- 
    ///////////////////////////////////////////////////////////////////////////////////////
    //
    // General axioms
    //
    ///////////////////////////////////////////////////////////////////////////////////////
     -->

    <rdf:Description>
        <rdf:type rdf:resource="http://www.w3.org/2002/07/owl#AllDisjointClasses"/>
        <owl:members rdf:parseType="Collection">
            <rdf:Description rdf:about="http://vcd.vicomtech.org/ontology/automotive#AmbulanceTruck"/>
            <rdf:Description rdf:about="http://vcd.vicomtech.org/ontology/automotive#FireTruck"/>
            <rdf:Description rdf:about="http://vcd.vicomtech.org/ontology/automotive#MilitaryTruck"/>
            <rdf:Description rdf:about="http://vcd.vicomtech.org/ontology/automotive#PoliceTruck"/>
        </owl:members>
    </rdf:Description>
    


    <!-- 
    ///////////////////////////////////////////////////////////////////////////////////////
    //
    // Rules
    //
    ///////////////////////////////////////////////////////////////////////////////////////
     -->

    <rdf:Description rdf:about="http://vcd.vicomtech.org/ontology/automotive#x">
        <rdf:type rdf:resource="http://www.w3.org/2003/11/swrl#Variable"/>
    </rdf:Description>
    <rdf:Description rdf:about="http://vcd.vicomtech.org/ontology/automotive#y">
        <rdf:type rdf:resource="http://www.w3.org/2003/11/swrl#Variable"/>
    </rdf:Description>
    <rdf:Description rdf:about="http://vcd.vicomtech.org/ontology/automotive#dx">
        <rdf:type rdf:resource="http://www.w3.org/2003/11/swrl#Variable"/>
    </rdf:Description>
    <rdf:Description rdf:about="http://vcd.vicomtech.org/ontology/automotive#dy">
        <rdf:type rdf:resource="http://www.w3.org/2003/11/swrl#Variable"/>
    </rdf:Description>
    <rdf:Description rdf:about="http://vcd.vicomtech.org/ontology/automotive#l">
        <rdf:type rdf:resource="http://www.w3.org/2003/11/swrl#Variable"/>
    </rdf:Description>
    <rdf:Description rdf:about="http://vcd.vicomtech.org/ontology/automotive#fa">
        <rdf:type rdf:resource="http://www.w3.org/2003/11/swrl#Variable"/>
    </rdf:Description>
    <rdf:Description rdf:about="http://vcd.vicomtech.org/ontology/automotive#f">
        <rdf:type rdf:resource="http://www.w3.org/2003/11/swrl#Variable"/>
    </rdf:Description>
    <rdf:Description rdf:about="http://vcd.vicomtech.org/ontology/automotive#a">
        <rdf:type rdf:resource="http://www.w3.org/2003/11/swrl#Variable"/>
    </rdf:Description>
    <rdf:Description rdf:about="http://vcd.vicomtech.org/ontology/automotive#oa">
        <rdf:type rdf:resource="http://www.w3.org/2003/11/swrl#Variable"/>
    </rdf:Description>
    <rdf:Description rdf:about="http://vcd.vicomtech.org/ontology/automotive#sx">
        <rdf:type rdf:resource="http://www.w3.org/2003/11/swrl#Variable"/>
    </rdf:Description>
    <rdf:Description rdf:about="http://vcd.vicomtech.org/ontology/automotive#sy">
        <rdf:type rdf:resource="http://www.w3.org/2003/11/swrl#Variable"/>
    </rdf:Description>
    <rdf:Description rdf:about="http://vcd.vicomtech.org/ontology/automotive#pe">
        <rdf:type rdf:resource="http://www.w3.org/2003/11/swrl#Variable"/>
    </rdf:Description>
    <rdf:Description rdf:about="http://vcd.vicomtech.org/ontology/automotive#pa">
        <rdf:type rdf:resource="http://www.w3.org/2003/11/swrl#Variable"/>
    </rdf:Description>
    <rdf:Description rdf:about="http://vcd.vicomtech.org/ontology/automotive#z">
        <rdf:type rdf:resource="http://www.w3.org/2003/11/swrl#Variable"/>
    </rdf:Description>
    <rdf:Description>
        <swrla:isRuleEnabled rdf:datatype="http://www.w3.org/2001/XMLSchema#boolean">true</swrla:isRuleEnabled>
        <rdfs:comment rdf:datatype="http://www.w3.org/2001/XMLSchema#string">If vehicle X is performing a pass event where Y is the object, then X is moving faster than Y.</rdfs:comment>
        <rdfs:label rdf:datatype="http://www.w3.org/2001/XMLSchema#string">S12</rdfs:label>
        <rdf:type rdf:resource="http://www.w3.org/2003/11/swrl#Imp"/>
        <swrl:body>
            <rdf:Description>
                <rdf:type rdf:resource="http://www.w3.org/2003/11/swrl#AtomList"/>
                <rdf:first>
                    <rdf:Description>
                        <rdf:type rdf:resource="http://www.w3.org/2003/11/swrl#ClassAtom"/>
                        <swrl:classPredicate rdf:resource="http://vcd.vicomtech.org/ontology/automotive#Pass"/>
                        <swrl:argument1 rdf:resource="http://vcd.vicomtech.org/ontology/automotive#pe"/>
                    </rdf:Description>
                </rdf:first>
                <rdf:rest>
                    <rdf:Description>
                        <rdf:type rdf:resource="http://www.w3.org/2003/11/swrl#AtomList"/>
                        <rdf:first>
                            <rdf:Description>
                                <rdf:type rdf:resource="http://www.w3.org/2003/11/swrl#IndividualPropertyAtom"/>
                                <swrl:propertyPredicate rdf:resource="http://vcd.vicomtech.org/ontology/automotive#isSubjectOfAction"/>
                                <swrl:argument1 rdf:resource="http://vcd.vicomtech.org/ontology/automotive#pe"/>
                                <swrl:argument2 rdf:resource="http://vcd.vicomtech.org/ontology/automotive#x"/>
                            </rdf:Description>
                        </rdf:first>
                        <rdf:rest>
                            <rdf:Description>
                                <rdf:type rdf:resource="http://www.w3.org/2003/11/swrl#AtomList"/>
                                <rdf:first>
                                    <rdf:Description>
                                        <rdf:type rdf:resource="http://www.w3.org/2003/11/swrl#IndividualPropertyAtom"/>
                                        <swrl:propertyPredicate rdf:resource="http://vcd.vicomtech.org/ontology/automotive#isObjectOfAction"/>
                                        <swrl:argument1 rdf:resource="http://vcd.vicomtech.org/ontology/automotive#pe"/>
                                        <swrl:argument2 rdf:resource="http://vcd.vicomtech.org/ontology/automotive#y"/>
                                    </rdf:Description>
                                </rdf:first>
                                <rdf:rest>
                                    <rdf:Description>
                                        <rdf:type rdf:resource="http://www.w3.org/2003/11/swrl#AtomList"/>
                                        <rdf:first>
                                            <rdf:Description>
                                                <rdf:type rdf:resource="http://www.w3.org/2003/11/swrl#ClassAtom"/>
                                                <swrl:classPredicate rdf:resource="http://vcd.vicomtech.org/ontology/automotive#Vehicle"/>
                                                <swrl:argument1 rdf:resource="http://vcd.vicomtech.org/ontology/automotive#x"/>
                                            </rdf:Description>
                                        </rdf:first>
                                        <rdf:rest>
                                            <rdf:Description>
                                                <rdf:type rdf:resource="http://www.w3.org/2003/11/swrl#AtomList"/>
                                                <rdf:first>
                                                    <rdf:Description>
                                                        <rdf:type rdf:resource="http://www.w3.org/2003/11/swrl#ClassAtom"/>
                                                        <swrl:classPredicate rdf:resource="http://vcd.vicomtech.org/ontology/automotive#Vehicle"/>
                                                        <swrl:argument1 rdf:resource="http://vcd.vicomtech.org/ontology/automotive#y"/>
                                                    </rdf:Description>
                                                </rdf:first>
                                                <rdf:rest>
                                                    <rdf:Description>
                                                        <rdf:type rdf:resource="http://www.w3.org/2003/11/swrl#AtomList"/>
                                                        <rdf:first>
                                                            <rdf:Description>
                                                                <rdf:type rdf:resource="http://www.w3.org/2003/11/swrl#DatavaluedPropertyAtom"/>
                                                                <swrl:propertyPredicate rdf:resource="http://vcd.vicomtech.org/ontology/automotive#hasSpeed"/>
                                                                <swrl:argument1 rdf:resource="http://vcd.vicomtech.org/ontology/automotive#x"/>
                                                                <swrl:argument2 rdf:resource="http://vcd.vicomtech.org/ontology/automotive#sx"/>
                                                            </rdf:Description>
                                                        </rdf:first>
                                                        <rdf:rest>
                                                            <rdf:Description>
                                                                <rdf:type rdf:resource="http://www.w3.org/2003/11/swrl#AtomList"/>
                                                                <rdf:first>
                                                                    <rdf:Description>
                                                                        <rdf:type rdf:resource="http://www.w3.org/2003/11/swrl#DatavaluedPropertyAtom"/>
                                                                        <swrl:propertyPredicate rdf:resource="http://vcd.vicomtech.org/ontology/automotive#hasSpeed"/>
                                                                        <swrl:argument1 rdf:resource="http://vcd.vicomtech.org/ontology/automotive#y"/>
                                                                        <swrl:argument2 rdf:resource="http://vcd.vicomtech.org/ontology/automotive#sy"/>
                                                                    </rdf:Description>
                                                                </rdf:first>
                                                                <rdf:rest rdf:resource="http://www.w3.org/1999/02/22-rdf-syntax-ns#nil"/>
                                                            </rdf:Description>
                                                        </rdf:rest>
                                                    </rdf:Description>
                                                </rdf:rest>
                                            </rdf:Description>
                                        </rdf:rest>
                                    </rdf:Description>
                                </rdf:rest>
                            </rdf:Description>
                        </rdf:rest>
                    </rdf:Description>
                </rdf:rest>
            </rdf:Description>
        </swrl:body>
        <swrl:head>
            <rdf:Description>
                <rdf:type rdf:resource="http://www.w3.org/2003/11/swrl#AtomList"/>
                <rdf:first>
                    <rdf:Description>
                        <rdf:type rdf:resource="http://www.w3.org/2003/11/swrl#BuiltinAtom"/>
                        <swrl:builtin rdf:resource="http://www.w3.org/2003/11/swrlb#greaterThan"/>
                        <swrl:arguments rdf:parseType="Collection">
                            <rdf:Description rdf:about="http://vcd.vicomtech.org/ontology/automotive#sx"/>
                            <rdf:Description rdf:about="http://vcd.vicomtech.org/ontology/automotive#sy"/>
                        </swrl:arguments>
                    </rdf:Description>
                </rdf:first>
                <rdf:rest rdf:resource="http://www.w3.org/1999/02/22-rdf-syntax-ns#nil"/>
            </rdf:Description>
        </swrl:head>
    </rdf:Description>
    <rdf:Description>
        <swrla:isRuleEnabled rdf:datatype="http://www.w3.org/2001/XMLSchema#boolean">true</swrla:isRuleEnabled>
        <rdfs:comment rdf:datatype="http://www.w3.org/2001/XMLSchema#string">If X is subject and Y is the object of the pass Event, then X is behind Y.</rdfs:comment>
        <rdfs:label rdf:datatype="http://www.w3.org/2001/XMLSchema#string">S8</rdfs:label>
        <rdf:type rdf:resource="http://www.w3.org/2003/11/swrl#Imp"/>
        <swrl:body>
            <rdf:Description>
                <rdf:type rdf:resource="http://www.w3.org/2003/11/swrl#AtomList"/>
                <rdf:first>
                    <rdf:Description>
                        <rdf:type rdf:resource="http://www.w3.org/2003/11/swrl#ClassAtom"/>
                        <swrl:classPredicate rdf:resource="http://vcd.vicomtech.org/ontology/automotive#Pass"/>
                        <swrl:argument1 rdf:resource="http://vcd.vicomtech.org/ontology/automotive#pe"/>
                    </rdf:Description>
                </rdf:first>
                <rdf:rest>
                    <rdf:Description>
                        <rdf:type rdf:resource="http://www.w3.org/2003/11/swrl#AtomList"/>
                        <rdf:first>
                            <rdf:Description>
                                <rdf:type rdf:resource="http://www.w3.org/2003/11/swrl#IndividualPropertyAtom"/>
                                <swrl:propertyPredicate rdf:resource="http://vcd.vicomtech.org/ontology/automotive#isSubjectOfEvent"/>
                                <swrl:argument1 rdf:resource="http://vcd.vicomtech.org/ontology/automotive#x"/>
                                <swrl:argument2 rdf:resource="http://vcd.vicomtech.org/ontology/automotive#pe"/>
                            </rdf:Description>
                        </rdf:first>
                        <rdf:rest>
                            <rdf:Description>
                                <rdf:type rdf:resource="http://www.w3.org/2003/11/swrl#AtomList"/>
                                <rdf:first>
                                    <rdf:Description>
                                        <rdf:type rdf:resource="http://www.w3.org/2003/11/swrl#IndividualPropertyAtom"/>
                                        <swrl:propertyPredicate rdf:resource="http://vcd.vicomtech.org/ontology/automotive#isObjectOfEvent"/>
                                        <swrl:argument1 rdf:resource="http://vcd.vicomtech.org/ontology/automotive#y"/>
                                        <swrl:argument2 rdf:resource="http://vcd.vicomtech.org/ontology/automotive#pe"/>
                                    </rdf:Description>
                                </rdf:first>
                                <rdf:rest rdf:resource="http://www.w3.org/1999/02/22-rdf-syntax-ns#nil"/>
                            </rdf:Description>
                        </rdf:rest>
                    </rdf:Description>
                </rdf:rest>
            </rdf:Description>
        </swrl:body>
        <swrl:head>
            <rdf:Description>
                <rdf:type rdf:resource="http://www.w3.org/2003/11/swrl#AtomList"/>
                <rdf:first>
                    <rdf:Description>
                        <rdf:type rdf:resource="http://www.w3.org/2003/11/swrl#IndividualPropertyAtom"/>
                        <swrl:propertyPredicate rdf:resource="http://vcd.vicomtech.org/ontology/automotive#behindOf"/>
                        <swrl:argument1 rdf:resource="http://vcd.vicomtech.org/ontology/automotive#x"/>
                        <swrl:argument2 rdf:resource="http://vcd.vicomtech.org/ontology/automotive#y"/>
                    </rdf:Description>
                </rdf:first>
                <rdf:rest rdf:resource="http://www.w3.org/1999/02/22-rdf-syntax-ns#nil"/>
            </rdf:Description>
        </swrl:head>
    </rdf:Description>
    <rdf:Description>
        <swrla:isRuleEnabled rdf:datatype="http://www.w3.org/2001/XMLSchema#boolean">true</swrla:isRuleEnabled>
        <rdfs:comment rdf:datatype="http://www.w3.org/2001/XMLSchema#string">If vehicle X is passing vehicle Y, then the speed of vehicle X is greater than the speed of vehicle Y.</rdfs:comment>
        <rdfs:label rdf:datatype="http://www.w3.org/2001/XMLSchema#string">S11</rdfs:label>
        <rdf:type rdf:resource="http://www.w3.org/2003/11/swrl#Imp"/>
        <swrl:body>
            <rdf:Description>
                <rdf:type rdf:resource="http://www.w3.org/2003/11/swrl#AtomList"/>
                <rdf:first>
                    <rdf:Description>
                        <rdf:type rdf:resource="http://www.w3.org/2003/11/swrl#ClassAtom"/>
                        <swrl:classPredicate rdf:resource="http://vcd.vicomtech.org/ontology/automotive#Passing"/>
                        <swrl:argument1 rdf:resource="http://vcd.vicomtech.org/ontology/automotive#pa"/>
                    </rdf:Description>
                </rdf:first>
                <rdf:rest>
                    <rdf:Description>
                        <rdf:type rdf:resource="http://www.w3.org/2003/11/swrl#AtomList"/>
                        <rdf:first>
                            <rdf:Description>
                                <rdf:type rdf:resource="http://www.w3.org/2003/11/swrl#IndividualPropertyAtom"/>
                                <swrl:propertyPredicate rdf:resource="http://vcd.vicomtech.org/ontology/automotive#isSubjectOfAction"/>
                                <swrl:argument1 rdf:resource="http://vcd.vicomtech.org/ontology/automotive#pa"/>
                                <swrl:argument2 rdf:resource="http://vcd.vicomtech.org/ontology/automotive#x"/>
                            </rdf:Description>
                        </rdf:first>
                        <rdf:rest>
                            <rdf:Description>
                                <rdf:type rdf:resource="http://www.w3.org/2003/11/swrl#AtomList"/>
                                <rdf:first>
                                    <rdf:Description>
                                        <rdf:type rdf:resource="http://www.w3.org/2003/11/swrl#IndividualPropertyAtom"/>
                                        <swrl:propertyPredicate rdf:resource="http://vcd.vicomtech.org/ontology/automotive#isObjectOfAction"/>
                                        <swrl:argument1 rdf:resource="http://vcd.vicomtech.org/ontology/automotive#pa"/>
                                        <swrl:argument2 rdf:resource="http://vcd.vicomtech.org/ontology/automotive#y"/>
                                    </rdf:Description>
                                </rdf:first>
                                <rdf:rest>
                                    <rdf:Description>
                                        <rdf:type rdf:resource="http://www.w3.org/2003/11/swrl#AtomList"/>
                                        <rdf:first>
                                            <rdf:Description>
                                                <rdf:type rdf:resource="http://www.w3.org/2003/11/swrl#ClassAtom"/>
                                                <swrl:classPredicate rdf:resource="http://vcd.vicomtech.org/ontology/automotive#Vehicle"/>
                                                <swrl:argument1 rdf:resource="http://vcd.vicomtech.org/ontology/automotive#x"/>
                                            </rdf:Description>
                                        </rdf:first>
                                        <rdf:rest>
                                            <rdf:Description>
                                                <rdf:type rdf:resource="http://www.w3.org/2003/11/swrl#AtomList"/>
                                                <rdf:first>
                                                    <rdf:Description>
                                                        <rdf:type rdf:resource="http://www.w3.org/2003/11/swrl#ClassAtom"/>
                                                        <swrl:classPredicate rdf:resource="http://vcd.vicomtech.org/ontology/automotive#Vehicle"/>
                                                        <swrl:argument1 rdf:resource="http://vcd.vicomtech.org/ontology/automotive#y"/>
                                                    </rdf:Description>
                                                </rdf:first>
                                                <rdf:rest>
                                                    <rdf:Description>
                                                        <rdf:type rdf:resource="http://www.w3.org/2003/11/swrl#AtomList"/>
                                                        <rdf:first>
                                                            <rdf:Description>
                                                                <rdf:type rdf:resource="http://www.w3.org/2003/11/swrl#DatavaluedPropertyAtom"/>
                                                                <swrl:propertyPredicate rdf:resource="http://vcd.vicomtech.org/ontology/automotive#hasSpeed"/>
                                                                <swrl:argument1 rdf:resource="http://vcd.vicomtech.org/ontology/automotive#x"/>
                                                                <swrl:argument2 rdf:resource="http://vcd.vicomtech.org/ontology/automotive#sx"/>
                                                            </rdf:Description>
                                                        </rdf:first>
                                                        <rdf:rest>
                                                            <rdf:Description>
                                                                <rdf:type rdf:resource="http://www.w3.org/2003/11/swrl#AtomList"/>
                                                                <rdf:first>
                                                                    <rdf:Description>
                                                                        <rdf:type rdf:resource="http://www.w3.org/2003/11/swrl#DatavaluedPropertyAtom"/>
                                                                        <swrl:propertyPredicate rdf:resource="http://vcd.vicomtech.org/ontology/automotive#hasSpeed"/>
                                                                        <swrl:argument1 rdf:resource="http://vcd.vicomtech.org/ontology/automotive#y"/>
                                                                        <swrl:argument2 rdf:resource="http://vcd.vicomtech.org/ontology/automotive#sy"/>
                                                                    </rdf:Description>
                                                                </rdf:first>
                                                                <rdf:rest rdf:resource="http://www.w3.org/1999/02/22-rdf-syntax-ns#nil"/>
                                                            </rdf:Description>
                                                        </rdf:rest>
                                                    </rdf:Description>
                                                </rdf:rest>
                                            </rdf:Description>
                                        </rdf:rest>
                                    </rdf:Description>
                                </rdf:rest>
                            </rdf:Description>
                        </rdf:rest>
                    </rdf:Description>
                </rdf:rest>
            </rdf:Description>
        </swrl:body>
        <swrl:head>
            <rdf:Description>
                <rdf:type rdf:resource="http://www.w3.org/2003/11/swrl#AtomList"/>
                <rdf:first>
                    <rdf:Description>
                        <rdf:type rdf:resource="http://www.w3.org/2003/11/swrl#BuiltinAtom"/>
                        <swrl:builtin rdf:resource="http://www.w3.org/2003/11/swrlb#greaterThan"/>
                        <swrl:arguments rdf:parseType="Collection">
                            <rdf:Description rdf:about="http://vcd.vicomtech.org/ontology/automotive#sx"/>
                            <rdf:Description rdf:about="http://vcd.vicomtech.org/ontology/automotive#sy"/>
                        </swrl:arguments>
                    </rdf:Description>
                </rdf:first>
                <rdf:rest rdf:resource="http://www.w3.org/1999/02/22-rdf-syntax-ns#nil"/>
            </rdf:Description>
        </swrl:head>
    </rdf:Description>
    <rdf:Description>
        <swrla:isRuleEnabled rdf:datatype="http://www.w3.org/2001/XMLSchema#boolean">true</swrla:isRuleEnabled>
        <rdfs:comment rdf:datatype="http://www.w3.org/2001/XMLSchema#string">if Y is behind X and Z is behind Y, then Z is behind X.</rdfs:comment>
        <rdfs:label rdf:datatype="http://www.w3.org/2001/XMLSchema#string">S6</rdfs:label>
        <rdf:type rdf:resource="http://www.w3.org/2003/11/swrl#Imp"/>
        <swrl:body>
            <rdf:Description>
                <rdf:type rdf:resource="http://www.w3.org/2003/11/swrl#AtomList"/>
                <rdf:first>
                    <rdf:Description>
                        <rdf:type rdf:resource="http://www.w3.org/2003/11/swrl#IndividualPropertyAtom"/>
                        <swrl:propertyPredicate rdf:resource="http://vcd.vicomtech.org/ontology/automotive#behindOf"/>
                        <swrl:argument1 rdf:resource="http://vcd.vicomtech.org/ontology/automotive#x"/>
                        <swrl:argument2 rdf:resource="http://vcd.vicomtech.org/ontology/automotive#y"/>
                    </rdf:Description>
                </rdf:first>
                <rdf:rest>
                    <rdf:Description>
                        <rdf:type rdf:resource="http://www.w3.org/2003/11/swrl#AtomList"/>
                        <rdf:first>
                            <rdf:Description>
                                <rdf:type rdf:resource="http://www.w3.org/2003/11/swrl#IndividualPropertyAtom"/>
                                <swrl:propertyPredicate rdf:resource="http://vcd.vicomtech.org/ontology/automotive#behindOf"/>
                                <swrl:argument1 rdf:resource="http://vcd.vicomtech.org/ontology/automotive#y"/>
                                <swrl:argument2 rdf:resource="http://vcd.vicomtech.org/ontology/automotive#z"/>
                            </rdf:Description>
                        </rdf:first>
                        <rdf:rest rdf:resource="http://www.w3.org/1999/02/22-rdf-syntax-ns#nil"/>
                    </rdf:Description>
                </rdf:rest>
            </rdf:Description>
        </swrl:body>
        <swrl:head>
            <rdf:Description>
                <rdf:type rdf:resource="http://www.w3.org/2003/11/swrl#AtomList"/>
                <rdf:first>
                    <rdf:Description>
                        <rdf:type rdf:resource="http://www.w3.org/2003/11/swrl#IndividualPropertyAtom"/>
                        <swrl:propertyPredicate rdf:resource="http://vcd.vicomtech.org/ontology/automotive#behindOf"/>
                        <swrl:argument1 rdf:resource="http://vcd.vicomtech.org/ontology/automotive#x"/>
                        <swrl:argument2 rdf:resource="http://vcd.vicomtech.org/ontology/automotive#z"/>
                    </rdf:Description>
                </rdf:first>
                <rdf:rest rdf:resource="http://www.w3.org/1999/02/22-rdf-syntax-ns#nil"/>
            </rdf:Description>
        </swrl:head>
    </rdf:Description>
    <rdf:Description>
        <swrla:isRuleEnabled rdf:datatype="http://www.w3.org/2001/XMLSchema#boolean">true</swrla:isRuleEnabled>
        <rdfs:comment rdf:datatype="http://www.w3.org/2001/XMLSchema#string">if X is in front of Y and Y is in front of Z, then X is in front if Z.</rdfs:comment>
        <rdfs:label rdf:datatype="http://www.w3.org/2001/XMLSchema#string">S7</rdfs:label>
        <rdf:type rdf:resource="http://www.w3.org/2003/11/swrl#Imp"/>
        <swrl:body>
            <rdf:Description>
                <rdf:type rdf:resource="http://www.w3.org/2003/11/swrl#AtomList"/>
                <rdf:first>
                    <rdf:Description>
                        <rdf:type rdf:resource="http://www.w3.org/2003/11/swrl#IndividualPropertyAtom"/>
                        <swrl:propertyPredicate rdf:resource="http://vcd.vicomtech.org/ontology/automotive#inFrontOf"/>
                        <swrl:argument1 rdf:resource="http://vcd.vicomtech.org/ontology/automotive#x"/>
                        <swrl:argument2 rdf:resource="http://vcd.vicomtech.org/ontology/automotive#y"/>
                    </rdf:Description>
                </rdf:first>
                <rdf:rest>
                    <rdf:Description>
                        <rdf:type rdf:resource="http://www.w3.org/2003/11/swrl#AtomList"/>
                        <rdf:first>
                            <rdf:Description>
                                <rdf:type rdf:resource="http://www.w3.org/2003/11/swrl#IndividualPropertyAtom"/>
                                <swrl:propertyPredicate rdf:resource="http://vcd.vicomtech.org/ontology/automotive#inFrontOf"/>
                                <swrl:argument1 rdf:resource="http://vcd.vicomtech.org/ontology/automotive#y"/>
                                <swrl:argument2 rdf:resource="http://vcd.vicomtech.org/ontology/automotive#z"/>
                            </rdf:Description>
                        </rdf:first>
                        <rdf:rest rdf:resource="http://www.w3.org/1999/02/22-rdf-syntax-ns#nil"/>
                    </rdf:Description>
                </rdf:rest>
            </rdf:Description>
        </swrl:body>
        <swrl:head>
            <rdf:Description>
                <rdf:type rdf:resource="http://www.w3.org/2003/11/swrl#AtomList"/>
                <rdf:first>
                    <rdf:Description>
                        <rdf:type rdf:resource="http://www.w3.org/2003/11/swrl#IndividualPropertyAtom"/>
                        <swrl:propertyPredicate rdf:resource="http://vcd.vicomtech.org/ontology/automotive#inFrontOf"/>
                        <swrl:argument1 rdf:resource="http://vcd.vicomtech.org/ontology/automotive#x"/>
                        <swrl:argument2 rdf:resource="http://vcd.vicomtech.org/ontology/automotive#z"/>
                    </rdf:Description>
                </rdf:first>
                <rdf:rest rdf:resource="http://www.w3.org/1999/02/22-rdf-syntax-ns#nil"/>
            </rdf:Description>
        </swrl:head>
    </rdf:Description>
    <rdf:Description>
        <swrla:isRuleEnabled rdf:datatype="http://www.w3.org/2001/XMLSchema#boolean">true</swrla:isRuleEnabled>
        <rdfs:comment rdf:datatype="http://www.w3.org/2001/XMLSchema#string">If two vehicles (X and Y) are driving straight at the same time and vehicle X is in front of vehicle Y, then vehicle Y&apos;s driving activity is also a following activity.</rdfs:comment>
        <rdfs:label rdf:datatype="http://www.w3.org/2001/XMLSchema#string">S5</rdfs:label>
        <rdf:type rdf:resource="http://www.w3.org/2003/11/swrl#Imp"/>
        <swrl:body>
            <rdf:Description>
                <rdf:type rdf:resource="http://www.w3.org/2003/11/swrl#AtomList"/>
                <rdf:first>
                    <rdf:Description>
                        <rdf:type rdf:resource="http://www.w3.org/2003/11/swrl#ClassAtom"/>
                        <swrl:classPredicate rdf:resource="http://vcd.vicomtech.org/ontology/automotive#Vehicle"/>
                        <swrl:argument1 rdf:resource="http://vcd.vicomtech.org/ontology/automotive#x"/>
                    </rdf:Description>
                </rdf:first>
                <rdf:rest>
                    <rdf:Description>
                        <rdf:type rdf:resource="http://www.w3.org/2003/11/swrl#AtomList"/>
                        <rdf:first>
                            <rdf:Description>
                                <rdf:type rdf:resource="http://www.w3.org/2003/11/swrl#ClassAtom"/>
                                <swrl:classPredicate rdf:resource="http://vcd.vicomtech.org/ontology/automotive#Vehicle"/>
                                <swrl:argument1 rdf:resource="http://vcd.vicomtech.org/ontology/automotive#y"/>
                            </rdf:Description>
                        </rdf:first>
                        <rdf:rest>
                            <rdf:Description>
                                <rdf:type rdf:resource="http://www.w3.org/2003/11/swrl#AtomList"/>
                                <rdf:first>
                                    <rdf:Description>
                                        <rdf:type rdf:resource="http://www.w3.org/2003/11/swrl#IndividualPropertyAtom"/>
                                        <swrl:propertyPredicate rdf:resource="http://vcd.vicomtech.org/ontology/automotive#inFrontOf"/>
                                        <swrl:argument1 rdf:resource="http://vcd.vicomtech.org/ontology/automotive#x"/>
                                        <swrl:argument2 rdf:resource="http://vcd.vicomtech.org/ontology/automotive#y"/>
                                    </rdf:Description>
                                </rdf:first>
                                <rdf:rest>
                                    <rdf:Description>
                                        <rdf:type rdf:resource="http://www.w3.org/2003/11/swrl#AtomList"/>
                                        <rdf:first>
                                            <rdf:Description>
                                                <rdf:type rdf:resource="http://www.w3.org/2003/11/swrl#ClassAtom"/>
                                                <swrl:classPredicate rdf:resource="http://vcd.vicomtech.org/ontology/automotive#DrivingStraight"/>
                                                <swrl:argument1 rdf:resource="http://vcd.vicomtech.org/ontology/automotive#dx"/>
                                            </rdf:Description>
                                        </rdf:first>
                                        <rdf:rest>
                                            <rdf:Description>
                                                <rdf:type rdf:resource="http://www.w3.org/2003/11/swrl#AtomList"/>
                                                <rdf:first>
                                                    <rdf:Description>
                                                        <rdf:type rdf:resource="http://www.w3.org/2003/11/swrl#IndividualPropertyAtom"/>
                                                        <swrl:propertyPredicate rdf:resource="http://vcd.vicomtech.org/ontology/automotive#isSubjectOfAction"/>
                                                        <swrl:argument1 rdf:resource="http://vcd.vicomtech.org/ontology/automotive#x"/>
                                                        <swrl:argument2 rdf:resource="http://vcd.vicomtech.org/ontology/automotive#dx"/>
                                                    </rdf:Description>
                                                </rdf:first>
                                                <rdf:rest>
                                                    <rdf:Description>
                                                        <rdf:type rdf:resource="http://www.w3.org/2003/11/swrl#AtomList"/>
                                                        <rdf:first>
                                                            <rdf:Description>
                                                                <rdf:type rdf:resource="http://www.w3.org/2003/11/swrl#ClassAtom"/>
                                                                <swrl:classPredicate rdf:resource="http://vcd.vicomtech.org/ontology/automotive#DrivingStraight"/>
                                                                <swrl:argument1 rdf:resource="http://vcd.vicomtech.org/ontology/automotive#dy"/>
                                                            </rdf:Description>
                                                        </rdf:first>
                                                        <rdf:rest>
                                                            <rdf:Description>
                                                                <rdf:type rdf:resource="http://www.w3.org/2003/11/swrl#AtomList"/>
                                                                <rdf:first>
                                                                    <rdf:Description>
                                                                        <rdf:type rdf:resource="http://www.w3.org/2003/11/swrl#IndividualPropertyAtom"/>
                                                                        <swrl:propertyPredicate rdf:resource="http://vcd.vicomtech.org/ontology/automotive#isSubjectOfAction"/>
                                                                        <swrl:argument1 rdf:resource="http://vcd.vicomtech.org/ontology/automotive#x"/>
                                                                        <swrl:argument2 rdf:resource="http://vcd.vicomtech.org/ontology/automotive#dy"/>
                                                                    </rdf:Description>
                                                                </rdf:first>
                                                                <rdf:rest>
                                                                    <rdf:Description>
                                                                        <rdf:type rdf:resource="http://www.w3.org/2003/11/swrl#AtomList"/>
                                                                        <rdf:first>
                                                                            <rdf:Description>
                                                                                <rdf:type rdf:resource="http://www.w3.org/2003/11/swrl#DatavaluedPropertyAtom"/>
                                                                                <swrl:propertyPredicate rdf:resource="http://vcd.vicomtech.org/ontology/automotive#hasPosition"/>
                                                                                <swrl:argument1 rdf:resource="http://vcd.vicomtech.org/ontology/automotive#x"/>
                                                                                <swrl:argument2 rdf:resource="http://vcd.vicomtech.org/ontology/automotive#l"/>
                                                                            </rdf:Description>
                                                                        </rdf:first>
                                                                        <rdf:rest>
                                                                            <rdf:Description>
                                                                                <rdf:type rdf:resource="http://www.w3.org/2003/11/swrl#AtomList"/>
                                                                                <rdf:first>
                                                                                    <rdf:Description>
                                                                                        <rdf:type rdf:resource="http://www.w3.org/2003/11/swrl#DatavaluedPropertyAtom"/>
                                                                                        <swrl:propertyPredicate rdf:resource="http://vcd.vicomtech.org/ontology/automotive#hasPosition"/>
                                                                                        <swrl:argument1 rdf:resource="http://vcd.vicomtech.org/ontology/automotive#y"/>
                                                                                        <swrl:argument2 rdf:resource="http://vcd.vicomtech.org/ontology/automotive#l"/>
                                                                                    </rdf:Description>
                                                                                </rdf:first>
                                                                                <rdf:rest rdf:resource="http://www.w3.org/1999/02/22-rdf-syntax-ns#nil"/>
                                                                            </rdf:Description>
                                                                        </rdf:rest>
                                                                    </rdf:Description>
                                                                </rdf:rest>
                                                            </rdf:Description>
                                                        </rdf:rest>
                                                    </rdf:Description>
                                                </rdf:rest>
                                            </rdf:Description>
                                        </rdf:rest>
                                    </rdf:Description>
                                </rdf:rest>
                            </rdf:Description>
                        </rdf:rest>
                    </rdf:Description>
                </rdf:rest>
            </rdf:Description>
        </swrl:body>
        <swrl:head>
            <rdf:Description>
                <rdf:type rdf:resource="http://www.w3.org/2003/11/swrl#AtomList"/>
                <rdf:first>
                    <rdf:Description>
                        <rdf:type rdf:resource="http://www.w3.org/2003/11/swrl#ClassAtom"/>
                        <swrl:classPredicate rdf:resource="http://vcd.vicomtech.org/ontology/automotive#Following"/>
                        <swrl:argument1 rdf:resource="http://vcd.vicomtech.org/ontology/automotive#dy"/>
                    </rdf:Description>
                </rdf:first>
                <rdf:rest>
                    <rdf:Description>
                        <rdf:type rdf:resource="http://www.w3.org/2003/11/swrl#AtomList"/>
                        <rdf:first>
                            <rdf:Description>
                                <rdf:type rdf:resource="http://www.w3.org/2003/11/swrl#IndividualPropertyAtom"/>
                                <swrl:propertyPredicate rdf:resource="http://vcd.vicomtech.org/ontology/automotive#isObjectOfAction"/>
                                <swrl:argument1 rdf:resource="http://vcd.vicomtech.org/ontology/automotive#y"/>
                                <swrl:argument2 rdf:resource="http://vcd.vicomtech.org/ontology/automotive#dy"/>
                            </rdf:Description>
                        </rdf:first>
                        <rdf:rest rdf:resource="http://www.w3.org/1999/02/22-rdf-syntax-ns#nil"/>
                    </rdf:Description>
                </rdf:rest>
            </rdf:Description>
        </swrl:head>
    </rdf:Description>
    <rdf:Description>
        <swrla:isRuleEnabled rdf:datatype="http://www.w3.org/2001/XMLSchema#boolean">true</swrla:isRuleEnabled>
        <rdfs:comment rdf:datatype="http://www.w3.org/2001/XMLSchema#string">If vehicle X is following vehicle Y, then vehicle X is behind of vehicle Y.</rdfs:comment>
        <rdfs:label rdf:datatype="http://www.w3.org/2001/XMLSchema#string">S1</rdfs:label>
        <rdf:type rdf:resource="http://www.w3.org/2003/11/swrl#Imp"/>
        <swrl:body>
            <rdf:Description>
                <rdf:type rdf:resource="http://www.w3.org/2003/11/swrl#AtomList"/>
                <rdf:first>
                    <rdf:Description>
                        <rdf:type rdf:resource="http://www.w3.org/2003/11/swrl#ClassAtom"/>
                        <swrl:classPredicate rdf:resource="http://vcd.vicomtech.org/ontology/automotive#Following"/>
                        <swrl:argument1 rdf:resource="http://vcd.vicomtech.org/ontology/automotive#fa"/>
                    </rdf:Description>
                </rdf:first>
                <rdf:rest>
                    <rdf:Description>
                        <rdf:type rdf:resource="http://www.w3.org/2003/11/swrl#AtomList"/>
                        <rdf:first>
                            <rdf:Description>
                                <rdf:type rdf:resource="http://www.w3.org/2003/11/swrl#IndividualPropertyAtom"/>
                                <swrl:propertyPredicate rdf:resource="http://vcd.vicomtech.org/ontology/automotive#isSubjectOfAction"/>
                                <swrl:argument1 rdf:resource="http://vcd.vicomtech.org/ontology/automotive#fa"/>
                                <swrl:argument2 rdf:resource="http://vcd.vicomtech.org/ontology/automotive#x"/>
                            </rdf:Description>
                        </rdf:first>
                        <rdf:rest>
                            <rdf:Description>
                                <rdf:type rdf:resource="http://www.w3.org/2003/11/swrl#AtomList"/>
                                <rdf:first>
                                    <rdf:Description>
                                        <rdf:type rdf:resource="http://www.w3.org/2003/11/swrl#IndividualPropertyAtom"/>
                                        <swrl:propertyPredicate rdf:resource="http://vcd.vicomtech.org/ontology/automotive#isObjectOfAction"/>
                                        <swrl:argument1 rdf:resource="http://vcd.vicomtech.org/ontology/automotive#fa"/>
                                        <swrl:argument2 rdf:resource="http://vcd.vicomtech.org/ontology/automotive#y"/>
                                    </rdf:Description>
                                </rdf:first>
                                <rdf:rest rdf:resource="http://www.w3.org/1999/02/22-rdf-syntax-ns#nil"/>
                            </rdf:Description>
                        </rdf:rest>
                    </rdf:Description>
                </rdf:rest>
            </rdf:Description>
        </swrl:body>
        <swrl:head>
            <rdf:Description>
                <rdf:type rdf:resource="http://www.w3.org/2003/11/swrl#AtomList"/>
                <rdf:first>
                    <rdf:Description>
                        <rdf:type rdf:resource="http://www.w3.org/2003/11/swrl#IndividualPropertyAtom"/>
                        <swrl:propertyPredicate rdf:resource="http://vcd.vicomtech.org/ontology/automotive#behindOf"/>
                        <swrl:argument1 rdf:resource="http://vcd.vicomtech.org/ontology/automotive#x"/>
                        <swrl:argument2 rdf:resource="http://vcd.vicomtech.org/ontology/automotive#y"/>
                    </rdf:Description>
                </rdf:first>
                <rdf:rest rdf:resource="http://www.w3.org/1999/02/22-rdf-syntax-ns#nil"/>
            </rdf:Description>
        </swrl:head>
    </rdf:Description>
    <rdf:Description>
        <swrla:isRuleEnabled rdf:datatype="http://www.w3.org/2001/XMLSchema#boolean">true</swrla:isRuleEnabled>
        <rdfs:comment rdf:datatype="http://www.w3.org/2001/XMLSchema#string">If vehicle X is following vehicle Y, then vehicle Y is in front of vehicle X.</rdfs:comment>
        <rdfs:label rdf:datatype="http://www.w3.org/2001/XMLSchema#string">S2</rdfs:label>
        <rdf:type rdf:resource="http://www.w3.org/2003/11/swrl#Imp"/>
        <swrl:body>
            <rdf:Description>
                <rdf:type rdf:resource="http://www.w3.org/2003/11/swrl#AtomList"/>
                <rdf:first>
                    <rdf:Description>
                        <rdf:type rdf:resource="http://www.w3.org/2003/11/swrl#ClassAtom"/>
                        <swrl:classPredicate rdf:resource="http://vcd.vicomtech.org/ontology/automotive#Following"/>
                        <swrl:argument1 rdf:resource="http://vcd.vicomtech.org/ontology/automotive#fa"/>
                    </rdf:Description>
                </rdf:first>
                <rdf:rest>
                    <rdf:Description>
                        <rdf:type rdf:resource="http://www.w3.org/2003/11/swrl#AtomList"/>
                        <rdf:first>
                            <rdf:Description>
                                <rdf:type rdf:resource="http://www.w3.org/2003/11/swrl#IndividualPropertyAtom"/>
                                <swrl:propertyPredicate rdf:resource="http://vcd.vicomtech.org/ontology/automotive#isSubjectOfAction"/>
                                <swrl:argument1 rdf:resource="http://vcd.vicomtech.org/ontology/automotive#fa"/>
                                <swrl:argument2 rdf:resource="http://vcd.vicomtech.org/ontology/automotive#x"/>
                            </rdf:Description>
                        </rdf:first>
                        <rdf:rest>
                            <rdf:Description>
                                <rdf:type rdf:resource="http://www.w3.org/2003/11/swrl#AtomList"/>
                                <rdf:first>
                                    <rdf:Description>
                                        <rdf:type rdf:resource="http://www.w3.org/2003/11/swrl#IndividualPropertyAtom"/>
                                        <swrl:propertyPredicate rdf:resource="http://vcd.vicomtech.org/ontology/automotive#isObjectOfAction"/>
                                        <swrl:argument1 rdf:resource="http://vcd.vicomtech.org/ontology/automotive#fa"/>
                                        <swrl:argument2 rdf:resource="http://vcd.vicomtech.org/ontology/automotive#y"/>
                                    </rdf:Description>
                                </rdf:first>
                                <rdf:rest rdf:resource="http://www.w3.org/1999/02/22-rdf-syntax-ns#nil"/>
                            </rdf:Description>
                        </rdf:rest>
                    </rdf:Description>
                </rdf:rest>
            </rdf:Description>
        </swrl:body>
        <swrl:head>
            <rdf:Description>
                <rdf:type rdf:resource="http://www.w3.org/2003/11/swrl#AtomList"/>
                <rdf:first>
                    <rdf:Description>
                        <rdf:type rdf:resource="http://www.w3.org/2003/11/swrl#IndividualPropertyAtom"/>
                        <swrl:propertyPredicate rdf:resource="http://vcd.vicomtech.org/ontology/automotive#inFrontOf"/>
                        <swrl:argument1 rdf:resource="http://vcd.vicomtech.org/ontology/automotive#y"/>
                        <swrl:argument2 rdf:resource="http://vcd.vicomtech.org/ontology/automotive#x"/>
                    </rdf:Description>
                </rdf:first>
                <rdf:rest rdf:resource="http://www.w3.org/1999/02/22-rdf-syntax-ns#nil"/>
            </rdf:Description>
        </swrl:head>
    </rdf:Description>
    <rdf:Description>
        <swrla:isRuleEnabled rdf:datatype="http://www.w3.org/2001/XMLSchema#boolean">true</swrla:isRuleEnabled>
        <rdfs:comment rdf:datatype="http://www.w3.org/2001/XMLSchema#string">If X is the subject of an activity whose object is Footwalk F, then X has position  F.</rdfs:comment>
        <rdfs:label rdf:datatype="http://www.w3.org/2001/XMLSchema#string">S4</rdfs:label>
        <rdf:type rdf:resource="http://www.w3.org/2003/11/swrl#Imp"/>
        <swrl:body>
            <rdf:Description>
                <rdf:type rdf:resource="http://www.w3.org/2003/11/swrl#AtomList"/>
                <rdf:first>
                    <rdf:Description>
                        <rdf:type rdf:resource="http://www.w3.org/2003/11/swrl#IndividualPropertyAtom"/>
                        <swrl:propertyPredicate rdf:resource="http://vcd.vicomtech.org/ontology/automotive#isObjectOfAction"/>
                        <swrl:argument1 rdf:resource="http://vcd.vicomtech.org/ontology/automotive#f"/>
                        <swrl:argument2 rdf:resource="http://vcd.vicomtech.org/ontology/automotive#a"/>
                    </rdf:Description>
                </rdf:first>
                <rdf:rest>
                    <rdf:Description>
                        <rdf:type rdf:resource="http://www.w3.org/2003/11/swrl#AtomList"/>
                        <rdf:first>
                            <rdf:Description>
                                <rdf:type rdf:resource="http://www.w3.org/2003/11/swrl#IndividualPropertyAtom"/>
                                <swrl:propertyPredicate rdf:resource="http://vcd.vicomtech.org/ontology/automotive#isSubjectOfAction"/>
                                <swrl:argument1 rdf:resource="http://vcd.vicomtech.org/ontology/automotive#x"/>
                                <swrl:argument2 rdf:resource="http://vcd.vicomtech.org/ontology/automotive#a"/>
                            </rdf:Description>
                        </rdf:first>
                        <rdf:rest>
                            <rdf:Description>
                                <rdf:type rdf:resource="http://www.w3.org/2003/11/swrl#AtomList"/>
                                <rdf:first>
                                    <rdf:Description>
                                        <rdf:type rdf:resource="http://www.w3.org/2003/11/swrl#ClassAtom"/>
                                        <swrl:classPredicate rdf:resource="http://vcd.vicomtech.org/ontology/automotive#Footwalk"/>
                                        <swrl:argument1 rdf:resource="http://vcd.vicomtech.org/ontology/automotive#f"/>
                                    </rdf:Description>
                                </rdf:first>
                                <rdf:rest rdf:resource="http://www.w3.org/1999/02/22-rdf-syntax-ns#nil"/>
                            </rdf:Description>
                        </rdf:rest>
                    </rdf:Description>
                </rdf:rest>
            </rdf:Description>
        </swrl:body>
        <swrl:head>
            <rdf:Description>
                <rdf:type rdf:resource="http://www.w3.org/2003/11/swrl#AtomList"/>
                <rdf:first>
                    <rdf:Description>
                        <rdf:type rdf:resource="http://www.w3.org/2003/11/swrl#DatavaluedPropertyAtom"/>
                        <swrl:propertyPredicate rdf:resource="http://vcd.vicomtech.org/ontology/automotive#hasPosition"/>
                        <swrl:argument1 rdf:resource="http://vcd.vicomtech.org/ontology/automotive#x"/>
                        <swrl:argument2 rdf:resource="http://vcd.vicomtech.org/ontology/automotive#f"/>
                    </rdf:Description>
                </rdf:first>
                <rdf:rest rdf:resource="http://www.w3.org/1999/02/22-rdf-syntax-ns#nil"/>
            </rdf:Description>
        </swrl:head>
    </rdf:Description>
    <rdf:Description>
        <swrla:isRuleEnabled rdf:datatype="http://www.w3.org/2001/XMLSchema#boolean">true</swrla:isRuleEnabled>
        <rdfs:comment rdf:datatype="http://www.w3.org/2001/XMLSchema#string">If X is the subject of an activity whose object is lane L, then X has position L.</rdfs:comment>
        <rdfs:label rdf:datatype="http://www.w3.org/2001/XMLSchema#string">S3</rdfs:label>
        <rdf:type rdf:resource="http://www.w3.org/2003/11/swrl#Imp"/>
        <swrl:body>
            <rdf:Description>
                <rdf:type rdf:resource="http://www.w3.org/2003/11/swrl#AtomList"/>
                <rdf:first>
                    <rdf:Description>
                        <rdf:type rdf:resource="http://www.w3.org/2003/11/swrl#IndividualPropertyAtom"/>
                        <swrl:propertyPredicate rdf:resource="http://vcd.vicomtech.org/ontology/automotive#isObjectOfAction"/>
                        <swrl:argument1 rdf:resource="http://vcd.vicomtech.org/ontology/automotive#l"/>
                        <swrl:argument2 rdf:resource="http://vcd.vicomtech.org/ontology/automotive#a"/>
                    </rdf:Description>
                </rdf:first>
                <rdf:rest>
                    <rdf:Description>
                        <rdf:type rdf:resource="http://www.w3.org/2003/11/swrl#AtomList"/>
                        <rdf:first>
                            <rdf:Description>
                                <rdf:type rdf:resource="http://www.w3.org/2003/11/swrl#IndividualPropertyAtom"/>
                                <swrl:propertyPredicate rdf:resource="http://vcd.vicomtech.org/ontology/automotive#isSubjectOfAction"/>
                                <swrl:argument1 rdf:resource="http://vcd.vicomtech.org/ontology/automotive#x"/>
                                <swrl:argument2 rdf:resource="http://vcd.vicomtech.org/ontology/automotive#a"/>
                            </rdf:Description>
                        </rdf:first>
                        <rdf:rest>
                            <rdf:Description>
                                <rdf:type rdf:resource="http://www.w3.org/2003/11/swrl#AtomList"/>
                                <rdf:first>
                                    <rdf:Description>
                                        <rdf:type rdf:resource="http://www.w3.org/2003/11/swrl#ClassAtom"/>
                                        <swrl:classPredicate rdf:resource="http://vcd.vicomtech.org/ontology/automotive#Lane"/>
                                        <swrl:argument1 rdf:resource="http://vcd.vicomtech.org/ontology/automotive#l"/>
                                    </rdf:Description>
                                </rdf:first>
                                <rdf:rest rdf:resource="http://www.w3.org/1999/02/22-rdf-syntax-ns#nil"/>
                            </rdf:Description>
                        </rdf:rest>
                    </rdf:Description>
                </rdf:rest>
            </rdf:Description>
        </swrl:body>
        <swrl:head>
            <rdf:Description>
                <rdf:type rdf:resource="http://www.w3.org/2003/11/swrl#AtomList"/>
                <rdf:first>
                    <rdf:Description>
                        <rdf:type rdf:resource="http://www.w3.org/2003/11/swrl#DatavaluedPropertyAtom"/>
                        <swrl:propertyPredicate rdf:resource="http://vcd.vicomtech.org/ontology/automotive#hasPosition"/>
                        <swrl:argument1 rdf:resource="http://vcd.vicomtech.org/ontology/automotive#x"/>
                        <swrl:argument2 rdf:resource="http://vcd.vicomtech.org/ontology/automotive#l"/>
                    </rdf:Description>
                </rdf:first>
                <rdf:rest rdf:resource="http://www.w3.org/1999/02/22-rdf-syntax-ns#nil"/>
            </rdf:Description>
        </swrl:head>
    </rdf:Description>
    <rdf:Description>
        <swrla:isRuleEnabled rdf:datatype="http://www.w3.org/2001/XMLSchema#boolean">true</swrla:isRuleEnabled>
        <rdfs:comment rdf:datatype="http://www.w3.org/2001/XMLSchema#string">If vehicle X is overtaking vehicle Y, then the speed of vehicle X is greater than the speed of vehicle Y.</rdfs:comment>
        <rdfs:label rdf:datatype="http://www.w3.org/2001/XMLSchema#string">S10</rdfs:label>
        <rdf:type rdf:resource="http://www.w3.org/2003/11/swrl#Imp"/>
        <swrl:body>
            <rdf:Description>
                <rdf:type rdf:resource="http://www.w3.org/2003/11/swrl#AtomList"/>
                <rdf:first>
                    <rdf:Description>
                        <rdf:type rdf:resource="http://www.w3.org/2003/11/swrl#ClassAtom"/>
                        <swrl:classPredicate rdf:resource="http://vcd.vicomtech.org/ontology/automotive#Overtaking"/>
                        <swrl:argument1 rdf:resource="http://vcd.vicomtech.org/ontology/automotive#oa"/>
                    </rdf:Description>
                </rdf:first>
                <rdf:rest>
                    <rdf:Description>
                        <rdf:type rdf:resource="http://www.w3.org/2003/11/swrl#AtomList"/>
                        <rdf:first>
                            <rdf:Description>
                                <rdf:type rdf:resource="http://www.w3.org/2003/11/swrl#IndividualPropertyAtom"/>
                                <swrl:propertyPredicate rdf:resource="http://vcd.vicomtech.org/ontology/automotive#isSubjectOfAction"/>
                                <swrl:argument1 rdf:resource="http://vcd.vicomtech.org/ontology/automotive#oa"/>
                                <swrl:argument2 rdf:resource="http://vcd.vicomtech.org/ontology/automotive#x"/>
                            </rdf:Description>
                        </rdf:first>
                        <rdf:rest>
                            <rdf:Description>
                                <rdf:type rdf:resource="http://www.w3.org/2003/11/swrl#AtomList"/>
                                <rdf:first>
                                    <rdf:Description>
                                        <rdf:type rdf:resource="http://www.w3.org/2003/11/swrl#IndividualPropertyAtom"/>
                                        <swrl:propertyPredicate rdf:resource="http://vcd.vicomtech.org/ontology/automotive#isObjectOfAction"/>
                                        <swrl:argument1 rdf:resource="http://vcd.vicomtech.org/ontology/automotive#oa"/>
                                        <swrl:argument2 rdf:resource="http://vcd.vicomtech.org/ontology/automotive#y"/>
                                    </rdf:Description>
                                </rdf:first>
                                <rdf:rest>
                                    <rdf:Description>
                                        <rdf:type rdf:resource="http://www.w3.org/2003/11/swrl#AtomList"/>
                                        <rdf:first>
                                            <rdf:Description>
                                                <rdf:type rdf:resource="http://www.w3.org/2003/11/swrl#ClassAtom"/>
                                                <swrl:classPredicate rdf:resource="http://vcd.vicomtech.org/ontology/automotive#Vehicle"/>
                                                <swrl:argument1 rdf:resource="http://vcd.vicomtech.org/ontology/automotive#x"/>
                                            </rdf:Description>
                                        </rdf:first>
                                        <rdf:rest>
                                            <rdf:Description>
                                                <rdf:type rdf:resource="http://www.w3.org/2003/11/swrl#AtomList"/>
                                                <rdf:first>
                                                    <rdf:Description>
                                                        <rdf:type rdf:resource="http://www.w3.org/2003/11/swrl#ClassAtom"/>
                                                        <swrl:classPredicate rdf:resource="http://vcd.vicomtech.org/ontology/automotive#Vehicle"/>
                                                        <swrl:argument1 rdf:resource="http://vcd.vicomtech.org/ontology/automotive#y"/>
                                                    </rdf:Description>
                                                </rdf:first>
                                                <rdf:rest>
                                                    <rdf:Description>
                                                        <rdf:type rdf:resource="http://www.w3.org/2003/11/swrl#AtomList"/>
                                                        <rdf:first>
                                                            <rdf:Description>
                                                                <rdf:type rdf:resource="http://www.w3.org/2003/11/swrl#DatavaluedPropertyAtom"/>
                                                                <swrl:propertyPredicate rdf:resource="http://vcd.vicomtech.org/ontology/automotive#hasSpeed"/>
                                                                <swrl:argument1 rdf:resource="http://vcd.vicomtech.org/ontology/automotive#x"/>
                                                                <swrl:argument2 rdf:resource="http://vcd.vicomtech.org/ontology/automotive#sx"/>
                                                            </rdf:Description>
                                                        </rdf:first>
                                                        <rdf:rest>
                                                            <rdf:Description>
                                                                <rdf:type rdf:resource="http://www.w3.org/2003/11/swrl#AtomList"/>
                                                                <rdf:first>
                                                                    <rdf:Description>
                                                                        <rdf:type rdf:resource="http://www.w3.org/2003/11/swrl#DatavaluedPropertyAtom"/>
                                                                        <swrl:propertyPredicate rdf:resource="http://vcd.vicomtech.org/ontology/automotive#hasSpeed"/>
                                                                        <swrl:argument1 rdf:resource="http://vcd.vicomtech.org/ontology/automotive#y"/>
                                                                        <swrl:argument2 rdf:resource="http://vcd.vicomtech.org/ontology/automotive#sy"/>
                                                                    </rdf:Description>
                                                                </rdf:first>
                                                                <rdf:rest rdf:resource="http://www.w3.org/1999/02/22-rdf-syntax-ns#nil"/>
                                                            </rdf:Description>
                                                        </rdf:rest>
                                                    </rdf:Description>
                                                </rdf:rest>
                                            </rdf:Description>
                                        </rdf:rest>
                                    </rdf:Description>
                                </rdf:rest>
                            </rdf:Description>
                        </rdf:rest>
                    </rdf:Description>
                </rdf:rest>
            </rdf:Description>
        </swrl:body>
        <swrl:head>
            <rdf:Description>
                <rdf:type rdf:resource="http://www.w3.org/2003/11/swrl#AtomList"/>
                <rdf:first>
                    <rdf:Description>
                        <rdf:type rdf:resource="http://www.w3.org/2003/11/swrl#BuiltinAtom"/>
                        <swrl:builtin rdf:resource="http://www.w3.org/2003/11/swrlb#greaterThan"/>
                        <swrl:arguments rdf:parseType="Collection">
                            <rdf:Description rdf:about="http://vcd.vicomtech.org/ontology/automotive#sx"/>
                            <rdf:Description rdf:about="http://vcd.vicomtech.org/ontology/automotive#sy"/>
                        </swrl:arguments>
                    </rdf:Description>
                </rdf:first>
                <rdf:rest rdf:resource="http://www.w3.org/1999/02/22-rdf-syntax-ns#nil"/>
            </rdf:Description>
        </swrl:head>
    </rdf:Description>
    <rdf:Description>
        <swrla:isRuleEnabled rdf:datatype="http://www.w3.org/2001/XMLSchema#boolean">true</swrla:isRuleEnabled>
        <rdfs:comment rdf:datatype="http://www.w3.org/2001/XMLSchema#string">If X is the subject of an overtaking Action (oa) and Y is the object, then X is behind Y and Y is in front of X.</rdfs:comment>
        <rdfs:label rdf:datatype="http://www.w3.org/2001/XMLSchema#string">S9</rdfs:label>
        <rdf:type rdf:resource="http://www.w3.org/2003/11/swrl#Imp"/>
        <swrl:body>
            <rdf:Description>
                <rdf:type rdf:resource="http://www.w3.org/2003/11/swrl#AtomList"/>
                <rdf:first>
                    <rdf:Description>
                        <rdf:type rdf:resource="http://www.w3.org/2003/11/swrl#ClassAtom"/>
                        <swrl:classPredicate rdf:resource="http://vcd.vicomtech.org/ontology/automotive#Overtaking"/>
                        <swrl:argument1 rdf:resource="http://vcd.vicomtech.org/ontology/automotive#oa"/>
                    </rdf:Description>
                </rdf:first>
                <rdf:rest>
                    <rdf:Description>
                        <rdf:type rdf:resource="http://www.w3.org/2003/11/swrl#AtomList"/>
                        <rdf:first>
                            <rdf:Description>
                                <rdf:type rdf:resource="http://www.w3.org/2003/11/swrl#IndividualPropertyAtom"/>
                                <swrl:propertyPredicate rdf:resource="http://vcd.vicomtech.org/ontology/automotive#isSubjectOfAction"/>
                                <swrl:argument1 rdf:resource="http://vcd.vicomtech.org/ontology/automotive#x"/>
                                <swrl:argument2 rdf:resource="http://vcd.vicomtech.org/ontology/automotive#oa"/>
                            </rdf:Description>
                        </rdf:first>
                        <rdf:rest>
                            <rdf:Description>
                                <rdf:type rdf:resource="http://www.w3.org/2003/11/swrl#AtomList"/>
                                <rdf:first>
                                    <rdf:Description>
                                        <rdf:type rdf:resource="http://www.w3.org/2003/11/swrl#IndividualPropertyAtom"/>
                                        <swrl:propertyPredicate rdf:resource="http://vcd.vicomtech.org/ontology/automotive#isObjectOfAction"/>
                                        <swrl:argument1 rdf:resource="http://vcd.vicomtech.org/ontology/automotive#y"/>
                                        <swrl:argument2 rdf:resource="http://vcd.vicomtech.org/ontology/automotive#oa"/>
                                    </rdf:Description>
                                </rdf:first>
                                <rdf:rest rdf:resource="http://www.w3.org/1999/02/22-rdf-syntax-ns#nil"/>
                            </rdf:Description>
                        </rdf:rest>
                    </rdf:Description>
                </rdf:rest>
            </rdf:Description>
        </swrl:body>
        <swrl:head>
            <rdf:Description>
                <rdf:type rdf:resource="http://www.w3.org/2003/11/swrl#AtomList"/>
                <rdf:first>
                    <rdf:Description>
                        <rdf:type rdf:resource="http://www.w3.org/2003/11/swrl#IndividualPropertyAtom"/>
                        <swrl:propertyPredicate rdf:resource="http://vcd.vicomtech.org/ontology/automotive#behindOf"/>
                        <swrl:argument1 rdf:resource="http://vcd.vicomtech.org/ontology/automotive#x"/>
                        <swrl:argument2 rdf:resource="http://vcd.vicomtech.org/ontology/automotive#y"/>
                    </rdf:Description>
                </rdf:first>
                <rdf:rest>
                    <rdf:Description>
                        <rdf:type rdf:resource="http://www.w3.org/2003/11/swrl#AtomList"/>
                        <rdf:first>
                            <rdf:Description>
                                <rdf:type rdf:resource="http://www.w3.org/2003/11/swrl#IndividualPropertyAtom"/>
                                <swrl:propertyPredicate rdf:resource="http://vcd.vicomtech.org/ontology/automotive#inFrontOf"/>
                                <swrl:argument1 rdf:resource="http://vcd.vicomtech.org/ontology/automotive#y"/>
                                <swrl:argument2 rdf:resource="http://vcd.vicomtech.org/ontology/automotive#x"/>
                            </rdf:Description>
                        </rdf:first>
                        <rdf:rest rdf:resource="http://www.w3.org/1999/02/22-rdf-syntax-ns#nil"/>
                    </rdf:Description>
                </rdf:rest>
            </rdf:Description>
        </swrl:head>
    </rdf:Description>
</rdf:RDF>



<!-- Generated by the OWL API (version 4.5.9.2019-02-01T07:24:44Z) https://github.com/owlcs/owlapi -->

